format-version: 1.2
data-version: t4fs/releases/2023-03-02/t4fs-simple.owl
remark: terms4FAIRskills by the terms4FAIRskills developers is licensed under CC BY 4.0. You are free to share (copy and redistribute the material in any medium or format) and adapt (remix, transform, and build upon the material) for any purpose, even commercially. for any purpose, even commercially. The licensor cannot revoke these freedoms as long as you follow the license terms. You must give appropriate credit (by using the original ontology IRI for the whole ontology and original term IRIs for individual terms), provide a link to the license, and indicate if any changes were made. You may do so in any reasonable manner, but not in any way that suggests the licensor endorses you or your use.
ontology: t4fs/t4fs-simple
property_value: http://purl.org/dc/terms/description "terms4FAIRskills describes the competencies, skills and knowledge associated with making and keeping data FAIR.\\nThis terminology applies to a variety of use cases, including: assisting with the creation and assessment of stewardship curricula; facilitating the annotation, discovery and evaluation of FAIR-enabling materials \\(e.g. training\\) and resources; enabling the formalisation of job descriptions and CVs with recognised, structured competencies.\\nIt is intended to be of use to trainers who teach FAIR data skills, researchers who wish to identify skill gaps in their teams and managers who need to recruit individuals to relevant roles." xsd:string
property_value: http://purl.org/dc/terms/license http://creativecommons.org/licenses/by/4.0/
property_value: http://purl.org/dc/terms/title "terms4FAIRskills (T4FS)" xsd:string
property_value: owl:versionInfo "2023-03-02" xsd:string

[Term]
id: T4FS:0000002
name: pipe separated values
def: "A file that contains the values in a table as a series of ASCII text lines organized so that each column value is separated by a pipe." [] {http://purl.obolibrary.org/obo/IAO_0000119="CASRAI. https://casrai.org/term/pipe-separated-values/"}
is_a: T4FS:0000372 ! data stewardship technical concept
relationship: T4FS:0000563 T4FS:0000137 ! contributes to the implementation of I1. (meta)data use a formal, accessible, shared, and broadly applicable language for knowledge representation
property_value: IAO:0000117 "https://orcid.org/0000-0002-7702-4495" xsd:string
property_value: IAO:0000117 "Peter McQuilton" xsd:string

[Term]
id: T4FS:0000004
name: software preservation
def: "Software preservation involves the collection and long-term storage of software for archiving as well as maintaining availability and accessibility." [] {http://purl.obolibrary.org/obo/IAO_0000119="https://orcid.org/0000-0002-7702-4495 8.2.22"}
comment: AL 8.2.22: Refactored "software review and preservation" to "software preservation", as the review process is not within the remit of terms4FAIRskills. Added definition and source.
is_a: T4FS:0000156 ! archiving
property_value: IAO:0000117 "https://orcid.org/0000-0002-7702-4495" xsd:string
property_value: IAO:0000117 "Kristina Hettne" xsd:string
property_value: IAO:0000117 "Victoria Dominguez Del Angel" xsd:string
property_value: IAO:0000117 "Yann Le Franc" xsd:string

[Term]
id: T4FS:0000005
name: repository access
def: "In accessing a repository one uses a client (application) to discover relevant digital objects within a repository, and then retrieve a copy of a desired digital object." [] {http://purl.obolibrary.org/obo/IAO_0000119="CASRAI. https://casrai.org/term/repository-access"}
is_a: T4FS:0000489 ! repository
property_value: IAO:0000117 "https://orcid.org/0000-0002-7702-4495" xsd:string
property_value: IAO:0000117 "Peter McQuilton" xsd:string

[Term]
id: T4FS:0000006
name: develop fair and open research vision
def: "Include FAIR and open research in the strategic framework for the organization and set objectives and timeframe." []
is_a: T4FS:0000008 ! develop open research strategy and vision
property_value: IAO:0000117 "Angus Whyte" xsd:string
property_value: IAO:0000117 "Celia van Gelder" xsd:string
property_value: IAO:0000117 "Mateusz Kuzak" xsd:string
property_value: IAO:0000117 "Yan Wang" xsd:string

[Term]
id: T4FS:0000008
name: develop open research strategy and vision
def: "The activity of developing an open research strategy and vision." [] {http://purl.obolibrary.org/obo/IAO_0000119="PMQ 3.2022"}
is_a: T4FS:0000514 ! strategic/long-term planning
property_value: IAO:0000117 "Angus Whyte" xsd:string
property_value: IAO:0000117 "Celia van Gelder" xsd:string
property_value: IAO:0000117 "Mateusz Kuzak" xsd:string
property_value: IAO:0000117 "Yan Wang" xsd:string

[Term]
id: T4FS:0000009
name: data management policy
def: "A written document backed by management describing policy and providing guidance to ensure that appropriate standards, consistent guidelines, and common strategies are used, providing linkages to and consistency with other similar systems, and fostering a true network across an organization producing data." [] {http://purl.obolibrary.org/obo/IAO_0000119="CASRAI. https://casrai.org/term/data-management-policy/"}
is_a: T4FS:0000372 ! data stewardship technical concept
relationship: T4FS:0000563 T4FS:0000447 ! contributes to the implementation of fair principle
property_value: IAO:0000117 "Peter McQuilton" xsd:string

[Term]
id: T4FS:0000010
name: understand research code of conduct
def: "Understand how the governing principles of research integrity and FAIR overlap" []
is_a: T4FS:0000525 ! research integrity, attribution, impact awareness
property_value: IAO:0000117 "Angus Whyte" xsd:string
property_value: IAO:0000117 "Celia van Gelder" xsd:string

[Term]
id: T4FS:0000011
name: choosing the appropriate reporting guideline for your data
def: "To be able to choose the appropriate reporting guideline/checklist for your data, based on community-adopted standards." [] {http://purl.obolibrary.org/obo/IAO_0000119="[PMQ]"}
is_a: T4FS:0000175 ! fair evaluation of repositories for data deposition
property_value: IAO:0000117 "Peter McQuilton" xsd:string

[Term]
id: T4FS:0000012
name: data stewardship activity
def: "A specific deed, action, function or sphere of action in relation with the role of data stewardship" []
relationship: T4FS:0000556 T4FS:0000548 ! requires/improves personal attribute data stewardship soft skill
property_value: IAO:0000117 "https://orcid.org/0000-0002-7702-4495" xsd:string
property_value: IAO:0000117 "Peter McQuilton" xsd:string
property_value: IAO:0000117 "Yann Le Franc" xsd:string
property_value: T4FS:0000564 "Set of actions carried out during data stewardship processes" xsd:string

[Term]
id: T4FS:0000013
name: data munging
def: "A series of potentially destructive or irrevocable changes to a piece of data or a file. Common munging operations include removing punctuation or html tags, data parsing, filtering, and transformation." [] {http://purl.obolibrary.org/obo/IAO_0000119="CASRAI. https://casrai.org/term/data-munging/"}
is_a: T4FS:0000036 ! curation
property_value: IAO:0000117 "Peter McQuilton" xsd:string

[Term]
id: T4FS:0000014
name: interoperability of digital assets
is_a: T4FS:0000447 ! fair principle
property_value: IAO:0000117 "Peter McQuilton" xsd:string

[Term]
id: T4FS:0000016
name: skills for resource management
def: "Bin for Skills related to Resource management" []
is_a: T4FS:0000353 ! resource management
property_value: IAO:0000117 "leightonlc" xsd:string

[Term]
id: T4FS:0000017
name: preservation
def: "An activity within archiving in which specific items of data are maintained over time so that they can still be accessed and understood through changes in technology." [] {http://purl.obolibrary.org/obo/IAO_0000119="CASRAI. https://casrai.org/term/preservation/"}
is_a: T4FS:0000156 ! archiving
property_value: IAO:0000117 "https://orcid.org/0000-0002-7702-4495" xsd:string
property_value: IAO:0000117 "Peter McQuilton" xsd:string
property_value: IAO:0000118 "Conservation" xsd:string

[Term]
id: T4FS:0000018
name: data categorisation
is_a: T4FS:0000036 ! curation
property_value: IAO:0000118 "Data Categorization" xsd:string
property_value: IAO:0000118 "Data Classification" xsd:string
created_by: Peter McQuilton
creation_date: 2021-02-17T22:30:31.531624Z

[Term]
id: T4FS:0000019
name: data registration
def: "A curation process on a data object by which it receives a persistent object identifier (PID) from a trusted registration authority. Registration must be accompanied by the step(s) to upload the data object to a persistent repository." [] {http://purl.obolibrary.org/obo/IAO_0000119="CASRAI. https://casrai.org/term/data-registration/ RELATED TERM. Repository; Persistent identifierREFERENCE. Research Data Alliance http://smw-rda.esc.rzg.mpg.de/index.php/Main_Page ; NISO (2004) Understanding Metadata. Bethesda, MD: NISO Press."}
is_a: T4FS:0000021 ! exposing data
property_value: IAO:0000117 "https://orcid.org/0000-0002-7702-4495" xsd:string
property_value: IAO:0000117 "Peter McQuilton" xsd:string

[Term]
id: T4FS:0000020
name: interoperability
def: "The capability to communicate, execute programs, or transfer data among various functional units in a useful and meaningful manner that requires the user to have little or no knowledge of the unique characteristics of those units. Foundational, syntactic, and semantic interoperability are the three necessary aspects of interoperability." [] {http://purl.obolibrary.org/obo/IAO_0000119="CASRAI. https://casrai.org/term/interoperability/"}
is_a: T4FS:0000372 ! data stewardship technical concept
relationship: T4FS:0000563 T4FS:0000014 ! contributes to the implementation of interoperability of digital assets
property_value: IAO:0000117 "Peter McQuilton" xsd:string

[Term]
id: T4FS:0000021
name: exposing data
def: "Exposing data is the activity of exposing your data to collaborators, the public, or other interested parties. A data producer makes the data accessible to external users in a machine- and/or human-readable way." [] {http://purl.obolibrary.org/obo/IAO_0000119="[PMQ 3.2022, AL 15.3.22]"}
comment: AL 15.3.22: Was "expose your data", which was not in the style of other term labels. Also updated definition, but might need revisiting later for a more formal definition.
is_a: T4FS:0000012 ! data stewardship activity
property_value: IAO:0000117 "https://orcid.org/0000-0002-7702-4495" xsd:string
property_value: IAO:0000117 "Peter McQuilton" xsd:string

[Term]
id: T4FS:0000023
name: aptitudes for workflow technologies management
def: "Bin for Aptitudes related to Workflow technologies management." []
is_a: T4FS:0000177 ! workflow technologies management
property_value: IAO:0000117 "leightonlc" xsd:string

[Term]
id: T4FS:0000024
name: de facto standard
def: "A standard that is widely accepted and used, but lacks formal approval by a recognized standards developing organization (e.g., the QWERTY keyboard)." [] {http://purl.obolibrary.org/obo/IAO_0000119="CASRAI. https://casrai.org/term/de-facto-standard/"}
is_a: T4FS:0000372 ! data stewardship technical concept
relationship: T4FS:0000563 T4FS:0000137 ! contributes to the implementation of I1. (meta)data use a formal, accessible, shared, and broadly applicable language for knowledge representation
property_value: IAO:0000117 "Peter McQuilton" xsd:string

[Term]
id: T4FS:0000025
name: data entity
def: "An object, event, or phenomenon about which data are stored in a database and which has intermediate representation in a Data Model." [] {http://purl.obolibrary.org/obo/IAO_0000119="CASRAI. https://casrai.org/term/data-entity/"}
is_a: T4FS:0000372 ! data stewardship technical concept
property_value: IAO:0000117 "Peter McQuilton" xsd:string

[Term]
id: T4FS:0000026
name: real-time data
def: "Data that are being received, processed and stored at the time of their occurrence with only small delays. Examples include: stock quotes, manufacturing statistics, Web server loads, data warehouse activity and sensor feeds to data collectors. Real-time data are data streams that are typically generated by sensors and received via direct networking connections." [] {http://purl.obolibrary.org/obo/IAO_0000119="CASRAI. https://casrai.org/term/real-time-data"}
is_a: T4FS:0000430 ! data
property_value: IAO:0000117 "https://orcid.org/0000-0002-7702-4495" xsd:string
property_value: IAO:0000117 "Peter McQuilton" xsd:string

[Term]
id: T4FS:0000027
name: storage security risk assessment and mitigation
def: "Detect and analysis security risk of storage periodically, and minimize the impact of the risks detected" []
is_a: T4FS:0000470 ! storage security management
property_value: IAO:0000117 "Angus Whyte" xsd:string
property_value: IAO:0000117 "Celia van Gelder" xsd:string
property_value: IAO:0000117 "Mateusz Kuzak" xsd:string
property_value: IAO:0000117 "Yan Wang" xsd:string

[Term]
id: T4FS:0000028
name: remote access
def: "The ability to get access to a computer or a network from a remote distance. Access may be through an Internet service provider (ISP) or through a dedicated line between a computer or a remote local area network and the central or main corporate local area network. A dedicated line is more expensive and less flexible but offers faster data rates." [] {http://purl.obolibrary.org/obo/IAO_0000119="CASRAI. https://casrai.org/term/remote-access"}
is_a: T4FS:0000372 ! data stewardship technical concept
property_value: IAO:0000117 "https://orcid.org/0000-0002-7702-4495" xsd:string
property_value: IAO:0000117 "Peter McQuilton" xsd:string

[Term]
id: T4FS:0000029
name: fair stewardship supervising
def: "The activity of supervision of other people to ensure FAIR data practices." [] {http://purl.obolibrary.org/obo/IAO_0000119="PMQ"}
is_a: T4FS:0000259 ! fair training
property_value: IAO:0000117 "https://orcid.org/0000-0002-7702-4495" xsd:string
property_value: IAO:0000117 "Peter McQuilton" xsd:string
property_value: IAO:0000117 "Philippe Rocca-Serra" xsd:string
property_value: IAO:0000117 "Susanna Sansone" xsd:string

[Term]
id: T4FS:0000030
name: skills related to high performance computing management
def: "Bin for Skills needed for High performance computing management." []
is_a: T4FS:0000308 ! high performance computing management
property_value: IAO:0000117 "leightonlc" xsd:string

[Term]
id: T4FS:0000031
name: fair metrics selection skills
def: "Ability to select the appropriate FAIR metrics among the existing ones in relation to the type of digital object concerned." []
is_a: T4FS:0000252 ! fairness assessment
property_value: IAO:0000117 "Kristina Hettne" xsd:string
property_value: IAO:0000117 "Victoria Dominguez Del Angel" xsd:string
property_value: IAO:0000117 "Yann Le Franc" xsd:string

[Term]
id: T4FS:0000032
name: relational database
def: "A collection of data items organized as a set of formally-described tables from which data can be accessed or reassembled in many different ways without having to reorganize the database tables. The standard user and application program interface to a relational database is the structured query language (SQL)." [] {http://purl.obolibrary.org/obo/IAO_0000119="CASRAI. https://casrai.org/term/relational-database"}
is_a: T4FS:0000372 ! data stewardship technical concept
property_value: IAO:0000117 "https://orcid.org/0000-0002-7702-4495" xsd:string
property_value: IAO:0000117 "Peter McQuilton" xsd:string

[Term]
id: T4FS:0000033
name: non identifiable data
def: "Data that could not lead to the identification of a specific object of interest. These may be data that have been de-identified, or that could not lead to identifiable information in the first place." [] {http://purl.obolibrary.org/obo/IAO_0000119="Modified by AL on 6.5.22 from CASRAI. https://casrai.org/term/non-identifiable-data/"}
comment: AL 6.5.22: Modifed CASRAI definition to distinguish this term from 'non personally identifiable information.' Further work may determine whether or not both terms are required.
is_a: T4FS:0000430 ! data
property_value: IAO:0000117 "https://orcid.org/0000-0002-7702-4495" xsd:string
property_value: IAO:0000117 "Peter McQuilton" xsd:string

[Term]
id: T4FS:0000034
name: database developer
relationship: T4FS:0000558 T4FS:0000012 ! has/wants competency in data stewardship activity
relationship: T4FS:0000559 T4FS:0000372 ! has/wants knowledge about data stewardship technical concept
relationship: T4FS:0000559 T4FS:0000446 ! has/wants knowledge about data stewardship guideline
relationship: T4FS:0000561 T4FS:0000372 ! has/wants practical skill about data stewardship technical concept
relationship: T4FS:0000562 T4FS:0000548 ! has aptitude for data stewardship soft skill

[Term]
id: T4FS:0000036
name: curation
def: "The activity of managing and promoting the use of data from their point of creation to ensure that they are fit for contemporary purpose and available for discovery and reuse." [] {http://purl.obolibrary.org/obo/IAO_0000119="CASRAI. https://casrai.org/term/curation/"}
is_a: T4FS:0000012 ! data stewardship activity
property_value: IAO:0000117 "Peter McQuilton" xsd:string

[Term]
id: T4FS:0000038
name: A1. (meta)data are retrievable by their identifier using a standardised communications protocol
is_a: T4FS:0000478 ! accessibility of digital assets
property_value: IAO:0000117 "Peter McQuilton" xsd:string

[Term]
id: T4FS:0000039
name: version control
def: "Control over time of data, computer code, software, and documents that allows for the ability to revert to a previous revision, which is critical for data traceability, tracking edits, and correcting mistakes. Version control generates a (changed) copy of a data object that is uniquely labeled with a version number. The intent is to track changes to a data object, by making versioned copies. Note that a version is different from a backup copy, which is typically a copy made at a specific point in time, or a replica." [] {http://purl.obolibrary.org/obo/IAO_0000119="CASRAI. https://casrai.org/term/version-control"}
is_a: T4FS:0000372 ! data stewardship technical concept
property_value: IAO:0000117 "https://orcid.org/0000-0002-7702-4495" xsd:string
property_value: IAO:0000117 "Peter McQuilton" xsd:string

[Term]
id: T4FS:0000041
name: understanding fair and open research challenges in your organization
def: "Understand the FAIR and open research practices, and the research landscape / current data management practices in the organization." []
is_a: T4FS:0000008 ! develop open research strategy and vision
property_value: IAO:0000117 "Angus Whyte" xsd:string
property_value: IAO:0000117 "Celia van Gelder" xsd:string
property_value: IAO:0000117 "Mateusz Kuzak" xsd:string
property_value: IAO:0000117 "Yan Wang" xsd:string

[Term]
id: T4FS:0000042
name: ethical application of patents, licenses
is_a: T4FS:0000106 ! publish data

[Term]
id: T4FS:0000043
name: data access protocol
def: "A system that allows outsiders to be granted access to databases without overloading the system." [] {http://purl.obolibrary.org/obo/IAO_0000119="CASRAI. https://casrai.org/term/data-access-protocol/"}
is_a: T4FS:0000283 ! access
property_value: IAO:0000117 "Peter McQuilton" xsd:string

[Term]
id: T4FS:0000044
name: data processing
def: "A generic concept referring to all kinds of procedures being executed on data at any point in the data life cycle." [] {http://purl.obolibrary.org/obo/IAO_0000119="CASRAI. https://casrai.org/term/data-processing/"}
is_a: T4FS:0000036 ! curation
property_value: IAO:0000117 "Peter McQuilton" xsd:string

[Term]
id: T4FS:0000045
name: data organization
def: "Denotes the complexity of measures that are used by a repository to form aggregations of data objects (including collections and metadata) to describe the properties of data objects, to register PIDs, to build the PID records, to link between all components, and to set up the containers (software stack) that are used to store all..." [] {http://purl.obolibrary.org/obo/IAO_0000119="CASRAI. https://casrai.org/term/data-organization/"}
is_a: T4FS:0000372 ! data stewardship technical concept
relationship: T4FS:0000563 T4FS:0000447 ! contributes to the implementation of fair principle
property_value: IAO:0000117 "Peter McQuilton" xsd:string

[Term]
id: T4FS:0000046
name: data rescue
def: "Recovery and/or transformation and digitization of dark data and at-risk data so that they can be preserved, accessed, shared, and used. Data rescue also involves the addition of rich metadata to make the content understandable and more easily re-usable." [] {http://purl.obolibrary.org/obo/IAO_0000119="CASRAI. https://casrai.org/term/data-rescue/ REFERENCE. http://www.wmo.int/pages/prog/hwrp/datarescue.php ; http://iedro.org/data-rescue-process/ ;"}
is_a: T4FS:0000156 ! archiving
property_value: IAO:0000117 "https://orcid.org/0000-0002-7702-4495" xsd:string
property_value: IAO:0000117 "Peter McQuilton" xsd:string

[Term]
id: T4FS:0000047
name: understand societal impact of research
def: "Anticipate possible implications of the research and making its outputs FAIR, reflecting on rmotivations and areas of uncertainty" []
is_a: T4FS:0000525 ! research integrity, attribution, impact awareness
property_value: IAO:0000117 "Angus Whyte" xsd:string
property_value: IAO:0000117 "Celia van Gelder" xsd:string
property_value: IAO:0000117 "Mateusz Kuzak" xsd:string
property_value: IAO:0000117 "Yan Wang" xsd:string

[Term]
id: T4FS:0000048
name: searching via algorithms and software
def: "To be able to search using software with a GUI or terminal access. For example using BLAST or genomic search tools in the life sciences." [] {http://purl.obolibrary.org/obo/IAO_0000119="[PMQ]"}
is_a: T4FS:0000145 ! search repositories and knowledge-bases
property_value: IAO:0000117 "Peter McQuilton" xsd:string
property_value: IAO:0000118 "Algorithm searching" xsd:string
property_value: IAO:0000118 "batch search" xsd:string
property_value: IAO:0000118 "Programmatic search" xsd:string

[Term]
id: T4FS:0000049
name: audit
def: "An independent evaluation of an organization, system, process, project or product." [] {http://purl.obolibrary.org/obo/IAO_0000119="CASRAI. https://casrai.org/term/audit/"}
is_a: T4FS:0000126 ! assessment
property_value: IAO:0000117 "Peter McQuilton" xsd:string

[Term]
id: T4FS:0000050
name: wiki site
is_a: T4FS:0000095 ! online documentation
created_by: Peter McQuilton
creation_date: 2020-10-01T21:03:37.147424Z

[Term]
id: T4FS:0000051
name: skills related to authorisation management
def: "Bin for Skills needed for Authorization management." []
is_a: T4FS:0000142 ! authorisation management
property_value: IAO:0000117 "leightonlc" xsd:string

[Term]
id: T4FS:0000053
name: storage management
def: "The term storage management encompasses the technologies and processes organizations use to maximize or improve the performance of their data storage resources. It is a broad category that includes  virtualization, replication, mirroring, security, compression, traffic analysis, process automation, storage provisioning and related techniques." [] {http://purl.obolibrary.org/obo/IAO_0000119="(webopedia.com/TERM/S/storage_management.html)[VDA]"}
is_a: T4FS:0000353 ! resource management
property_value: IAO:0000117 "Kristina Hettne" xsd:string
property_value: IAO:0000117 "Simon Hodson" xsd:string
property_value: IAO:0000117 "Victoria Dominguez Del Angel" xsd:string

[Term]
id: T4FS:0000054
name: data warehouse
def: "A central repository for all or significant parts of the data that an organization's various business systems collect. A data warehouse tends to be a strategic but somewhat unfinished concept. Data warehousing emphasizes the capture of data from diverse sources for useful analysis and access, but does not generally start from the point-of-view of the &hellip; <a href=CASRAI. https://casrai.org/term/data-warehouse/ class=more-link" [] {http://purl.obolibrary.org/obo/IAO_0000119="CASRAI. https://casrai.org/term/data-warehouse/"}
is_a: T4FS:0000215 ! data store
property_value: IAO:0000117 "Peter McQuilton" xsd:string

[Term]
id: T4FS:0000055
name: data driven disaster
def: "A serious problem caused by one or more ineffective data analysis processes. In addition to the financial burden, problems with data quality and analysis can have a serious impact on security, compliance, project management and human resource management, among others." [] {http://purl.obolibrary.org/obo/IAO_0000119="CASRAI. https://casrai.org/term/data-driven-disaster/"}
is_a: T4FS:0000012 ! data stewardship activity
property_value: IAO:0000117 "Peter McQuilton" xsd:string

[Term]
id: T4FS:0000056
name: data identifier
def: "An identifier that uniquely distinguishes one set of data from all others." [] {http://purl.obolibrary.org/obo/IAO_0000119="CASRAI. https://casrai.org/term/data-identifier/"}
is_a: T4FS:0000453 ! persistent identifier
property_value: IAO:0000117 "Peter McQuilton" xsd:string

[Term]
id: T4FS:0000057
name: data splitting
def: "An approach to protecting sensitive data from unauthorized access by encrypting the data and storing different portions of a file on different servers. An unauthorized person would need to know the locations of the servers containing the parts, be able to get access to each server, know what data to combine, and how to decrypt it. Data splitting can be made even more effective by periodically retrieving and recombining the parts, and then splitting the data in a different way among different servers, and using a different encryption key." [] {http://purl.obolibrary.org/obo/IAO_0000119="CASRAI. https://casrai.org/term/data-splitting/"}
is_a: T4FS:0000107 ! information security
property_value: IAO:0000117 "https://orcid.org/0000-0002-7702-4495" xsd:string
property_value: IAO:0000117 "Peter McQuilton" xsd:string

[Term]
id: T4FS:0000058
name: manage access
def: "Monitor the status of information access of different stakeholder groups. Evaluate new access request and authorize or decline it. Update the organizational information access overview." []
is_a: T4FS:0000107 ! information security
property_value: IAO:0000117 "Angus Whyte" xsd:string
property_value: IAO:0000117 "Celia van Gelder" xsd:string
property_value: IAO:0000117 "Mateusz Kuzak" xsd:string
property_value: IAO:0000117 "Yan Wang" xsd:string

[Term]
id: T4FS:0000059
name: system metadata
def: "Digital entity properties that are generated by the data management system (e.g., creation time; owner; storage location; data retention period; the length of time a digital entity will be retained)." [] {http://purl.obolibrary.org/obo/IAO_0000119="CASRAI. https://casrai.org/term/system-metadata/"}
is_a: T4FS:0000527 ! metadata
property_value: IAO:0000117 "https://orcid.org/0000-0002-7702-4495" xsd:string
property_value: IAO:0000117 "Peter McQuilton" xsd:string

[Term]
id: T4FS:0000060
name: tactical/short-term planning
is_a: T4FS:0000320 ! project management activities
property_value: IAO:0000117 "https://orcid.org/0000-0002-7702-4495" xsd:string
property_value: IAO:0000117 "Peter McQuilton" xsd:string
property_value: IAO:0000117 "Philippe Rocca-Serra" xsd:string
property_value: IAO:0000117 "Susanna Sansone" xsd:string

[Term]
id: T4FS:0000061
name: electronic medical record
def: "An electronic version of the paper record that doctors have traditionally maintained for their patients and which is typically only accessible within the facility or office that controls it." [] {http://purl.obolibrary.org/obo/IAO_0000119="CASRAI. https://casrai.org/term/electronic-medical-record/"}
is_a: T4FS:0000372 ! data stewardship technical concept
property_value: IAO:0000117 "Peter McQuilton" xsd:string

[Term]
id: T4FS:0000062
name: aptitudes for provenance information management
def: "Bin for Aptitudes related to Provenance information management." []
is_a: T4FS:0000368 ! provenance information management
property_value: IAO:0000117 "leightonlc" xsd:string

[Term]
id: T4FS:0000065
name: data modeling
def: "Data modeling formalizes and documents existing processes and events. It captures and translates complex system designs into easily understood representations of the data flows and processes, creating a blueprint for construction and/or re-engineering." [] {http://purl.obolibrary.org/obo/IAO_0000119="CASRAI. https://casrai.org/term/data-modeling/"}
is_a: T4FS:0000036 ! curation
property_value: IAO:0000117 "Peter McQuilton" xsd:string

[Term]
id: T4FS:0000067
name: use of aggregator sites
def: "To be able to search and understand the results from dataset aggregrator sites. To understand the implications of the provenance of the data and how to integrate and analyse data with differing metadata." [] {http://purl.obolibrary.org/obo/IAO_0000119="[PMQ]"}
is_a: T4FS:0000145 ! search repositories and knowledge-bases
property_value: IAO:0000117 "Peter McQuilton" xsd:string
property_value: IAO:0000118 "Searching aggregator sites" xsd:string

[Term]
id: T4FS:0000068
name: manage metadata catalog
def: "Implement the policies that govern the choice of metadata schema, reserved vocabularies, metadata organization in tables, and metadata properties (creation date, access control, ownership, etc.)." [] {http://purl.obolibrary.org/obo/IAO_0000119="CASRAI. https://casrai.org/term/manage-metadata-catalog"}
is_a: T4FS:0000353 ! resource management
property_value: IAO:0000117 "https://orcid.org/0000-0002-7702-4495" xsd:string
property_value: IAO:0000117 "Peter McQuilton" xsd:string

[Term]
id: T4FS:0000069
name: data transformation
def: "Manipulation of raw data to produce a single output." [] {http://purl.obolibrary.org/obo/IAO_0000119="CASRAI. https://casrai.org/term/data-transformation/"}
is_a: T4FS:0000352 ! data analysis
property_value: IAO:0000117 "https://orcid.org/0000-0002-7702-4495" xsd:string
property_value: IAO:0000117 "Peter McQuilton" xsd:string

[Term]
id: T4FS:0000070
name: cataloguing
def: "An intellectual process of describing objects in accordance with accepted library principles, particularly those of subject and classification order." [] {http://purl.obolibrary.org/obo/IAO_0000119="CASRAI. https://casrai.org/term/cataloguing/"}
is_a: T4FS:0000036 ! curation
property_value: IAO:0000117 "Peter McQuilton" xsd:string

[Term]
id: T4FS:0000071
name: design and apply processes for attribution
def: "Iniitate and develop processes for crediting the contributions of researchers and professional groups towards making FAIR outputs" []
is_a: T4FS:0000525 ! research integrity, attribution, impact awareness
property_value: IAO:0000117 "Angus Whyte" xsd:string
property_value: IAO:0000117 "Celia van Gelder" xsd:string
property_value: IAO:0000117 "Mateusz Kuzak" xsd:string
property_value: IAO:0000117 "Yan Wang" xsd:string

[Term]
id: T4FS:0000072
name: dataset series
def: "A collection of datasets sharing the same product specification. A dataset series is a type of aggregation or collection with some logical grouping such as by a topic (specification) with the (product) unit being a dataset series. Example: A series of earth observations. Each year, month or week (depending on the volume) might be a &hellip; <a href=CASRAI. https://casrai.org/term/dataset-series/ class=more-link" [] {http://purl.obolibrary.org/obo/IAO_0000119="CASRAI. https://casrai.org/term/dataset-series/"}
is_a: T4FS:0000397 ! database
property_value: IAO:0000117 "Peter McQuilton" xsd:string

[Term]
id: T4FS:0000073
name: data dictionary
def: "A collection of descriptions of the data objects or items in a data model." [] {http://purl.obolibrary.org/obo/IAO_0000119="CASRAI. https://casrai.org/term/data-dictionary/"}
is_a: T4FS:0000372 ! data stewardship technical concept
property_value: IAO:0000117 "Peter McQuilton" xsd:string

[Term]
id: T4FS:0000074
name: data selection
def: "A process that creates a new dataset from an original source. Examples include: creating a subset of the data,querying a database." [] {http://purl.obolibrary.org/obo/IAO_0000119="CASRAI. https://casrai.org/term/data-selection/"}
is_a: T4FS:0000231 ! data acquisition
property_value: IAO:0000117 "https://orcid.org/0000-0002-7702-4495" xsd:string
property_value: IAO:0000117 "Peter McQuilton" xsd:string

[Term]
id: T4FS:0000075
name: apply data access policy
def: "Define data access policy based on project requirements. Provide access to autorised parties." []
is_a: T4FS:0000469 ! access control and management
property_value: IAO:0000117 "Celia van Gelder" xsd:string
property_value: IAO:0000117 "Mateusz Kuzak" xsd:string
property_value: IAO:0000117 "Yan Wang" xsd:string

[Term]
id: T4FS:0000076
name: data discovery
def: "The ability to find and comprehend data produced by people other than yourself." [] {http://purl.obolibrary.org/obo/IAO_0000119="[PMQ]"}
comment: AL 15.3.22: tidied label from "discover other peoples data" to "Data discovery
is_a: T4FS:0000012 ! data stewardship activity
property_value: IAO:0000117 "https://orcid.org/0000-0002-7702-4495" xsd:string
property_value: IAO:0000117 "Peter McQuilton" xsd:string
property_value: IAO:0000118 "Data search" xsd:string

[Term]
id: T4FS:0000078
name: documented data
def: "Data that are delivered with all associated metadata, data dictionary, description of methods and instruments used to collect and process the data, and other supporting data (e.g., duplicate sample results, replicate analyses, percent recovery, etc.)." [] {http://purl.obolibrary.org/obo/IAO_0000119="CASRAI. https://casrai.org/term/documented-data/"}
is_a: T4FS:0000430 ! data
property_value: IAO:0000117 "Peter McQuilton" xsd:string

[Term]
id: T4FS:0000079
name: conducting operations
is_a: T4FS:0000320 ! project management activities
property_value: IAO:0000117 "https://orcid.org/0000-0002-7702-4495" xsd:string
property_value: IAO:0000117 "Peter McQuilton" xsd:string
property_value: IAO:0000117 "Philippe Rocca-Serra" xsd:string
property_value: IAO:0000117 "Susanna Sansone" xsd:string

[Term]
id: T4FS:0000080
name: dynamic data
def: "Data the content of which is changing frequently and at asynchronous moments. Examples include: Data streams that are generated by sensors when it is unpredictable when data segments will appear in time (i.e. data streams have gaps); Data streams that are generated by humans in crowdsourcing scenarios where it is not clear when which cell in a database will be filled." [] {http://purl.obolibrary.org/obo/IAO_0000119="CASRAI. https://casrai.org/term/dynamic-data/"}
is_a: T4FS:0000372 ! data stewardship technical concept
property_value: IAO:0000117 "https://orcid.org/0000-0002-7702-4495" xsd:string
property_value: IAO:0000117 "Peter McQuilton" xsd:string

[Term]
id: T4FS:0000081
name: reference model
def: "A design covering a class of frameworks with the following characteristics: (1) it can be used to generate more specific models that still belong to the class and (2) it can be used to compare a concrete framework design to identify whether it belongs to the same class." [] {http://purl.obolibrary.org/obo/IAO_0000119="CASRAI. https://casrai.org/term/reference-model"}
is_a: T4FS:0000372 ! data stewardship technical concept
relationship: T4FS:0000563 T4FS:0000137 ! contributes to the implementation of I1. (meta)data use a formal, accessible, shared, and broadly applicable language for knowledge representation
property_value: IAO:0000117 "https://orcid.org/0000-0002-7702-4495" xsd:string
property_value: IAO:0000117 "Peter McQuilton" xsd:string

[Term]
id: T4FS:0000082
name: online workbook
is_a: T4FS:0000095 ! online documentation
created_by: Peter McQuilton
creation_date: 2020-10-01T20:52:57.551905Z

[Term]
id: T4FS:0000084
name: engaging in open innovation beyond academia
is_a: T4FS:0000106 ! publish data

[Term]
id: T4FS:0000085
name: registered data
def: "Data that have gone through a registration process and have been assigned an identifier metadata to aid in their search and retrieval." [] {http://purl.obolibrary.org/obo/IAO_0000119="CASRAI. https://casrai.org/term/registered-data"}
is_a: T4FS:0000430 ! data
property_value: IAO:0000117 "https://orcid.org/0000-0002-7702-4495" xsd:string
property_value: IAO:0000117 "Peter McQuilton" xsd:string

[Term]
id: T4FS:0000086
name: integrity
def: "In the context of data and network security: The assurance that information can only be accessed or modified by those authorized to do so. Measures taken to ensure integrity include controlling the physical environment of networked terminals and servers, restricting access to data, and maintaining rigorous authentication practices. Data integrity can also be threatened by environmental hazards, such as heat, dust, and electrical surges." [] {http://purl.obolibrary.org/obo/IAO_0000119="CASRAI. https://casrai.org/term/integrity/"}
is_a: T4FS:0000012 ! data stewardship activity
property_value: IAO:0000117 "https://orcid.org/0000-0002-7702-4495" xsd:string
property_value: IAO:0000117 "Peter McQuilton" xsd:string

[Term]
id: T4FS:0000087
name: digital scholarship
def: "Incorporates: building a digital collection of information for further study and analysis; creating appropriate tools for collection- building; creating appropriate tools for the analysis and study of collections; using digital collections and analytical tools to generate new intellectual products; and, Creating authoring tools for these new intellectual products, either in traditional forms or in digital form." [] {http://purl.obolibrary.org/obo/IAO_0000119="CASRAI. https://casrai.org/term/digital-scholarship/"}
is_a: T4FS:0000012 ! data stewardship activity
property_value: IAO:0000117 "https://orcid.org/0000-0002-7702-4495" xsd:string
property_value: IAO:0000117 "Peter McQuilton" xsd:string

[Term]
id: T4FS:0000088
name: a knowledge for resource management
def: "Bin for types of Knowledge related to Resource management" []
is_a: T4FS:0000353 ! resource management
property_value: IAO:0000117 "leightonlc" xsd:string

[Term]
id: T4FS:0000089
name: aptitudes for resource management
def: "Bin for Aptitudes related to Resource management." []
is_a: T4FS:0000353 ! resource management
property_value: IAO:0000117 "leightonlc" xsd:string

[Term]
id: T4FS:0000091
name: knowledge of storage management
def: "Bin for types of Knowledge related to Storage management." []
is_a: T4FS:0000053 ! storage management
property_value: IAO:0000117 "leightonlc" xsd:string

[Term]
id: T4FS:0000092
name: understand open access publishing
def: "Know about the open access publishing procedure, journals' policies on OA publishing, project funder and institutions policy as well as the financial support on OA publishing" []
is_a: T4FS:0000193 ! open access publishing
property_value: IAO:0000117 "Celia van Gelder" xsd:string
property_value: IAO:0000117 "Mateusz Kuzak" xsd:string
property_value: IAO:0000117 "Yan Wang" xsd:string

[Term]
id: T4FS:0000093
name: use of persistent, resolvable identifiers (pids)
def: "OBSOLETE. The use of persistent identifiers or PIDs to uniquely and persistently identify an entity." [] {http://purl.obolibrary.org/obo/IAO_0000119="[PMQ 3.2022]"}
comment: This term is redundant with http://purl.obolibrary.org/obo/T4FS_0000388 and has been deprecated.
property_value: IAO:0000117 "https://orcid.org/0000-0002-7702-4495" xsd:string
property_value: IAO:0000117 "Nancy Hoebelheinrich" xsd:string
property_value: IAO:0000117 "Peter McQuilton" xsd:string
property_value: IAO:0000233 "https://github.com/terms4fairskills/FAIRterminology/issues/21" xsd:string
is_obsolete: true

[Term]
id: T4FS:0000094
name: record standardization
def: "A process in which files are first parsed (assigned to appropriate fields in a record) and then translated to a common format. For example, if an original record had the client’s name and address as “Bob Jones, VP Acme. Co., 15 S. Main St, Brooklyn” the standardized record might read “Bob Jones, Vice President, Acme Corporation, 15 South Main Street, Brooklyn, New York”. Data often lack consistency simply because there are a many of ways of saying the same thing. Standardizing the record ensures that when a query is run for a particular field, accurate results will be returned." [] {http://purl.obolibrary.org/obo/IAO_0000119="CASRAI. https://casrai.org/term/record-standardization"}
is_a: T4FS:0000372 ! data stewardship technical concept
property_value: IAO:0000117 "https://orcid.org/0000-0002-7702-4495" xsd:string
property_value: IAO:0000117 "Peter McQuilton" xsd:string

[Term]
id: T4FS:0000095
name: online documentation
is_a: T4FS:0000519 ! learning medium
property_value: IAO:0000117 "Peter McQuilton" xsd:string
created_by: Peter McQuilton
creation_date: 2020-10-01T20:53:59.107153Z

[Term]
id: T4FS:0000096
name: metadata catalogue
def: "A catalogue containing metadata records in XML-encoded (machine-readable and human-readable) format that enables services to find data and services." [] {http://purl.obolibrary.org/obo/IAO_0000119="https://casrai.org/term/metadata-catalogue/"}
is_a: T4FS:0000372 ! data stewardship technical concept
relationship: T4FS:0000563 T4FS:0000393 ! contributes to the implementation of F4. (meta)data are registered or indexed in a searchable resource
property_value: IAO:0000117 "https://orcid.org/0000-0002-7702-4495" xsd:string
property_value: IAO:0000117 "Peter McQuilton" xsd:string
created_by: Peter McQuilton

[Term]
id: T4FS:0000097
name: understand legal background of patents
def: "Learn about the types of patents and its legal implications. Understand the application procedure of patents." []
is_a: T4FS:0000042 ! ethical application of patents, licenses
property_value: IAO:0000117 "Celia van Gelder" xsd:string
property_value: IAO:0000117 "Mateusz Kuzak" xsd:string
property_value: IAO:0000117 "Yan Wang" xsd:string

[Term]
id: T4FS:0000098
name: data file format
def: "The layout of a file in terms of how the data within the file are organized. A program that uses the data in a file must be able to recognize and possibly access data within the file." [] {http://purl.obolibrary.org/obo/IAO_0000119="CASRAI. https://casrai.org/term/data-file-format/"}
is_a: T4FS:0000372 ! data stewardship technical concept
property_value: IAO:0000117 "Peter McQuilton" xsd:string

[Term]
id: T4FS:0000100
name: data catalogue
def: "A curated collection of metadata about datasets and their data elements." [] {http://purl.obolibrary.org/obo/IAO_0000119="CASRAI. https://casrai.org/term/data-catalogue/"}
is_a: T4FS:0000215 ! data store
property_value: IAO:0000117 "Peter McQuilton" xsd:string

[Term]
id: T4FS:0000102
name: curation workflow
def: "A type of workflow that includes active steps to curate data as an aid to on-going management of data through its lifecycle." [] {http://purl.obolibrary.org/obo/IAO_0000119="CASRAI. https://casrai.org/term/curation-workflow/"}
is_a: T4FS:0000372 ! data stewardship technical concept
property_value: IAO:0000117 "Peter McQuilton" xsd:string

[Term]
id: T4FS:0000103
name: A1.1 the protocol is open, free, and universally implementable
is_a: T4FS:0000038 ! A1. (meta)data are retrievable by their identifier using a standardised communications protocol
property_value: IAO:0000117 "Peter McQuilton" xsd:string

[Term]
id: T4FS:0000104
name: preservation costs management
def: "Planning for and controlling the present and future costs of the conservation of data, including technical storage, fixed costs, and staff resources." [] {http://purl.obolibrary.org/obo/IAO_0000119="Based on https://www.cessda.eu/About/Projects/Past-projects/CESSDA-SaW/WP4/Cost-Benefit-Advocacy-Toolkit/Costs-Factsheet [LLC]"}
is_a: T4FS:0000353 ! resource management
property_value: IAO:0000117 "Kristina Hettne" xsd:string
property_value: IAO:0000117 "Leighton Christiansen" xsd:string
property_value: IAO:0000117 "Simon Hodson" xsd:string
property_value: IAO:0000117 "Victoria Dominguez Del Angel" xsd:string

[Term]
id: T4FS:0000105
name: project manager
def: "The person who is tasked with delivering a project within the boundaries and framework established by the program manager. The project manager is and should be delivery and execution focused and is judged on the elements of time, cost, and scope of the project. The person responsible for ensuring that the Project Team completes the project. The Project Manager develops the Project Plan with the team and manages the teamís performance of project tasks. It is also the responsibility of the Project Manager to secure acceptance and approval of deliverables from the Project Sponsor and Stakeholders. The Project Manager is responsible for communication, including status reporting, risk management, escalation of issues that cannot be resolved in the team, and, in general, making sure the project is delivered in budget, on schedule, and within scope." [] {http://purl.obolibrary.org/obo/IAO_0000119="CASRAI. https://casrai.org/term/project-manager"}
is_a: T4FS:0000415 ! manager
property_value: IAO:0000117 "https://orcid.org/0000-0002-7702-4495" xsd:string
property_value: IAO:0000117 "Peter McQuilton" xsd:string

[Term]
id: T4FS:0000106
name: publish data
comment: AL 9.3.22. Removed from 'FAIR4S defined activity' class to better integrate with the T4FS hierarchy. AL 5.5.22: removed "Publishing and archiving data" and "Publish and archive data" alternative terms, as the two actions are not the same.
is_a: T4FS:0000021 ! exposing data
property_value: IAO:0000117 "Celia van Gelder" xsd:string
property_value: IAO:0000117 "https://orcid.org/0000-0002-7702-4495" xsd:string
property_value: IAO:0000117 "Mateusz Kuzak" xsd:string
property_value: IAO:0000117 "Peter McQuilton" xsd:string
property_value: IAO:0000117 "Yan Wang" xsd:string
property_value: IAO:0000118 "Release data" xsd:string

[Term]
id: T4FS:0000107
name: information security
comment: AL 16.3.22: Changed 'information security and access management' such that access management went in as an alternative term. If required in future, we may wish to separate it out completely.
is_a: T4FS:0000012 ! data stewardship activity
property_value: IAO:0000117 "https://orcid.org/0000-0002-7702-4495" xsd:string
property_value: IAO:0000118 "Access management" xsd:string

[Term]
id: T4FS:0000108
name: data production
def: "Includes all activities involved in the planning, collecting, processing, analysis and maintenance of data in the original research project. Among these activities are selecting a study design, constructing instruments for data collection, conducting data collection/creation, performing data editing/verification/validation, analyzing data, backing up data versions and preparing and tagging metadata." [] {http://purl.obolibrary.org/obo/IAO_0000119="CASRAI. https://casrai.org/term/data-production/"}
is_a: T4FS:0000231 ! data acquisition
property_value: IAO:0000117 "Peter McQuilton" xsd:string

[Term]
id: T4FS:0000109
name: raw data
def: "Data that have not been processed for meaningful use. Although raw data have the potential to become information, they require selective extraction, organization, and sometimes analysis and formatting for presentation. As a result of processing, raw data sometimes end up in a database, which enables the data to become accessible for further processing and analysis." [] {http://purl.obolibrary.org/obo/IAO_0000119="CASRAI. https://casrai.org/term/raw-data"}
is_a: T4FS:0000430 ! data
property_value: IAO:0000117 "https://orcid.org/0000-0002-7702-4495" xsd:string
property_value: IAO:0000117 "Peter McQuilton" xsd:string

[Term]
id: T4FS:0000112
name: interface testing
def: "Testing conducted to evaluate whether systems or components pass data and control correctly to each other." [] {http://purl.obolibrary.org/obo/IAO_0000119="CASRAI. https://casrai.org/term/interface-testing/"}
is_a: T4FS:0000126 ! assessment
property_value: IAO:0000117 "https://orcid.org/0000-0002-7702-4495" xsd:string
property_value: IAO:0000117 "Peter McQuilton" xsd:string

[Term]
id: T4FS:0000113
name: digital object
def: "A digital object is editable, interactive, accessible and modifiable by means of digital objects other than the one governing its behaviour, and is distributed over information infrastructures. It is a machine-independent data structure consisting of one or more elements in digital form that can be parsed by different information systems; the structure helps to enable interoperability among diverse information systems in the Internet." [] {http://purl.obolibrary.org/obo/IAO_0000119="CASRAI. https://casrai.org/term/digital-object/"}
is_a: T4FS:0000372 ! data stewardship technical concept
property_value: IAO:0000117 "https://orcid.org/0000-0002-7702-4495" xsd:string
property_value: IAO:0000117 "Peter McQuilton" xsd:string

[Term]
id: T4FS:0000114
name: digital materials
def: "A broad term encompassing: (a) digital surrogates created as a result of converting analogue materials to digital form (digitisation); (b) born digital for which there has never been and is never intended to be an analogue equivalent; and, (c) digital records." [] {http://purl.obolibrary.org/obo/IAO_0000119="CASRAI. https://casrai.org/term/digital-materials/"}
is_a: T4FS:0000372 ! data stewardship technical concept
property_value: IAO:0000117 "https://orcid.org/0000-0002-7702-4495" xsd:string
property_value: IAO:0000117 "Peter McQuilton" xsd:string

[Term]
id: T4FS:0000116
name: define access policy
def: "Understand the needs and conditions of information access for different stakeholder groups. Identify the responsibility and rights for each stakeholder group on informaiton access. Build up a catalogue of risk profiles. For each risk profile, develope mitigation protocols." []
is_a: T4FS:0000107 ! information security
property_value: IAO:0000117 "Angus Whyte" xsd:string
property_value: IAO:0000117 "Celia van Gelder" xsd:string
property_value: IAO:0000117 "Mateusz Kuzak" xsd:string
property_value: IAO:0000117 "Yan Wang" xsd:string

[Term]
id: T4FS:0000117
name: skills related to provenance information management
def: "Bin for Skills needed for Provenance information management." []
is_a: T4FS:0000368 ! provenance information management
created_by: leightonlc
creation_date: 2019-10-17T15:17:02.313138Z

[Term]
id: T4FS:0000118
name: remote data access
def: "The ability to access and download data from a repository." [] {http://purl.obolibrary.org/obo/IAO_0000119="CASRAI. https://casrai.org/term/remote-data-access"}
is_a: T4FS:0000372 ! data stewardship technical concept
property_value: IAO:0000117 "https://orcid.org/0000-0002-7702-4495" xsd:string
property_value: IAO:0000117 "Peter McQuilton" xsd:string

[Term]
id: T4FS:0000119
name: disambiguation
def: "The act of interpreting an author's intended use of a word that has multiple meanings or spellings." [] {http://purl.obolibrary.org/obo/IAO_0000119="CASRAI. https://casrai.org/term/dissambuation/"}
is_a: T4FS:0000036 ! curation
property_value: IAO:0000117 "https://orcid.org/0000-0002-7702-4495" xsd:string
property_value: IAO:0000117 "Peter McQuilton" xsd:string

[Term]
id: T4FS:0000120
name: data compliance
def: "Data compliance consists of the ongoing processes to ensure adherence of data to both enterprise business rules (government department, university, industry, or agency), and to legal, regulatory and accreditation requirements." [] {http://purl.obolibrary.org/obo/IAO_0000119="CASRAI. https://casrai.org/term/data-compliance/"}
is_a: T4FS:0000372 ! data stewardship technical concept
property_value: IAO:0000117 "Peter McQuilton" xsd:string

[Term]
id: T4FS:0000121
name: re-use
def: "OBSOLETE. Use of content outside of its original intention." [] {http://purl.obolibrary.org/obo/IAO_0000119="CASRAI. https://casrai.org/term/re-use"}
comment: AL 2.3.23: Removed because of its high level of similarity with the 'R' FAIR principle.
property_value: IAO:0000117 "https://orcid.org/0000-0002-7702-4495" xsd:string
property_value: IAO:0000117 "Peter McQuilton" xsd:string
property_value: IAO:0000233 "https://github.com/terms4fairskills/FAIRterminology/issues/15" xsd:string
is_obsolete: true

[Term]
id: T4FS:0000122
name: trainer/teacher
relationship: T4FS:0000558 T4FS:0000012 ! has/wants competency in data stewardship activity
relationship: T4FS:0000559 T4FS:0000372 ! has/wants knowledge about data stewardship technical concept
relationship: T4FS:0000559 T4FS:0000446 ! has/wants knowledge about data stewardship guideline
relationship: T4FS:0000561 T4FS:0000372 ! has/wants practical skill about data stewardship technical concept
relationship: T4FS:0000562 T4FS:0000548 ! has aptitude for data stewardship soft skill

[Term]
id: T4FS:0000123
name: aptitudes for identity management
def: "Bin for Aptitudes related to Identity management." []
is_a: T4FS:0000169 ! identity management
property_value: IAO:0000117 "leightonlc" xsd:string

[Term]
id: T4FS:0000124
name: understand information security challenges
def: "Know the security requirements on the organization regarding different types of information Know the current organizational policy, infrastructure and capacity on information security." []
is_a: T4FS:0000107 ! information security
property_value: IAO:0000117 "Angus Whyte" xsd:string
property_value: IAO:0000117 "Celia van Gelder" xsd:string
property_value: IAO:0000117 "Mateusz Kuzak" xsd:string
property_value: IAO:0000117 "Yan Wang" xsd:string

[Term]
id: T4FS:0000125
name: aptitudes for authorisation management
def: "Bin for Aptitudes related to Authorization management." []
is_a: T4FS:0000142 ! authorisation management
property_value: IAO:0000117 "leightonlc" xsd:string

[Term]
id: T4FS:0000126
name: assessment
comment: AL 17.3.22: Updated to "Assessment" to match the style of its sibling classes. AL 3.22: Was "govern and assess", which is a compound concept. Split into two classes, Assess and Governance. Original source: FAIR4S defined activity.
is_a: T4FS:0000012 ! data stewardship activity
property_value: IAO:0000117 "Angus Whyte" xsd:string
property_value: IAO:0000117 "Celia van Gelder" xsd:string
property_value: IAO:0000117 "https://orcid.org/0000-0002-7702-4495" xsd:string
property_value: IAO:0000117 "Mateusz Kuzak" xsd:string
property_value: IAO:0000117 "Yan Wang" xsd:string

[Term]
id: T4FS:0000127
name: personal information privacy
def: "The World Wide Web Consortium’s Platform for Personal Privacy Project (P3P) offers specific recommendations for practices that will let users define and share personal information with Web sites that they agree to share it with. The P3P incorporates a number of industry proposals, including the Open Profiling Standard (OPS). Using software that adheres to the P3P recommendations, users will be able to create a personal profile, all or parts of which can be made accessible to a Web site as the user directs. A tool that will help a user decide whether to trust a given Website with personal information is a Statement of Privacy Policy that a Web site can post." [] {http://purl.obolibrary.org/obo/IAO_0000119="CASRAI. https://casrai.org/term/personal-information-privacy"}
is_a: T4FS:0000372 ! data stewardship technical concept
property_value: IAO:0000117 "https://orcid.org/0000-0002-7702-4495" xsd:string
property_value: IAO:0000117 "Peter McQuilton" xsd:string

[Term]
id: T4FS:0000129
name: ability to solve fair implementation problems collaboratively
def: "Demonstrate ability to involve others and share responsibility for applying FAIR principles." [] {http://purl.obolibrary.org/obo/IAO_0000119="[PMQ, 3.2022]"}
is_a: T4FS:0000399 ! ability to learn new techniques for fair implementation
property_value: IAO:0000117 "Angus Whyte" xsd:string

[Term]
id: T4FS:0000131
name: skills related to cloud computing environment management
def: "Bin for Skills needed for Cloud computing environment management." []
is_a: T4FS:0000479 ! cloud computing environment management
created_by: leightonlc
creation_date: 2019-10-17T15:14:37.180683Z

[Term]
id: T4FS:0000132
name: data curation
def: "A managed process, throughout the data lifecycle, by which data &amp; data collections are cleansed, documented, standardized, formatted and inter-related. This includes versioning data, or forming a new collection from several data sources, annotating with metadata, adding codes to raw data (e.g., classifying a galaxy image with a galaxy type such as spiral)." [] {http://purl.obolibrary.org/obo/IAO_0000119="CASRAI. https://casrai.org/term/data-curation/"}
is_a: T4FS:0000036 ! curation
property_value: IAO:0000117 "Peter McQuilton" xsd:string

[Term]
id: T4FS:0000133
name: cite contributions
def: "Cite contributions to data work in published literature which draws upon that data." [] {http://purl.obolibrary.org/obo/IAO_0000119="[LM]"}
is_a: T4FS:0000021 ! exposing data
property_value: IAO:0000117 "Laura Molloy" xsd:string
property_value: IAO:0000117 "Peter McQuilton" xsd:string

[Term]
id: T4FS:0000134
name: operational management
def: "Ongoing organizational activities associated with supporting functional elements, as opposed to project elements. Operational management also includes support of products that the organization has created through project activity." [] {http://purl.obolibrary.org/obo/IAO_0000119="CASRAI. https://casrai.org/term/operational-management/"}
is_a: T4FS:0000548 ! data stewardship soft skill
property_value: IAO:0000117 "https://orcid.org/0000-0002-7702-4495" xsd:string
property_value: IAO:0000117 "Peter McQuilton" xsd:string

[Term]
id: T4FS:0000135
name: high quality data
def: "High-quality data are complete, timely, accurate, consistent, relevant, reliable, traceable, cleaned, validated, and well documented." [] {http://purl.obolibrary.org/obo/IAO_0000119="CASRAI. https://casrai.org/term/high-quality-data/"}
is_a: T4FS:0000372 ! data stewardship technical concept
property_value: IAO:0000117 "Peter McQuilton" xsd:string

[Term]
id: T4FS:0000136
name: how to make your data reuseable
def: "Understand what reuse is permitted according to the licenses or terms and conditions applicable to services, tools and their content." []
is_a: T4FS:0000481 ! the use of fair and open research tools or services
property_value: IAO:0000117 "Angus Whyte" xsd:string

[Term]
id: T4FS:0000137
name: I1. (meta)data use a formal, accessible, shared, and broadly applicable language for knowledge representation
is_a: T4FS:0000014 ! interoperability of digital assets
property_value: IAO:0000117 "Peter McQuilton" xsd:string

[Term]
id: T4FS:0000138
name: schema
def: "1. The organization or structure for a database. The activity of data modeling leads to a schema. (The plural form is schemata.) The term is used in discussing both relational databases and object-oriented databases. The term sometimes seems to refer to a visualization of a structure and sometimes to a formal text-oriented description. Two common types of database schemata are the star schema and the snowflake schema. 2. A formal expression of an inference rule for artificial intelligence (AI) computing. The expression is a generalized axiom in which specific values or cases are substituted for each symbol in the axiom to derive a specific inference." [] {http://purl.obolibrary.org/obo/IAO_0000119="CASRAI. https://casrai.org/term/schema"}
is_a: T4FS:0000372 ! data stewardship technical concept
property_value: IAO:0000117 "https://orcid.org/0000-0002-7702-4495" xsd:string
property_value: IAO:0000117 "Peter McQuilton" xsd:string

[Term]
id: T4FS:0000139
name: pid service
def: "A service that provides a connection between a PID and its target object." [] {http://purl.obolibrary.org/obo/IAO_0000119="CASRAI. https://casrai.org/term/pid-service/"}
is_a: T4FS:0000453 ! persistent identifier
property_value: IAO:0000117 "https://orcid.org/0000-0002-7702-4495" xsd:string
property_value: IAO:0000117 "Peter McQuilton" xsd:string

[Term]
id: T4FS:0000140
name: foundational interoperability
def: "Foundational interoperability allows data exchange from one information technology system to be received by another and does not require the ability for the receiving information technology system to interpret the data.REFERENCE. Healthcare information management and systems society" [] {http://purl.obolibrary.org/obo/IAO_0000119="CASRAI. https://casrai.org/term/foundational-interoperability/"}
is_a: T4FS:0000020 ! interoperability
property_value: IAO:0000117 "Peter McQuilton" xsd:string

[Term]
id: T4FS:0000141
name: data management
def: "The activities of data policies, data planning, data element standardization, information management control, data synchronization, data sharing, and database development, including practices and projects that acquire, control, protect, deliver and enhance the value of data and information." [] {http://purl.obolibrary.org/obo/IAO_0000119="CASRAI. https://casrai.org/term/data-management/"}
is_a: T4FS:0000353 ! resource management
property_value: IAO:0000117 "Peter McQuilton" xsd:string

[Term]
id: T4FS:0000142
name: authorisation management
def: "Authorization management is concerned with people's access to different objects, most often to data or physical objects, such as land, buildings, rooms or infrastructure." [] {http://purl.obolibrary.org/obo/IAO_0000119="https://managementmania.com/en/authorization-management"}
is_a: T4FS:0000353 ! resource management
property_value: IAO:0000117 "Kristina Hettne" xsd:string
property_value: IAO:0000117 "Leighton Christiansen" xsd:string
property_value: IAO:0000117 "Simon Hodson" xsd:string
property_value: IAO:0000117 "Victoria Dominguez Del Angel" xsd:string

[Term]
id: T4FS:0000143
name: knowledge of authorisation management
def: "Bin for types of Knowledge related to Authorization management." []
is_a: T4FS:0000142 ! authorisation management
property_value: IAO:0000117 "leightonlc" xsd:string

[Term]
id: T4FS:0000145
name: search repositories and knowledge-bases
def: "The ability to search repositories and knowledge-bases." [] {http://purl.obolibrary.org/obo/IAO_0000119="[PMQ]"}
is_a: T4FS:0000076 ! data discovery
property_value: IAO:0000117 "Peter McQuilton" xsd:string
property_value: IAO:0000118 "database search" xsd:string
property_value: IAO:0000118 "Repository search" xsd:string
property_value: IAO:0000118 "searching databases" xsd:string
property_value: IAO:0000118 "searching repositories" xsd:string

[Term]
id: T4FS:0000146
name: cloud ecosystem
def: "An ecosystem that includes not only traditional elements of cloud computing such as software and infrastructure, but also consultants, integrators, partners, third parties and anything in their environments that has a bearing on the other components." [] {http://purl.obolibrary.org/obo/IAO_0000119="CASRAI. https://casrai.org/term/cloud-ecosystem/"}
is_a: T4FS:0000372 ! data stewardship technical concept
property_value: IAO:0000117 "Peter McQuilton" xsd:string

[Term]
id: T4FS:0000148
name: understand legal background of licensing
def: "Learn about  data licensing, the types of data licences and its legal implications. Understand the application procedure of data licences." []
is_a: T4FS:0000042 ! ethical application of patents, licenses
property_value: IAO:0000117 "Celia van Gelder" xsd:string
property_value: IAO:0000117 "Mateusz Kuzak" xsd:string
property_value: IAO:0000117 "Yan Wang" xsd:string

[Term]
id: T4FS:0000149
name: archive
def: "A place or collection containing static records, documents, or other materials for long-term preservation." [] {http://purl.obolibrary.org/obo/IAO_0000119="CASRAI. https://casrai.org/term/archive/"}
is_a: T4FS:0000372 ! data stewardship technical concept
property_value: IAO:0000117 "Peter McQuilton" xsd:string

[Term]
id: T4FS:0000150
name: trusted digital repository
def: "An infrastructure component that provides reliable, long-term access to managed digital resources. It stores, manages, and curates digital objects and returns their bit streams when a request is issued. Trusted repositories undergo regular assessments according to a set of rules such as defined by Data Seal of Approval (DSA) or TRAC (ISO 16363). It is well understood that such an assessment has the potential of increasing trust from its depositors and users, but it will not be the only criterion for users. Repositories can be at different stages of assessments. However, it is evident that certain quality criteria need to be met to distinguish trusted repositories from all types of other entities that store data such as notebooks or lab servers." [] {http://purl.obolibrary.org/obo/IAO_0000119="CASRAI. https://casrai.org/term/trusted-digital-repository/"}
is_a: T4FS:0000372 ! data stewardship technical concept
property_value: IAO:0000117 "https://orcid.org/0000-0002-7702-4495" xsd:string
property_value: IAO:0000117 "Peter McQuilton" xsd:string

[Term]
id: T4FS:0000151
name: database administration
def: "The function of managing the physical aspects of data resources, including database design and integrity, backup and recovery, performance and tuning." [] {http://purl.obolibrary.org/obo/IAO_0000119="CASRAI. https://casrai.org/term/database-administration/ REFERENCE. DAMA Dictionary of Data Management"}
is_a: T4FS:0000141 ! data management
property_value: IAO:0000117 "https://orcid.org/0000-0002-7702-4495" xsd:string
property_value: IAO:0000117 "Peter McQuilton" xsd:string

[Term]
id: T4FS:0000152
name: knowledge of identity management
def: "Bin for types of Knowledge related to Identity management" []
is_a: T4FS:0000169 ! identity management
property_value: IAO:0000117 "leightonlc" xsd:string

[Term]
id: T4FS:0000153
name: quality assessment
is_a: T4FS:0000126 ! assessment
property_value: IAO:0000117 "Angus Whyte" xsd:string
property_value: IAO:0000117 "Celia van Gelder" xsd:string
property_value: IAO:0000117 "Mateusz Kuzak" xsd:string
property_value: IAO:0000117 "Yan Wang" xsd:string

[Term]
id: T4FS:0000154
name: data structure
def: "A specialized format for organizing and storing data. General data structure types include the array, the file, the record, the table, the tree, and so on. Any data structure is designed to organize data to suit a specific purpose so that it can be accessed and worked with in appropriate ways...." [] {http://purl.obolibrary.org/obo/IAO_0000119="CASRAI. https://casrai.org/term/data-structure/"}
is_a: T4FS:0000372 ! data stewardship technical concept
property_value: IAO:0000117 "Peter McQuilton" xsd:string
property_value: IAO:0000118 "Data format" xsd:string

[Term]
id: T4FS:0000155
name: information technology specialist
def: "Information systems and technology infrastructure manager, expert, or technician." [] {http://purl.obolibrary.org/obo/IAO_0000119="CASRAI. https://casrai.org/term/information-technology-specialist/"}
relationship: T4FS:0000558 T4FS:0000012 ! has/wants competency in data stewardship activity
relationship: T4FS:0000559 T4FS:0000372 ! has/wants knowledge about data stewardship technical concept
relationship: T4FS:0000559 T4FS:0000446 ! has/wants knowledge about data stewardship guideline
relationship: T4FS:0000561 T4FS:0000372 ! has/wants practical skill about data stewardship technical concept
relationship: T4FS:0000562 T4FS:0000548 ! has aptitude for data stewardship soft skill
property_value: IAO:0000117 "Peter McQuilton" xsd:string

[Term]
id: T4FS:0000156
name: archiving
def: "A curation activity that ensures that data are properly selected, stored, and can be accessed, and for which logical and physical integrity are maintained over time, including security and authenticity." [] {http://purl.obolibrary.org/obo/IAO_0000119="CASRAI. https://casrai.org/term/archiving/"}
is_a: T4FS:0000012 ! data stewardship activity
property_value: IAO:0000117 "Peter McQuilton" xsd:string

[Term]
id: T4FS:0000157
name: knowledge of preservation costs management
def: "Bin for types of Knowledge related to Preservation costs management." []
is_a: T4FS:0000104 ! preservation costs management
created_by: leightonlc
creation_date: 2019-10-17T15:17:32.816776Z

[Term]
id: T4FS:0000158
name: user acceptance testing
def: "A phase of development where the product is tested in the real world by the intended audience. The experiences of the early users are forwarded back to the developers who make final changes before releasing the product." [] {http://purl.obolibrary.org/obo/IAO_0000119="CASRAI. https://casrai.org/term/user-acceptance-testing/"}
is_a: T4FS:0000012 ! data stewardship activity
property_value: IAO:0000117 "https://orcid.org/0000-0002-7702-4495" xsd:string
property_value: IAO:0000117 "Peter McQuilton" xsd:string

[Term]
id: T4FS:0000159
name: minimal metadata
def: "A description with very little curation that would include at least a name and PID of a data object. Minimal metadata is only marginally targeted at discovery since there is much better infrastructure to accomplish this." [] {http://purl.obolibrary.org/obo/IAO_0000119="CASRAI, https://casrai.org/term/minimal-metadata/"}
is_a: T4FS:0000527 ! metadata
property_value: IAO:0000117 "https://orcid.org/0000-0002-7702-4495" xsd:string

[Term]
id: T4FS:0000160
name: metadata exposure
def: "Metadata exposure is the process of finding, identifying, selecting and acquiring/obtaining access to a metadata entity." [] {http://purl.obolibrary.org/obo/IAO_0000119="AL 22.3.22, and see also FRBR User Tasks at: https://sites.google.com/site/metadatastandards/chapter-6/6-3-frbr-user-tasks."}
comment: AL 22.3.22: Refactored from 'metadata creation and exposure'. Metadata creation has moved to the Curation hierarchy.
is_a: T4FS:0000021 ! exposing data
property_value: IAO:0000117 "https://orcid.org/0000-0002-7702-4495" xsd:string
property_value: IAO:0000117 "Nancy Hoebelheinrich" xsd:string

[Term]
id: T4FS:0000161
name: data destruction
def: "The process of destroying data stored on tapes, hard disks and other forms of electronic media so that it is completely unreadable and cannot be accessed or used." [] {http://purl.obolibrary.org/obo/IAO_0000119="CASRAI. https://casrai.org/term/data-destruction/"}
is_a: T4FS:0000107 ! information security

[Term]
id: T4FS:0000162
name: fair stewardship training
def: "The provision of training materials and events in and around good data stewardship." [] {http://purl.obolibrary.org/obo/IAO_0000119="PMQ"}
is_a: T4FS:0000259 ! fair training
property_value: IAO:0000117 "https://orcid.org/0000-0002-7702-4495" xsd:string
property_value: IAO:0000117 "Peter McQuilton" xsd:string
property_value: IAO:0000117 "Philippe Rocca-Serra" xsd:string
property_value: IAO:0000117 "Susanna Sansone" xsd:string

[Term]
id: T4FS:0000165
name: creativity
def: "The ability to have an innovative approach to research by creating new or modified current concepts, theories, approaches and/or solutions." [] {http://purl.obolibrary.org/obo/IAO_0000119="CASRAI. https://casrai.org/term/creativity/"}
is_a: T4FS:0000548 ! data stewardship soft skill
property_value: IAO:0000117 "Peter McQuilton" xsd:string

[Term]
id: T4FS:0000166
name: data table attribute
def: "1. A field or column in a database table. It is an abbreviation for 'physical data attribute' which is a single data element related to a data object, such as a table in a database. The database schema associates one or more attributes with each database entity (i.e. table). 2. A term for a logical or conceptual attribute such as in an entity-attribute-relationship (EAR) data model." [] {http://purl.obolibrary.org/obo/IAO_0000119="CASRAI. https://casrai.org/term/data-table-attribute/"}
is_a: T4FS:0000372 ! data stewardship technical concept
property_value: IAO:0000117 "Peter McQuilton" xsd:string

[Term]
id: T4FS:0000168
name: consensus standard
def: "A standard developed through the cooperation of all parties who have an interest in participating in its development and/or use." [] {http://purl.obolibrary.org/obo/IAO_0000119="CASRAI. https://casrai.org/term/consensus-standard/"}
is_a: T4FS:0000372 ! data stewardship technical concept
relationship: T4FS:0000563 T4FS:0000137 ! contributes to the implementation of I1. (meta)data use a formal, accessible, shared, and broadly applicable language for knowledge representation
property_value: IAO:0000117 "Peter McQuilton" xsd:string
property_value: IAO:0000118 "Community standard" xsd:string

[Term]
id: T4FS:0000169
name: identity management
def: "Identity Management (IdM), also called Identity and Access Management (IAM) refers to a framework of policies and technologies for ensuring that the proper  user in an organisation has the appropriate access to technology resources  systems fall under the overarching umbrella of IT security.  IdM systems not only identify, but authenticate and authorize individuals  who will be using IT resources, but also the hardware and applications users need to access." [] {http://purl.obolibrary.org/obo/IAO_0000119="https://en.wikipedia.org/wiki/Identity_management"}
is_a: T4FS:0000353 ! resource management
property_value: IAO:0000117 "Kristina Hettne" xsd:string
property_value: IAO:0000117 "Leighton Christiansen" xsd:string
property_value: IAO:0000117 "Simon Hodson" xsd:string
property_value: IAO:0000117 "Victoria Dominguez Del Angel" xsd:string
property_value: IAO:0000118 "IAM" xsd:string
property_value: IAO:0000118 "Identity and Access Management" xsd:string
property_value: IAO:0000118 "IdM" xsd:string

[Term]
id: T4FS:0000170
name: reuse of digital assets
is_a: T4FS:0000447 ! fair principle
property_value: IAO:0000117 "Peter McQuilton" xsd:string

[Term]
id: T4FS:0000172
name: investigate open innovation opportunities
def: "Explore the potential application domain/sociental implication of the project work and the communities of users/partners." []
is_a: T4FS:0000084 ! engaging in open innovation beyond academia
property_value: IAO:0000117 "Celia van Gelder" xsd:string
property_value: IAO:0000117 "Mateusz Kuzak" xsd:string
property_value: IAO:0000117 "Yan Wang" xsd:string

[Term]
id: T4FS:0000173
name: data recovery
def: "The process of restoring data that have been lost, accidentally deleted, corrupted or made inaccessible for any reason. The data recovery process may vary, depending on the circumstances of the data loss, the data recovery software used to create backups, and backup target media. In some cases, end users may be able to restore lost..." [] {http://purl.obolibrary.org/obo/IAO_0000119="CASRAI. https://casrai.org/term/data-quality-review/"}
is_a: T4FS:0000156 ! archiving
property_value: IAO:0000117 "Peter McQuilton" xsd:string

[Term]
id: T4FS:0000174
name: R1. (meta)data are richly described with a plurality of accurate and relevant attributes
is_a: T4FS:0000170 ! reuse of digital assets
property_value: IAO:0000117 "Peter McQuilton" xsd:string

[Term]
id: T4FS:0000175
name: fair evaluation of repositories for data deposition
def: "To be able to define and deploy appropriate criteria, based on the FAIR principles, to identify the appropriate repository for a dataset. This may, for example, involve discovering the mark-up of the repository, the exchange formats and data models used, and the licensing information for each repository. Tools such as the FAIR evaluator or FAIRshake may be used to assess the FAIRness of a repository based on human-entered questionnaires or FAIRsharing resource metadata." [] {http://purl.obolibrary.org/obo/IAO_0000119="[PMQ]"}
is_a: T4FS:0000021 ! exposing data
property_value: IAO:0000117 "Peter McQuilton" xsd:string
property_value: IAO:0000118 "FAIR data submission" xsd:string
property_value: IAO:0000118 "Repository FAIRness" xsd:string

[Term]
id: T4FS:0000176
name: regional standard
def: "A Regional standard is one that applies across a multi-nation region. Most countries have their own national standards-making bodies, which in turn may also group together to make regional standards. For example, national standards bodies in Europe are also members of the European Committee for Standardization (CEN) as well as members of ISO. The use of such standards may be voluntary, or they may be referenced in regulation (therefore mandatory)." [] {http://purl.obolibrary.org/obo/IAO_0000119="Adapted by AL from ISO. https://www.iso.org/sites/ConsumersStandards/1_standards.html#section1_2"}
comment: AL 9.3.22: Removed reference to CASRAI (https://casrai.org/term/regional-standard/), as the definition was unsuitable.
is_a: T4FS:0000372 ! data stewardship technical concept
property_value: IAO:0000117 "https://orcid.org/0000-0002-7702-4495" xsd:string
property_value: IAO:0000117 "Peter McQuilton" xsd:string

[Term]
id: T4FS:0000177
name: workflow technologies management
def: "The process of setting up environments for workflow technologies." [] {http://purl.obolibrary.org/obo/IAO_0000119="KH"}
is_a: T4FS:0000353 ! resource management
property_value: IAO:0000117 "Kristina Hettne" xsd:string
property_value: IAO:0000117 "Simon Hodson" xsd:string
property_value: IAO:0000117 "Victoria Dominguez Del Angel" xsd:string

[Term]
id: T4FS:0000178
name: data steward
def: "Data stewardship is a shared responsibility between Principal Investigators and data stewards. Principal Investigators are responsible for, and data stewards provide support for: (a) Data collection, data integration, or reuse of existing data; (b) Review of data quality; (c) Description of scientific workflow/process; (d) Provision of standards-compliant metadata; and, (e) Submission of data and data." [] {http://purl.obolibrary.org/obo/IAO_0000119="CASRAI. https://casrai.org/term/data-steward/"}
relationship: T4FS:0000558 T4FS:0000162 ! has/wants competency in fair stewardship training
relationship: T4FS:0000558 T4FS:0000297 ! has/wants competency in research data management
relationship: T4FS:0000558 T4FS:0000492 ! has/wants competency in understanding persistent identifiers
relationship: T4FS:0000559 T4FS:0000372 ! has/wants knowledge about data stewardship technical concept
relationship: T4FS:0000559 T4FS:0000446 ! has/wants knowledge about data stewardship guideline
relationship: T4FS:0000561 T4FS:0000372 ! has/wants practical skill about data stewardship technical concept
relationship: T4FS:0000562 T4FS:0000548 ! has aptitude for data stewardship soft skill
property_value: IAO:0000117 "Peter McQuilton" xsd:string
created_by: Peter McQuilton

[Term]
id: T4FS:0000180
name: skills related to preservation costs management
def: "Bin for Skills needed for Preservation costs management." []
is_a: T4FS:0000104 ! preservation costs management
created_by: leightonlc
creation_date: 2019-10-17T15:17:32.816013Z

[Term]
id: T4FS:0000181
name: repository certification schemes
is_a: T4FS:0000489 ! repository
created_by: Peter McQuilton
creation_date: 2021-02-17T22:10:11.837519Z

[Term]
id: T4FS:0000182
name: registry
def: "A database containing information about trusted repositories that are provided by the repository managers and are useful for human and machine users. It is a registry information system on which a register is maintained. These registries do not contain information about all metadata descriptions of digital objects, nor do they offer a list of PIDs of all stored digital objects. They do offer information based on standardized types on how to retrieve such information (e.g., the port under which OAI-PMH can be accessed to offer metadata). It is a set of files containing identifiers assigned to items with descriptions of the associated items. It is assignment of a permanent, unique and unambiguous identifier to an item." [] {http://purl.obolibrary.org/obo/IAO_0000119="CASRAI. https://casrai.org/term/registry"}
is_a: T4FS:0000372 ! data stewardship technical concept
property_value: IAO:0000117 "https://orcid.org/0000-0002-7702-4495" xsd:string
property_value: IAO:0000117 "Peter McQuilton" xsd:string

[Term]
id: T4FS:0000183
name: recognise and acknowledge contributions
def: "To clearly communicate the existence of contributions from different individuals / projects to the compilation of a given dataset, in such a way that can be consistently cited." [] {http://purl.obolibrary.org/obo/IAO_0000119="[LM]"}
is_a: T4FS:0000021 ! exposing data
property_value: IAO:0000117 "Laura Molloy" xsd:string
property_value: IAO:0000118 "attribution" xsd:string
property_value: IAO:0000118 "credit" xsd:string

[Term]
id: T4FS:0000184
name: linked open data
def: "Data where relationships/connections between them are available to allow easy data access. A typical case of a large Linked dataset is DBPedia (http://dbpedia.org/), which essentially makes the content of Wikipedia available in RDF. This related collection of interrelated datasets is stored on the Web and available via a common format -RDF." [] {http://purl.obolibrary.org/obo/IAO_0000119="CASRAI. https://casrai.org/term/linked-open-data/"}
is_a: T4FS:0000372 ! data stewardship technical concept
property_value: IAO:0000117 "https://orcid.org/0000-0002-7702-4495" xsd:string
property_value: IAO:0000117 "Peter McQuilton" xsd:string

[Term]
id: T4FS:0000185
name: research data format
def: "Research data format is a generic term encompassing the concept of a standardised format for research data." [] {http://purl.obolibrary.org/obo/IAO_0000119="AL, 9.3.22"}
comment: AL 9.3.2022: The original CASRAI definition is unsuitable (https://casrai.org/term/research-data-format), therefore I have changed the definition to something more generic.
is_a: T4FS:0000372 ! data stewardship technical concept
property_value: IAO:0000117 "https://orcid.org/0000-0002-7702-4495" xsd:string
property_value: IAO:0000117 "Peter McQuilton" xsd:string

[Term]
id: T4FS:0000186
name: research governance
def: "Ensures that the benefits to society of research outweigh any risks, from both an ethical and legal perspective." [] {http://purl.obolibrary.org/obo/IAO_0000119="CASRAI. https://casrai.org/term/research-governance/"}
is_a: T4FS:0000472 ! governance
property_value: IAO:0000117 "https://orcid.org/0000-0002-7702-4495" xsd:string
property_value: IAO:0000117 "Peter McQuilton" xsd:string

[Term]
id: T4FS:0000188
name: semantic interoperability
def: "The ability of computer systems to transmit data with unambiguous, shared meaning. Semantic interoperability is a requirement to enable machine computable logic, inferencing, knowledge discovery, and data federation between information systems. Semantic interoperability is achieved when the information transferred has, in its communicated form, all of the meaning required for the receiving system to interpret it correctly, even when the algorithms used by the receiving system are unknown to the sending system. Syntactic interoperability is a prerequisite to semantic interoperability." [] {http://purl.obolibrary.org/obo/IAO_0000119="CASRAI. https://casrai.org/term/semantic-interoperability"}
is_a: T4FS:0000372 ! data stewardship technical concept
relationship: T4FS:0000563 T4FS:0000361 ! contributes to the implementation of I2. (meta)data use vocabularies that follow fair principles
property_value: IAO:0000117 "https://orcid.org/0000-0002-7702-4495" xsd:string
property_value: IAO:0000117 "Peter McQuilton" xsd:string

[Term]
id: T4FS:0000189
name: international chemical identifier
def: "In the context of chemistry: The International Chemical Identifier is a non-proprietary identifier for chemical substances that can be used in printed and electronic data sources thus enabling easier linking of diverse data compilations. International Union of Pure and Applied Chemistry (IUPAC)REFERENCE. MIT data management and publishing" [] {http://purl.obolibrary.org/obo/IAO_0000119="CASRAI. https://casrai.org/term/international-chemical-identifier/"}
is_a: T4FS:0000453 ! persistent identifier
property_value: IAO:0000117 "Peter McQuilton" xsd:string

[Term]
id: T4FS:0000190
name: research data publication workflow
def: "Activities and processes in a digital environment that lead to the publication of research data, associated metadata and accompanying documentation and software code on the Web. In contrast to interim or final published products, workflows are the means to curate, document, and review, and thus ensure and enhance the value of the published product. Workflows can involve both humans and machines and often humans are supported by technology as they perform steps in the workflow. Similar workflows may vary in the details depending on the research discipline, data publishing product and/or the host institution of the workflow (e.g., individual publisher/journal, institutional repository, discipline-specific repository)." [] {http://purl.obolibrary.org/obo/IAO_0000119="CASRAI. https://casrai.org/term/research-data-publication-workflow/"}
is_a: T4FS:0000012 ! data stewardship activity
property_value: IAO:0000117 "https://orcid.org/0000-0002-7702-4495" xsd:string
property_value: IAO:0000117 "Peter McQuilton" xsd:string

[Term]
id: T4FS:0000191
name: data completeness
def: "The degree to which all required measures are known. Values may be designated as missing in order not to have empty cells, or missing values may be replaced with default or interpolated values. In the case of default or interpolated values, these must be flagged as such to distinguish them from actual measurements or observations." [] {http://purl.obolibrary.org/obo/IAO_0000119="CASRAI. https://casrai.org/term/data-completeness/"}
is_a: T4FS:0000372 ! data stewardship technical concept
property_value: IAO:0000117 "Peter McQuilton" xsd:string

[Term]
id: T4FS:0000192
name: privacy-preserving data linkage
def: "Data linkage where the resulting product has been de-identified." [] {http://purl.obolibrary.org/obo/IAO_0000119="CASRAI. https://casrai.org/term/privacy-preserving-data-linkage"}
is_a: T4FS:0000372 ! data stewardship technical concept
property_value: IAO:0000117 "https://orcid.org/0000-0002-7702-4495" xsd:string
property_value: IAO:0000117 "Peter McQuilton" xsd:string

[Term]
id: T4FS:0000193
name: open access publishing
comment: AL 22.3.22: refactored 'open access publishing and self-archiving' to be two separate concepts ('open access publishing', and 'self-archiving') according to T4FS best practices. Self-archiving did not have to be created because we already had self-archive, which was then moved to the Archiving hierarchy. 'publish open access' was also removed in favour of this term as they were too similar to have without the potential for confusion by users.
is_a: T4FS:0000106 ! publish data
property_value: IAO:0000117 "Celia van Gelder" xsd:string
property_value: IAO:0000117 "https://orcid.org/0000-0002-7702-4495" xsd:string
property_value: IAO:0000117 "Mateusz Kuzak" xsd:string
property_value: IAO:0000117 "Yan Wang" xsd:string

[Term]
id: T4FS:0000194
name: self-archiving
def: "Prepare the data in preferred types and the data documentation. Choose the data repository and data license, deposit the data in the repository." []
is_a: T4FS:0000534 ! data archiving
property_value: IAO:0000117 "Celia van Gelder" xsd:string
property_value: IAO:0000117 "https://orcid.org/0000-0002-7702-4495" xsd:string
property_value: IAO:0000117 "Mateusz Kuzak" xsd:string
property_value: IAO:0000117 "Yan Wang" xsd:string

[Term]
id: T4FS:0000195
name: information management advisor
def: "A person having a broad knowledge of information management disciplines and who provides guidance and support to program and staff functions on all aspects of managing the information resource." [] {http://purl.obolibrary.org/obo/IAO_0000119="CASRAI. https://casrai.org/term/information-management-advisor/"}
relationship: T4FS:0000558 T4FS:0000012 ! has/wants competency in data stewardship activity
relationship: T4FS:0000559 T4FS:0000372 ! has/wants knowledge about data stewardship technical concept
relationship: T4FS:0000559 T4FS:0000446 ! has/wants knowledge about data stewardship guideline
relationship: T4FS:0000561 T4FS:0000372 ! has/wants practical skill about data stewardship technical concept
relationship: T4FS:0000562 T4FS:0000548 ! has aptitude for data stewardship soft skill
property_value: IAO:0000117 "Peter McQuilton" xsd:string

[Term]
id: T4FS:0000196
name: data management plan
def: "A formal statement describing how research data will be managed and documented throughout a research project and the terms regarding the subsequent deposit of the data with a data repository for long-term management and preservation." [] {http://purl.obolibrary.org/obo/IAO_0000119="CASRAI. https://casrai.org/term/data-management-plan/"}
is_a: T4FS:0000372 ! data stewardship technical concept
relationship: T4FS:0000563 T4FS:0000447 ! contributes to the implementation of fair principle
property_value: IAO:0000117 "Peter McQuilton" xsd:string

[Term]
id: T4FS:0000199
name: F2. data are described with rich metadata
is_a: T4FS:0000248 ! findability of digital assets
property_value: IAO:0000117 "Peter McQuilton" xsd:string

[Term]
id: T4FS:0000200
name: R1.1 (meta)data are released with a clear and accessible data usage license
is_a: T4FS:0000174 ! R1. (meta)data are richly described with a plurality of accurate and relevant attributes
property_value: IAO:0000117 "Peter McQuilton" xsd:string
property_value: IAO:0000118 "Data license" xsd:string

[Term]
id: T4FS:0000201
name: data stream
def: "A sequence of digitally encoded, coherent signals used to send or receive a representation of information content as transmitted." [] {http://purl.obolibrary.org/obo/IAO_0000119="CASRAI. https://casrai.org/term/data-stream/"}
is_a: T4FS:0000372 ! data stewardship technical concept
property_value: IAO:0000117 "Peter McQuilton" xsd:string

[Term]
id: T4FS:0000202
name: data librarian
def: "Data experts who have a librarian background. Data librarians often carry out curation and metadata related work. There is much overlap between data librarians, data managers, and data stewards." [] {http://purl.obolibrary.org/obo/IAO_0000119="CASRAI. https://casrai.org/term/data-librarian/"}
relationship: T4FS:0000558 T4FS:0000012 ! has/wants competency in data stewardship activity
relationship: T4FS:0000559 T4FS:0000372 ! has/wants knowledge about data stewardship technical concept
relationship: T4FS:0000559 T4FS:0000446 ! has/wants knowledge about data stewardship guideline
relationship: T4FS:0000561 T4FS:0000372 ! has/wants practical skill about data stewardship technical concept
relationship: T4FS:0000562 T4FS:0000548 ! has aptitude for data stewardship soft skill
property_value: IAO:0000117 "Peter McQuilton" xsd:string

[Term]
id: T4FS:0000203
name: program governance
def: "The process of developing, communicating, implementing, monitoring, and assuring the policies, procedures, organizational structures, and practices associated with a given program." [] {http://purl.obolibrary.org/obo/IAO_0000119="CASRAI. https://casrai.org/term/program-governance/"}
is_a: T4FS:0000472 ! governance
property_value: IAO:0000117 "https://orcid.org/0000-0002-7702-4495" xsd:string
property_value: IAO:0000117 "Peter McQuilton" xsd:string

[Term]
id: T4FS:0000206
name: knowledge of workflow technologies management
def: "Bin for types of Knowledge related to Workflow technologies management." []
is_a: T4FS:0000177 ! workflow technologies management
created_by: leightonlc
creation_date: 2019-10-17T15:16:10.561925Z

[Term]
id: T4FS:0000209
name: access risk assessment and mitigation
def: "Obtain an overview of information access status for different stakeholder groups. Check this overview against the organizational information access policy and risk catalogue, identify the type of information security risks based on the mismatch between the current status and policy. Choose and implement the right protocal to mitigate the risk." []
is_a: T4FS:0000107 ! information security
property_value: IAO:0000117 "Angus Whyte" xsd:string
property_value: IAO:0000117 "Celia van Gelder" xsd:string
property_value: IAO:0000117 "Mateusz Kuzak" xsd:string
property_value: IAO:0000117 "Yan Wang" xsd:string

[Term]
id: T4FS:0000210
name: usable data
def: "Data that can be understood and used without additional information. Usable data are delivered in a form that meets the needs of different end-user audiences, is ready for the tasks that the end-user needs to accomplish, and that has been adapted to the end-user’s needs (not the other way around). Usable data have been cleaned, structured, are in machine readable format, fully documented, and ready for analysis and interpretation." [] {http://purl.obolibrary.org/obo/IAO_0000119="CASRAI. https://casrai.org/term/usable-data"}
is_a: T4FS:0000430 ! data
property_value: IAO:0000117 "https://orcid.org/0000-0002-7702-4495" xsd:string
property_value: IAO:0000117 "Peter McQuilton" xsd:string

[Term]
id: T4FS:0000211
name: presentation slides
is_a: T4FS:0000519 ! learning medium
property_value: IAO:0000117 "Peter McQuilton" xsd:string
created_by: Peter McQuilton
creation_date: 2020-10-01T20:52:43.543314Z

[Term]
id: T4FS:0000212
name: implement secure storage
def: "Configure secure storage and monitor its usage" []
is_a: T4FS:0000470 ! storage security management
property_value: IAO:0000117 "Angus Whyte" xsd:string
property_value: IAO:0000117 "Celia van Gelder" xsd:string
property_value: IAO:0000117 "Mateusz Kuzak" xsd:string
property_value: IAO:0000117 "Yan Wang" xsd:string

[Term]
id: T4FS:0000213
name: data lifecycle
def: "Refers to all the stages in the existence of digital information from creation to destruction. A lifecycle view is used to enable active management of the data objects and resource over time, thus maintaining accessibility and usability." [] {http://purl.obolibrary.org/obo/IAO_0000119="CASRAI. https://casrai.org/term/data-lifecycle/"}
is_a: T4FS:0000372 ! data stewardship technical concept
property_value: IAO:0000117 "Peter McQuilton" xsd:string

[Term]
id: T4FS:0000214
name: format and media migration
is_a: T4FS:0000156 ! archiving
property_value: IAO:0000117 "Kristina Hettne" xsd:string
property_value: IAO:0000117 "Victoria Dominguez Del Angel" xsd:string
property_value: IAO:0000117 "Yann Le Franc" xsd:string

[Term]
id: T4FS:0000215
name: data store
def: "A repository for persistently storing collections of data, such as a database, a file system or a directory. The data stored can be of any type that can be rendered in digital format and placed in electronic media. Examples include text, image, video files and audio files." [] {http://purl.obolibrary.org/obo/IAO_0000119="CASRAI. https://casrai.org/term/data-store/"}
is_a: T4FS:0000372 ! data stewardship technical concept
property_value: IAO:0000117 "Peter McQuilton" xsd:string

[Term]
id: T4FS:0000216
name: design processes for research integrity
def: "Initiate and develop processes to ensure outputs are made FAIR consistently with research integrity principles, and with ethical oversight." []
is_a: T4FS:0000525 ! research integrity, attribution, impact awareness
property_value: IAO:0000117 "Angus Whyte" xsd:string
property_value: IAO:0000117 "Celia van Gelder" xsd:string
property_value: IAO:0000117 "Mateusz Kuzak" xsd:string
property_value: IAO:0000117 "Yan Wang" xsd:string

[Term]
id: T4FS:0000217
name: core trust seal
def: "CoreTrustSeal offers to any interested data repository a core level certification based on the DSA–WDS Core Trustworthy Data Repositories Requirements catalogue and procedures. This universal catalogue of requirements reflects the core characteristics of trustworthy data repositories and is the culmination of a cooperative effort between DSA and WDS under the umbrella of the Research Data Alliance to merge their data repositories certifications." [] {http://purl.obolibrary.org/obo/IAO_0000119="https://www.coretrustseal.org/about/"}
is_a: T4FS:0000181 ! repository certification schemes
property_value: IAO:0000117 "Peter McQuilton" xsd:string
property_value: IAO:0000118 "CTS" xsd:string
created_by: Peter McQuilton
creation_date: 2021-02-17T22:12:12.996581Z

[Term]
id: T4FS:0000218
name: project management lifecycle
def: "Defines how to manage a project. It will always be the same, regardless of the project lifecycle being employed." [] {http://purl.obolibrary.org/obo/IAO_0000119="CASRAI. https://casrai.org/term/project-management-lifecycle"}
is_a: T4FS:0000372 ! data stewardship technical concept
property_value: IAO:0000117 "https://orcid.org/0000-0002-7702-4495" xsd:string
property_value: IAO:0000117 "Peter McQuilton" xsd:string

[Term]
id: T4FS:0000219
name: authenticity metadata
def: "A type of metadata that conveys information needed to link a data object to its original source." [] {http://purl.obolibrary.org/obo/IAO_0000119="CASRAI. https://casrai.org/term/authenticity-metadata/"}
is_a: T4FS:0000372 ! data stewardship technical concept
relationship: T4FS:0000563 T4FS:0000137 ! contributes to the implementation of I1. (meta)data use a formal, accessible, shared, and broadly applicable language for knowledge representation
property_value: IAO:0000117 "Peter McQuilton" xsd:string

[Term]
id: T4FS:0000220
name: researcher
relationship: T4FS:0000558 T4FS:0000012 ! has/wants competency in data stewardship activity
relationship: T4FS:0000559 T4FS:0000372 ! has/wants knowledge about data stewardship technical concept
relationship: T4FS:0000559 T4FS:0000446 ! has/wants knowledge about data stewardship guideline
relationship: T4FS:0000561 T4FS:0000372 ! has/wants practical skill about data stewardship technical concept
relationship: T4FS:0000562 T4FS:0000548 ! has aptitude for data stewardship soft skill

[Term]
id: T4FS:0000221
name: skills related to service level management
def: "Bin for Skills needed for Service level management." []
is_a: T4FS:0000466 ! service level management
created_by: leightonlc
creation_date: 2019-10-17T15:18:53.731967Z

[Term]
id: T4FS:0000222
name: personally identifiable information
def: "1. Data which relate to a living individual who can be identified (a) from those data, or (b) from those data and other information which is in the possession of, or is likely to come into the possession of, the data controller, and includes any expression of opinion about the individual and any indication of the intentions of the data controller or any other person in respect of the individual. 2. Any data that could potentially identify a specific individual. Any information that can be used to distinguish one person from another and can be used for de-anonymizing anonymous data can be considered personally identifiable data. 3. Data are identifiable if the information contains the name of an individual, or other identifying items such as birth date, address or geocoding. Data will be identifiable if the information contains a unique personal identifier and the holder of the information also has the master list linking the identifiers to individuals. Data may also be identifiable because of the number of different pieces of information known about a particular individual. It may also be possible to ascertain the identity of individuals from aggregated data where there are very few individuals in a particular category. Identifiability is dependent on the amount of information held and also on the skills and technology of the holder." [] {http://purl.obolibrary.org/obo/IAO_0000119="CASRAI. https://casrai.org/term/personally-identifiable-information"}
is_a: T4FS:0000127 ! personal information privacy
property_value: IAO:0000117 "https://orcid.org/0000-0002-7702-4495" xsd:string
property_value: IAO:0000117 "Peter McQuilton" xsd:string

[Term]
id: T4FS:0000223
name: understand storage security challanges
def: "Understand the current storage security status and the preferred status, as well as the barriers between them." []
is_a: T4FS:0000470 ! storage security management
property_value: IAO:0000117 "Angus Whyte" xsd:string
property_value: IAO:0000117 "Celia van Gelder" xsd:string
property_value: IAO:0000117 "Mateusz Kuzak" xsd:string
property_value: IAO:0000117 "Yan Wang" xsd:string

[Term]
id: T4FS:0000224
name: normalization
def: "The process of organizing data into tables in such a way that the results of using the database are always unambiguous and as intended. Normalization is typically a refinement process after the initial exercise of identifying the data objects that should be in the database, identifying their relationships, and defining the tables required and the columns within each table." [] {http://purl.obolibrary.org/obo/IAO_0000119="CASRAI. https://casrai.org/term/normalization/"}
is_a: T4FS:0000372 ! data stewardship technical concept
property_value: IAO:0000117 "https://orcid.org/0000-0002-7702-4495" xsd:string
property_value: IAO:0000117 "Peter McQuilton" xsd:string

[Term]
id: T4FS:0000225
name: evaluation
def: "Evaluation is a decision about significance, value, or quality of something, based on careful study of its good and bad features." [] {http://purl.obolibrary.org/obo/IAO_0000119="CASRAI. https://casrai.org/term/evaluation/"}
comment: AL 17.3.22: We may wish to make this an alternative term of Assessment.
is_a: T4FS:0000126 ! assessment
property_value: IAO:0000117 "https://orcid.org/0000-0002-7702-4495" xsd:string
property_value: IAO:0000117 "Peter McQuilton" xsd:string

[Term]
id: T4FS:0000226
name: data item
def: "A type of data element that expresses a proposition that binds one or more property values to some data entity." [] {http://purl.obolibrary.org/obo/IAO_0000119="CASRAI. https://casrai.org/term/data-item/"}
is_a: T4FS:0000372 ! data stewardship technical concept
property_value: IAO:0000117 "Peter McQuilton" xsd:string

[Term]
id: T4FS:0000227
name: confidentiality
def: "The duties and practices of people and organizations to ensure that individual's personal information only flows from one entity to another according to legislated or otherwise broadly accepted norms and policies." [] {http://purl.obolibrary.org/obo/IAO_0000119="CASRAI. https://casrai.org/term/confidentiality/"}
is_a: T4FS:0000372 ! data stewardship technical concept
property_value: IAO:0000117 "Peter McQuilton" xsd:string

[Term]
id: T4FS:0000228
name: knowledge of data management costs management
def: "Bin for types of Knowledge needed for Data management costs management." []
is_a: T4FS:0000232 ! data management costs management
property_value: IAO:0000117 "leightonlc" xsd:string

[Term]
id: T4FS:0000229
name: logistical support
is_a: T4FS:0000320 ! project management activities
property_value: IAO:0000117 "https://orcid.org/0000-0002-7702-4495" xsd:string
property_value: IAO:0000117 "Peter McQuilton" xsd:string
property_value: IAO:0000117 "Philippe Rocca-Serra" xsd:string
property_value: IAO:0000117 "Susanna Sansone" xsd:string

[Term]
id: T4FS:0000230
name: aptitudes for data management costs management
def: "Bin for Aptitudes related to Data management costs management." []
is_a: T4FS:0000232 ! data management costs management
property_value: IAO:0000117 "leightonlc" xsd:string

[Term]
id: T4FS:0000231
name: data acquisition
def: "The process of acquiring data from some source. For example, data may be acquired by download from a repository, transfer from a data logger, data capture, etc." [] {http://purl.obolibrary.org/obo/IAO_0000119="CASRAI. https://casrai.org/term/data-acquisition/"}
comment: AL 15.3.22: Removed "data and metadata capture" as was too similar to this term. Added alternative term "data capture".
is_a: T4FS:0000012 ! data stewardship activity
property_value: IAO:0000117 "https://orcid.org/0000-0002-7702-4495" xsd:string
property_value: IAO:0000117 "Peter McQuilton" xsd:string
property_value: IAO:0000118 "Data capture" xsd:string

[Term]
id: T4FS:0000232
name: data management costs management
def: "Planning for and controlling expenditures related to the data management lifecycle, including, but not limited to, labor and infrastructure expenses for data collection; data documentation; data storage; data access and security; data preservation; data sharing; and data disposition." [] {http://purl.obolibrary.org/obo/IAO_0000119="Written by LLC, based on list at https://www.uu.nl/en/research/research-data-management/guides/costs-of-data-management"}
is_a: T4FS:0000353 ! resource management
property_value: IAO:0000117 "Kristina Hettne" xsd:string
property_value: IAO:0000117 "Simon Hodson" xsd:string
property_value: IAO:0000117 "Victoria Dominguez Del Angel" xsd:string

[Term]
id: T4FS:0000233
name: text file
def: "A Text file is a kind of computer file that is structured as a sequence of lines of electronic text. A text file exists stored as data within a computer file system." [] {http://purl.obolibrary.org/obo/IAO_0000119="AL, Adapted from Wikipedia. https://en.wikipedia.org/wiki/Text_file"}
comment: AL 9.3.22: The CASRAI term (https://casrai.org/term/text-file) had an unsuitable definition, and therefore was removed.
is_a: T4FS:0000372 ! data stewardship technical concept
relationship: T4FS:0000563 T4FS:0000137 ! contributes to the implementation of I1. (meta)data use a formal, accessible, shared, and broadly applicable language for knowledge representation
property_value: IAO:0000117 "https://orcid.org/0000-0002-7702-4495" xsd:string
property_value: IAO:0000117 "Peter McQuilton" xsd:string

[Term]
id: T4FS:0000236
name: human-readable format
def: "Data and code that are commented so that humans can understand what it represents, it's design, and purpose.REFERENCE. Wilson G, Aruliah DA, Brown CT, Hong NPC, Davis M, Guy RT, Haddock SHD, Huff K, Mitchell IM, Plumbley MD, Waugh B, White EP, Wilson P (2012). Best practices for scientific computing , arXiv, 29 November, 1-6." [] {http://purl.obolibrary.org/obo/IAO_0000119="CASRAI. https://casrai.org/term/human-readable-format/"}
is_a: T4FS:0000372 ! data stewardship technical concept
relationship: T4FS:0000563 T4FS:0000137 ! contributes to the implementation of I1. (meta)data use a formal, accessible, shared, and broadly applicable language for knowledge representation
property_value: IAO:0000117 "Peter McQuilton" xsd:string

[Term]
id: T4FS:0000238
name: data validation
def: "Provides well-defined guarantees for fitness, accuracy, and consistency for any of various kinds of user input into an application or automated system. Data validation checks that data are valid, sensible, reasonable, clean, usable, and secure before they are processed. Failures or omissions in data validation can lead to data corruption, security vulnerability. Improperly validated data &hellip; <a href=CASRAI. https://casrai.org/term/data-validation/ class=more-link" [] {http://purl.obolibrary.org/obo/IAO_0000119="CASRAI. https://casrai.org/term/data-validation/"}
is_a: T4FS:0000036 ! curation
property_value: IAO:0000117 "Peter McQuilton" xsd:string

[Term]
id: T4FS:0000239
name: pid record
def: "A type of record (and organization) that stores an instance of an executable/understandable PID. The content of a PID record distinguishes a registered digital or data object from other DOs. A PID record is a type of record that includes property information that characterizes the digital object it is identifying. Important parts of a PID record are location and checksum. However there is a large variation in usage. In some data models the PID is simply used as a unique label with an empty record. A PID record has a lifecycle including creation, publication, Curation and the destruction." [] {http://purl.obolibrary.org/obo/IAO_0000119="CASRAI, https://casrai.org/term/pid-record/"}
is_a: T4FS:0000453 ! persistent identifier
property_value: IAO:0000117 "https://orcid.org/0000-0002-7702-4495" xsd:string
property_value: IAO:0000117 "Peter McQuilton" xsd:string

[Term]
id: T4FS:0000240
name: appreciate importance of research integrity
def: "Take proactive approach to ensure outputs are made FAIR consistently with research integrity principles." []
is_a: T4FS:0000525 ! research integrity, attribution, impact awareness
property_value: IAO:0000117 "Angus Whyte" xsd:string
property_value: IAO:0000117 "Celia van Gelder" xsd:string
property_value: IAO:0000117 "Mateusz Kuzak" xsd:string
property_value: IAO:0000117 "Yan Wang" xsd:string

[Term]
id: T4FS:0000241
name: structural metadata
def: "A type of metadata that indicates how compound objects are put together (e.g., how pages are ordered to form chapters; how data are organized in a table; how datasets are organized in a collection) 2. The underlying structural metadata of digital objects that tells computers how to assemble them." [] {http://purl.obolibrary.org/obo/IAO_0000119="CASRAI. https://casrai.org/term/structural-metadata/"}
is_a: T4FS:0000527 ! metadata
property_value: IAO:0000117 "https://orcid.org/0000-0002-7702-4495" xsd:string
property_value: IAO:0000117 "Peter McQuilton" xsd:string

[Term]
id: T4FS:0000244
name: non personally identifiable information
def: "Data that could not lead to the identification of a specific individual, to distinguishing one person from another, or to personally identifiable information. These may be data that have been de-identified, or that could not lead to personally identifiable information in the first place." [] {http://purl.obolibrary.org/obo/IAO_0000119="CASRAI. https://casrai.org/term/non-personally-identifiable-information/"}
is_a: T4FS:0000372 ! data stewardship technical concept
property_value: IAO:0000117 "https://orcid.org/0000-0002-7702-4495" xsd:string
property_value: IAO:0000117 "Peter McQuilton" xsd:string

[Term]
id: T4FS:0000245
name: digitisation
def: "The process of creating digital files by scanning or otherwise converting analogue materials. The resulting digital copy, or digital surrogate, would then be classed as digital material and then subject to the same broad challenges involved in preserving access to it, as born digital materials." [] {http://purl.obolibrary.org/obo/IAO_0000119="CASRAI. https://casrai.org/term/digitisation/ REFERENCE. Digital preservation coalitionhttp://www.dpconline.org/advice/preservationhandbook/introduction/definitions-and-concepts"}
is_a: T4FS:0000036 ! curation
property_value: IAO:0000117 "https://orcid.org/0000-0002-7702-4495" xsd:string
property_value: IAO:0000117 "Peter McQuilton" xsd:string

[Term]
id: T4FS:0000247
name: data publication
def: "The release of research data, associated metadata, accompanying documentation, and software code (in cases where the raw data have been processed or manipulated) for re-use and analysis in such a manner that they can be discovered on the Web and referred to in a unique and persistent way. Data publishing occurs via dedicated data repositories..." [] {http://purl.obolibrary.org/obo/IAO_0000119="CASRAI. https://casrai.org/term/data-publication/"}
is_a: T4FS:0000021 ! exposing data
property_value: IAO:0000117 "Peter McQuilton" xsd:string

[Term]
id: T4FS:0000248
name: findability of digital assets
is_a: T4FS:0000447 ! fair principle
property_value: IAO:0000117 "Peter McQuilton" xsd:string

[Term]
id: T4FS:0000249
name: community building
comment: AL 9.3.22: renamed to prevent compound term. Was 'Influencing/community building'
is_a: T4FS:0000320 ! project management activities
property_value: IAO:0000117 "https://orcid.org/0000-0002-7702-4495" xsd:string
property_value: IAO:0000117 "Peter McQuilton" xsd:string
property_value: IAO:0000117 "Philippe Rocca-Serra" xsd:string
property_value: IAO:0000117 "Susanna Sansone" xsd:string

[Term]
id: T4FS:0000250
name: citable data
def: "A type of referable data that has undergone quality assessment and can be referred to as citations in publications and as part of research objects." [] {http://purl.obolibrary.org/obo/IAO_0000119="CASRAI. https://casrai.org/term/citable-data/"}
is_a: T4FS:0000430 ! data
relationship: T4FS:0000563 T4FS:0000512 ! contributes to the implementation of F1. (meta)data are assigned a globally unique and persistent identifier
property_value: IAO:0000117 "Peter McQuilton" xsd:string

[Term]
id: T4FS:0000251
name: big data
def: "An evolving term that describes any voluminous amount of structured, semi-structured and unstructured data that have the potential to be mined for information." [] {http://purl.obolibrary.org/obo/IAO_0000119="CASRAI. https://casrai.org/term/big-data/"}
is_a: T4FS:0000430 ! data
property_value: IAO:0000117 "Peter McQuilton" xsd:string

[Term]
id: T4FS:0000252
name: fairness assessment
def: "Ability to apply knowledge about FAIR metrics and assessing FAIRness using FAIR assessment tools." []
is_a: T4FS:0000126 ! assessment
property_value: IAO:0000117 "Kristina Hettne" xsd:string
property_value: IAO:0000117 "Victoria Dominguez Del Angel" xsd:string
property_value: IAO:0000117 "Yann Le Franc" xsd:string

[Term]
id: T4FS:0000254
name: data archive
def: "An archival service providing the long-term permanent care and accessibility for digital objects with research value." [] {http://purl.obolibrary.org/obo/IAO_0000119="CASRAI. https://casrai.org/term/data-archive/"}
is_a: T4FS:0000372 ! data stewardship technical concept
property_value: IAO:0000117 "Peter McQuilton" xsd:string

[Term]
id: T4FS:0000255
name: technical metadata
def: "Describes the technical processes used to produce, or required to use a digital object." [] {http://purl.obolibrary.org/obo/IAO_0000119="CASRAI. https://casrai.org/term/technical-metadata/"}
is_a: T4FS:0000527 ! metadata
property_value: IAO:0000117 "https://orcid.org/0000-0002-7702-4495" xsd:string
property_value: IAO:0000117 "Peter McQuilton" xsd:string

[Term]
id: T4FS:0000256
name: machine readable
def: "OBSOLETE. In a form that can be used and understood by a computer." [] {http://purl.obolibrary.org/obo/IAO_0000119="CASRAI. https://casrai.org/term/machine-readable/"}
comment: AL 5.12.22: Deprecated because of its similarity with http://purl.obolibrary.org/obo/T4FS_0000551. We don't need to be going to the level of granularity that the concept of machine readability needs to be modelled as well as machine readable format.
property_value: IAO:0000117 "https://orcid.org/0000-0002-7702-4495" xsd:string
property_value: IAO:0000117 "Peter McQuilton" xsd:string
is_obsolete: true

[Term]
id: T4FS:0000257
name: integrated access management
def: "A combination of business processes, policies and technologies that allows organizations to provide secure access to confidential data. Integrated access management software is used by enterprises to control the flow of sensitive data in and out of the network." [] {http://purl.obolibrary.org/obo/IAO_0000119="CASRAI. https://casrai.org/term/integrated-access-management/"}
is_a: T4FS:0000012 ! data stewardship activity
property_value: IAO:0000117 "https://orcid.org/0000-0002-7702-4495" xsd:string
property_value: IAO:0000117 "Peter McQuilton" xsd:string

[Term]
id: T4FS:0000258
name: noisy data
def: "Meaningless data, including: Any data that cannot be understood and interpreted correctly by machines, such as unstructured text; any data that has been received, stored, or changed in such a manner that it cannot be read or used by the program that originally created it." [] {http://purl.obolibrary.org/obo/IAO_0000119="CASRAI. https://casrai.org/term/noisy-data/"}
is_a: T4FS:0000430 ! data
property_value: IAO:0000117 "https://orcid.org/0000-0002-7702-4495" xsd:string
property_value: IAO:0000117 "Peter McQuilton" xsd:string

[Term]
id: T4FS:0000259
name: fair training
def: "Activities in and around the provision of training, mentorship and teaching opportunities for good data management and the implementation of FAIR practices." [] {http://purl.obolibrary.org/obo/IAO_0000119="PMQ"}
is_a: T4FS:0000012 ! data stewardship activity
property_value: IAO:0000117 "https://orcid.org/0000-0002-7702-4495" xsd:string
property_value: IAO:0000117 "Peter McQuilton" xsd:string
property_value: IAO:0000117 "Philippe Rocca-Serra" xsd:string
property_value: IAO:0000117 "Susanna Sansone" xsd:string

[Term]
id: T4FS:0000260
name: software
def: "A set of instructions that direct a computer to do a specific task." [] {http://purl.obolibrary.org/obo/IAO_0000119="CASRAI. https://casrai.org/term/software"}
is_a: T4FS:0000372 ! data stewardship technical concept
property_value: IAO:0000117 "https://orcid.org/0000-0002-7702-4495" xsd:string
property_value: IAO:0000117 "Peter McQuilton" xsd:string

[Term]
id: T4FS:0000263
name: data standardization
def: "In the context of data analysis and data mining: Where V represents the value of the variable in the original datasets: Transformation of data to have zero mean and unit variance. Techniques used include: (a) Data normalization; (b) z-score scaling; (c) Dividing each value by the range: recalculates each variable as V /(max V - ..." [] {http://purl.obolibrary.org/obo/IAO_0000119="CASRAI. https://casrai.org/term/data-standardization/"}
is_a: T4FS:0000372 ! data stewardship technical concept
property_value: IAO:0000117 "Peter McQuilton" xsd:string

[Term]
id: T4FS:0000264
name: open data
def: "Strutured data that are accessible, machine-readable, usable, intelligible, and freely shared. Open data can be freely used, re-used, built on, and redistributed by anyone - subject only, at most, to the requirement to attribute and sharealike." [] {http://purl.obolibrary.org/obo/IAO_0000119="CASRAI. https://casrai.org/term/open-data/"}
is_a: T4FS:0000430 ! data
property_value: IAO:0000117 "https://orcid.org/0000-0002-7702-4495" xsd:string
property_value: IAO:0000117 "Peter McQuilton" xsd:string

[Term]
id: T4FS:0000265
name: curated data
def: "The output of a data curation activity. Such data has generally already been cleaned, standardised, documented. Additional metadata relevant to the data object has also been added, via either manual or automatic methods." [] {http://purl.obolibrary.org/obo/IAO_0000119="AL 9.5.22"}
comment: AL 9.5.22: The orginal label ("data curation") matched a term within the Data stewardship activity hierarchy. Changing the class label to "Curated data" better fit the model.
is_a: T4FS:0000430 ! data
relationship: T4FS:0000563 T4FS:0000174 ! contributes to the implementation of R1. (meta)data are richly described with a plurality of accurate and relevant attributes
relationship: T4FS:0000563 T4FS:0000361 ! contributes to the implementation of I2. (meta)data use vocabularies that follow fair principles
relationship: T4FS:0000563 T4FS:0000435 ! contributes to the implementation of F3. metadata clearly and explicitly include the identifier of the data they describe
property_value: IAO:0000117 "https://orcid.org/0000-0002-7702-4495" xsd:string
property_value: IAO:0000117 "Peter McQuilton" xsd:string
created_by: Peter McQuilton

[Term]
id: T4FS:0000267
name: skills related to funding acquisition management
def: "Bin for Skills needed for Funding acquisition management." []
is_a: T4FS:0000426 ! funding acquisition management
property_value: IAO:0000117 "leightonlc" xsd:string

[Term]
id: T4FS:0000268
name: universally unique identifier
def: "A 128-bit number used to guarantee unique identity for different objects on the internet over time. File system partitions." [] {http://purl.obolibrary.org/obo/IAO_0000119="CASRAI. https://casrai.org/term/universally-unique-identifier/"}
is_a: T4FS:0000529 ! identifier
property_value: IAO:0000117 "https://orcid.org/0000-0002-7702-4495" xsd:string
property_value: IAO:0000117 "Peter McQuilton" xsd:string
property_value: IAO:0000118 "UUID" xsd:string

[Term]
id: T4FS:0000270
name: authentication
def: "The process of confirming the identity of a principal entity." [] {http://purl.obolibrary.org/obo/IAO_0000119="CASRAI. https://casrai.org/term/authentication/"}
is_a: T4FS:0000107 ! information security
property_value: IAO:0000117 "Peter McQuilton" xsd:string

[Term]
id: T4FS:0000271
name: cloud computing
def: "A large-scale distributed computing paradigm that is driven by economies of scale, in which a pool of abstracted, virtualized, dynamically- scalable, managed computing power, storage, platforms and services are delivered on demand to external customers over the Internet." [] {http://purl.obolibrary.org/obo/IAO_0000119="CASRAI. https://casrai.org/term/cloud-computing/"}
is_a: T4FS:0000372 ! data stewardship technical concept
property_value: IAO:0000117 "Peter McQuilton" xsd:string

[Term]
id: T4FS:0000273
name: short-term preservation
def: "Short-term preservation. Access to digital materials either for a defined period of time while use is predicted but which does not extend beyond the foreseeable future and/or until it becomes inaccessible because of changes in technology." [] {http://purl.obolibrary.org/obo/IAO_0000119="CASRAI. https://casrai.org/term/short-term-preservation"}
is_a: T4FS:0000372 ! data stewardship technical concept
property_value: IAO:0000117 "https://orcid.org/0000-0002-7702-4495" xsd:string
property_value: IAO:0000117 "Peter McQuilton" xsd:string

[Term]
id: T4FS:0000274
name: international standard
def: "A standard that is used in multiple nations and whose development process is open to representatives from all countries." [] {http://purl.obolibrary.org/obo/IAO_0000119="CASRAI. https://casrai.org/term/international-standard/"}
is_a: T4FS:0000372 ! data stewardship technical concept
relationship: T4FS:0000563 T4FS:0000137 ! contributes to the implementation of I1. (meta)data use a formal, accessible, shared, and broadly applicable language for knowledge representation
property_value: IAO:0000117 "Peter McQuilton" xsd:string

[Term]
id: T4FS:0000275
name: conformance
def: "The state of having satisfied the requirements of some specific standard(s) and/or specification(s)." [] {http://purl.obolibrary.org/obo/IAO_0000119="CASRAI. https://casrai.org/term/conformance/"}
is_a: T4FS:0000372 ! data stewardship technical concept
property_value: IAO:0000117 "Peter McQuilton" xsd:string

[Term]
id: T4FS:0000276
name: data custodian
def: "A data custodian is an IT individual or organization responsible for the IT infrastructure providing and protecting data in conformance with the policies and practices prescribed by data governance." [] {http://purl.obolibrary.org/obo/IAO_0000119="CASRAI. https://casrai.org/term/data-custodian/"}
relationship: T4FS:0000558 T4FS:0000012 ! has/wants competency in data stewardship activity
relationship: T4FS:0000559 T4FS:0000372 ! has/wants knowledge about data stewardship technical concept
relationship: T4FS:0000559 T4FS:0000446 ! has/wants knowledge about data stewardship guideline
relationship: T4FS:0000561 T4FS:0000372 ! has/wants practical skill about data stewardship technical concept
relationship: T4FS:0000562 T4FS:0000548 ! has aptitude for data stewardship soft skill
property_value: IAO:0000117 "Peter McQuilton" xsd:string

[Term]
id: T4FS:0000277
name: aptitudes for high performance computing management
def: "Bin for Aptitudes related to High performance computing management." []
is_a: T4FS:0000308 ! high performance computing management
property_value: IAO:0000117 "leightonlc" xsd:string

[Term]
id: T4FS:0000278
name: manage datasets in a repository
def: "Implement the policies that govern the arrangement, naming, descriptive metadata, provenance metadata, representation metadata, administrative metadata, access controls, retention, disposition, integrity, and replication of digital objects." [] {http://purl.obolibrary.org/obo/IAO_0000119="CASRAI. https://casrai.org/term/manage-datasets-in-a-repository"}
is_a: T4FS:0000141 ! data management
property_value: IAO:0000117 "https://orcid.org/0000-0002-7702-4495" xsd:string
property_value: IAO:0000117 "Peter McQuilton" xsd:string

[Term]
id: T4FS:0000280
name: data de-noising
def: "Removing noise from data." [] {http://purl.obolibrary.org/obo/IAO_0000119="CASRAI. https://casrai.org/term/data-de-noising/"}
is_a: T4FS:0000036 ! curation
property_value: IAO:0000117 "Peter McQuilton" xsd:string

[Term]
id: T4FS:0000282
name: governance and accountability model
def: "Provides the relationship and process context for working together to ensure outcomes are achieved." [] {http://purl.obolibrary.org/obo/IAO_0000119="CASRAI. https://casrai.org/term/governance-and-accountability-model"}
is_a: T4FS:0000372 ! data stewardship technical concept
property_value: IAO:0000117 "https://orcid.org/0000-0002-7702-4495" xsd:string
property_value: IAO:0000117 "Peter McQuilton" xsd:string

[Term]
id: T4FS:0000283
name: access
def: "The continued, available for use, ongoing usability of a digital resource, retaining all qualities of authenticity, accuracy and functionality deemed to be essential for the purposes the digital material was created and/or acquired for. Users who have access can retrieve, manipulate, copy, and store copies on a wide range of hard drives and external devices." [] {http://purl.obolibrary.org/obo/IAO_0000119="CASRAI. https://casrai.org/term/access"}
is_a: T4FS:0000372 ! data stewardship technical concept
property_value: IAO:0000117 "Peter McQuilton" xsd:string

[Term]
id: T4FS:0000285
name: develop fair and open research strategy
def: "Find the people with a good understand of FAIR and open research challenges in your organiation, and create a work agenda." []
is_a: T4FS:0000008 ! develop open research strategy and vision
property_value: IAO:0000117 "Angus Whyte" xsd:string
property_value: IAO:0000117 "Celia van Gelder" xsd:string
property_value: IAO:0000117 "Mateusz Kuzak" xsd:string
property_value: IAO:0000117 "Yan Wang" xsd:string

[Term]
id: T4FS:0000286
name: patent application
def: "Choose the proper type of patent for the project data and apply for the patent chosen." []
is_a: T4FS:0000042 ! ethical application of patents, licenses
property_value: IAO:0000117 "Celia van Gelder" xsd:string
property_value: IAO:0000117 "Mateusz Kuzak" xsd:string
property_value: IAO:0000117 "Yan Wang" xsd:string

[Term]
id: T4FS:0000287
name: collection management identification
def: "A type of data provenance that adds metadata to identify data collections." [] {http://purl.obolibrary.org/obo/IAO_0000119="CASRAI. https://casrai.org/term/collection-management-identification/"}
is_a: T4FS:0000372 ! data stewardship technical concept
property_value: IAO:0000117 "Peter McQuilton" xsd:string

[Term]
id: T4FS:0000288
name: assess fairness
def: "Activity/Process whereby digital objects are evaluated with the relevant FAIR metrics and assessment tools." [] {http://purl.obolibrary.org/obo/IAO_0000119="[YLF, VDA, KH]"}
is_a: T4FS:0000126 ! assessment
property_value: IAO:0000117 "Kristina Hettne" xsd:string
property_value: IAO:0000117 "Victoria Dominguez Del Angel" xsd:string
property_value: IAO:0000117 "Yann Le Franc" xsd:string

[Term]
id: T4FS:0000289
name: knowledge of change management
def: "Bin for types of Knowledge related to Change management." []
is_a: T4FS:0000411 ! change management
property_value: IAO:0000117 "leightonlc" xsd:string

[Term]
id: T4FS:0000290
name: data ingestion
def: "The process of obtaining, importing, and processing data for later use or storage in a database. This process often involves altering individual files by editing their content and/or formatting them to fit into a larger document." [] {http://purl.obolibrary.org/obo/IAO_0000119="CASRAI. https://casrai.org/term/data-ingestion/"}
is_a: T4FS:0000231 ! data acquisition
property_value: IAO:0000117 "Peter McQuilton" xsd:string

[Term]
id: T4FS:0000291
name: data wrangling
def: "The process of manually or semi-automatically converting or mapping data from one form into another format that allows for more convenient consumption of the data with the help of semi-automated tools. Gathering and organizing disparate data from different sources, often collected by many different investigators. Activities include developing and supporting search tools that utilize standardized &hellip; <a href=CASRAI. https://casrai.org/term/data-wrangling/ class=more-link" [] {http://purl.obolibrary.org/obo/IAO_0000119="CASRAI. https://casrai.org/term/data-wrangling/"}
is_a: T4FS:0000036 ! curation
property_value: IAO:0000117 "Peter McQuilton" xsd:string

[Term]
id: T4FS:0000292
name: research data management infrastructure
def: "The configuration of staff, services and tools assembled to support data management across the research lifecycle and more specifically to provide comprehensive coverage of the stages making up the data lifecycle. It can be organized locally and/or globally to support research data activities across the research lifecycle." [] {http://purl.obolibrary.org/obo/IAO_0000119="CASRAI. https://casrai.org/term/research-data-management-infrastructure"}
is_a: T4FS:0000372 ! data stewardship technical concept
property_value: IAO:0000117 "https://orcid.org/0000-0002-7702-4495" xsd:string
property_value: IAO:0000117 "Peter McQuilton" xsd:string

[Term]
id: T4FS:0000293
name: flexibility in relating fair criteria to openness
def: "Appreciate the need for flexibility in applying FAIR criteria to make data as open as possible, as closed as necessary." []
is_a: T4FS:0000259 ! fair training
property_value: IAO:0000117 "Angus Whyte" xsd:string

[Term]
id: T4FS:0000294
name: choosing the appropriate terminology for your data
def: "To be able to research and identify the appropriate taxonomy for your project. This may involve using resources such as FAIRsharing, which captures metadata on taxonomies and provides an assessment of their FAIRness." [] {http://purl.obolibrary.org/obo/IAO_0000119="[PMQ]"}
is_a: T4FS:0000175 ! fair evaluation of repositories for data deposition
property_value: IAO:0000117 "Peter McQuilton" xsd:string
property_value: IAO:0000118 "Controlled Vocabulary identification" xsd:string
property_value: IAO:0000118 "Ontology identification" xsd:string
property_value: IAO:0000118 "Taxonomy identification" xsd:string
property_value: IAO:0000118 "Thesaurus identification" xsd:string

[Term]
id: T4FS:0000295
name: structured data
def: "Data whose elements have been organized into a consistent format and data structure within a defined data model such that the elements can be easily addressed, organized and accessed in various combinations to make better use of the information, such as in a relational database." [] {http://purl.obolibrary.org/obo/IAO_0000119="CASRAI. https://casrai.org/term/structured-data/"}
is_a: T4FS:0000430 ! data
property_value: IAO:0000117 "https://orcid.org/0000-0002-7702-4495" xsd:string
property_value: IAO:0000117 "Peter McQuilton" xsd:string

[Term]
id: T4FS:0000296
name: knowledge to contextualise fair principles to domain
def: "Know how data handling practices in the domain make FAIR criteria more or less easy to implement." []
is_a: T4FS:0000259 ! fair training
property_value: IAO:0000117 "Angus Whyte" xsd:string

[Term]
id: T4FS:0000297
name: research data management
def: "Data Management refers to the storage, access and preservation of data produced from a given investigation. Data management practices cover the entire lifecycle of the data, from planning the investigation to conducting it, and from backing up data as it is created and used to long term preservation of data deliverables after the research investigation has concluded. Specific activities and issues that fall within the category of data management include: File naming (the proper way to name computer files); data quality control and quality assurance; data access; data documentation (including levels of uncertainty); metadata creation and controlled vocabularies; data storage; data archiving and preservation; data sharing and reuse; data integrity; data security; data privacy; data rights; notebook protocols (lab or field)." [] {http://purl.obolibrary.org/obo/IAO_0000119="CASRAI. https://casrai.org/term/research-data-management/"}
is_a: T4FS:0000141 ! data management
property_value: IAO:0000117 "https://orcid.org/0000-0002-7702-4495" xsd:string
property_value: IAO:0000117 "Peter McQuilton" xsd:string

[Term]
id: T4FS:0000298
name: publish output in a repository
def: "Deposit research output (software, data and publication together with documentation) in  previousy selected repositories." []
is_a: T4FS:0000106 ! publish data
property_value: IAO:0000117 "Celia van Gelder" xsd:string
property_value: IAO:0000117 "Mateusz Kuzak" xsd:string
property_value: IAO:0000117 "Yan Wang" xsd:string

[Term]
id: T4FS:0000300
name: metadata search via metadata providers
def: "To be able to identify and process metadata over the internet, sourced from a variety of metadata providers and schemata." [] {http://purl.obolibrary.org/obo/IAO_0000119="[PMQ]"}
is_a: T4FS:0000076 ! data discovery
property_value: IAO:0000117 "Peter McQuilton" xsd:string
property_value: IAO:0000118 "Metadata processing" xsd:string
property_value: IAO:0000118 "Metadata search" xsd:string

[Term]
id: T4FS:0000301
name: record provenance information
def: "Information for a data object that includes: * the person who deposited the data object in the repository, * the source of the data object, * the date when the object was deposited, and * authenticity information needed to link the data object to its original source." [] {http://purl.obolibrary.org/obo/IAO_0000119="CASRAI. https://casrai.org/term/record-provenance-information/"}
is_a: T4FS:0000527 ! metadata
property_value: IAO:0000117 "https://orcid.org/0000-0002-7702-4495" xsd:string
property_value: IAO:0000117 "Peter McQuilton" xsd:string

[Term]
id: T4FS:0000302
name: data citation
def: "Offers proper recognition to authors as well as permanent identification through the use of global persistent identifiers in place of URLs which can change frequently." [] {http://purl.obolibrary.org/obo/IAO_0000119="CASRAI. https://casrai.org/term/data-citation/"}
is_a: T4FS:0000021 ! exposing data
property_value: IAO:0000117 "Peter McQuilton" xsd:string

[Term]
id: T4FS:0000305
name: book
is_a: T4FS:0000519 ! learning medium
property_value: IAO:0000117 "Peter McQuilton" xsd:string
created_by: Peter McQuilton
creation_date: 2020-10-01T20:54:08.535183Z

[Term]
id: T4FS:0000306
name: intellectual leadership
def: "The capacity to influence stakeholders and the direction of research activities; the ability to shape others' understanding in ways that capture interest, inform and gain support; and, the capacity to influence the actions and opinions of others." [] {http://purl.obolibrary.org/obo/IAO_0000119="CASRAI. https://casrai.org/term/intellectual-leadership/"}
is_a: T4FS:0000548 ! data stewardship soft skill
property_value: IAO:0000117 "https://orcid.org/0000-0002-7702-4495" xsd:string
property_value: IAO:0000117 "Peter McQuilton" xsd:string

[Term]
id: T4FS:0000307
name: innovation
def: "In the context of a researcher's activities, innovation is the development of modified or novel approaches, theories, concepts, ideas or solutions. Innovation is one of four valued outcomes." [] {http://purl.obolibrary.org/obo/IAO_0000119="CASRAI. https://casrai.org/term/innovation/"}
is_a: T4FS:0000012 ! data stewardship activity
property_value: IAO:0000117 "https://orcid.org/0000-0002-7702-4495" xsd:string
property_value: IAO:0000117 "Peter McQuilton" xsd:string

[Term]
id: T4FS:0000308
name: high performance computing management
def: "High-performance computing (HPC) is a process for using of super computers and parallel processing techniques for solving complex computational problems. HPC technology focuses on developing parallel processing algorithms and systems by incorporating both administration and parallel computational techniques." [] {http://purl.obolibrary.org/obo/IAO_0000119="(modified from wikipedia)[VDA]"}
is_a: T4FS:0000353 ! resource management
property_value: IAO:0000117 "Kristina Hettne" xsd:string
property_value: IAO:0000117 "Simon Hodson" xsd:string
property_value: IAO:0000117 "Victoria Dominguez Del Angel" xsd:string
property_value: IAO:0000118 "HPC management" xsd:string

[Term]
id: T4FS:0000309
name: provenance
def: "A type of historical information or metadata about the origin, location or the source of something, or the history of the ownership or location of an object or resource including digital objects. For example, information about the Principal Investigator who recorded the data, and the information concerning its storage, handling, and migration." [] {http://purl.obolibrary.org/obo/IAO_0000119="CASRAI. https://casrai.org/term/provenance"}
is_a: T4FS:0000372 ! data stewardship technical concept
relationship: T4FS:0000563 T4FS:0000014 ! contributes to the implementation of interoperability of digital assets
property_value: IAO:0000117 "https://orcid.org/0000-0002-7702-4495" xsd:string
property_value: IAO:0000117 "Peter McQuilton" xsd:string

[Term]
id: T4FS:0000310
name: digital record
def: "A record created digitally in the day-to-day business of the organisation and assigned formal status by the organisation. Examples include: word processing documents, emails, databases, or intranet web pages." [] {http://purl.obolibrary.org/obo/IAO_0000119="CASRAI. https://casrai.org/term/digital/"}
comment: AL 8.2.22: Updated label from the CASRAI "Digital" to "Digital record" to better match the definition and intent of the term, and to provide clarity.
is_a: T4FS:0000372 ! data stewardship technical concept
property_value: IAO:0000117 "https://orcid.org/0000-0002-7702-4495" xsd:string
property_value: IAO:0000117 "Peter McQuilton" xsd:string
property_value: IAO:0000118 "Electronic record" xsd:string

[Term]
id: T4FS:0000311
name: analytical quality control
def: "Processes and procedures designed to ensure that the results of laboratory analysis are consistent, comparable, accurate and within specified limits of precision." [] {http://purl.obolibrary.org/obo/IAO_0000119="CASRAI. https://casrai.org/term/analytical-quality-control/"}
is_a: T4FS:0000372 ! data stewardship technical concept
property_value: IAO:0000117 "Peter McQuilton" xsd:string

[Term]
id: T4FS:0000312
name: digital research data
def: "Research data which is in digital form. It may have been originally created in digital form, or it may have been converted from paper, or other form to a digital representation." [] {http://purl.obolibrary.org/obo/IAO_0000119="CASRAI. https://casrai.org/term/digital-research-data/"}
is_a: T4FS:0000430 ! data
property_value: IAO:0000117 "https://orcid.org/0000-0002-7702-4495" xsd:string
property_value: IAO:0000117 "Peter McQuilton" xsd:string

[Term]
id: T4FS:0000314
name: managing research
def: "In the context of a researcher’s activities, Managing research is the processes related to the planning, organizing, setting objectives, controlling and evaluating of RDA activities and their associated human and financial resources. It includes the provision of leadership to, and assessment of, other scientists, engineers, technologists, and/or other staff. Managing research is one of the three research contexts in which a researcher is expected to conduct his/her activities. Managing research is distinct from the position-based role of a research manager." [] {http://purl.obolibrary.org/obo/IAO_0000119="CASRAI. https://casrai.org/term/managing-research/"}
is_a: T4FS:0000012 ! data stewardship activity
property_value: IAO:0000117 "https://orcid.org/0000-0002-7702-4495" xsd:string
property_value: IAO:0000117 "Peter McQuilton" xsd:string

[Term]
id: T4FS:0000315
name: evaluation of how to publish your data
def: "To be able to define and deploy appropriate criteria, based on the FAIR principles, to identify the appropriate publishing platform for a dataset. This may, for example, involve discovering the mark-up of the platform, the exchange formats and data models used, and the licensing information for each repository. Tools such as the FAIR evaluator or FAIRshake may be used to assess the FAIRnessbased on human-entered questionnaires or FAIRsharing resource metadata." [] {http://purl.obolibrary.org/obo/IAO_0000119="[PMQ]"}
is_a: T4FS:0000021 ! exposing data
property_value: IAO:0000117 "Peter McQuilton" xsd:string

[Term]
id: T4FS:0000316
name: accession number
def: "Numbers used by the National Center for Biotechnology Information (NCBI) that are unique and citable." [] {http://purl.obolibrary.org/obo/IAO_0000119="CASRAI. https://casrai.org/term/accession-number/"}
is_a: T4FS:0000529 ! identifier
property_value: IAO:0000117 "Peter McQuilton" xsd:string

[Term]
id: T4FS:0000318
name: digital preservation
def: "The series of managed activities necessary to ensure continued access to digital materials for as long as necessary. Digital preservation is defined very broadly and refers to all of the actions required to maintain access to digital materials beyond the limits of media failure or technological change. Those materials may be records created during the day-to-day business of an organisation; “”born-digital”” materials created for a specific purpose (e.g. teaching resources); or the products of digitisation projects. This definition specifically excludes the potential use of digital technology to preserve the original artefacts through digitisation." [] {http://purl.obolibrary.org/obo/IAO_0000119="CASRAI. https://casrai.org/term/digital-preservation/"}
is_a: T4FS:0000372 ! data stewardship technical concept
property_value: IAO:0000117 "https://orcid.org/0000-0002-7702-4495" xsd:string
property_value: IAO:0000117 "Peter McQuilton" xsd:string

[Term]
id: T4FS:0000320
name: project management activities
def: "The practice of initiating, planning, executing, controlling, and closing the work of a team in relation to FAIR data stewardship." [] {http://purl.obolibrary.org/obo/IAO_0000119="PMQ"}
is_a: T4FS:0000012 ! data stewardship activity
property_value: IAO:0000117 "https://orcid.org/0000-0002-7702-4495" xsd:string
property_value: IAO:0000117 "Peter McQuilton" xsd:string
property_value: IAO:0000117 "Philippe Rocca-Serra" xsd:string
property_value: IAO:0000117 "Susanna Sansone" xsd:string

[Term]
id: T4FS:0000321
name: knowledge of funding acquisition management
def: "Bin for types of Knowledge related to Funding acquisition management." []
is_a: T4FS:0000426 ! funding acquisition management
property_value: IAO:0000117 "leightonlc" xsd:string

[Term]
id: T4FS:0000322
name: manage access control
def: "Monitor the authorised parties' access to data and keep it up to date." []
is_a: T4FS:0000469 ! access control and management
property_value: IAO:0000117 "Celia van Gelder" xsd:string
property_value: IAO:0000117 "Mateusz Kuzak" xsd:string
property_value: IAO:0000117 "Yan Wang" xsd:string

[Term]
id: T4FS:0000323
name: project management
def: "The practice of initiating, planning, executing, controlling, and closing the work of a team to achieve specific goals and meet specific success criteria at the specified time." [] {http://purl.obolibrary.org/obo/IAO_0000119="KH"}
is_a: T4FS:0000353 ! resource management
property_value: IAO:0000117 "Kristina Hettne" xsd:string
property_value: IAO:0000117 "Simon Hodson" xsd:string
property_value: IAO:0000117 "Victoria Dominguez Del Angel" xsd:string
property_value: IAO:0000118 "PM" xsd:string

[Term]
id: T4FS:0000324
name: data retention policy
def: "An organization's established protocol for retaining information for operational or regulatory compliance needs. The objectives of a data retention policy are to keep important information for future use or reference, to organize information so it can be searched and accessed at a later date, and to dispose of information that is no longer needed." [] {http://purl.obolibrary.org/obo/IAO_0000119="CASRAI. https://casrai.org/term/data-retention-policy/"}
is_a: T4FS:0000372 ! data stewardship technical concept
property_value: IAO:0000117 "Peter McQuilton" xsd:string

[Term]
id: T4FS:0000326
name: data representation
def: "An object describing the context of the data, including provenance, description, structural, and administrative information." [] {http://purl.obolibrary.org/obo/IAO_0000119="CASRAI. https://casrai.org/term/data-representation/"}
is_a: T4FS:0000036 ! curation
property_value: IAO:0000117 "https://orcid.org/0000-0002-7702-4495" xsd:string
property_value: IAO:0000117 "Peter McQuilton" xsd:string

[Term]
id: T4FS:0000327
name: metadata dataset
def: "The set of metadata describing a specific dataset." [] {http://purl.obolibrary.org/obo/IAO_0000119="CASRAI. https://casrai.org/term/metadata-dataset/"}
is_a: T4FS:0000517 ! metadata record
property_value: IAO:0000117 "https://orcid.org/0000-0002-7702-4495" xsd:string
property_value: IAO:0000117 "Peter McQuilton" xsd:string

[Term]
id: T4FS:0000328
name: long-term preservation
def: "Long-term preservation - Continued access to digital materials, or at least to the information contained in them, indefinitely." [] {http://purl.obolibrary.org/obo/IAO_0000119="CASRAI. https://casrai.org/term/long-term-preservation"}
is_a: T4FS:0000017 ! preservation
property_value: IAO:0000117 "https://orcid.org/0000-0002-7702-4495" xsd:string
property_value: IAO:0000117 "Peter McQuilton" xsd:string

[Term]
id: T4FS:0000329
name: research metadata format
def: "Research metadata format is a generic term encompassing the concept of a standardised format for research metadata." [] {http://purl.obolibrary.org/obo/IAO_0000119="AL, 9.3.2022"}
comment: AL 9.3.2022: The original CASRAI definition is unsuitable (https://casrai.org/term/research-metadata-format), therefore I have changed the definition to something more generic
is_a: T4FS:0000372 ! data stewardship technical concept
relationship: T4FS:0000563 T4FS:0000137 ! contributes to the implementation of I1. (meta)data use a formal, accessible, shared, and broadly applicable language for knowledge representation
property_value: IAO:0000117 "https://orcid.org/0000-0002-7702-4495" xsd:string
property_value: IAO:0000117 "Peter McQuilton" xsd:string

[Term]
id: T4FS:0000330
name: data residency
def: "The physical or geographic location of an organization's data or information. Data residency also refers to the legal or regulatory requirements imposed on data based on the country or region in which it resides. Cloud computing, which allows organizations to deliver hosted services over the Internet, can create data residency concerns." [] {http://purl.obolibrary.org/obo/IAO_0000119="CASRAI. https://casrai.org/term/data-residency/"}
is_a: T4FS:0000012 ! data stewardship activity
property_value: IAO:0000117 "Peter McQuilton" xsd:string

[Term]
id: T4FS:0000331
name: information governance
def: "Information governance, is the overall strategy for information at an organization. Information governance balances the risk that information presents with the value that information provides. Information governance helps with legal compliance, operational transparency, and reducing expenditures associated with legal discovery." [] {http://purl.obolibrary.org/obo/IAO_0000119="https://en.wikipedia.org/wiki/Information_governance, accessed 8.2.22"}
comment: CASRAI is the source for the term, with the definition provided separately.
is_a: T4FS:0000107 ! information security
property_value: IAO:0000117 "https://orcid.org/0000-0002-7702-4495" xsd:string
property_value: IAO:0000117 "Peter McQuilton" xsd:string

[Term]
id: T4FS:0000332
name: data element
def: "A unit of data for which the definition, identification, representation (term used to represent it), and permissible values are specified by means of a set of attributes." [] {http://purl.obolibrary.org/obo/IAO_0000119="CASRAI. https://casrai.org/term/data-element/"}
is_a: T4FS:0000372 ! data stewardship technical concept
property_value: IAO:0000117 "Peter McQuilton" xsd:string

[Term]
id: T4FS:0000333
name: data policy
def: "An organization's stated data/information management processes designed to assist and protect the organization's data research assets. It is a set of high-level principles that establish a guiding framework for data management. A data policy can be used to address strategic aspects such as data access, relevant legal matters, data stewardship issues and custodial duties, data..." [] {http://purl.obolibrary.org/obo/IAO_0000119="CASRAI. https://casrai.org/term/data-policy/"}
is_a: T4FS:0000372 ! data stewardship technical concept
relationship: T4FS:0000563 T4FS:0000447 ! contributes to the implementation of fair principle
property_value: IAO:0000117 "Peter McQuilton" xsd:string

[Term]
id: T4FS:0000334
name: legacy data
def: "Data that fall into the category of dark data or at-risk data." [] {http://purl.obolibrary.org/obo/IAO_0000119="CASRAI. https://casrai.org/term/legacy-data"}
is_a: T4FS:0000430 ! data
property_value: IAO:0000117 "https://orcid.org/0000-0002-7702-4495" xsd:string
property_value: IAO:0000117 "Peter McQuilton" xsd:string

[Term]
id: T4FS:0000335
name: controlled vocabulary
def: "A list of standardized terminology, words, or phrases, used for indexing or content analysis and information retrieval, usually in a defined information domain." [] {http://purl.obolibrary.org/obo/IAO_0000119="CASRAI. https://casrai.org/term/controlled-vocabulary/"}
is_a: T4FS:0000372 ! data stewardship technical concept
relationship: T4FS:0000563 T4FS:0000452 ! contributes to the implementation of I3. (meta)data include qualified references to other (meta)data
property_value: IAO:0000117 "Peter McQuilton" xsd:string

[Term]
id: T4FS:0000336
name: data integrity
def: "The assurance that information can only be accessed or modified by those authorized to do so." [] {http://purl.obolibrary.org/obo/IAO_0000119="CASRAI. https://casrai.org/term/data-integrity/"}
is_a: T4FS:0000372 ! data stewardship technical concept
property_value: IAO:0000117 "Peter McQuilton" xsd:string

[Term]
id: T4FS:0000337
name: pid attribute
def: "A single data element related to a PID and part of its record content." [] {http://purl.obolibrary.org/obo/IAO_0000119="CASRAI. https://casrai.org/term/pid-attribute/"}
is_a: T4FS:0000453 ! persistent identifier
property_value: IAO:0000117 "https://orcid.org/0000-0002-7702-4495" xsd:string
property_value: IAO:0000117 "Peter McQuilton" xsd:string

[Term]
id: T4FS:0000338
name: aptitudes for change management
def: "Bin for Aptitudes related to Change management." []
is_a: T4FS:0000411 ! change management
property_value: IAO:0000117 "leightonlc" xsd:string

[Term]
id: T4FS:0000339
name: medium-term preservation
def: "Medium-term preservation - Continued access to digital materials beyond changes in technology for a defined period of time but not indefinitely." [] {http://purl.obolibrary.org/obo/IAO_0000119="CASRAI. https://casrai.org/term/medium-term-preservation/"}
is_a: T4FS:0000017 ! preservation
property_value: IAO:0000117 "https://orcid.org/0000-0002-7702-4495" xsd:string
property_value: IAO:0000117 "Peter McQuilton" xsd:string

[Term]
id: T4FS:0000340
name: project lifecycle
def: "Describes the processes and tasks that must be completed to produce a product or service. Different project lifecycles exist for specific products and services. (For example, the lifecycle followed to build a house is very different from the lifecycle followed to develop a software package." [] {http://purl.obolibrary.org/obo/IAO_0000119="CASRAI. https://casrai.org/term/project-lifecycle"}
is_a: T4FS:0000372 ! data stewardship technical concept
property_value: IAO:0000117 "https://orcid.org/0000-0002-7702-4495" xsd:string
property_value: IAO:0000117 "Peter McQuilton" xsd:string

[Term]
id: T4FS:0000341
name: knowledge to relate fair data assessment to research community norms
def: "Know how the acceptability of research data FAIRness depends on the research community norms e.g. concepts of data and methods for deriving valid knowledge." []
is_a: T4FS:0000259 ! fair training
property_value: IAO:0000117 "Angus Whyte" xsd:string

[Term]
id: T4FS:0000342
name: data traceability
def: "Data traceability follows the lifecycle of data to track all access and changes to the data. It helps demonstrate transparency, compliance and adherence to regulations. Data traceability, along with data compliance, can be considered part of a data audit process. Data traceability is fundamental to reproducible research." [] {http://purl.obolibrary.org/obo/IAO_0000119="CASRAI. https://casrai.org/term/data-traceability/"}
is_a: T4FS:0000372 ! data stewardship technical concept
property_value: IAO:0000117 "Peter McQuilton" xsd:string

[Term]
id: T4FS:0000343
name: maintaining persistent identifiers
is_a: T4FS:0000492 ! understanding persistent identifiers
created_by: Peter McQuilton
creation_date: 2020-10-02T14:23:22.115275Z

[Term]
id: T4FS:0000345
name: select and apply license
def: "Choose the proper license considering types of project data and clearly indicate (apply) the license chosen in the project work." []
is_a: T4FS:0000042 ! ethical application of patents, licenses
property_value: IAO:0000117 "Celia van Gelder" xsd:string
property_value: IAO:0000117 "Mateusz Kuzak" xsd:string
property_value: IAO:0000117 "Yan Wang" xsd:string

[Term]
id: T4FS:0000346
name: relations
def: "Indicates how the different components within a system are linked to fulfill the tasks. Relations are thus defined by the services they are making use of and by the interface specifications." [] {http://purl.obolibrary.org/obo/IAO_0000119="CASRAI. https://casrai.org/term/relations"}
is_a: T4FS:0000372 ! data stewardship technical concept
property_value: IAO:0000117 "https://orcid.org/0000-0002-7702-4495" xsd:string
property_value: IAO:0000117 "Peter McQuilton" xsd:string

[Term]
id: T4FS:0000347
name: dataset
def: "Any organized collection of data in a computational format, defined by a theme or category that reflects what is being measured/observed/monitored. The presentation of the data in the application is enabled through metadata.REFERENCE. Research Data Alliance http://smw-rda.esc.rzg.mpg.de/index.php/Main_Page ; Mapping the Data Landscape 2011 Summit; TBS Standard on Geospatial Data (ISO 19115:2003); Environment Canada data stewardship &hellip; <a href=CASRAI. https://casrai.org/term/dataset/ class=more-link" [] {http://purl.obolibrary.org/obo/IAO_0000119="CASRAI. https://casrai.org/term/dataset/"}
is_a: T4FS:0000072 ! dataset series
property_value: IAO:0000117 "Peter McQuilton" xsd:string

[Term]
id: T4FS:0000348
name: aptitudes for service level management
def: "Bin for Aptitudes related to Service level management." []
is_a: T4FS:0000466 ! service level management
property_value: IAO:0000117 "leightonlc" xsd:string

[Term]
id: T4FS:0000350
name: extensible markup language
def: "Extensible Markup Language (XML) is a simple, very flexible text format derived from SGML (ISO 8879). Originally designed to meet the challenges of large-scale electronic publishing, XML is also playing an increasingly important role in the exchange of a wide variety of data on the Web and elsewhere." [] {http://purl.obolibrary.org/obo/IAO_0000119="CASRAI. https://casrai.org/term/extensible-markup-language/"}
is_a: T4FS:0000372 ! data stewardship technical concept
relationship: T4FS:0000563 T4FS:0000137 ! contributes to the implementation of I1. (meta)data use a formal, accessible, shared, and broadly applicable language for knowledge representation
property_value: IAO:0000117 "https://orcid.org/0000-0002-7702-4495" xsd:string
property_value: IAO:0000117 "Peter McQuilton" xsd:string
property_value: IAO:0000118 "XML" xsd:string

[Term]
id: T4FS:0000351
name: skills related to change management
def: "Bin for Skills needed for Change management." []
is_a: T4FS:0000411 ! change management
property_value: IAO:0000117 "leightonlc" xsd:string

[Term]
id: T4FS:0000352
name: data analysis
def: "A data lifecycle stage that involves the techniques that produce synthesized knowledge from organized information." [] {http://purl.obolibrary.org/obo/IAO_0000119="CASRAI. https://casrai.org/term/data-analysis/"}
is_a: T4FS:0000012 ! data stewardship activity
property_value: IAO:0000117 "Peter McQuilton" xsd:string

[Term]
id: T4FS:0000353
name: resource management
def: "Resource management is the efficient and effective development of an organization's resources when they are needed. Such resources may include the financial resources, inventory, human skills, production resources, or information technology (IT) and natural resources." [] {http://purl.obolibrary.org/obo/IAO_0000119="[LLC, https://en.wikipedia.org/wiki/Resource_management]"}
is_a: T4FS:0000012 ! data stewardship activity
property_value: IAO:0000117 "Kristina Hettne" xsd:string
property_value: IAO:0000117 "Leighton Christiansen" xsd:string
property_value: IAO:0000117 "Simon Hodson" xsd:string
property_value: IAO:0000117 "Victoria Dominguez Del Angel" xsd:string

[Term]
id: T4FS:0000354
name: data exploration
def: "Data exploration involves summarizing the main characteristics of a dataset using visualization and should be the first step in data analysis." [] {http://purl.obolibrary.org/obo/IAO_0000119="CASRAI. https://casrai.org/term/data-exploration/"}
is_a: T4FS:0000352 ! data analysis
property_value: IAO:0000117 "Peter McQuilton" xsd:string

[Term]
id: T4FS:0000355
name: aptitudes for storage management
def: "Bin for Aptitudes related to Storage management." []
is_a: T4FS:0000053 ! storage management
property_value: IAO:0000117 "leightonlc" xsd:string

[Term]
id: T4FS:0000356
name: advise and mentor
def: "Management and provision of good data stewardship practice." [] {http://purl.obolibrary.org/obo/IAO_0000119="PMQ"}
comment: AL 9.3.22. Removed from 'FAIR4S defined activity' class to better integrate with the T4FS hierarchy.
is_a: T4FS:0000012 ! data stewardship activity
property_value: IAO:0000117 "https://orcid.org/0000-0002-7702-4495" xsd:string
property_value: IAO:0000117 "Peter McQuilton" xsd:string
property_value: IAO:0000117 "Philippe Rocca-Serra" xsd:string
property_value: IAO:0000117 "Susanna Sansone" xsd:string
property_value: IAO:0000118 "Advise and enable" xsd:string
property_value: IAO:0000118 "data management and open research" xsd:string
property_value: IAO:0000118 "Data Stewardship and FAIR mentorship activity" xsd:string

[Term]
id: T4FS:0000357
name: skills related to workflow technologies management
def: "Bin for Skills needed for Workflow technologies management." []
is_a: T4FS:0000177 ! workflow technologies management
created_by: leightonlc
creation_date: 2019-10-17T15:15:55.86138Z

[Term]
id: T4FS:0000358
name: digital infrastructure
def: "Those layers that sit between base technology (a computer science concern) and discipline-specific science. The focus is on value-added systems and services that can be widely shared across scientific domains, both supporting and enabling large increases in multi- and interdisciplinary science while reducing duplication of effort and resources (e.g., including hardware, software, personnel, services and organizations)." [] {http://purl.obolibrary.org/obo/IAO_0000119="CASRAI. https://casrai.org/term/digital-infrastructure/"}
is_a: T4FS:0000372 ! data stewardship technical concept
property_value: IAO:0000117 "https://orcid.org/0000-0002-7702-4495" xsd:string
property_value: IAO:0000117 "Peter McQuilton" xsd:string
property_value: IAO:0000118 "Cyber infrastructure" xsd:string

[Term]
id: T4FS:0000359
name: skills related to data management cost management
def: "Bin for Skills needed for Data management cost management." []
is_a: T4FS:0000232 ! data management costs management
property_value: IAO:0000117 "leightonlc" xsd:string

[Term]
id: T4FS:0000360
name: pid system
def: "Consists of at least one PID resolver, a name schema and a defined mechanism for issuing PIDs that conform to the name schema. Examples include: DOI, Handle System, URN, ARK, PURL, etc." [] {http://purl.obolibrary.org/obo/IAO_0000119="CASRAI. https://casrai.org/term/pid-system/"}
is_a: T4FS:0000453 ! persistent identifier
property_value: IAO:0000117 "https://orcid.org/0000-0002-7702-4495" xsd:string
property_value: IAO:0000117 "Peter McQuilton" xsd:string

[Term]
id: T4FS:0000361
name: I2. (meta)data use vocabularies that follow fair principles
is_a: T4FS:0000014 ! interoperability of digital assets
property_value: IAO:0000117 "Peter McQuilton" xsd:string

[Term]
id: T4FS:0000362
name: cross-disciplinary
def: "Explains aspects of one discipline in terms of another (e.g., the physics of music; the politics of literature)." [] {http://purl.obolibrary.org/obo/IAO_0000119="CASRAI. https://casrai.org/term/cross-disciplinary/"}
is_a: T4FS:0000372 ! data stewardship technical concept
property_value: IAO:0000117 "Peter McQuilton" xsd:string

[Term]
id: T4FS:0000364
name: semantic data
def: "Data that are tagged with particular metadata that can be used to derive relationships between data." [] {http://purl.obolibrary.org/obo/IAO_0000119="CASRAI. https://casrai.org/term/semantic-data"}
is_a: T4FS:0000430 ! data
relationship: T4FS:0000563 T4FS:0000361 ! contributes to the implementation of I2. (meta)data use vocabularies that follow fair principles
property_value: IAO:0000117 "https://orcid.org/0000-0002-7702-4495" xsd:string
property_value: IAO:0000117 "Peter McQuilton" xsd:string

[Term]
id: T4FS:0000365
name: pid domain
def: "For a single identifier, the class of entity it refers to. For a PID system, the typical class of entities it is intended to be used for. Examples include: digital objects, physical objects, bodies, actors." [] {http://purl.obolibrary.org/obo/IAO_0000119="CASRAI. https://casrai.org/term/pid-domain/"}
is_a: T4FS:0000453 ! persistent identifier
property_value: IAO:0000117 "https://orcid.org/0000-0002-7702-4495" xsd:string
property_value: IAO:0000117 "Peter McQuilton" xsd:string

[Term]
id: T4FS:0000367
name: knowledge to choose fair data handling approaches appropriate to the research phenomena
def: "Select data handling approaches likely to make data as FAIR as possible, considering what the data is about and its purpose in the research." []
is_a: T4FS:0000259 ! fair training
property_value: IAO:0000117 "Angus Whyte" xsd:string

[Term]
id: T4FS:0000368
name: provenance information management
def: "The activity of recording provenance for data and software. Knowledge about provenance vocabularies, for example PROV-O and models provenance such as nanopublications." [] {http://purl.obolibrary.org/obo/IAO_0000119="KH"}
is_a: T4FS:0000353 ! resource management
property_value: IAO:0000117 "Kristina Hettne" xsd:string
property_value: IAO:0000117 "Simon Hodson" xsd:string
property_value: IAO:0000117 "Victoria Dominguez Del Angel" xsd:string

[Term]
id: T4FS:0000370
name: reproducible research
def: "Published results can be replicated using the documented data, code, and methods employed by the author or provider without the need for any additional information or needing to communicate with the author or provider." [] {http://purl.obolibrary.org/obo/IAO_0000119="CASRAI. https://casrai.org/term/reproducible-research"}
is_a: T4FS:0000170 ! reuse of digital assets
property_value: IAO:0000117 "https://orcid.org/0000-0002-7702-4495" xsd:string
property_value: IAO:0000117 "Peter McQuilton" xsd:string

[Term]
id: T4FS:0000371
name: A1.2 the protocol allows for an authentication and authorisation procedure, where necessary
is_a: T4FS:0000038 ! A1. (meta)data are retrievable by their identifier using a standardised communications protocol
property_value: IAO:0000117 "Peter McQuilton" xsd:string

[Term]
id: T4FS:0000372
name: data stewardship technical concept
relationship: T4FS:0000563 T4FS:0000446 ! contributes to the implementation of data stewardship guideline
property_value: IAO:0000117 "https://orcid.org/0000-0002-7702-4495" xsd:string
property_value: IAO:0000117 "Peter McQuilton" xsd:string

[Term]
id: T4FS:0000373
name: canonical data collection
def: "A data collection that has been normalized by some established criteria to allow for effective data management. Examples include: data files that belong to a certain experiment, all files that are created by one specific simulation, all files that belong to a specific observation (same day, same place, etc.)." [] {http://purl.obolibrary.org/obo/IAO_0000119="CASRAI. https://casrai.org/term/canonical-data-collection/"}
is_a: T4FS:0000372 ! data stewardship technical concept
property_value: IAO:0000117 "Peter McQuilton" xsd:string

[Term]
id: T4FS:0000374
name: archival documentation of software
def: "Ability to clean up existing source code and version control systems, get Unique ID for the code, choose the appropriate code repository/registry [YLF, VDA, KH]" []
is_a: T4FS:0000156 ! archiving
property_value: IAO:0000117 "https://orcid.org/0000-0002-7702-4495" xsd:string
property_value: IAO:0000117 "Kristina Hettne" xsd:string
property_value: IAO:0000117 "Victoria Dominguez Del Angel" xsd:string
property_value: IAO:0000117 "Yann Le Franc" xsd:string

[Term]
id: T4FS:0000375
name: data harmonization
def: "Data harmonization is the process of making data from different sources comparable." [] {http://purl.obolibrary.org/obo/IAO_0000119="Modified from CASRAI. https://casrai.org/term/data-harmonization/"}
is_a: T4FS:0000036 ! curation
property_value: IAO:0000117 "https://orcid.org/0000-0002-7702-4495" xsd:string
property_value: IAO:0000117 "Peter McQuilton" xsd:string
property_value: IAO:0000233 "https://github.com/terms4fairskills/FAIRterminology/issues/17" xsd:string

[Term]
id: T4FS:0000376
name: data mart
def: "A repository of data designed to serve a particular community of knowledge workers. The goal of a data mart is to meet the particular demands of a specific group of users." [] {http://purl.obolibrary.org/obo/IAO_0000119="CASRAI. https://casrai.org/term/data-mart/"}
is_a: T4FS:0000215 ! data store
property_value: IAO:0000117 "Peter McQuilton" xsd:string

[Term]
id: T4FS:0000377
name: access workflow
def: "A type of access entity that contains the services and functions which make the data object holdings and their information content and related services visible to data consumers." [] {http://purl.obolibrary.org/obo/IAO_0000119="CASRAI. https://casrai.org/term/access-workflow/"}
is_a: T4FS:0000283 ! access
property_value: IAO:0000117 "Peter McQuilton" xsd:string

[Term]
id: T4FS:0000378
name: knowledge of service level management
def: "Bin for types of Knowledge related to Service level management." []
is_a: T4FS:0000466 ! service level management
created_by: leightonlc
creation_date: 2019-10-17T15:18:53.73274Z

[Term]
id: T4FS:0000379
name: data model
def: "A model that specifies the structure or schema of a dataset. The model provides a documented description of the data and thus is an instance of metadata. It is a logical, relational data model showing an organized dataset as a collection of tables with entity, attributes and relations." [] {http://purl.obolibrary.org/obo/IAO_0000119="CASRAI. https://casrai.org/term/data-model/"}
is_a: T4FS:0000372 ! data stewardship technical concept
property_value: IAO:0000117 "Peter McQuilton" xsd:string

[Term]
id: T4FS:0000380
name: appreciate security and usability trade-offs
def: "Be aware of the potential conflicts between security and usability. Understand the importance of having information security policy and keeping a balance between the information security and usability. Willing to establish both organization and technical information security measurements." []
is_a: T4FS:0000107 ! information security
property_value: IAO:0000117 "Angus Whyte" xsd:string
property_value: IAO:0000117 "Celia van Gelder" xsd:string
property_value: IAO:0000117 "Mateusz Kuzak" xsd:string
property_value: IAO:0000117 "Yan Wang" xsd:string

[Term]
id: T4FS:0000381
name: standard
def: "A document that applies collectively to codes, specifications, recommended practices, classifications, test methods, and guides, which have been prepared by a standards developing organization or group, and published in accordance with established procedures." [] {http://purl.obolibrary.org/obo/IAO_0000119="CASRAI. https://casrai.org/term/standard"}
is_a: T4FS:0000372 ! data stewardship technical concept
property_value: IAO:0000117 "https://orcid.org/0000-0002-7702-4495" xsd:string
property_value: IAO:0000117 "Peter McQuilton" xsd:string

[Term]
id: T4FS:0000382
name: university teaching
def: "The application of a comprehensive knowledge of a discipline or disciplines to the development of expertise and the generation of new knowledge through research, and the planning and presentation of courses of study for undergraduates and graduates in universities." [] {http://purl.obolibrary.org/obo/IAO_0000119="CASRAI. https://casrai.org/term/university-teaching/"}
is_a: T4FS:0000012 ! data stewardship activity
property_value: IAO:0000117 "https://orcid.org/0000-0002-7702-4495" xsd:string
property_value: IAO:0000117 "Peter McQuilton" xsd:string

[Term]
id: T4FS:0000383
name: data migration
def: "The process of transferring data between storage types, formats, information technologies, or computer systems. A data migration project is usually undertaken to replace or upgrade servers or storage equipment, for a website consolidation, to conduct server maintenance or to relocate a data center." [] {http://purl.obolibrary.org/obo/IAO_0000119="CASRAI. https://casrai.org/term/data-migration/"}
is_a: T4FS:0000141 ! data management
property_value: IAO:0000117 "Peter McQuilton" xsd:string

[Term]
id: T4FS:0000384
name: data cleaning
def: "A continuous process that requires corrective actions throughout the data lifecycle." [] {http://purl.obolibrary.org/obo/IAO_0000119="CASRAI. https://casrai.org/term/data-cleaning/"}
is_a: T4FS:0000036 ! curation
property_value: IAO:0000117 "Peter McQuilton" xsd:string

[Term]
id: T4FS:0000385
name: R1.2 (meta)data are associated with detailed provenance
is_a: T4FS:0000174 ! R1. (meta)data are richly described with a plurality of accurate and relevant attributes
property_value: IAO:0000117 "Peter McQuilton" xsd:string

[Term]
id: T4FS:0000387
name: skills related to identity management
def: "Bin for Skills needed for Identity management." []
is_a: T4FS:0000169 ! identity management
property_value: IAO:0000117 "leightonlc" xsd:string

[Term]
id: T4FS:0000388
name: using persistent identifiers
def: "The use of persistent identifiers or PIDs to uniquely and persistently identify an entity." [] {http://purl.obolibrary.org/obo/IAO_0000119="[PMQ 3.2022]"}
is_a: T4FS:0000492 ! understanding persistent identifiers
property_value: IAO:0000117 "https://orcid.org/0000-0002-7702-4495" xsd:string
property_value: IAO:0000117 "Nancy Hoebelheinrich" xsd:string
property_value: IAO:0000117 "Peter McQuilton" xsd:string
created_by: Peter McQuilton
creation_date: 2020-10-02T14:22:51.569762Z

[Term]
id: T4FS:0000389
name: data curator
comment: AL 15.3.22: Updated label to 'data curator' to encompass curation beyond just in databases.
relationship: T4FS:0000558 T4FS:0000012 ! has/wants competency in data stewardship activity
relationship: T4FS:0000559 T4FS:0000372 ! has/wants knowledge about data stewardship technical concept
relationship: T4FS:0000559 T4FS:0000446 ! has/wants knowledge about data stewardship guideline
relationship: T4FS:0000561 T4FS:0000372 ! has/wants practical skill about data stewardship technical concept
relationship: T4FS:0000562 T4FS:0000548 ! has aptitude for data stewardship soft skill
property_value: IAO:0000117 "https://orcid.org/0000-0002-7702-4495" xsd:string
property_value: IAO:0000118 "database curator" xsd:string

[Term]
id: T4FS:0000390
name: engage innovation partners
def: "Learn about innovation partners' interests and concerns, analyze them and position the project work/outcome properly. Reach out to innovation partners with proactive and pragmatic innovation plan which is in compliance with FAIR principles." []
is_a: T4FS:0000084 ! engaging in open innovation beyond academia
property_value: IAO:0000117 "Celia van Gelder" xsd:string
property_value: IAO:0000117 "Mateusz Kuzak" xsd:string
property_value: IAO:0000117 "Yan Wang" xsd:string

[Term]
id: T4FS:0000391
name: R1.3 (meta)data meet domain-relevant community standards
is_a: T4FS:0000174 ! R1. (meta)data are richly described with a plurality of accurate and relevant attributes
property_value: IAO:0000117 "Peter McQuilton" xsd:string

[Term]
id: T4FS:0000392
name: data reduction
def: "The process of reducing the amount or size of stored data. This may be achieved by eliminating redundant copies of data files, deduplicating data files by removing redundant records, or by compressing the data files." [] {http://purl.obolibrary.org/obo/IAO_0000119="CASRAI. https://casrai.org/term/data-reduction/"}
is_a: T4FS:0000141 ! data management
property_value: IAO:0000117 "Peter McQuilton" xsd:string

[Term]
id: T4FS:0000393
name: F4. (meta)data are registered or indexed in a searchable resource
is_a: T4FS:0000248 ! findability of digital assets
property_value: IAO:0000117 "Peter McQuilton" xsd:string

[Term]
id: T4FS:0000394
name: data type registry
def: "1. A registry that links data types of all sorts with the executable data processing functions that can be useful for working with a specific data type. Examples include: complex file types in biology (diagnosis), registering categories that appear in PID records to describe data properties. Data types range from complex digital objects to simple..." [] {http://purl.obolibrary.org/obo/IAO_0000119="CASRAI. https://casrai.org/term/data-type-registry/"}
is_a: T4FS:0000215 ! data store
property_value: IAO:0000117 "Peter McQuilton" xsd:string

[Term]
id: T4FS:0000397
name: database
def: "A collection of data that is organised in a according to a conceptual structure/model describing the characteristics of these data and the relationships among their corresponding entities, supporting one or more application areas. A database allows its contents to be easily accessed, managed and updated. The type of database used depends on the requirements of &hellip; <a href=CASRAI. https://casrai.org/term/database/ class=more-link" [] {http://purl.obolibrary.org/obo/IAO_0000119="CASRAI. https://casrai.org/term/database/"}
is_a: T4FS:0000215 ! data store
property_value: IAO:0000117 "Peter McQuilton" xsd:string

[Term]
id: T4FS:0000398
name: appreciation of fair and open research
def: "Recognize the added value of FAIR and open research, encourage researchers to practise FAIR and open research." []
is_a: T4FS:0000008 ! develop open research strategy and vision
property_value: IAO:0000117 "Angus Whyte" xsd:string
property_value: IAO:0000117 "Celia van Gelder" xsd:string
property_value: IAO:0000117 "Mateusz Kuzak" xsd:string
property_value: IAO:0000117 "Yan Wang" xsd:string

[Term]
id: T4FS:0000399
name: ability to learn new techniques for fair implementation
def: "Demonstrate willingness to engage with new ways of applying FAIR principles." []
is_a: T4FS:0000408 ! aptitudes associated with using fair tools and services
relationship: T4FS:0000556 T4FS:0000548 {all_only="true"} ! requires/improves personal attribute data stewardship soft skill
property_value: IAO:0000117 "Angus Whyte" xsd:string

[Term]
id: T4FS:0000400
name: aptitudes for funding acquisition management
def: "Bin for Aptitudes related to Funding acquisition management." []
is_a: T4FS:0000426 ! funding acquisition management
property_value: IAO:0000117 "leightonlc" xsd:string

[Term]
id: T4FS:0000401
name: choosing the appropriate model or format for your data
def: "To be able to choose the correct data model and/or exchange format for your data, based on the repository where you plan to deposit your data." [] {http://purl.obolibrary.org/obo/IAO_0000119="[PMQ]"}
is_a: T4FS:0000175 ! fair evaluation of repositories for data deposition
property_value: IAO:0000117 "Peter McQuilton" xsd:string
property_value: IAO:0000118 "Which data model to use" xsd:string
property_value: IAO:0000118 "Which format to use" xsd:string

[Term]
id: T4FS:0000402
name: provenance metadata
def: "Information concerning the creation, attribution, or version history of managed data. Provenance metadata that indicates the relationship between two versions of data objects and is generated whenever a new version of a dataset is created. Examples include: (i) the name of the program that generated the new version, (ii) the commit id of the program." [] {http://purl.obolibrary.org/obo/IAO_0000119="CASRAI, https://casrai.org/term/provenance-metadata/"}
is_a: T4FS:0000527 ! metadata
property_value: IAO:0000117 "https://orcid.org/0000-0002-7702-4495" xsd:string

[Term]
id: T4FS:0000404
name: data availability
def: "The state when data are in the place needed by the user, at the time the user needs them, and in the form needed by the user." [] {http://purl.obolibrary.org/obo/IAO_0000119="CASRAI. https://casrai.org/term/data-availability/"}
is_a: T4FS:0000372 ! data stewardship technical concept
property_value: IAO:0000117 "Peter McQuilton" xsd:string

[Term]
id: T4FS:0000406
name: data review
def: "An activity through which the correctness conditions of the data are verified. It also includes the specification of the type of the error or condition not met, and the qualification of the data and its division into the error-free and erroneous data. Data review consists of both error detection and data analysis, and can be carried out in manual or automated mode." [] {http://purl.obolibrary.org/obo/IAO_0000119="CASRAI. https://casrai.org/term/data-review/"}
is_a: T4FS:0000352 ! data analysis
property_value: IAO:0000117 "https://orcid.org/0000-0002-7702-4495" xsd:string
property_value: IAO:0000117 "Peter McQuilton" xsd:string

[Term]
id: T4FS:0000408
name: aptitudes associated with using fair tools and services
is_a: T4FS:0000508 ! using fair and open research tools or services
created_by: HughShanahan
creation_date: 2019-10-18T08:56:32.673701Z

[Term]
id: T4FS:0000410
name: preservation metadata
def: "Documents actions that have been undertaken to preserve a digital resource such as migrations and checks sum calculations." [] {http://purl.obolibrary.org/obo/IAO_0000119="CASRAI. https://casrai.org/term/preservation-metadata/"}
is_a: T4FS:0000527 ! metadata
property_value: IAO:0000117 "https://orcid.org/0000-0002-7702-4495" xsd:string
property_value: IAO:0000117 "Peter McQuilton" xsd:string

[Term]
id: T4FS:0000411
name: change management
def: "Change management is a broad subject and can be applied to all different types of organizational change. The most common change drivers include:  technological evolution, process reviews, crisis, and consumer habit changes; pressure from new business entrants, acquisitions, mergers, and organizational restructuring." [] {http://purl.obolibrary.org/obo/IAO_0000119="https://www.hucmi.com/en/hcmbok/"}
is_a: T4FS:0000353 ! resource management
property_value: IAO:0000117 "Kristina Hettne" xsd:string
property_value: IAO:0000117 "Leighton Christiansen" xsd:string
property_value: IAO:0000117 "Simon Hodson" xsd:string
property_value: IAO:0000117 "Victoria Dominguez Del Angel" xsd:string
property_value: IAO:0000118 "CM" xsd:string

[Term]
id: T4FS:0000413
name: original repository
def: "A type of repository where the original copy of data was stored and probably a data identifier registered." [] {http://purl.obolibrary.org/obo/IAO_0000119="CASRAI. https://casrai.org/term/original repository"}
is_a: T4FS:0000215 ! data store
property_value: IAO:0000117 "https://orcid.org/0000-0002-7702-4495" xsd:string
property_value: IAO:0000117 "Peter McQuilton" xsd:string

[Term]
id: T4FS:0000414
name: de-identification
def: "1. The act of minimally perturbing individual-level data to decrease the probability of discovering an individualís identity. It involves masking direct identifiers (e.g., name, phone number, address) as well as transforming indirect identifiers that could be used alone or in combination to-identify an individual (e.g., birth dates, geographic details, dates of key events). If done correctly, de-identification is a defensible, repeatable, and auditable process that consistently provides assurance, based on generally accepted and repeatable statistical methodologies, that there is a very small risk of re-identification of any data that are released. 2. The use of one or more techniques designed to make it impossible — or at least more difficult — to identify a particular individual from stored data related to them. The purpose of data anonymization is to protect the privacy of the individual and to make it legal for governments and businesses to share their data without obtaining permission. Such data have proven to be very valuable for researchers, particularly in health care. Data anonymization methods include removing personally identifiable information (e.g., names, addresses, social insurance numbers, Medicare numbers, etc.), or using obfuscation methods such as encryption, hashing, generalization, pseudonymization, and perturbation." [] {http://purl.obolibrary.org/obo/IAO_0000119="CASRAI. https://casrai.org/term/de-identification/"}
is_a: T4FS:0000107 ! information security
property_value: IAO:0000117 "https://orcid.org/0000-0002-7702-4495" xsd:string
property_value: IAO:0000117 "Peter McQuilton" xsd:string
property_value: IAO:0000118 "Anonymization" xsd:string

[Term]
id: T4FS:0000415
name: manager
def: "Program delivery managers and support function managers, at all levels in an institution who are accountable for the direct delivery and support of programs and services within their domain of business responsibility." [] {http://purl.obolibrary.org/obo/IAO_0000119="CASRAI. https://casrai.org/term/manager"}
relationship: T4FS:0000558 T4FS:0000012 ! has/wants competency in data stewardship activity
relationship: T4FS:0000559 T4FS:0000372 ! has/wants knowledge about data stewardship technical concept
relationship: T4FS:0000559 T4FS:0000446 ! has/wants knowledge about data stewardship guideline
relationship: T4FS:0000561 T4FS:0000372 ! has/wants practical skill about data stewardship technical concept
relationship: T4FS:0000562 T4FS:0000548 ! has aptitude for data stewardship soft skill
property_value: IAO:0000117 "https://orcid.org/0000-0002-7702-4495" xsd:string
property_value: IAO:0000117 "Peter McQuilton" xsd:string

[Term]
id: T4FS:0000417
name: organizational leadership
def: "Organizational leadership is: (a) The ability to attract, assess, mobilize and focus energies and talent to work towards a shared purpose aligned with the mandate of the organization; (b) The ability to change culture, processes and priorities within the organization; and, (c) The ability to mentor." [] {http://purl.obolibrary.org/obo/IAO_0000119="CASRAI. https://casrai.org/term/organizational-leadership/"}
is_a: T4FS:0000548 ! data stewardship soft skill
property_value: IAO:0000117 "https://orcid.org/0000-0002-7702-4495" xsd:string
property_value: IAO:0000117 "Peter McQuilton" xsd:string

[Term]
id: T4FS:0000418
name: data dredging
def: "A data mining practice in which large volumes of data are analyzed seeking any possible relationships between data. The traditional scientific method, in contrast, begins with a hypothesis and follows with an examination of the data." [] {http://purl.obolibrary.org/obo/IAO_0000119="CASRAI. https://casrai.org/term/data-dredging/"}
is_a: T4FS:0000352 ! data analysis
property_value: IAO:0000117 "Peter McQuilton" xsd:string

[Term]
id: T4FS:0000420
name: unstructured data
def: "Data that have not been organized into a format and identifiable data structure that makes them easy to access and process. These data can often be searched as long as they are digital, but they are difficult to use for computer analyses." [] {http://purl.obolibrary.org/obo/IAO_0000119="CASRAI. https://casrai.org/term/unstructured-data"}
is_a: T4FS:0000430 ! data
property_value: IAO:0000117 "https://orcid.org/0000-0002-7702-4495" xsd:string
property_value: IAO:0000117 "Peter McQuilton" xsd:string

[Term]
id: T4FS:0000421
name: presentation slides with interactive exercises
is_a: T4FS:0000211 ! presentation slides
created_by: Peter McQuilton
creation_date: 2020-11-16T22:18:14.764875Z

[Term]
id: T4FS:0000422
name: creating persistent identifiers
is_a: T4FS:0000492 ! understanding persistent identifiers
created_by: Peter McQuilton
creation_date: 2020-10-02T14:23:05.600474Z

[Term]
id: T4FS:0000423
name: data linkage
def: "The process of bringing together from two or more different sources, data that relate to the same individual, family, place or event)." [] {http://purl.obolibrary.org/obo/IAO_0000119="CASRAI. https://casrai.org/term/data-linkage/"}
is_a: T4FS:0000372 ! data stewardship technical concept
property_value: IAO:0000117 "Peter McQuilton" xsd:string

[Term]
id: T4FS:0000425
name: catalogue
def: "A type of collection that describes, and points to features of another collection." [] {http://purl.obolibrary.org/obo/IAO_0000119="CASRAI. https://casrai.org/term/catalogue/"}
is_a: T4FS:0000372 ! data stewardship technical concept
property_value: IAO:0000117 "Peter McQuilton" xsd:string

[Term]
id: T4FS:0000426
name: funding acquisition management
def: "The consideration of available monetary resources for a specific time period to serve a specific purpose." [] {http://purl.obolibrary.org/obo/IAO_0000119="KH"}
is_a: T4FS:0000353 ! resource management
property_value: IAO:0000117 "Kristina Hettne" xsd:string
property_value: IAO:0000117 "Simon Hodson" xsd:string
property_value: IAO:0000117 "Victoria Dominguez Del Angel" xsd:string

[Term]
id: T4FS:0000427
name: machine access via api
def: "To be able to use programmatic methods to access a resource's API to query and extract an appropriate subset of data." [] {http://purl.obolibrary.org/obo/IAO_0000119="PMQ"}
is_a: T4FS:0000372 ! data stewardship technical concept
property_value: IAO:0000117 "Peter McQuilton" xsd:string
property_value: IAO:0000118 "API access" xsd:string
property_value: IAO:0000118 "Machine actionable search" xsd:string

[Term]
id: T4FS:0000428
name: data structure continuum
def: "The continuum of data structure that includes unstructured data, semi-structured data, and structured data." [] {http://purl.obolibrary.org/obo/IAO_0000119="CASRAI. https://casrai.org/term/data-structure-continuum/"}
is_a: T4FS:0000372 ! data stewardship technical concept
property_value: IAO:0000117 "Peter McQuilton" xsd:string

[Term]
id: T4FS:0000430
name: data
def: "Facts, measurements, recordings, records, or observations about the world collected by scientists and others, with a minimum of contextual interpretation." [] {http://purl.obolibrary.org/obo/IAO_0000119="CASRAI. https://casrai.org/term/data/"}
is_a: T4FS:0000372 ! data stewardship technical concept
property_value: IAO:0000117 "Peter McQuilton" xsd:string

[Term]
id: T4FS:0000431
name: semi-structured data
def: "Data that have not been organized into a specialized repository, such as a database, but that nevertheless have associated information, such as metadata, that makes them more amenable to processing than raw data. Semi-structured data lie somewhere between structured and unstructured data. They are not organized in a complex manner that makes sophisticated access and analysis possible. However, they may have information associated with them, such as metadata tagging that allows elements contained to be addressed. Example: A Word document is generally considered to be unstructured data. However, metadata tags could be added in the form of keywords and other metadata that represent the document content and make it easier for that document to be found when people search for those terms — the data are now semi-structured. Nevertheless, the document still lacks the complex organization of a database, so falls short of being fully structured data." [] {http://purl.obolibrary.org/obo/IAO_0000119="CASRAI. https://casrai.org/term/semi-structured-data"}
is_a: T4FS:0000430 ! data
property_value: IAO:0000117 "https://orcid.org/0000-0002-7702-4495" xsd:string
property_value: IAO:0000117 "Peter McQuilton" xsd:string

[Term]
id: T4FS:0000432
name: book chapter
is_a: T4FS:0000305 ! book
created_by: Peter McQuilton
creation_date: 2020-10-01T20:53:37.24517Z

[Term]
id: T4FS:0000433
name: research scientist
def: "A scientist who conducts activities in: (1) Research, development and analysis (RDA); (2) Managing research; and, (3) Representation and client services." [] {http://purl.obolibrary.org/obo/IAO_0000119="CASRAI. https://casrai.org/term/research-scientist"}
is_a: T4FS:0000220 ! researcher
property_value: IAO:0000117 "https://orcid.org/0000-0002-7702-4495" xsd:string
property_value: IAO:0000117 "Peter McQuilton" xsd:string

[Term]
id: T4FS:0000434
name: digital object identifier
def: "A name (not a location) for an entity on digital networks. It provides a system for persistent and actionable identification and interoperable exchange of managed information on digital networks. A DOI is a type of Persistent Identifier (PID) issued by the International DOI Foundation. This permanent identifier is associated with a digital object that permits it to be referenced reliably even if its location and metadata undergo change over time." [] {http://purl.obolibrary.org/obo/IAO_0000119="CASRAI. https://casrai.org/term/digital-object-identifier/"}
is_a: T4FS:0000453 ! persistent identifier
property_value: IAO:0000117 "https://orcid.org/0000-0002-7702-4495" xsd:string
property_value: IAO:0000117 "Peter McQuilton" xsd:string

[Term]
id: T4FS:0000435
name: F3. metadata clearly and explicitly include the identifier of the data they describe
is_a: T4FS:0000248 ! findability of digital assets
property_value: IAO:0000117 "Peter McQuilton" xsd:string

[Term]
id: T4FS:0000437
name: information management specialist
def: "A person who is expert in one or more of the information management disciplines that support the effective and efficient management of information." [] {http://purl.obolibrary.org/obo/IAO_0000119="CASRAI. https://casrai.org/term/information-management-specialist/"}
relationship: T4FS:0000558 T4FS:0000012 ! has/wants competency in data stewardship activity
relationship: T4FS:0000559 T4FS:0000372 ! has/wants knowledge about data stewardship technical concept
relationship: T4FS:0000559 T4FS:0000446 ! has/wants knowledge about data stewardship guideline
relationship: T4FS:0000561 T4FS:0000372 ! has/wants practical skill about data stewardship technical concept
relationship: T4FS:0000562 T4FS:0000548 ! has aptitude for data stewardship soft skill
property_value: IAO:0000117 "Peter McQuilton" xsd:string

[Term]
id: T4FS:0000438
name: A2. metadata are accessible, even when the data are no longer available
is_a: T4FS:0000478 ! accessibility of digital assets
property_value: IAO:0000117 "Peter McQuilton" xsd:string

[Term]
id: T4FS:0000439
name: stakeholder engagement on societal impact
def: "Identify and engage in dialogue with stakeholders affected by the research, or by making its outputs FAIR." []
is_a: T4FS:0000525 ! research integrity, attribution, impact awareness
property_value: IAO:0000117 "Angus Whyte" xsd:string
property_value: IAO:0000117 "Celia van Gelder" xsd:string
property_value: IAO:0000117 "Mateusz Kuzak" xsd:string
property_value: IAO:0000117 "Yan Wang" xsd:string

[Term]
id: T4FS:0000441
name: principal investigator
def: "The Principal Investigator (P.I.) is a researcher who has a research leadership role and is the point of contact for a project or partnership that applies the scientific method, historical method, or other research methodology for the advancement of knowledge resulting in independent, objective, high quality, traceable, and reproducible results. The P.I. has primary responsibility for the intellectual direction and integrity of the research or research-related activity, including data production, findings and results, and ensures ethical conduct in all aspects of the research process including but not limited to the treatment of human and animal subjects, conflicts of interest, data acquisition, sharing and ownership, publication practices, responsible authorship, and collaborative research and reporting. While various tasks may be delegated to team members, some of whom may have greater expertise in specific areas, the P.I. is familiar with the various technical and scientific aspects of a project and how they fit together, is able to identify and remediate gaps, and ensure communication within the team and with users of the research data and results." [] {http://purl.obolibrary.org/obo/IAO_0000119="CASRAI. https://casrai.org/term/principal-investigator"}
is_a: T4FS:0000415 ! manager
property_value: IAO:0000117 "https://orcid.org/0000-0002-7702-4495" xsd:string
property_value: IAO:0000117 "Peter McQuilton" xsd:string

[Term]
id: T4FS:0000442
name: program manager
def: "The person responsible for creating the organizational environment culture by providing clear direction and circumstances that allow people to be successful. The program manager is judged on the elements time, cost, and scope, cumulatively for all the projects and operations within the program. Program management decisions are both tactical and strategic in nature. The strategy aspects of these decisions must consider multidimensional impacts beyond the near-term delivery dates of the project. In addition to delivery and execution, the program manager has to also be concerned with the overall health and effectiveness of the program over the long term." [] {http://purl.obolibrary.org/obo/IAO_0000119="CASRAI. https://casrai.org/term/program-manager"}
is_a: T4FS:0000415 ! manager
property_value: IAO:0000117 "https://orcid.org/0000-0002-7702-4495" xsd:string
property_value: IAO:0000117 "Peter McQuilton" xsd:string

[Term]
id: T4FS:0000443
name: persistent uniform resource locator
def: "This is a URL. However, instead of pointing directly to the location of an Internet resource, a PURL points to an intermediate resolution service. The PURL resolution service associates the PURL with the actual URL and returns that URL to the client." [] {http://purl.obolibrary.org/obo/IAO_0000119="CASRAI. https://casrai.org/term/persistent-uniform-resource-locator"}
is_a: T4FS:0000453 ! persistent identifier
property_value: IAO:0000117 "https://orcid.org/0000-0002-7702-4495" xsd:string
property_value: IAO:0000117 "Peter McQuilton" xsd:string

[Term]
id: T4FS:0000445
name: dublin core
def: "An initiative to create a digital library card catalog for the Web. Dublin Core is made up of 15 metadata elements that offer expanded cataloging information and improved document indexing for search engine programs. The 15 metadata elements used by Dublin Core are: title (the name given the resource), creator (the person or organization responsible for the content), subject (the topic covered), description (a textual outline of the content), publisher (those responsible for making the resource available), contributor (those who added to the content), date (when the resource was made available), type (a category for the content), format (how the resource is presented), identifier (numerical identifier for the content such as a URL), source (where the content originally derived from), language (in what language the content is written), relation (how the content relates to other resources, for instance, if it is a chapter in a book), coverage (where the resource is physically located), and rights (a link to a copyright notice)." [] {http://purl.obolibrary.org/obo/IAO_0000119="CASRAI. https://casrai.org/term/dublin-core/"}
is_a: T4FS:0000372 ! data stewardship technical concept
relationship: T4FS:0000563 T4FS:0000137 ! contributes to the implementation of I1. (meta)data use a formal, accessible, shared, and broadly applicable language for knowledge representation
property_value: IAO:0000117 "https://orcid.org/0000-0002-7702-4495" xsd:string
property_value: IAO:0000117 "Peter McQuilton" xsd:string

[Term]
id: T4FS:0000446
name: data stewardship guideline
property_value: IAO:0000117 "Yann Le Franc" xsd:string
created_by: ylefranc
creation_date: 2021-03-17T16:34:14.943152Z

[Term]
id: T4FS:0000447
name: fair principle
def: "The FAIR principles are guidelines to improve the Findability, Accessibility, Interoperability, and Reuse of digital assets. The principles emphasise machine-actionability (i.e., the capacity of computational systems to find, access, interoperate, and reuse data with none or minimal human intervention) because humans increasingly rely on computational support to deal with data as a result of the increase in volume, complexity, and creation speed of data. The principles refer to three types of entities: data (or any digital object), metadata (information about that digital object), and infrastructure." [] {http://purl.obolibrary.org/obo/IAO_0000119="https://www.go-fair.org/fair-principles/"}
is_a: T4FS:0000446 ! data stewardship guideline
property_value: IAO:0000117 "Peter McQuilton" xsd:string
created_by: Peter McQuilton
creation_date: 2020-10-02T14:56:15.031154Z

[Term]
id: T4FS:0000448
name: aptitudes for cloud computing environment management
def: "Bin for Aptitudes related to Cloud computing environment management." []
is_a: T4FS:0000479 ! cloud computing environment management
property_value: IAO:0000117 "leightonlc" xsd:string

[Term]
id: T4FS:0000449
name: repurposed data
def: "New datasets obtained by combining data appropriately from a variety of existing files, generating new data products that did not previously exist. Repurposed data result from data wrangling." [] {http://purl.obolibrary.org/obo/IAO_0000119="CASRAI. https://casrai.org/term/repurposed-data/"}
is_a: T4FS:0000430 ! data
property_value: IAO:0000117 "https://orcid.org/0000-0002-7702-4495" xsd:string
property_value: IAO:0000117 "Peter McQuilton" xsd:string

[Term]
id: T4FS:0000450
name: document type definition
def: "The building blocks of an XML document." [] {http://purl.obolibrary.org/obo/IAO_0000119="CASRAI. https://casrai.org/term/document-type-definition/"}
is_a: T4FS:0000372 ! data stewardship technical concept
relationship: T4FS:0000563 T4FS:0000137 ! contributes to the implementation of I1. (meta)data use a formal, accessible, shared, and broadly applicable language for knowledge representation
property_value: IAO:0000117 "https://orcid.org/0000-0002-7702-4495" xsd:string
property_value: IAO:0000117 "Peter McQuilton" xsd:string

[Term]
id: T4FS:0000452
name: I3. (meta)data include qualified references to other (meta)data
is_a: T4FS:0000014 ! interoperability of digital assets
property_value: IAO:0000117 "Peter McQuilton" xsd:string

[Term]
id: T4FS:0000453
name: persistent identifier
def: "A persistent identifier is a long-lasting reference to a digital object that gives information about that object regardless what happens to it. Developed to address link rot, a persistent identifier can be resolved to provide an appropriate representation of an object whether that objects changes its online location or goes offline." [] {http://purl.obolibrary.org/obo/IAO_0000119="CASRAI. https://casrai.org/term/persistent-identifier"}
is_a: T4FS:0000529 ! identifier
property_value: IAO:0000117 "https://orcid.org/0000-0002-7702-4495" xsd:string
property_value: IAO:0000117 "Peter McQuilton" xsd:string

[Term]
id: T4FS:0000454
name: scientist
def: "A person who is studying or has expert knowledge of one or more of the natural or physical sciences." [] {http://purl.obolibrary.org/obo/IAO_0000119="CASRAI. https://casrai.org/term/scientist"}
is_a: T4FS:0000220 ! researcher
property_value: IAO:0000117 "https://orcid.org/0000-0002-7702-4495" xsd:string
property_value: IAO:0000117 "Peter McQuilton" xsd:string

[Term]
id: T4FS:0000455
name: integration
def: "1. The act of bringing together smaller components into a single system that functions as one. 2. In the context of information technology: The end result of a process that aims to stitch together different, often disparate, subsystems so that the data contained in each becomes part of a larger, more comprehensive system that, ideally, quickly and easily shares data when needed. This often requires that organizations build a customized architecture or structure of applications to combine new or existing hardware, software and other communications." [] {http://purl.obolibrary.org/obo/IAO_0000119="CASRAI. https://casrai.org/term/integration/"}
is_a: T4FS:0000012 ! data stewardship activity
property_value: IAO:0000117 "https://orcid.org/0000-0002-7702-4495" xsd:string
property_value: IAO:0000117 "Peter McQuilton" xsd:string

[Term]
id: T4FS:0000456
name: knowledge of high performance computing management
def: "Bin for types of Knowledge related to High performance computing management." []
is_a: T4FS:0000308 ! high performance computing management
property_value: IAO:0000117 "leightonlc" xsd:string

[Term]
id: T4FS:0000457
name: fair mentoring
def: "The act of mentoring around FAIR data stewardship." [] {http://purl.obolibrary.org/obo/IAO_0000119="PMQ"}
is_a: T4FS:0000259 ! fair training
property_value: IAO:0000117 "https://orcid.org/0000-0002-7702-4495" xsd:string
property_value: IAO:0000117 "Peter McQuilton" xsd:string
property_value: IAO:0000117 "Philippe Rocca-Serra" xsd:string
property_value: IAO:0000117 "Susanna Sansone" xsd:string

[Term]
id: T4FS:0000458
name: data governance
def: "The exercise of authority, control and shared decision making (planning, monitoring and enforcement) over the management of data assets." [] {http://purl.obolibrary.org/obo/IAO_0000119="CASRAI. https://casrai.org/term/data-governance/"}
is_a: T4FS:0000472 ! governance
property_value: IAO:0000117 "Peter McQuilton" xsd:string

[Term]
id: T4FS:0000460
name: extensible resource identifier
def: "A defining scheme used for identification of resources (including people and organizations) and the sharing of data across domains, enterprises, and applications. XRI TC will define a Uniform Resource Identifier (URI) scheme and a corresponding Uniform Resource (URN) namespace.n/aCASRAI. https://www.oasis-open.org/committees/tc_home.php?wg_abbrev=xri" [] {http://purl.obolibrary.org/obo/IAO_0000119="CASRAI. https://casrai.org/term/extensible-resource-identifier/"}
is_a: T4FS:0000529 ! identifier
property_value: IAO:0000117 "Peter McQuilton" xsd:string

[Term]
id: T4FS:0000462
name: impact
def: "In the context of a researcher's activities, impact is the consequence of the research and new knowledge on the advancement of the specialty. Science-based policies, regulations, services and technology transfers are some examples of ways target results can be achieved and impact demonstrated." [] {http://purl.obolibrary.org/obo/IAO_0000119="CASRAI. https://casrai.org/term/impact/"}
is_a: T4FS:0000372 ! data stewardship technical concept
property_value: IAO:0000117 "Peter McQuilton" xsd:string

[Term]
id: T4FS:0000463
name: access control list
def: "A list used to grant permission matched against credentials." [] {http://purl.obolibrary.org/obo/IAO_0000119="CASRAI. https://casrai.org/term/access-control-list/"}
is_a: T4FS:0000283 ! access
property_value: IAO:0000117 "Peter McQuilton" xsd:string

[Term]
id: T4FS:0000464
name: understand data ownership and access policies
def: "Learn about data copyright laws, licennsing and other legal aspects of data access. Understand the application of those laws at the project level." []
is_a: T4FS:0000469 ! access control and management
property_value: IAO:0000117 "Celia van Gelder" xsd:string
property_value: IAO:0000117 "Mateusz Kuzak" xsd:string
property_value: IAO:0000117 "Yan Wang" xsd:string

[Term]
id: T4FS:0000465
name: meeting/conference organisation
def: "Meeting/conference organisation is a project management activity that encompasses all of the steps required to run a meeting or conference." []
is_a: T4FS:0000320 ! project management activities
property_value: IAO:0000117 "https://orcid.org/0000-0002-7702-4495" xsd:string
property_value: IAO:0000117 "Peter McQuilton" xsd:string
property_value: IAO:0000117 "Philippe Rocca-Serra" xsd:string
property_value: IAO:0000117 "Susanna Sansone" xsd:string

[Term]
id: T4FS:0000466
name: service level management
def: "It can be considered as a negotiated agreement between the customer and vendor which are acceptable to both parties with respect to costs and expectations in order to support the business process." [] {http://purl.obolibrary.org/obo/IAO_0000119="https://www.techopedia.com/definition/13848/service-level-management-slm [LLC]"}
is_a: T4FS:0000353 ! resource management
property_value: IAO:0000117 "Kristina Hettne" xsd:string
property_value: IAO:0000117 "Leighton Christiansen" xsd:string
property_value: IAO:0000117 "Simon Hodson" xsd:string
property_value: IAO:0000117 "Victoria Dominguez Del Angel" xsd:string
property_value: IAO:0000118 "SLM" xsd:string

[Term]
id: T4FS:0000467
name: national standard
def: "From an official perspective, a national standard is adopted by a national standards body (e.g., Standards Council of Canada, American National Standards Institute, British Standards Institution) and made available to the public. Practically speaking, however, a national standard is any standard that is widely used and recognized within a country. In this context, even government standards, such as those issued by the Occupational Safety and Health Administration (OSHA), can be considered national standards." [] {http://purl.obolibrary.org/obo/IAO_0000119="CASRAI. https://casrai.org/term/national-standard/"}
is_a: T4FS:0000372 ! data stewardship technical concept
relationship: T4FS:0000563 T4FS:0000137 ! contributes to the implementation of I1. (meta)data use a formal, accessible, shared, and broadly applicable language for knowledge representation
property_value: IAO:0000117 "https://orcid.org/0000-0002-7702-4495" xsd:string
property_value: IAO:0000117 "Peter McQuilton" xsd:string

[Term]
id: T4FS:0000468
name: open government
def: "A governing culture that holds that the public has the right to access the documents and proceedings of government to allow for greater openness, accountability, and engagement." [] {http://purl.obolibrary.org/obo/IAO_0000119="CASRAI. https://casrai.org/term/open-government/"}
is_a: T4FS:0000372 ! data stewardship technical concept
property_value: IAO:0000117 "https://orcid.org/0000-0002-7702-4495" xsd:string
property_value: IAO:0000117 "Peter McQuilton" xsd:string

[Term]
id: T4FS:0000469
name: access control and management
is_a: T4FS:0000106 ! publish data

[Term]
id: T4FS:0000470
name: storage security management
def: "Manage the assessment, implementation and monitoring of secure storage protocols." []
is_a: T4FS:0000107 ! information security
property_value: IAO:0000117 "Angus Whyte" xsd:string
property_value: IAO:0000117 "Celia van Gelder" xsd:string
property_value: IAO:0000117 "Mateusz Kuzak" xsd:string
property_value: IAO:0000117 "Yan Wang" xsd:string

[Term]
id: T4FS:0000472
name: governance
def: "1. Exercising authority to provide direction and to undertake, coordinate, and regulate activities in support of achieving this direction and desired outcomes. Governance can be thought of as the role of an organization's board of directors or its equivalent that is focused on defining that organization's purpose and the development of the strategies, objectives, values, and policies that frame how that purpose will be pursued. It includes the development of such things as mission statements, statements of organizational objectives and values, logic models, organizational performance metrics, risk management frameworks, policies and guidelines for financial and operational matters, stakeholder relations, etc." [] {http://purl.obolibrary.org/obo/IAO_0000119="CASRAI. https://casrai.org/term/governance/"}
is_a: T4FS:0000012 ! data stewardship activity
property_value: IAO:0000117 "Peter McQuilton" xsd:string

[Term]
id: T4FS:0000474
name: open archives initiative protocol for metadata harvesting
def: "A low-barrier mechanism for repository interoperability. Data Providers are repositories that expose structured metadata via OAI-PMH. Service Providers then make OAI-PMH service requests to harvest that metadata. OAI-PMH is a set of six verbs or services that are invoked within HTTP." [] {http://purl.obolibrary.org/obo/IAO_0000119="CASRAI. https://casrai.org/term/open-archives-initiative-protocol-for-metadata-harvesting/"}
is_a: T4FS:0000427 ! machine access via api
property_value: IAO:0000117 "Peter McQuilton" xsd:string

[Term]
id: T4FS:0000475
name: computer code
def: "A series of computer instructions written in some human readable computer language, usually stored in a text file." [] {http://purl.obolibrary.org/obo/IAO_0000119="CASRAI. https://casrai.org/term/computer-code/"}
is_a: T4FS:0000372 ! data stewardship technical concept
property_value: IAO:0000117 "Peter McQuilton" xsd:string

[Term]
id: T4FS:0000476
name: syntactic interoperability
def: "Syntactic interoperability defines the structure or format of data exchange and is achieved through tools such as XML or SQL Standards." [] {http://purl.obolibrary.org/obo/IAO_0000119="CASRAI. https://casrai.org/term/syntactic-interoperability"}
is_a: T4FS:0000372 ! data stewardship technical concept
property_value: IAO:0000117 "https://orcid.org/0000-0002-7702-4495" xsd:string
property_value: IAO:0000117 "Peter McQuilton" xsd:string

[Term]
id: T4FS:0000477
name: aptitudes for preservation costs management
def: "Bin for Aptitudes related to Preservation costs management." []
is_a: T4FS:0000104 ! preservation costs management
property_value: IAO:0000117 "leightonlc" xsd:string

[Term]
id: T4FS:0000478
name: accessibility of digital assets
is_a: T4FS:0000447 ! fair principle
property_value: IAO:0000117 "Peter McQuilton" xsd:string

[Term]
id: T4FS:0000479
name: cloud computing environment management
def: "The activity of bringing computer system resources, especially data storage and computing power on demand via Internet." [] {http://purl.obolibrary.org/obo/IAO_0000119="(modified from wikipedia) [VDA]"}
is_a: T4FS:0000353 ! resource management
property_value: IAO:0000117 "Kristina Hettne" xsd:string
property_value: IAO:0000117 "Simon Hodson" xsd:string
property_value: IAO:0000117 "Victoria Dominguez Del Angel" xsd:string

[Term]
id: T4FS:0000480
name: corpus
def: "A set of documents that has a scientific meaning. A corpus can be produced by an individual researchers activity (including its archival materials), or from a laboratory research, field campaign or science and culture heritage project, a survey, etc." [] {http://purl.obolibrary.org/obo/IAO_0000119="CASRAI. https://casrai.org/term/corpus/"}
is_a: T4FS:0000372 ! data stewardship technical concept
property_value: IAO:0000117 "Peter McQuilton" xsd:string

[Term]
id: T4FS:0000481
name: the use of fair and open research tools or services
def: "Understand how to use FAIR and open research tools and services." []
is_a: T4FS:0000508 ! using fair and open research tools or services
property_value: IAO:0000117 "Hugh Shanahan" xsd:string

[Term]
id: T4FS:0000482
name: data sharing
def: "The practice of making data available for reuse. This may be done, for example, by depositing the data in a repository, through data publication." [] {http://purl.obolibrary.org/obo/IAO_0000119="CASRAI. https://casrai.org/term/data-sharing/"}
is_a: T4FS:0000021 ! exposing data
property_value: IAO:0000117 "https://orcid.org/0000-0002-7702-4495" xsd:string
property_value: IAO:0000117 "Peter McQuilton" xsd:string
property_value: IAO:0000118 "Data dissemination" xsd:string
property_value: IAO:0000118 "Data posting" xsd:string

[Term]
id: T4FS:0000483
name: appreciate importance of crediting research contributions
def: "Understand how the rewards for effort depend on crediting the contributions of researchers and professional groups towards making FAIR outputs." []
is_a: T4FS:0000525 ! research integrity, attribution, impact awareness
property_value: IAO:0000117 "Angus Whyte" xsd:string
property_value: IAO:0000117 "Celia van Gelder" xsd:string
property_value: IAO:0000117 "Mateusz Kuzak" xsd:string
property_value: IAO:0000117 "Yan Wang" xsd:string

[Term]
id: T4FS:0000485
name: reference resolution
def: "The process of resolving a reference to useful information by using a globally available system." [] {http://purl.obolibrary.org/obo/IAO_0000119="CASRAI. https://casrai.org/term/reference-resolution"}
is_a: T4FS:0000372 ! data stewardship technical concept
property_value: IAO:0000117 "https://orcid.org/0000-0002-7702-4495" xsd:string
property_value: IAO:0000117 "Peter McQuilton" xsd:string

[Term]
id: T4FS:0000486
name: research manager
def: "The person who manages or coordinates resources, personnel, facilities, and operating funds-allocations in an organization conducting research, development and analysis (RDA) in the natural and physical sciences. A research manager determines the nature, priority objectives and the resources committed to their achievement within and across the organizations, and evaluates program outputs in relation to organizational objectives and policies. A research manager provides scientific advice on the direction, conduct and management of these programs. A research manager does not personally conduct research development and analysis (RDA), control and coordinate projects, or control and coordinate contracted RDA." [] {http://purl.obolibrary.org/obo/IAO_0000119="CASRAI. https://casrai.org/term/research-manager"}
is_a: T4FS:0000220 ! researcher
property_value: IAO:0000117 "https://orcid.org/0000-0002-7702-4495" xsd:string
property_value: IAO:0000117 "Peter McQuilton" xsd:string

[Term]
id: T4FS:0000487
name: data integration
def: "Combining diverse datasets from disparate sources into one unified dataset or database. Data are accessed and extracted, moved, validated, cleaned, transformed and loaded." [] {http://purl.obolibrary.org/obo/IAO_0000119="CASRAI. https://casrai.org/term/data-integration"}
is_a: T4FS:0000036 ! curation
property_value: IAO:0000117 "https://orcid.org/0000-0002-7702-4495" xsd:string
property_value: IAO:0000117 "Peter McQuilton" xsd:string

[Term]
id: T4FS:0000488
name: standard operating procedure
def: "Detailed, written instructions to achieve uniformity of the performance of a specific function." [] {http://purl.obolibrary.org/obo/IAO_0000119="CASRAI. https://casrai.org/term/standard-operating-procedure"}
is_a: T4FS:0000372 ! data stewardship technical concept
property_value: IAO:0000117 "https://orcid.org/0000-0002-7702-4495" xsd:string
property_value: IAO:0000117 "Peter McQuilton" xsd:string

[Term]
id: T4FS:0000489
name: repository
def: "Repositories preserve, manage, and provide access to many types of digital materials in a variety of formats." [] {http://purl.obolibrary.org/obo/IAO_0000119="CASRAI. https://casrai.org/term/repository"}
is_a: T4FS:0000372 ! data stewardship technical concept
property_value: IAO:0000117 "https://orcid.org/0000-0002-7702-4495" xsd:string
property_value: IAO:0000117 "Peter McQuilton" xsd:string

[Term]
id: T4FS:0000490
name: knowledge of theories underlying fair implementation
def: "Understand the concepts underpinning FAIR criteria." []
is_a: T4FS:0000259 ! fair training
property_value: IAO:0000117 "Angus Whyte" xsd:string

[Term]
id: T4FS:0000491
name: document in lay terms
def: "Know the purpose of the public use, choose the proper subjects for the audience and describe the project work for the purpose/audience chosen." []
is_a: T4FS:0000106 ! publish data
property_value: IAO:0000117 "Celia van Gelder" xsd:string
property_value: IAO:0000117 "Mateusz Kuzak" xsd:string
property_value: IAO:0000117 "Yan Wang" xsd:string

[Term]
id: T4FS:0000492
name: understanding persistent identifiers
is_a: T4FS:0000021 ! exposing data
created_by: Peter McQuilton
creation_date: 2020-10-02T14:54:27.168274Z

[Term]
id: T4FS:0000493
name: data upload database
def: "A collection of interrelated data often with controlled redundancy, organized according to a scheme to serve one or more applications; the data are stored so that they can be used by several programs without concern for data structures or organization." [] {http://purl.obolibrary.org/obo/IAO_0000119="CASRAI. https://casrai.org/term/data-upload-database/"}
is_a: T4FS:0000215 ! data store
property_value: IAO:0000117 "Peter McQuilton" xsd:string

[Term]
id: T4FS:0000494
name: uniform resource identifier
def: "A string of characters used to identify or name a resource on the Internet. Such identification enables interaction with representations of the resource over a network, typically the World Wide Web, using specific protocols. MIT data management and publishing" [] {http://purl.obolibrary.org/obo/IAO_0000119="CASRAI. https://casrai.org/term/uniform-resource-identifier/"}
is_a: T4FS:0000529 ! identifier
property_value: IAO:0000117 "https://orcid.org/0000-0002-7702-4495" xsd:string
property_value: IAO:0000117 "Peter McQuilton" xsd:string

[Term]
id: T4FS:0000495
name: how to find fair research data tools/services (catalogues)
def: "Know how to search for and identify FAIR services or tools that fit project needs." []
is_a: T4FS:0000481 ! the use of fair and open research tools or services
property_value: IAO:0000117 "Angus Whyte" xsd:string

[Term]
id: T4FS:0000496
name: data reference model
def: "A framework whose primary purpose is to enable information sharing and reuse across the federal government via the standard description and discovery of common data and the promotion of uniform data management practices.n/aCASRAI. https://www.whitehouse.gov/sites/default/files/omb/assets/egov_docs/DRM_2_0_Final.pdf" [] {http://purl.obolibrary.org/obo/IAO_0000119="CASRAI. https://casrai.org/term/data-reference-model/"}
is_a: T4FS:0000379 ! data model
property_value: IAO:0000117 "Peter McQuilton" xsd:string

[Term]
id: T4FS:0000498
name: peer review
def: "A process by which a scholarly work (such as a paper or a research proposal) is checked by a group of experts in the same field to make sure it meets the necessary standards before it is published or accepted." [] {http://purl.obolibrary.org/obo/IAO_0000119="CASRAI. https://casrai.org/term/peer-review/"}
is_a: T4FS:0000126 ! assessment
property_value: IAO:0000117 "https://orcid.org/0000-0002-7702-4495" xsd:string
property_value: IAO:0000117 "Peter McQuilton" xsd:string

[Term]
id: T4FS:0000499
name: knowledge of provenance information management
def: "Bin for types of Knowledge related to Provenance information management." []
is_a: T4FS:0000368 ! provenance information management
created_by: leightonlc
creation_date: 2019-10-17T15:17:02.313897Z

[Term]
id: T4FS:0000500
name: record
def: "1. A collection of data items arranged for processing by a program. Multiple records are contained in a file or dataset. Typically, records can be of fixed-length or be of variable length with the length information contained within the record. 2. A record (sometimes called a row) is a group of fields (sometimes called columns) within a table that are relevant to a specific entity." [] {http://purl.obolibrary.org/obo/IAO_0000119="CASRAI. https://casrai.org/term/record"}
is_a: T4FS:0000372 ! data stewardship technical concept
property_value: IAO:0000117 "https://orcid.org/0000-0002-7702-4495" xsd:string
property_value: IAO:0000117 "Peter McQuilton" xsd:string

[Term]
id: T4FS:0000501
name: de-anonymization
def: "De-anonymization is a reverse engineering process in which de-identified data are cross-referenced with other data sources to re-identify the personally identifiable information. This could occur if a de-identification process had not been not successfully performed, or had not been undertaken in the first place." [] {http://purl.obolibrary.org/obo/IAO_0000119="CASRAI. https://casrai.org/term/de-anonymization/"}
is_a: T4FS:0000107 ! information security
property_value: IAO:0000117 "https://orcid.org/0000-0002-7702-4495" xsd:string
property_value: IAO:0000117 "Peter McQuilton" xsd:string

[Term]
id: T4FS:0000502
name: application of fair tools and services
is_a: T4FS:0000508 ! using fair and open research tools or services
created_by: HughShanahan
creation_date: 2019-10-18T08:45:02.980527Z

[Term]
id: T4FS:0000503
name: mandatory standard
def: "Requires compliance because of a government statute or regulation, an organization internal policy, or contractual requirement. Failure to comply with a mandatory standard usually carries a sanction, such as civil or criminal penalties, or loss of employment." [] {http://purl.obolibrary.org/obo/IAO_0000119="CASRAI. https://casrai.org/term/mandatory-standard/"}
is_a: T4FS:0000372 ! data stewardship technical concept
relationship: T4FS:0000563 T4FS:0000137 ! contributes to the implementation of I1. (meta)data use a formal, accessible, shared, and broadly applicable language for knowledge representation
property_value: IAO:0000117 "https://orcid.org/0000-0002-7702-4495" xsd:string
property_value: IAO:0000117 "Peter McQuilton" xsd:string

[Term]
id: T4FS:0000504
name: data driven decision management
def: "An approach to governance that values decisions that can be backed up with data that can be verified. The success of the data-driven approach is reliant upon the quality of the data gathered and the effectiveness of its analysis and interpretation." [] {http://purl.obolibrary.org/obo/IAO_0000119="CASRAI. https://casrai.org/term/data-driven-decision-management/"}
is_a: T4FS:0000472 ! governance
property_value: IAO:0000117 "Peter McQuilton" xsd:string

[Term]
id: T4FS:0000505
name: golden record
def: "1. A single, well-defined version of all the data entities in an organizational ecosystem. In this context, a golden record is sometimes called the single version of the truth, where truth is understood to mean the reference to which data users can turn when they want to ensure that they have the correct version of a piece of information. The golden record encompasses all the data in every system of record within a particular organization. A system of record is an information storage and retrieval system that serves as the authoritative source for a particular data element in a system containing multiple sources of the same element. To ensure data integrity, a single system of record must always exist for each and every data element. A well-maintained, current golden record should be a fundamental element of the Master Data Management policy for every enterprise. 2. The word “golden” is sometimes used in information technology to express the importance of some type of source. In the context of virtualization, for example, a golden image is a template for a virtual machine, virtual desktop, servers, or hard disk drive." [] {http://purl.obolibrary.org/obo/IAO_0000119="CASRAI. https://casrai.org/term/golden-record/"}
is_a: T4FS:0000372 ! data stewardship technical concept
property_value: IAO:0000117 "https://orcid.org/0000-0002-7702-4495" xsd:string
property_value: IAO:0000117 "Peter McQuilton" xsd:string

[Term]
id: T4FS:0000507
name: data quality
def: "The reliability and application efficiency of data. It is a perception or an assessment of dataset's fitness to serve its purpose in a given context. Aspects of data quality include: Accuracy, Completeness, Update status, Relevance, Consistency across data sources, Reliability, Appropriate presentation, Accessibility. Within an organization, acceptable data quality is crucial to operational and transactional..." [] {http://purl.obolibrary.org/obo/IAO_0000119="CASRAI. https://casrai.org/term/data-quality/"}
is_a: T4FS:0000372 ! data stewardship technical concept
property_value: IAO:0000117 "Peter McQuilton" xsd:string

[Term]
id: T4FS:0000508
name: using fair and open research tools or services
is_a: T4FS:0000259 ! fair training
created_by: HughShanahan
creation_date: 2019-10-18T08:38:59.038306Z

[Term]
id: T4FS:0000510
name: webinar
is_a: T4FS:0000519 ! learning medium
property_value: IAO:0000117 "Peter McQuilton" xsd:string
created_by: Peter McQuilton
creation_date: 2020-10-01T20:53:15.691824Z

[Term]
id: T4FS:0000511
name: digital data
def: "Data in the form of digital materials." [] {http://purl.obolibrary.org/obo/IAO_0000119="CASRAI. https://casrai.org/term/digital-data/"}
is_a: T4FS:0000430 ! data
property_value: IAO:0000117 "https://orcid.org/0000-0002-7702-4495" xsd:string
property_value: IAO:0000117 "Peter McQuilton" xsd:string

[Term]
id: T4FS:0000512
name: F1. (meta)data are assigned a globally unique and persistent identifier
is_a: T4FS:0000248 ! findability of digital assets
property_value: IAO:0000117 "Peter McQuilton" xsd:string

[Term]
id: T4FS:0000514
name: strategic/long-term planning
def: "An organization's process of defining its strategy or direction in the context of FAIR project management activities, both in the context of current knowledge and unknown factors in the future." [] {http://purl.obolibrary.org/obo/IAO_0000119="AL, and https://en.wikipedia.org/wiki/Strategic_planning [17.10.19]"}
is_a: T4FS:0000320 ! project management activities
property_value: IAO:0000117 "https://orcid.org/0000-0002-7702-4495" xsd:string
property_value: IAO:0000117 "Peter McQuilton" xsd:string
property_value: IAO:0000117 "Philippe Rocca-Serra" xsd:string
property_value: IAO:0000117 "Susanna Sansone" xsd:string

[Term]
id: T4FS:0000515
name: data hygiene
def: "The collective processes conducted to ensure the cleanliness of data. Data are considered clean when they are relatively error-free." [] {http://purl.obolibrary.org/obo/IAO_0000119="CASRAI. https://casrai.org/term/data-hygiene/"}
is_a: T4FS:0000036 ! curation
property_value: IAO:0000117 "Peter McQuilton" xsd:string

[Term]
id: T4FS:0000516
name: data profiling
def: "The statistical analysis and assessment of the quality of data values within a dataset for consistency, uniqueness and logic. The data profiling process cannot identify inaccurate data; it can only identify business rules violations and anomalies. The insight gained by data profiling can be used to determine how difficult it will be to use existing data for other purposes. It can also be used to provide metrics to assess data quality and help determine whether or not metadata accurately describes the source data. Profiling tools evaluate the actual content, structure and quality of the data by exploring relationships that exist between value collections both within and across datasets. For example, by examining the frequency distribution of different values for each column in a table, an analyst can gain insight into the type and use of each column. Cross-column analysis can be used to expose embedded value dependencies and inter-table analysis allows the analyst to discover overlapping value sets that represent foreign key relationships between entities." [] {http://purl.obolibrary.org/obo/IAO_0000119="CASRAI. https://casrai.org/term/data-profiling/"}
is_a: T4FS:0000352 ! data analysis
property_value: IAO:0000117 "Peter McQuilton" xsd:string

[Term]
id: T4FS:0000517
name: metadata record
def: "A collection of data defined by a theme, category, which reflects what is being measured, observed, monitored at the various sites. The Metadata Record is an information resource of business value." [] {http://purl.obolibrary.org/obo/IAO_0000119="CASRAI. https://casrai.org/term/metadata-record/"}
is_a: T4FS:0000096 ! metadata catalogue
property_value: IAO:0000117 "https://orcid.org/0000-0002-7702-4495" xsd:string
property_value: IAO:0000117 "Peter McQuilton" xsd:string

[Term]
id: T4FS:0000518
name: research data
def: "Data that are used as primary sources to support technical or scientific enquiry, research, scholarship, or artistic activity, and that are used as evidence in the research process and/or are commonly accepted in the research community as necessary to validate research findings and results. All other digital and non-digital content have the potential of becoming research data. Research data may be experimental data, observational data, operational data, third party data, public sector data, monitoring data, processed data, or repurposed data." [] {http://purl.obolibrary.org/obo/IAO_0000119="CASRAI. https://casrai.org/term/research-data"}
is_a: T4FS:0000430 ! data
property_value: IAO:0000117 "https://orcid.org/0000-0002-7702-4495" xsd:string
property_value: IAO:0000117 "Peter McQuilton" xsd:string

[Term]
id: T4FS:0000519
name: learning medium
def: "The medium through which learning has been provided. For example, through a course, slides, video presentation, online documentation, wiki pages or others." []
relationship: T4FS:0000554 T4FS:0000012 ! confers competency about data stewardship activity
relationship: T4FS:0000555 T4FS:0000372 ! confers knowledge about data stewardship technical concept
relationship: T4FS:0000556 T4FS:0000548 ! requires/improves personal attribute data stewardship soft skill
relationship: T4FS:0000557 T4FS:0000372 ! confers practical skill about data stewardship technical concept
relationship: T4FS:0000560 T4FS:0000446 ! supports implementation of data stewardship guideline
relationship: T4FS:0000576 T4FS:0000012 ! requires competency about data stewardship activity
relationship: T4FS:0000577 T4FS:0000372 ! requires knowledge about data stewardship technical concept
relationship: T4FS:0000578 T4FS:0000372 ! requires practical skill about data stewardship technical concept
property_value: IAO:0000117 "https://orcid.org/0000-0002-7702-4495" xsd:string
property_value: IAO:0000117 "Peter McQuilton" xsd:string
created_by: Peter McQuilton
creation_date: 2020-09-22T13:19:57.012225Z

[Term]
id: T4FS:0000520
name: data manager
is_a: T4FS:0000415 ! manager

[Term]
id: T4FS:0000521
name: electronic health record
def: "1. A compilation of core electronic health data submitted by various healthcare providers and organizations, accessible by numerous authorized parties from a number of points of care, possibly even from different jurisdictions. 2. An official health record for an individual that is shared among multiple facilities and agencies. 3. Electronic health records typically include: Contact information, Information about visits to health care professionals, Allergies, Insurance information, Family history, Immunization status, Information about any conditions or diseases, A list of medications, Records of hospitalization, Information about any surgeries or procedures performed. Digitized health information systems are expected to improve efficiency and quality of care and, ultimately, reduce costs. The benefits of electronic health records include: The ability to automatically share and update information among different offices and organizations, More efficient storage and retrieval, The ability to share multimedia information, such as medical imaging results, among locations, The ability to link records to sources of relevant and current research, Easier standardization of services and patient care, Provision of decision support systems (DSS) for healthcare professionals, Less redundancy of effort, Lower cost to the medical system once implementation is complete, The governments of many countries are working to ensure that all citizens have standardized electronic health records and that all records include the same types of information. The major barrier for the adoption of electronic health records is cost." [] {http://purl.obolibrary.org/obo/IAO_0000119="CASRAI. https://casrai.org/term/electronic-health-record/"}
is_a: T4FS:0000372 ! data stewardship technical concept
property_value: IAO:0000117 "https://orcid.org/0000-0002-7702-4495" xsd:string
property_value: IAO:0000117 "Peter McQuilton" xsd:string

[Term]
id: T4FS:0000522
name: data scaling
def: "Techniques used to deal with parameters having different units and scales." [] {http://purl.obolibrary.org/obo/IAO_0000119="CASRAI. https://casrai.org/term/data-scaling/"}
is_a: T4FS:0000352 ! data analysis
property_value: IAO:0000117 "https://orcid.org/0000-0002-7702-4495" xsd:string
property_value: IAO:0000117 "Peter McQuilton" xsd:string
property_value: IAO:0000118 "Data rescaling" xsd:string

[Term]
id: T4FS:0000523
name: access controls
def: "Given a data object name, access controls define access relationships between the following metadata: data object name, a user name (or user group, or user role), and access permission. The information can be stored as metadata information associated with each data object. The information can be generated dynamically by applying the access controls of the collection that organizes the data objects." [] {http://purl.obolibrary.org/obo/IAO_0000119="CASRAI. https://casrai.org/term/access-controls/"}
is_a: T4FS:0000283 ! access
property_value: IAO:0000117 "Peter McQuilton" xsd:string

[Term]
id: T4FS:0000524
name: privacy governance
def: "Monitoring the risk to privacy posed by data requests from researchers, and the practices of data custodians in providing data (information governance) to ensure that confidentiality is protected. Such governance requires specialized knowledge of technology, law, and statistical methods." [] {http://purl.obolibrary.org/obo/IAO_0000119="CASRAI. https://casrai.org/term/privacy-governance/"}
is_a: T4FS:0000472 ! governance
property_value: IAO:0000117 "https://orcid.org/0000-0002-7702-4495" xsd:string
property_value: IAO:0000117 "Peter McQuilton" xsd:string

[Term]
id: T4FS:0000525
name: research integrity, attribution, impact awareness
is_a: T4FS:0000126 ! assessment
property_value: IAO:0000117 "Angus Whyte" xsd:string
property_value: IAO:0000117 "Celia van Gelder" xsd:string
property_value: IAO:0000117 "Mateusz Kuzak" xsd:string
property_value: IAO:0000117 "Yan Wang" xsd:string

[Term]
id: T4FS:0000526
name: knowledge of cloud computing environment management
def: "Bin for types of Knowledge related to Cloud computing environment management." []
is_a: T4FS:0000479 ! cloud computing environment management
property_value: IAO:0000117 "leightonlc" xsd:string

[Term]
id: T4FS:0000527
name: metadata
def: "Literally, “data about data”; data that defines and describes the characteristics of other data, used to improve both business and technical understanding of data and data-related processes. Business metadata includes the names and business definitions of subject areas, entities and attributes, attribute data types and other attribute properties, range descriptions, valid domain values and their definitions. Technical metadata includes physical database table and column names, column properties, and the properties of other database objects, including how data is stored. Process metadata is data that defines and describes the characteristics of other system elements (processes, business rules, programs, jobs, tools, etc.). Data stewardship metadata is data about data stewards, stewardship processes and responsibility assignments." [] {http://purl.obolibrary.org/obo/IAO_0000119="CASRAI. https://casrai.org/term/metadata/"}
is_a: T4FS:0000372 ! data stewardship technical concept
relationship: T4FS:0000563 T4FS:0000199 ! contributes to the implementation of F2. data are described with rich metadata
property_value: IAO:0000117 "https://orcid.org/0000-0002-7702-4495" xsd:string
property_value: IAO:0000117 "Peter McQuilton" xsd:string
property_value: IAO:0000118 "Data documentation" xsd:string

[Term]
id: T4FS:0000528
name: comma separated values
def: "A file that contains the values in a table as a series of ASCII text lines organized so that each column value is separated by a comma from the next column's value and each row starts a new line." [] {http://purl.obolibrary.org/obo/IAO_0000119="CASRAI. https://casrai.org/term/comma-separated-values/"}
comment: Maybe remove as shouldn't have formats here.
is_a: T4FS:0000372 ! data stewardship technical concept
relationship: T4FS:0000563 T4FS:0000137 ! contributes to the implementation of I1. (meta)data use a formal, accessible, shared, and broadly applicable language for knowledge representation
property_value: IAO:0000117 "Peter McQuilton" xsd:string

[Term]
id: T4FS:0000529
name: identifier
is_a: T4FS:0000372 ! data stewardship technical concept
relationship: T4FS:0000563 T4FS:0000512 ! contributes to the implementation of F1. (meta)data are assigned a globally unique and persistent identifier
property_value: IAO:0000117 "Peter McQuilton" xsd:string

[Term]
id: T4FS:0000530
name: project team member
def: "Responsible for executing tasks and producing deliverables as outlined in the Project Plan and directed by the Project Manager, at whatever level of effort or participation has been defined for them." [] {http://purl.obolibrary.org/obo/IAO_0000119="CASRAI. https://casrai.org/term/project-team-member"}
relationship: T4FS:0000558 T4FS:0000012 ! has/wants competency in data stewardship activity
relationship: T4FS:0000559 T4FS:0000372 ! has/wants knowledge about data stewardship technical concept
relationship: T4FS:0000559 T4FS:0000446 ! has/wants knowledge about data stewardship guideline
relationship: T4FS:0000561 T4FS:0000372 ! has/wants practical skill about data stewardship technical concept
relationship: T4FS:0000562 T4FS:0000548 ! has aptitude for data stewardship soft skill
property_value: IAO:0000117 "https://orcid.org/0000-0002-7702-4495" xsd:string
property_value: IAO:0000117 "Peter McQuilton" xsd:string

[Term]
id: T4FS:0000531
name: descriptive metadata
def: "Enables identification, location, and retrieval of information resources by users, often including the use of controlled vocabularies for classification and indexing and links to related resources.REFERENCE. DCC/TC3+" [] {http://purl.obolibrary.org/obo/IAO_0000119="CASRAI. https://casrai.org/term/descriptive-metadata/"}
is_a: T4FS:0000527 ! metadata
property_value: IAO:0000117 "https://orcid.org/0000-0002-7702-4495" xsd:string
property_value: IAO:0000117 "Peter McQuilton" xsd:string
property_value: IAO:0000233 "https://github.com/terms4fairskills/FAIRterminology/issues/13" xsd:string

[Term]
id: T4FS:0000532
name: github repository
is_a: T4FS:0000519 ! learning medium
property_value: IAO:0000117 "Peter McQuilton" xsd:string
created_by: Peter McQuilton
creation_date: 2020-10-01T21:03:55.425579Z

[Term]
id: T4FS:0000533
name: data mining
def: "The process of analyzing multivariate datasets using pattern recognition or other knowledge discovery techniques to identify potentially unknown and potentially meaningful data content, relationships, classification, or trends." [] {http://purl.obolibrary.org/obo/IAO_0000119="CASRAI. https://casrai.org/term/data-mining/"}
is_a: T4FS:0000352 ! data analysis
property_value: IAO:0000117 "Peter McQuilton" xsd:string

[Term]
id: T4FS:0000534
name: data archiving
is_a: T4FS:0000156 ! archiving
property_value: IAO:0000117 "https://orcid.org/0000-0002-7702-4495" xsd:string
property_value: IAO:0000117 "Peter McQuilton" xsd:string
property_value: IAO:0000118 "Data preservation" xsd:string
created_by: Peter McQuilton
creation_date: 2021-02-17T22:18:22.641817Z

[Term]
id: T4FS:0000535
name: encoding schema
def: "Machine processable specifications which define the structure and syntax of metadata specifications in a formal schema language." [] {http://purl.obolibrary.org/obo/IAO_0000119="CASRAI. https://casrai.org/term/encoding-schema/"}
comment: AL 5.12.22 Moved from 'findability of digital assets' as it is definitely not a particular data stewardship guideline.
is_a: T4FS:0000372 ! data stewardship technical concept
property_value: IAO:0000117 "https://orcid.org/0000-0002-7702-4495" xsd:string
property_value: IAO:0000117 "Peter McQuilton" xsd:string

[Term]
id: T4FS:0000537
name: digital archiving
def: "1. In the context of library and archiving communities: Digital archiving is often used interchangeably with digital preservation. 2. In the context of computing: Digital archiving is process of backup and ongoing maintenance as opposed to strategies for long-term digital preservation." [] {http://purl.obolibrary.org/obo/IAO_0000119="CASRAI. https://casrai.org/term/digital-archiving/"}
is_a: T4FS:0000156 ! archiving
property_value: IAO:0000117 "https://orcid.org/0000-0002-7702-4495" xsd:string
property_value: IAO:0000117 "Peter McQuilton" xsd:string

[Term]
id: T4FS:0000540
name: pid resolution
def: "The process of resolving a PID to a useful state of information about a digital object by using a globally available system." [] {http://purl.obolibrary.org/obo/IAO_0000119="CASRAI. https://casrai.org/term/pid-resolution/"}
is_a: T4FS:0000453 ! persistent identifier
property_value: IAO:0000117 "https://orcid.org/0000-0002-7702-4495" xsd:string
property_value: IAO:0000117 "Peter McQuilton" xsd:string

[Term]
id: T4FS:0000541
name: skills related to storage management
def: "Bin for Skills needed for Storage management." []
is_a: T4FS:0000053 ! storage management
property_value: IAO:0000117 "leightonlc" xsd:string

[Term]
id: T4FS:0000544
name: data repository management
def: "A type of data management using repositories. It is the set of policies that govern the organization, control, and properties of the repository such as: required file formats, access control restrictions, integrity, replication, retention, disposition, etc." [] {http://purl.obolibrary.org/obo/IAO_0000119="CASRAI. https://casrai.org/term/data-repository-management/"}
is_a: T4FS:0000353 ! resource management
property_value: IAO:0000117 "https://orcid.org/0000-0002-7702-4495" xsd:string
property_value: IAO:0000117 "Peter McQuilton" xsd:string

[Term]
id: T4FS:0000546
name: darwin information typing architecture
def: "A document creation and management specification that builds content reuse into the authoring process." [] {http://purl.obolibrary.org/obo/IAO_0000119="CASRAI. https://casrai.org/term/darwin-information-typing-architecture/"}
is_a: T4FS:0000372 ! data stewardship technical concept
property_value: IAO:0000117 "Peter McQuilton" xsd:string

[Term]
id: T4FS:0000547
name: analytics
def: "The discovery of meaningful multidimensional patterns in data." [] {http://purl.obolibrary.org/obo/IAO_0000119="CASRAI. https://casrai.org/term/analytics/"}
is_a: T4FS:0000372 ! data stewardship technical concept
property_value: IAO:0000117 "Peter McQuilton" xsd:string

[Term]
id: T4FS:0000548
name: data stewardship soft skill
def: "The personal attributes necessary to perform a task." []
property_value: IAO:0000117 "Peter McQuilton" xsd:string
property_value: T4FS:0000564 "Aptitude is the innate trait or talent that a person brings to a task or situation. It is the quality of being able to do something. An aptitude is not something that can be learned or developed unless it is there to begin with." xsd:string
property_value: T4FS:0000565 "Laura Molloy, Celia van Gelder:https://docs.google.com/presentation/d/12oNBFix39ZtsLAR4tkqESBXxMU5rVg3cCKoEDG2oK-M/edit#slide=id.p5" xsd:string

[Term]
id: T4FS:0000550
name: archival documentation of data
def: "Ability to apply the FAIR principles i.e. describe the data with community metadata standard for machine and human, align with existing semantic models (ontologies, controlled vocabularies, ...), get a persistent ID, attribute licence and credit for data creators, legal aspect related to data (ownership, confidentiality, ethics, ...) add data provenance." [] {http://purl.obolibrary.org/obo/IAO_0000119="[YLF, VDA, KH]"}
is_a: T4FS:0000156 ! archiving
property_value: IAO:0000117 "https://orcid.org/0000-0002-7702-4495" xsd:string
property_value: IAO:0000117 "Kristina Hettne" xsd:string
property_value: IAO:0000117 "Victoria Dominguez Del Angel" xsd:string
property_value: IAO:0000117 "Yann Le Franc" xsd:string

[Term]
id: T4FS:0000551
name: machine-readable format
def: "A machine-readable format is a structured format that can be processed by a computer. Such formats can either be intended solely for machine processing (e.g. XML or RDF), or may be both human and machine accessible via appropriate markup (e.g. HTML)." [] {http://purl.obolibrary.org/obo/IAO_0000119="Modified by AL from Wikipedia, https://en.wikipedia.org/wiki/Machine-readable_data, accessed 6.5.22"}
comment: AL 5.12.22: Merged with now-obsolete 'machine readable' (http://purl.obolibrary.org/obo/T4FS_0000256), as we do not need that level of granularity. AL 6.5.22: The original CASRAI term (https://casrai.org/term/machine-readable-format/) has an identical source definition with 'Digital materials', and therefore has been removed.
is_a: T4FS:0000372 ! data stewardship technical concept
property_value: IAO:0000117 "https://orcid.org/0000-0002-7702-4495" xsd:string
property_value: IAO:0000117 "Peter McQuilton" xsd:string

[Term]
id: T4FS:0000552
name: confidential information
def: "Any information obtained by a person on the understanding that they will not disclose it to others, or obtained in circumstances where it is expected that they will not disclose it." [] {http://purl.obolibrary.org/obo/IAO_0000119="CASRAI. https://casrai.org/term/confidential-information/"}
is_a: T4FS:0000372 ! data stewardship technical concept
property_value: IAO:0000117 "Peter McQuilton" xsd:string

[Term]
id: T4FS:0000579
name: fair cookbook recipe
def: "The FAIR Cookbook’s recipes are a combination of guidance, technical, hands-on, background and review types to cover the operation steps of FAIR data management, and are classified according to the audience types, to serve all those involved in the data management life cycle. The FAIR Cookbook is for anyone working in the Life Sciences who needs guidance on applying the FAIR Principles in practice." [] {http://purl.obolibrary.org/obo/IAO_0000119="https://faircookbook.elixir-europe.org/content/recipes/introduction/FAIR-cookbook-audience.html"}
is_a: T4FS:0000095 ! online documentation
property_value: IAO:0000117 "https://orcid.org/0000-0002-7702-4495" xsd:string

[Term]
id: T4FS:0000580
name: evaluation indicator
def: "Evaluation indicators are designed to enable the measurement of the degree of compliance against a guideline using a set of criteria. The goals of such indicators are varied, but a good example would be to improve the re-usability of the digital asset being measured for increased discoverability, interoperability and overall machine actionability." [] {http://purl.obolibrary.org/obo/IAO_0000119="Definition by https://orcid.org/0000-0002-7702-4495 and drawn in part from https://fairplus.github.io/Data-Maturity/docs/Indicators"}
property_value: IAO:0000233 "https://github.com/terms4fairskills/FAIRterminology/issues/22" xsd:string

[Term]
id: T4FS:0000583
name: fairplus dataset maturity model indicator
def: "The fairplus dataset maturity model indicators are used within the context of the model, which is intended as a comprehensive reference model for state-of-FAIRness improvement in research datasets. Based on the FAIR guiding principles, the DSM model defines and classifies requirements that constitute an incremental path towards improving FAIRness level for a given research dataset." [] {http://purl.obolibrary.org/obo/IAO_0000119="https://fairplus.github.io/Data-Maturity/"}
is_a: T4FS:0000580 ! evaluation indicator
property_value: IAO:0000117 "https://orcid.org/0000-0002-7702-4495" xsd:string
property_value: IAO:0000118 "fairplus DSM model indicator" xsd:string

[Term]
id: T4FS:0000584
name: fairplus DSM content-related indicator
def: "The fairplus DSM content-related indicators relate to what is reported in the Dataset (data) & the Dataset Descriptor (metadata)." [] {http://purl.obolibrary.org/obo/IAO_0000119="https://fairplus.github.io/Data-Maturity/"}
is_a: T4FS:0000583 ! fairplus dataset maturity model indicator
property_value: IAO:0000117 "https://orcid.org/0000-0002-7702-4495" xsd:string

[Term]
id: T4FS:0000585
name: fairplus DSM representation and format indicator
def: "The fairplus DSM representation and format indicators relate to how the data object & metadata object are represented and formatted." [] {http://purl.obolibrary.org/obo/IAO_0000119="https://fairplus.github.io/Data-Maturity/"}
comment: AL 5.12.22: Please note that the 'and' in this label is a direct representation of the fairplus DSM model, and not a ontological design choice.
is_a: T4FS:0000583 ! fairplus dataset maturity model indicator
property_value: IAO:0000117 "https://orcid.org/0000-0002-7702-4495" xsd:string

[Term]
id: T4FS:0000586
name: fairplus DSM hosting-environment capabilities indicator
def: "The fairplus DSM hosting-environment capabilities indicator relate to the capabilities of the hosting environment that enables and supports the use of FAIR data" [] {http://purl.obolibrary.org/obo/IAO_0000119="https://fairplus.github.io/Data-Maturity/"}
is_a: T4FS:0000583 ! fairplus dataset maturity model indicator
property_value: IAO:0000117 "https://orcid.org/0000-0002-7702-4495" xsd:string

[Term]
id: T4FS:0000587
name: DSM-0-R2
def: "No representation of Data purposed for FAIR sharing is available" [] {http://purl.obolibrary.org/obo/IAO_0000119="https://fairplus.github.io/Data-Maturity/docs/Indicators/"}
is_a: T4FS:0000585 ! fairplus DSM representation and format indicator
property_value: IAO:0000117 "https://orcid.org/0000-0002-7702-4495" xsd:string

[Term]
id: T4FS:0000588
name: DSM-1-R2
def: "Structured and/or Unstructured Data are organised into Dataset(s) created for the purpose of FAIR sharing" [] {http://purl.obolibrary.org/obo/IAO_0000119="https://fairplus.github.io/Data-Maturity/docs/Indicators/"}
is_a: T4FS:0000585 ! fairplus DSM representation and format indicator
property_value: IAO:0000117 "https://orcid.org/0000-0002-7702-4495" xsd:string

[Term]
id: T4FS:0000589
name: DSM-2-R2
def: "Project collected Data are organized into structured Dataset(s) and conform to a locally defined Dataset Model" [] {http://purl.obolibrary.org/obo/IAO_0000119="https://fairplus.github.io/Data-Maturity/docs/Indicators/"}
is_a: T4FS:0000585 ! fairplus DSM representation and format indicator
property_value: IAO:0000117 "https://orcid.org/0000-0002-7702-4495" xsd:string

[Term]
id: T4FS:0000590
name: DSM-3-R2
def: "Structured Data are represented as Datasets and conform to relevant Standard Dataset Model(s) for FAIR sharing" [] {http://purl.obolibrary.org/obo/IAO_0000119="https://fairplus.github.io/Data-Maturity/docs/Indicators/"}
is_a: T4FS:0000585 ! fairplus DSM representation and format indicator
property_value: IAO:0000117 "https://orcid.org/0000-0002-7702-4495" xsd:string

[Term]
id: T4FS:0000591
name: DSM-4-R2
def: "Dataset(s) content is semantically represented using Linked Data Represetations conforming to a Semantic Data Model" [] {http://purl.obolibrary.org/obo/IAO_0000119="https://fairplus.github.io/Data-Maturity/docs/Indicators/"}
is_a: T4FS:0000585 ! fairplus DSM representation and format indicator
property_value: IAO:0000117 "https://orcid.org/0000-0002-7702-4495" xsd:string

[Term]
id: T4FS:0000592
name: DSM-5-R2
def: "Dataset(s) are granularly represented and managed at the Data Element Level (e.g. ISO 11179 MDR standard)" [] {http://purl.obolibrary.org/obo/IAO_0000119="https://fairplus.github.io/Data-Maturity/docs/Indicators/"}
is_a: T4FS:0000585 ! fairplus DSM representation and format indicator
property_value: IAO:0000117 "https://orcid.org/0000-0002-7702-4495" xsd:string

[Term]
id: T4FS:0000593
name: DSM-0-R3
def: "Dataset Metadata is NOT formally represented in a structured Dataset Descriptor" [] {http://purl.obolibrary.org/obo/IAO_0000119="https://fairplus.github.io/Data-Maturity/docs/Indicators/"}
is_a: T4FS:0000585 ! fairplus DSM representation and format indicator
property_value: IAO:0000117 "https://orcid.org/0000-0002-7702-4495" xsd:string

[Term]
id: T4FS:0000594
name: DSM-1-R0
def: "Dataset Metadata is formally represented in the form of an Identifiable Dataset Descriptor" [] {http://purl.obolibrary.org/obo/IAO_0000119="https://fairplus.github.io/Data-Maturity/docs/Indicators/"}
is_a: T4FS:0000585 ! fairplus DSM representation and format indicator
property_value: IAO:0000117 "https://orcid.org/0000-0002-7702-4495" xsd:string

[Term]
id: T4FS:0000595
name: DSM-1-R3
def: "A representation of the Dataset Descriptor conforming to a relevant General Purpose Metadata Schema is available" [] {http://purl.obolibrary.org/obo/IAO_0000119="https://fairplus.github.io/Data-Maturity/docs/Indicators/"}
is_a: T4FS:0000585 ! fairplus DSM representation and format indicator
property_value: IAO:0000117 "https://orcid.org/0000-0002-7702-4495" xsd:string

[Term]
id: T4FS:0000596
name: DSM-2-R3
def: "Dataset Descriptor(s) conforms to or extends a Standard Generic Dataset Descriptor Model to describe and represent structural metadata of Dataset(s)" [] {http://purl.obolibrary.org/obo/IAO_0000119="https://fairplus.github.io/Data-Maturity/docs/Indicators/"}
is_a: T4FS:0000585 ! fairplus DSM representation and format indicator
property_value: IAO:0000117 "https://orcid.org/0000-0002-7702-4495" xsd:string

[Term]
id: T4FS:0000597
name: DSM-3-R3
def: "Dataset Descriptor(s) use community-defined or domain-specific metadata standard" [] {http://purl.obolibrary.org/obo/IAO_0000119="https://fairplus.github.io/Data-Maturity/docs/Indicators/"}
is_a: T4FS:0000585 ! fairplus DSM representation and format indicator
relationship: T4FS:0000581 T4FS:0000391 ! confers compliance with R1.3 (meta)data meet domain-relevant community standards
property_value: IAO:0000117 "https://orcid.org/0000-0002-7702-4495" xsd:string

[Term]
id: T4FS:0000598
name: DSM-4-R3
def: "A Semantic Data Model (Metadata) used for data harmonisation across Datasets is formally defined and represented using Linked Data Representations" [] {http://purl.obolibrary.org/obo/IAO_0000119="https://fairplus.github.io/Data-Maturity/docs/Indicators/"}
is_a: T4FS:0000585 ! fairplus DSM representation and format indicator
relationship: T4FS:0000581 T4FS:0000137 ! confers compliance with I1. (meta)data use a formal, accessible, shared, and broadly applicable language for knowledge representation
property_value: IAO:0000117 "https://orcid.org/0000-0002-7702-4495" xsd:string

[Term]
id: T4FS:0000599
name: DSM-5-R3
def: "Common Data Elements and their value sets are defined and registered in a managed Metadata Registry" [] {http://purl.obolibrary.org/obo/IAO_0000119="https://fairplus.github.io/Data-Maturity/docs/Indicators/"}
is_a: T4FS:0000585 ! fairplus DSM representation and format indicator
property_value: IAO:0000117 "https://orcid.org/0000-0002-7702-4495" xsd:string

[Term]
id: T4FS:0000600
name: DSM-0-R1
def: "Contextual Metadata is NOT formally represented in any form" [] {http://purl.obolibrary.org/obo/IAO_0000119="https://fairplus.github.io/Data-Maturity/docs/Indicators/"}
is_a: T4FS:0000585 ! fairplus DSM representation and format indicator
property_value: IAO:0000117 "https://orcid.org/0000-0002-7702-4495" xsd:string

[Term]
id: T4FS:0000601
name: DSM-1-R1
def: "Contextual Metadata is reported at summary level and represented in the Dataset Descriptor" [] {http://purl.obolibrary.org/obo/IAO_0000119="https://fairplus.github.io/Data-Maturity/docs/Indicators/"}
is_a: T4FS:0000585 ! fairplus DSM representation and format indicator
property_value: IAO:0000117 "https://orcid.org/0000-0002-7702-4495" xsd:string

[Term]
id: T4FS:0000602
name: DSM-2-R1
def: "Contextual Metadata is formally represented in the form of a locally defined Domain Model" [] {http://purl.obolibrary.org/obo/IAO_0000119="https://fairplus.github.io/Data-Maturity/docs/Indicators/"}
is_a: T4FS:0000585 ! fairplus DSM representation and format indicator
property_value: IAO:0000117 "https://orcid.org/0000-0002-7702-4495" xsd:string

[Term]
id: T4FS:0000603
name: DSM-3-R1
def: "Contextual Metadata is formally represented and conforms to a standard defined Domain Model if available" [] {http://purl.obolibrary.org/obo/IAO_0000119="https://fairplus.github.io/Data-Maturity/docs/Indicators/"}
is_a: T4FS:0000585 ! fairplus DSM representation and format indicator
property_value: IAO:0000117 "https://orcid.org/0000-0002-7702-4495" xsd:string

[Term]
id: T4FS:0000604
name: DSM-4-R1
def: "Contextual Metadata is formally represented by a defined set Common Data Elements" [] {http://purl.obolibrary.org/obo/IAO_0000119="https://fairplus.github.io/Data-Maturity/docs/Indicators/"}
is_a: T4FS:0000585 ! fairplus DSM representation and format indicator
property_value: IAO:0000117 "https://orcid.org/0000-0002-7702-4495" xsd:string

[Term]
id: T4FS:0000605
name: DSM-5-R1
def: "Domain entities are represented by Managed Master Data Objects conforming to a Master Data Model used for data consolidation" [] {http://purl.obolibrary.org/obo/IAO_0000119="https://fairplus.github.io/Data-Maturity/docs/Indicators/"}
is_a: T4FS:0000585 ! fairplus DSM representation and format indicator
property_value: IAO:0000117 "https://orcid.org/0000-0002-7702-4495" xsd:string

[Term]
id: T4FS:0000606
name: DSM-0-R4
def: "Dataset Descriptor (metadata) is NOT available in a Machine Readable Format" [] {http://purl.obolibrary.org/obo/IAO_0000119="https://fairplus.github.io/Data-Maturity/docs/Indicators/"}
is_a: T4FS:0000585 ! fairplus DSM representation and format indicator
property_value: IAO:0000117 "https://orcid.org/0000-0002-7702-4495" xsd:string

[Term]
id: T4FS:0000607
name: DSM-1-R4
def: "Dataset Descriptor is available in Machine Readable Format" [] {http://purl.obolibrary.org/obo/IAO_0000119="https://fairplus.github.io/Data-Maturity/docs/Indicators/"}
is_a: T4FS:0000585 ! fairplus DSM representation and format indicator
property_value: IAO:0000117 "https://orcid.org/0000-0002-7702-4495" xsd:string

[Term]
id: T4FS:0000608
name: DSM-2-R4
def: "Contextual Metadata represented in the form of a Domain Model is available in a Human Readable Format" [] {http://purl.obolibrary.org/obo/IAO_0000119="https://fairplus.github.io/Data-Maturity/docs/Indicators/"}
is_a: T4FS:0000585 ! fairplus DSM representation and format indicator
property_value: IAO:0000117 "https://orcid.org/0000-0002-7702-4495" xsd:string

[Term]
id: T4FS:0000609
name: DSM-3-R4
def: "A formal documentation of the adopted Standard Dataset Model is available in a Machine Readable Format" [] {http://purl.obolibrary.org/obo/IAO_0000119="https://fairplus.github.io/Data-Maturity/docs/Indicators/"}
is_a: T4FS:0000585 ! fairplus DSM representation and format indicator
property_value: IAO:0000117 "https://orcid.org/0000-0002-7702-4495" xsd:string

[Term]
id: T4FS:0000610
name: DSM-4-R4
def: "A Semantic Data Model (Metadata) describing the data is represented in a Machine Readable and Machine Interptretable format" [] {http://purl.obolibrary.org/obo/IAO_0000119="https://fairplus.github.io/Data-Maturity/docs/Indicators/"}
is_a: T4FS:0000585 ! fairplus DSM representation and format indicator
property_value: IAO:0000117 "https://orcid.org/0000-0002-7702-4495" xsd:string

[Term]
id: T4FS:0000611
name: DSM-0-R5
def: "Dataset(s) are NOT available in a Machine Readable Format" [] {http://purl.obolibrary.org/obo/IAO_0000119="https://fairplus.github.io/Data-Maturity/docs/Indicators/"}
is_a: T4FS:0000585 ! fairplus DSM representation and format indicator
property_value: IAO:0000117 "https://orcid.org/0000-0002-7702-4495" xsd:string

[Term]
id: T4FS:0000612
name: DSM-1-R5
def: "Dataset(s) available in Machine Readable Format" [] {http://purl.obolibrary.org/obo/IAO_0000119="https://fairplus.github.io/Data-Maturity/docs/Indicators/"}
is_a: T4FS:0000585 ! fairplus DSM representation and format indicator
property_value: IAO:0000117 "https://orcid.org/0000-0002-7702-4495" xsd:string

[Term]
id: T4FS:0000613
name: DSM-3-R5
def: "If applicable, Dataset(s) available in non-proprietary Machine Readable Format relevant to the adopted standard Dataset Model" [] {http://purl.obolibrary.org/obo/IAO_0000119="https://fairplus.github.io/Data-Maturity/docs/Indicators/"}
is_a: T4FS:0000585 ! fairplus DSM representation and format indicator
property_value: IAO:0000117 "https://orcid.org/0000-0002-7702-4495" xsd:string

[Term]
id: T4FS:0000614
name: DSM-4-R5
def: "Datasets are available in a Machine Readable and Machine Interpretable format" [] {http://purl.obolibrary.org/obo/IAO_0000119="https://fairplus.github.io/Data-Maturity/docs/Indicators/"}
is_a: T4FS:0000585 ! fairplus DSM representation and format indicator
property_value: IAO:0000117 "https://orcid.org/0000-0002-7702-4495" xsd:string

[Term]
id: T4FS:0000615
name: DSM-4-R6
def: "If applicable, license information and/or permitted use and accessability to parts of the dataset is formally represented and encoded in a Machine Readable Format" [] {http://purl.obolibrary.org/obo/IAO_0000119="https://fairplus.github.io/Data-Maturity/docs/Indicators/"}
is_a: T4FS:0000585 ! fairplus DSM representation and format indicator
relationship: T4FS:0000581 T4FS:0000200 ! confers compliance with R1.1 (meta)data are released with a clear and accessible data usage license
property_value: IAO:0000117 "https://orcid.org/0000-0002-7702-4495" xsd:string

[Term]
id: T4FS:0000616
name: DSM-0-C0
def: "Dataset(s) are NOT Identifiable via Unique Identifiers" [] {http://purl.obolibrary.org/obo/IAO_0000119="https://fairplus.github.io/Data-Maturity/docs/Indicators/"}
is_a: T4FS:0000584 ! fairplus DSM content-related indicator
property_value: IAO:0000117 "https://orcid.org/0000-0002-7702-4495" xsd:string

[Term]
id: T4FS:0000617
name: DSM-1-C0
def: "Each Dataset purposed for FAIR sharing is assigned a unique identifier" [] {http://purl.obolibrary.org/obo/IAO_0000119="https://fairplus.github.io/Data-Maturity/docs/Indicators/"}
is_a: T4FS:0000584 ! fairplus DSM content-related indicator
relationship: T4FS:0000581 T4FS:0000512 ! confers compliance with F1. (meta)data are assigned a globally unique and persistent identifier
property_value: IAO:0000117 "https://orcid.org/0000-0002-7702-4495" xsd:string

[Term]
id: T4FS:0000618
name: DSM-2-C2
def: "Where applicable, data is structured in the Dataset according to the Tidy Data Principles" [] {http://purl.obolibrary.org/obo/IAO_0000119="https://fairplus.github.io/Data-Maturity/docs/Indicators/"}
is_a: T4FS:0000584 ! fairplus DSM content-related indicator
relationship: T4FS:0000581 T4FS:0000174 ! confers compliance with R1. (meta)data are richly described with a plurality of accurate and relevant attributes
property_value: IAO:0000117 "https://orcid.org/0000-0002-7702-4495" xsd:string

[Term]
id: T4FS:0000619
name: DSM-3-C2
def: "Where applicable, Dataset(s) scope and content are reported in compliance with relevant community-defined Data Reporting Guidelines" [] {http://purl.obolibrary.org/obo/IAO_0000119="https://fairplus.github.io/Data-Maturity/docs/Indicators/"}
is_a: T4FS:0000584 ! fairplus DSM content-related indicator
relationship: T4FS:0000581 T4FS:0000391 ! confers compliance with R1.3 (meta)data meet domain-relevant community standards
property_value: IAO:0000117 "https://orcid.org/0000-0002-7702-4495" xsd:string

[Term]
id: T4FS:0000620
name: DSM-4-C2
def: "Dataset(s) content is harmonised against a designed-for-purpose Semantic Data Model" [] {http://purl.obolibrary.org/obo/IAO_0000119="https://fairplus.github.io/Data-Maturity/docs/Indicators/"}
is_a: T4FS:0000584 ! fairplus DSM content-related indicator
relationship: T4FS:0000581 T4FS:0000137 ! confers compliance with I1. (meta)data use a formal, accessible, shared, and broadly applicable language for knowledge representation
property_value: IAO:0000117 "https://orcid.org/0000-0002-7702-4495" xsd:string

[Term]
id: T4FS:0000621
name: DSM-2-C3
def: "Dataset(s) include Reference Fields that enable joining related datasets" [] {http://purl.obolibrary.org/obo/IAO_0000119="https://fairplus.github.io/Data-Maturity/docs/Indicators/"}
is_a: T4FS:0000584 ! fairplus DSM content-related indicator
relationship: T4FS:0000581 T4FS:0000452 ! confers compliance with I3. (meta)data include qualified references to other (meta)data
property_value: IAO:0000117 "https://orcid.org/0000-0002-7702-4495" xsd:string

[Term]
id: T4FS:0000622
name: DSM-3-C3
def: "Where applicable, Dataset Field Names use standard controlled terms as recommended by the adopted Standard" [] {http://purl.obolibrary.org/obo/IAO_0000119="https://fairplus.github.io/Data-Maturity/docs/Indicators/"}
is_a: T4FS:0000584 ! fairplus DSM content-related indicator
relationship: T4FS:0000581 T4FS:0000137 ! confers compliance with I1. (meta)data use a formal, accessible, shared, and broadly applicable language for knowledge representation
property_value: IAO:0000117 "https://orcid.org/0000-0002-7702-4495" xsd:string

[Term]
id: T4FS:0000623
name: DSM-4-C3
def: "Key Dataset Fields are mapped to Common Data Elements as defined by the Semantic Data Model" [] {http://purl.obolibrary.org/obo/IAO_0000119="https://fairplus.github.io/Data-Maturity/docs/Indicators/"}
is_a: T4FS:0000584 ! fairplus DSM content-related indicator
property_value: IAO:0000117 "https://orcid.org/0000-0002-7702-4495" xsd:string

[Term]
id: T4FS:0000624
name: DSM-5-C3
def: "Dataset Fields are linked and harmonized against enterprise managed Metadata Elements (e.g. MDR registered Data Elements)" [] {http://purl.obolibrary.org/obo/IAO_0000119="https://fairplus.github.io/Data-Maturity/docs/Indicators/"}
is_a: T4FS:0000584 ! fairplus DSM content-related indicator
property_value: IAO:0000117 "https://orcid.org/0000-0002-7702-4495" xsd:string

[Term]
id: T4FS:0000625
name: DSM-2-C4
def: "Where applicable, Dataset Field Values are standardized against a locally defined Data Dictionary within and across related Datasets" [] {http://purl.obolibrary.org/obo/IAO_0000119="https://fairplus.github.io/Data-Maturity/docs/Indicators/"}
is_a: T4FS:0000584 ! fairplus DSM content-related indicator
relationship: T4FS:0000581 T4FS:0000174 ! confers compliance with R1. (meta)data are richly described with a plurality of accurate and relevant attributes
relationship: T4FS:0000581 T4FS:0000199 ! confers compliance with F2. data are described with rich metadata
property_value: IAO:0000117 "https://orcid.org/0000-0002-7702-4495" xsd:string

[Term]
id: T4FS:0000626
name: DSM-3-C4
def: "Where applicable, Dataset Field Values are standardised against domain-specific Controlled Terminologies and/or Ontology Terms" [] {http://purl.obolibrary.org/obo/IAO_0000119="https://fairplus.github.io/Data-Maturity/docs/Indicators/"}
is_a: T4FS:0000584 ! fairplus DSM content-related indicator
relationship: T4FS:0000581 T4FS:0000361 ! confers compliance with I2. (meta)data use vocabularies that follow fair principles
relationship: T4FS:0000581 T4FS:0000391 ! confers compliance with R1.3 (meta)data meet domain-relevant community standards
property_value: IAO:0000117 "https://orcid.org/0000-0002-7702-4495" xsd:string

[Term]
id: T4FS:0000627
name: DSM-4-C4
def: "Values for key Domain Entities reported in the Dataset(s) are standardised and assigned unique Standard Identifiers" [] {http://purl.obolibrary.org/obo/IAO_0000119="https://fairplus.github.io/Data-Maturity/docs/Indicators/"}
is_a: T4FS:0000584 ! fairplus DSM content-related indicator
relationship: T4FS:0000581 T4FS:0000435 ! confers compliance with F3. metadata clearly and explicitly include the identifier of the data they describe
property_value: IAO:0000117 "https://orcid.org/0000-0002-7702-4495" xsd:string

[Term]
id: T4FS:0000628
name: DSM-5-C4
def: "Dataset Field values are controlled and managed via enterprise managed Reference and Master Data" [] {http://purl.obolibrary.org/obo/IAO_0000119="https://fairplus.github.io/Data-Maturity/docs/Indicators/"}
is_a: T4FS:0000584 ! fairplus DSM content-related indicator
property_value: IAO:0000117 "https://orcid.org/0000-0002-7702-4495" xsd:string

[Term]
id: T4FS:0000629
name: DSM-0-C1
def: "Study/Project-Level metadata is NOT reported" [] {http://purl.obolibrary.org/obo/IAO_0000119="https://fairplus.github.io/Data-Maturity/docs/Indicators/"}
is_a: T4FS:0000584 ! fairplus DSM content-related indicator
property_value: IAO:0000117 "https://orcid.org/0000-0002-7702-4495" xsd:string

[Term]
id: T4FS:0000630
name: DSM-1-C1
def: "Dataset Descriptor includes Descriptive Study/Project-Level summary information" [] {http://purl.obolibrary.org/obo/IAO_0000119="https://fairplus.github.io/Data-Maturity/docs/Indicators/"}
is_a: T4FS:0000584 ! fairplus DSM content-related indicator
relationship: T4FS:0000581 T4FS:0000174 ! confers compliance with R1. (meta)data are richly described with a plurality of accurate and relevant attributes
relationship: T4FS:0000581 T4FS:0000199 ! confers compliance with F2. data are described with rich metadata
property_value: IAO:0000117 "https://orcid.org/0000-0002-7702-4495" xsd:string

[Term]
id: T4FS:0000631
name: DSM-2-C1
def: "A locally defined Domain Model contains concepts that describes the overall project/study design, the relationships between the Datasets, the key entities reported within the Datasets and the relationships between them." [] {http://purl.obolibrary.org/obo/IAO_0000119="https://fairplus.github.io/Data-Maturity/docs/Indicators/"}
is_a: T4FS:0000584 ! fairplus DSM content-related indicator
relationship: T4FS:0000581 T4FS:0000174 ! confers compliance with R1. (meta)data are richly described with a plurality of accurate and relevant attributes
property_value: IAO:0000117 "https://orcid.org/0000-0002-7702-4495" xsd:string

[Term]
id: T4FS:0000632
name: DSM-3-C1
def: "Where applicable, study-level / experimental metadata is reported in compliance with relevant Minimum Information Reporting Guidelines" [] {http://purl.obolibrary.org/obo/IAO_0000119="https://fairplus.github.io/Data-Maturity/docs/Indicators/"}
is_a: T4FS:0000584 ! fairplus DSM content-related indicator
relationship: T4FS:0000581 T4FS:0000391 ! confers compliance with R1.3 (meta)data meet domain-relevant community standards
property_value: IAO:0000117 "https://orcid.org/0000-0002-7702-4495" xsd:string

[Term]
id: T4FS:0000633
name: DSM-4-C1
def: "A Semantic Data Model includes study design Data Elements and the relationships between them" [] {http://purl.obolibrary.org/obo/IAO_0000119="https://fairplus.github.io/Data-Maturity/docs/Indicators/"}
is_a: T4FS:0000372 ! data stewardship technical concept
is_a: T4FS:0000584 ! fairplus DSM content-related indicator
relationship: T4FS:0000563 T4FS:0000137 ! contributes to the implementation of I1. (meta)data use a formal, accessible, shared, and broadly applicable language for knowledge representation
relationship: T4FS:0000581 T4FS:0000199 ! confers compliance with F2. data are described with rich metadata
property_value: IAO:0000117 "https://orcid.org/0000-0002-7702-4495" xsd:string

[Term]
id: T4FS:0000634
name: DSM-0-C2
def: "Dataset Descriptor does NOT include a reference to the Dataset it describes" [] {http://purl.obolibrary.org/obo/IAO_0000119="https://fairplus.github.io/Data-Maturity/docs/Indicators/"}
is_a: T4FS:0000584 ! fairplus DSM content-related indicator
property_value: IAO:0000117 "https://orcid.org/0000-0002-7702-4495" xsd:string

[Term]
id: T4FS:0000635
name: DSM-1-C2
def: "Dataset Descriptor includes Identifying & Descriptive Dataset-Level metadata" [] {http://purl.obolibrary.org/obo/IAO_0000119="https://fairplus.github.io/Data-Maturity/docs/Indicators/"}
is_a: T4FS:0000584 ! fairplus DSM content-related indicator
relationship: T4FS:0000581 T4FS:0000174 ! confers compliance with R1. (meta)data are richly described with a plurality of accurate and relevant attributes
relationship: T4FS:0000581 T4FS:0000435 ! confers compliance with F3. metadata clearly and explicitly include the identifier of the data they describe
property_value: IAO:0000117 "https://orcid.org/0000-0002-7702-4495" xsd:string

[Term]
id: T4FS:0000636
name: DSM-1-C3
def: "Dataset Descriptor contains access information for the Dataset" [] {http://purl.obolibrary.org/obo/IAO_0000119="https://fairplus.github.io/Data-Maturity/docs/Indicators/"}
is_a: T4FS:0000584 ! fairplus DSM content-related indicator
relationship: T4FS:0000581 T4FS:0000038 ! confers compliance with A1. (meta)data are retrievable by their identifier using a standardised communications protocol
property_value: IAO:0000117 "https://orcid.org/0000-0002-7702-4495" xsd:string

[Term]
id: T4FS:0000637
name: DSM-2-C5
def: "Dataset Descriptor includes reference to related Datasets and if applicable the relevant joining Dataset Fields" [] {http://purl.obolibrary.org/obo/IAO_0000119="https://fairplus.github.io/Data-Maturity/docs/Indicators/"}
is_a: T4FS:0000584 ! fairplus DSM content-related indicator
property_value: IAO:0000117 "https://orcid.org/0000-0002-7702-4495" xsd:string

[Term]
id: T4FS:0000638
name: DSM-3-C7
def: "Dataset Descriptor references a standard license under which the dataset can be re-used." [] {http://purl.obolibrary.org/obo/IAO_0000119="https://fairplus.github.io/Data-Maturity/docs/Indicators/"}
is_a: T4FS:0000584 ! fairplus DSM content-related indicator
relationship: T4FS:0000581 T4FS:0000199 ! confers compliance with F2. data are described with rich metadata
property_value: IAO:0000117 "https://orcid.org/0000-0002-7702-4495" xsd:string

[Term]
id: T4FS:0000639
name: DSM-2-C6
def: "Dataset Descriptor includes Field-level Metadata as prescribed by a locally defined Dataset Model" [] {http://purl.obolibrary.org/obo/IAO_0000119="https://fairplus.github.io/Data-Maturity/docs/Indicators/"}
is_a: T4FS:0000584 ! fairplus DSM content-related indicator
relationship: T4FS:0000581 T4FS:0000174 ! confers compliance with R1. (meta)data are richly described with a plurality of accurate and relevant attributes
relationship: T4FS:0000581 T4FS:0000199 ! confers compliance with F2. data are described with rich metadata
property_value: IAO:0000117 "https://orcid.org/0000-0002-7702-4495" xsd:string

[Term]
id: T4FS:0000640
name: DSM-3-C6
def: "Dataset Descriptor includes standard-compliant Field-level Metadata as prescribed by the adopted standard Dataset Model." [] {http://purl.obolibrary.org/obo/IAO_0000119="https://fairplus.github.io/Data-Maturity/docs/Indicators/"}
is_a: T4FS:0000584 ! fairplus DSM content-related indicator
property_value: IAO:0000117 "https://orcid.org/0000-0002-7702-4495" xsd:string

[Term]
id: T4FS:0000641
name: DSM-4-C5
def: "The Semantic Data Model includes a pre-defined set of Common Data Elements reported within the Datasets and the relationships between them" [] {http://purl.obolibrary.org/obo/IAO_0000119="https://fairplus.github.io/Data-Maturity/docs/Indicators/"}
is_a: T4FS:0000584 ! fairplus DSM content-related indicator
relationship: T4FS:0000581 T4FS:0000199 ! confers compliance with F2. data are described with rich metadata
property_value: IAO:0000117 "https://orcid.org/0000-0002-7702-4495" xsd:string

[Term]
id: T4FS:0000642
name: DSM-2-C7
def: "Dataset Descriptor includes Value-level Metadata or if applicable includes a reference to a locally defined Data Dictionary" [] {http://purl.obolibrary.org/obo/IAO_0000119="https://fairplus.github.io/Data-Maturity/docs/Indicators/"}
is_a: T4FS:0000584 ! fairplus DSM content-related indicator
relationship: T4FS:0000581 T4FS:0000174 ! confers compliance with R1. (meta)data are richly described with a plurality of accurate and relevant attributes
relationship: T4FS:0000581 T4FS:0000199 ! confers compliance with F2. data are described with rich metadata
property_value: IAO:0000117 "https://orcid.org/0000-0002-7702-4495" xsd:string

[Term]
id: T4FS:0000643
name: DSM-3-C5
def: "Value Level Metadata includes Resolvable Identifiers for Controlled and/or Standard Terms reported in the Dataset" [] {http://purl.obolibrary.org/obo/IAO_0000119="https://fairplus.github.io/Data-Maturity/docs/Indicators/"}
is_a: T4FS:0000584 ! fairplus DSM content-related indicator
relationship: T4FS:0000581 T4FS:0000038 ! confers compliance with A1. (meta)data are retrievable by their identifier using a standardised communications protocol
relationship: T4FS:0000581 T4FS:0000199 ! confers compliance with F2. data are described with rich metadata
relationship: T4FS:0000581 T4FS:0000361 ! confers compliance with I2. (meta)data use vocabularies that follow fair principles
relationship: T4FS:0000581 T4FS:0000435 ! confers compliance with F3. metadata clearly and explicitly include the identifier of the data they describe
relationship: T4FS:0000581 T4FS:0000452 ! confers compliance with I3. (meta)data include qualified references to other (meta)data
property_value: IAO:0000117 "https://orcid.org/0000-0002-7702-4495" xsd:string

[Term]
id: T4FS:0000644
name: DSM-0-H1
def: "Data or metadata is hosted in non-accessible storage (e.g., personal desktop, local file system or archive)" [] {http://purl.obolibrary.org/obo/IAO_0000119="https://fairplus.github.io/Data-Maturity/docs/Indicators/"}
is_a: T4FS:0000586 ! fairplus DSM hosting-environment capabilities indicator
property_value: IAO:0000117 "https://orcid.org/0000-0002-7702-4495" xsd:string

[Term]
id: T4FS:0000645
name: DSM-1-H1
def: "Metadata hosting environment stores and maintains an identifiable Dataset Descriptor for each identifiable Dataset" [] {http://purl.obolibrary.org/obo/IAO_0000119="https://fairplus.github.io/Data-Maturity/docs/Indicators/"}
is_a: T4FS:0000586 ! fairplus DSM hosting-environment capabilities indicator
relationship: T4FS:0000581 T4FS:0000038 ! confers compliance with A1. (meta)data are retrievable by their identifier using a standardised communications protocol
relationship: T4FS:0000581 T4FS:0000435 ! confers compliance with F3. metadata clearly and explicitly include the identifier of the data they describe
property_value: IAO:0000117 "https://orcid.org/0000-0002-7702-4495" xsd:string

[Term]
id: T4FS:0000646
name: DSM-2-H1
def: "The Data hosting environment's Persistence Model is aligned with a locally defined Domain Model to enable interpretation of Datasets" [] {http://purl.obolibrary.org/obo/IAO_0000119="https://fairplus.github.io/Data-Maturity/docs/Indicators/"}
is_a: T4FS:0000586 ! fairplus DSM hosting-environment capabilities indicator
relationship: T4FS:0000581 T4FS:0000174 ! confers compliance with R1. (meta)data are richly described with a plurality of accurate and relevant attributes
property_value: IAO:0000117 "https://orcid.org/0000-0002-7702-4495" xsd:string

[Term]
id: T4FS:0000647
name: DSM-3-H1
def: "The Data hosting environment's Persistence Model is aligned with a standard Dataset model or compliant with relevant Minimum Information Reporting Guidelines" [] {http://purl.obolibrary.org/obo/IAO_0000119="https://fairplus.github.io/Data-Maturity/docs/Indicators/"}
is_a: T4FS:0000586 ! fairplus DSM hosting-environment capabilities indicator
relationship: T4FS:0000581 T4FS:0000391 ! confers compliance with R1.3 (meta)data meet domain-relevant community standards
property_value: IAO:0000117 "https://orcid.org/0000-0002-7702-4495" xsd:string

[Term]
id: T4FS:0000648
name: DSM-4-H1
def: "Data Hosting environment stores data in a relevant linked data store (e.g., Triple Store or Graph Databaase)" [] {http://purl.obolibrary.org/obo/IAO_0000119="https://fairplus.github.io/Data-Maturity/docs/Indicators/"}
is_a: T4FS:0000586 ! fairplus DSM hosting-environment capabilities indicator
property_value: IAO:0000117 "https://orcid.org/0000-0002-7702-4495" xsd:string

[Term]
id: T4FS:0000649
name: DSM-0-H2
def: "Data or metadata hosted in an accessible resource but with no retrieval capability" [] {http://purl.obolibrary.org/obo/IAO_0000119="https://fairplus.github.io/Data-Maturity/docs/Indicators/"}
is_a: T4FS:0000586 ! fairplus DSM hosting-environment capabilities indicator
property_value: IAO:0000117 "https://orcid.org/0000-0002-7702-4495" xsd:string

[Term]
id: T4FS:0000650
name: DSM-1-H2
def: "The Dataset and its Descriptor are indexed and retrievable (in the same or separate hosting environments) via unique and persistent identifiers" [] {http://purl.obolibrary.org/obo/IAO_0000119="https://fairplus.github.io/Data-Maturity/docs/Indicators/"}
is_a: T4FS:0000586 ! fairplus DSM hosting-environment capabilities indicator
relationship: T4FS:0000581 T4FS:0000038 ! confers compliance with A1. (meta)data are retrievable by their identifier using a standardised communications protocol
property_value: IAO:0000117 "https://orcid.org/0000-0002-7702-4495" xsd:string

[Term]
id: T4FS:0000651
name: DSM-1-H3
def: "Retrieval of the Dataset and the Dataset Descriptor utilises a standardized communication protocol that is open, free and universally implementable" [] {http://purl.obolibrary.org/obo/IAO_0000119="https://fairplus.github.io/Data-Maturity/docs/Indicators/"}
is_a: T4FS:0000586 ! fairplus DSM hosting-environment capabilities indicator
relationship: T4FS:0000581 T4FS:0000103 ! confers compliance with A1.1 the protocol is open, free, and universally implementable
property_value: IAO:0000117 "https://orcid.org/0000-0002-7702-4495" xsd:string

[Term]
id: T4FS:0000652
name: DSM-2-H2
def: "Metadata hosting environment provides programmatic access and retrieval (API) for the Dataset Descriptor" [] {http://purl.obolibrary.org/obo/IAO_0000119="https://fairplus.github.io/Data-Maturity/docs/Indicators/"}
is_a: T4FS:0000586 ! fairplus DSM hosting-environment capabilities indicator
relationship: T4FS:0000581 T4FS:0000038 ! confers compliance with A1. (meta)data are retrievable by their identifier using a standardised communications protocol
property_value: IAO:0000117 "https://orcid.org/0000-0002-7702-4495" xsd:string

[Term]
id: T4FS:0000653
name: DSM-3-H2
def: "For each dataset, the hosting environment maintains a globally unique, persistent and resolvable identifier for access and retrieval" [] {http://purl.obolibrary.org/obo/IAO_0000119="https://fairplus.github.io/Data-Maturity/docs/Indicators/"}
is_a: T4FS:0000586 ! fairplus DSM hosting-environment capabilities indicator
relationship: T4FS:0000581 T4FS:0000512 ! confers compliance with F1. (meta)data are assigned a globally unique and persistent identifier
property_value: IAO:0000117 "https://orcid.org/0000-0002-7702-4495" xsd:string

[Term]
id: T4FS:0000654
name: DSM-3-H4
def: "If applicable, Dataset hosting environment offers dataset-level authentication and authorisation capabilities" [] {http://purl.obolibrary.org/obo/IAO_0000119="https://fairplus.github.io/Data-Maturity/docs/Indicators/"}
is_a: T4FS:0000586 ! fairplus DSM hosting-environment capabilities indicator
relationship: T4FS:0000581 T4FS:0000371 ! confers compliance with A1.2 the protocol allows for an authentication and authorisation procedure, where necessary
property_value: IAO:0000117 "https://orcid.org/0000-0002-7702-4495" xsd:string

[Term]
id: T4FS:0000655
name: DSM-4-H2
def: "Data Hosting Environment provides semantic querying capability" [] {http://purl.obolibrary.org/obo/IAO_0000119="https://fairplus.github.io/Data-Maturity/docs/Indicators/"}
is_a: T4FS:0000586 ! fairplus DSM hosting-environment capabilities indicator
property_value: IAO:0000117 "https://orcid.org/0000-0002-7702-4495" xsd:string

[Term]
id: T4FS:0000656
name: DSM-0-H3
def: "Dataset's Metadata is NOT searchable via keywords or elements within the Descriptor" [] {http://purl.obolibrary.org/obo/IAO_0000119="https://fairplus.github.io/Data-Maturity/docs/Indicators/"}
is_a: T4FS:0000586 ! fairplus DSM hosting-environment capabilities indicator
property_value: IAO:0000117 "https://orcid.org/0000-0002-7702-4495" xsd:string

[Term]
id: T4FS:0000657
name: DSM-1-H4
def: "Metadata hosting environment offers the capability to browse and search contents of the Dataset Descriptor" [] {http://purl.obolibrary.org/obo/IAO_0000119="https://fairplus.github.io/Data-Maturity/docs/Indicators/"}
is_a: T4FS:0000586 ! fairplus DSM hosting-environment capabilities indicator
relationship: T4FS:0000581 T4FS:0000393 ! confers compliance with F4. (meta)data are registered or indexed in a searchable resource
property_value: IAO:0000117 "https://orcid.org/0000-0002-7702-4495" xsd:string

[Term]
id: T4FS:0000658
name: DSM-2-H3
def: "Data hosting environment offers the capability to browse and search related Datasets" [] {http://purl.obolibrary.org/obo/IAO_0000119="https://fairplus.github.io/Data-Maturity/docs/Indicators/"}
is_a: T4FS:0000586 ! fairplus DSM hosting-environment capabilities indicator
relationship: T4FS:0000581 T4FS:0000393 ! confers compliance with F4. (meta)data are registered or indexed in a searchable resource
property_value: IAO:0000117 "https://orcid.org/0000-0002-7702-4495" xsd:string

[Term]
id: T4FS:0000659
name: DSM-3-H3
def: "Data Hosting environment utilises controlled terms and/or ontology terms to search within Dataset content." [] {http://purl.obolibrary.org/obo/IAO_0000119="https://fairplus.github.io/Data-Maturity/docs/Indicators/"}
is_a: T4FS:0000586 ! fairplus DSM hosting-environment capabilities indicator
relationship: T4FS:0000581 T4FS:0000512 ! confers compliance with F1. (meta)data are assigned a globally unique and persistent identifier
property_value: IAO:0000117 "https://orcid.org/0000-0002-7702-4495" xsd:string

[Term]
id: T4FS:0000660
name: DSM-4-H2
def: "Data Hosting Environment provides semantic querying capability" [] {http://purl.obolibrary.org/obo/IAO_0000119="https://fairplus.github.io/Data-Maturity/docs/Indicators/"}
is_a: T4FS:0000586 ! fairplus DSM hosting-environment capabilities indicator
property_value: IAO:0000117 "https://orcid.org/0000-0002-7702-4495" xsd:string

[Typedef]
id: T4FS:0000554
name: confers competency about
def: "Describes how a learning medium is intended to confer a competence or capability regarding a particular data stewardship activity, e.g. a presentation confering competency in metadata creation." [] {http://purl.obolibrary.org/obo/IAO_0000119="https://orcid.org/0000-0002-7702-4495"}
property_value: IAO:0000117 "https://orcid.org/0000-0002-7702-4495" xsd:string
property_value: IAO:0000117 "Peter McQuilton" xsd:string
domain: T4FS:0000519 ! learning medium
range: T4FS:0000012 ! data stewardship activity
inverse_of: T4FS:0000575 ! competency gained through
created_by: Peter McQuilton
creation_date: 2020-10-01T21:36:11.080721Z

[Typedef]
id: T4FS:0000555
name: confers knowledge about
def: "Describes how a learning medium is intended to confer knowledge of a particular data stewardship technical concept in order for that learning medium to perform its function, e.g. a presentation conferring competency in metadata." [] {http://purl.obolibrary.org/obo/IAO_0000119="https://orcid.org/0000-0002-7702-4495"}
property_value: IAO:0000117 "https://orcid.org/0000-0002-7702-4495" xsd:string
property_value: IAO:0000117 "Peter McQuilton" xsd:string
domain: T4FS:0000519 ! learning medium
range: T4FS:0000372 ! data stewardship technical concept
created_by: Peter McQuilton
creation_date: 2020-12-06 00:00:00

[Typedef]
id: T4FS:0000556
name: requires/improves personal attribute
property_value: IAO:0000117 "https://orcid.org/0000-0002-7702-4495" xsd:string
range: T4FS:0000548 ! data stewardship soft skill
created_by: Peter McQuilton

[Typedef]
id: T4FS:0000557
name: confers practical skill about
def: "Describes how a learning medium confers practical skills regarding a particular data stewardship technical concept in order for that learning medium to perform its function e.g. a workshop conferring a practical skill in repository access." [] {http://purl.obolibrary.org/obo/IAO_0000119="https://orcid.org/0000-0002-7702-4495"}
property_value: IAO:0000117 "https://orcid.org/0000-0002-7702-4495" xsd:string
property_value: IAO:0000117 "Peter McQuilton" xsd:string
domain: T4FS:0000519 ! learning medium
range: T4FS:0000372 ! data stewardship technical concept
created_by: Peter McQuilton
creation_date: 2020-12-06 00:00:00

[Typedef]
id: T4FS:0000558
name: has/wants competency in
def: "Describes how an expertise level or role (e.g. \"data steward\") is associated with a data stewardship activity (e.g. ‘workflow set-up and management’) to indicate whether someone has an awareness of the area, or an ability to do it, or expert knowledge of it." [] {http://purl.obolibrary.org/obo/IAO_0000119="https://orcid.org/0000-0002-7702-4495"}
comment: Definition added 8.2.22
property_value: IAO:0000117 "https://orcid.org/0000-0002-7702-4495" xsd:string
property_value: IAO:0000117 "Peter McQuilton" xsd:string
range: T4FS:0000012 ! data stewardship activity

[Typedef]
id: T4FS:0000559
name: has/wants knowledge about
property_value: IAO:0000117 "https://orcid.org/0000-0002-7702-4495" xsd:string
property_value: IAO:0000117 "Peter McQuilton" xsd:string

[Typedef]
id: T4FS:0000560
name: supports implementation of
property_value: IAO:0000117 "https://orcid.org/0000-0002-7702-4495" xsd:string
domain: T4FS:0000519 ! learning medium
range: T4FS:0000446 ! data stewardship guideline
created_by: Peter McQuilton

[Typedef]
id: T4FS:0000561
name: has/wants practical skill about
def: "Desires/has a competence or capability acquired or applied in a specific context, e.g. producing a research output or deploying a service. A skill may be specified in a ‘skills user story’. A badge or certificate may provide evidence that a skill has been acquired, and a publication, personal profile, portfolio or CV may provide evidence that a skill has been applied." [] {http://purl.obolibrary.org/obo/IAO_0000119="FAIR4S"}
property_value: IAO:0000117 "https://orcid.org/0000-0002-7702-4495" xsd:string
property_value: IAO:0000117 "Peter McQuilton" xsd:string
range: T4FS:0000372 ! data stewardship technical concept
created_by: Peter McQuilton

[Typedef]
id: T4FS:0000562
name: has aptitude for
property_value: IAO:0000117 "https://orcid.org/0000-0002-7702-4495" xsd:string
property_value: IAO:0000117 "Peter McQuilton" xsd:string
range: T4FS:0000548 ! data stewardship soft skill
created_by: Peter McQuilton
creation_date: 2021-03-24T15:33:43.476917Z

[Typedef]
id: T4FS:0000563
name: contributes to the implementation of
property_value: IAO:0000117 "https://orcid.org/0000-0002-7702-4495" xsd:string
property_value: IAO:0000117 "Peter McQuilton" xsd:string
domain: T4FS:0000372 ! data stewardship technical concept
range: T4FS:0000446 ! data stewardship guideline
created_by: Peter McQuilton
creation_date: 2021-03-22T15:25:13.443153Z

[Typedef]
id: T4FS:0000575
name: competency gained through
def: "The learning media that creates a competence or capability." [] {http://purl.obolibrary.org/obo/IAO_0000119="https://orcid.org/0000-0002-7702-4495"}
comment: Allyson Lister 13.9.22: This class is created as the inverse of confers/requires competency about to allow consistent reasoning and access to the Data stewardship guidelines for Data stewardship activities. It needs to be revisited by the entire team to check the model.
property_value: IAO:0000117 "https://orcid.org/0000-0002-7702-4495" xsd:string
domain: T4FS:0000012 ! data stewardship activity
range: T4FS:0000519 ! learning medium
created_by: https://orcid.org/0000-0002-7702-4495

[Typedef]
id: T4FS:0000576
name: requires competency about
def: "Describes how a learning medium requires competency in a particular data stewardship activity in order for that learning medium to perform its function, e.g. a presentation requiring competency in metadata creation prior to engaging with that learning medium." [] {http://purl.obolibrary.org/obo/IAO_0000119="https://orcid.org/0000-0002-7702-4495"}
domain: T4FS:0000519 ! learning medium
range: T4FS:0000012 ! data stewardship activity

[Typedef]
id: T4FS:0000577
name: requires knowledge about
def: "Describes how a learning medium requires knowledge of a particular data stewardship technical concept in order for that learning medium to perform its function, e.g. a presentation requiring knowledge of metadata." [] {http://purl.obolibrary.org/obo/IAO_0000119="https://orcid.org/0000-0002-7702-4495"}
domain: T4FS:0000519 ! learning medium
range: T4FS:0000372 ! data stewardship technical concept

[Typedef]
id: T4FS:0000578
name: requires practical skill about
def: "Describes how a learning medium requires practical skills of a particular data stewardship technical concept in order for that learning medium to perform its function e.g. a workshop requiring a practical skill in repository access." [] {http://purl.obolibrary.org/obo/IAO_0000119="https://orcid.org/0000-0002-7702-4495"}
domain: T4FS:0000519 ! learning medium
range: T4FS:0000372 ! data stewardship technical concept

[Typedef]
id: T4FS:0000581
name: confers compliance with
def: "Describes how an evaluation indicator may confer compliance with a particular guideline or set of guidelines" [] {http://purl.obolibrary.org/obo/IAO_0000119="https://orcid.org/0000-0002-7702-4495"}
property_value: IAO:0000117 "https://orcid.org/0000-0002-7702-4495" xsd:string
property_value: IAO:0000233 "https://github.com/terms4fairskills/FAIRterminology/issues/22" xsd:string
domain: T4FS:0000580 ! evaluation indicator
range: T4FS:0000446 ! data stewardship guideline

[Typedef]
id: T4FS:0000582
name: demonstrates how to fulfil the requirements for
def: "A learning medium may demonstrate how to meet the requirements for a particular evaluation indicator(s)." [] {http://purl.obolibrary.org/obo/IAO_0000119="https://orcid.org/0000-0002-7702-4495"}
property_value: IAO:0000117 "https://orcid.org/0000-0002-7702-4495" xsd:string
property_value: IAO:0000233 "https://github.com/terms4fairskills/FAIRterminology/issues/22" xsd:string
domain: T4FS:0000519 ! learning medium
range: T4FS:0000580 ! evaluation indicator

