format-version: 1.2
data-version: t4fs/releases/2025-02-09/t4fs-simple.owl
idspace: oboInOwl http://www.geneontology.org/formats/oboInOwl# 
idspace: terms http://purl.org/dc/terms/ 
remark: terms4FAIRskills by the terms4FAIRskills developers is licensed under CC BY 4.0. You are free to share (copy and redistribute the material in any medium or format) and adapt (remix, transform, and build upon the material) for any purpose, even commercially. for any purpose, even commercially. The licensor cannot revoke these freedoms as long as you follow the license terms. You must give appropriate credit (by using the original ontology IRI for the whole ontology and original term IRIs for individual terms), provide a link to the license, and indicate if any changes were made. You may do so in any reasonable manner, but not in any way that suggests the licensor endorses you or your use.
ontology: t4fs/t4fs-simple
property_value: owl:versionInfo "2025-02-09" xsd:string
property_value: terms:description "terms4FAIRskills describes the competencies, skills and knowledge associated with making and keeping data FAIR.\\nThis terminology applies to a variety of use cases, including: assisting with the creation and assessment of stewardship curricula; facilitating the annotation, discovery and evaluation of FAIR-enabling materials \\(e.g. training\\) and resources; enabling the formalisation of job descriptions and CVs with recognised, structured competencies.\\nIt is intended to be of use to trainers who teach FAIR data skills, researchers who wish to identify skill gaps in their teams and managers who need to recruit individuals to relevant roles." xsd:string
property_value: terms:license http://creativecommons.org/licenses/by/4.0/
property_value: terms:title "terms4FAIRskills (T4FS)" xsd:string

[Term]
id: T4FS:0000002
name: pipe separated values
def: "Values in a table presented as a series of ASCII text lines organised so that each column value is separated by a pipe ( | )." [] {IAO:0000119="RDMT. https://terms.codata.org/rdmt/pipe-separated-values"}
is_a: T4FS:0000372 ! data stewardship technical concept
relationship: T4FS:0000563 T4FS:0000137 ! contributes to the implementation of I1. (meta)data use a formal, accessible, shared, and broadly applicable language for knowledge representation
property_value: IAO:0000117 "https://orcid.org/0000-0002-5214-4466" xsd:string
property_value: IAO:0000117 "https://orcid.org/0000-0002-7702-4495" xsd:string
property_value: IAO:0000117 "https://orcid.org/0000-0003-2687-1982" xsd:string

[Term]
id: T4FS:0000004
name: software preservation
def: "Software preservation involves the collection and long-term storage of software for archiving as well as maintaining availability and accessibility." [] {IAO:0000119="https://orcid.org/0000-0002-7702-4495 8.2.22"}
comment: AL 8.2.22: Refactored "software review and preservation" to "software preservation", as the review process is not within the remit of terms4FAIRskills. Added definition and source.
is_a: T4FS:0000156 ! archiving
property_value: IAO:0000117 "https://orcid.org/0000-0002-7702-4495" xsd:string
property_value: IAO:0000117 "Kristina Hettne" xsd:string
property_value: IAO:0000117 "Victoria Dominguez Del Angel" xsd:string
property_value: IAO:0000117 "Yann Le Franc" xsd:string

[Term]
id: T4FS:0000005
name: repository access
def: "In accessing a repository one uses a client (application) to discover relevant digital objects within a repository, and then retrieve a copy of a desired digital object." [] {IAO:0000119="Definition from now-deprecated CASRAI Glossary term: repository-access"}
is_a: T4FS:0000489 ! repository
property_value: IAO:0000117 "https://orcid.org/0000-0002-5214-4466" xsd:string
property_value: IAO:0000117 "https://orcid.org/0000-0002-7702-4495" xsd:string
property_value: IAO:0000117 "https://orcid.org/0000-0003-2687-1982" xsd:string

[Term]
id: T4FS:0000006
name: develop fair and open research vision
def: "Include FAIR and open research in the strategic framework for the organization and set objectives and timeframe." []
is_a: T4FS:0000008 ! develop open research strategy and vision
property_value: IAO:0000117 "Angus Whyte" xsd:string
property_value: IAO:0000117 "Celia van Gelder" xsd:string
property_value: IAO:0000117 "Mateusz Kuzak" xsd:string
property_value: IAO:0000117 "Yan Wang" xsd:string

[Term]
id: T4FS:0000008
name: develop open research strategy and vision
def: "The activity of developing an open research strategy and vision." [] {IAO:0000119="PMQ 3.2022"}
is_a: T4FS:0000514 ! strategic/long-term planning
property_value: IAO:0000117 "Angus Whyte" xsd:string
property_value: IAO:0000117 "Celia van Gelder" xsd:string
property_value: IAO:0000117 "Mateusz Kuzak" xsd:string
property_value: IAO:0000117 "Yan Wang" xsd:string

[Term]
id: T4FS:0000009
name: data management policy
def: "Statement of an organisation’s processes for the management of a specified set of data assets." [] {IAO:0000119="RDMT. https://terms.codata.org/rdmt/data-management-policy"}
is_a: T4FS:0000372 ! data stewardship technical concept
relationship: T4FS:0000563 T4FS:0000447 ! contributes to the implementation of fair principle
property_value: IAO:0000117 "https://orcid.org/0000-0002-5214-4466" xsd:string
property_value: IAO:0000117 "https://orcid.org/0000-0003-2687-1982" xsd:string

[Term]
id: T4FS:0000010
name: understand research code of conduct
def: "Understand how the governing principles of research integrity and FAIR overlap" []
is_a: T4FS:0000525 ! research integrity, attribution, impact awareness
property_value: IAO:0000117 "Angus Whyte" xsd:string
property_value: IAO:0000117 "Celia van Gelder" xsd:string

[Term]
id: T4FS:0000011
name: choosing the appropriate reporting guideline for your data
def: "To be able to choose the appropriate reporting guideline/checklist for your data, based on community-adopted standards." [] {IAO:0000119="[PMQ]"}
is_a: T4FS:0000175 ! fair evaluation of repositories for data deposition
property_value: IAO:0000117 "https://orcid.org/0000-0003-2687-1982" xsd:string

[Term]
id: T4FS:0000012
name: data stewardship activity
def: "A specific deed, action, function or sphere of action in relation with the role of data stewardship" []
relationship: T4FS:0000556 T4FS:0000548 ! requires/improves personal attribute data stewardship soft skill
property_value: IAO:0000117 "https://orcid.org/0000-0002-7702-4495" xsd:string
property_value: IAO:0000117 "https://orcid.org/0000-0003-2687-1982" xsd:string
property_value: IAO:0000117 "Yann Le Franc" xsd:string
property_value: T4FS:0000564 "Set of actions carried out during data stewardship processes" xsd:string

[Term]
id: T4FS:0000013
name: data munging
def: "A series of potentially destructive or irrevocable changes to a piece of data or a file. Common munging operations include removing punctuation or html tags, data parsing, filtering, and transformation." [] {IAO:0000119="Definition from now-deprecated CASRAI Glossary term: data-munging"}
is_a: T4FS:0000036 ! curation
property_value: IAO:0000117 "https://orcid.org/0000-0002-5214-4466" xsd:string
property_value: IAO:0000117 "https://orcid.org/0000-0003-2687-1982" xsd:string

[Term]
id: T4FS:0000014
name: interoperability of digital assets
is_a: T4FS:0000447 ! fair principle
property_value: IAO:0000117 "https://orcid.org/0000-0003-2687-1982" xsd:string

[Term]
id: T4FS:0000016
name: skills for resource management
def: "Bin for Skills related to Resource management" []
is_a: T4FS:0000353 ! resource management
property_value: IAO:0000117 "leightonlc" xsd:string

[Term]
id: T4FS:0000017
name: preservation
def: "An activity within archiving in which specific items of data are maintained over time so that they can still be accessed and understood through changes in technology." [] {IAO:0000119="RDMT. https://terms.codata.org/rdmt/preservation"}
is_a: T4FS:0000156 ! archiving
property_value: IAO:0000117 "https://orcid.org/0000-0002-5214-4466" xsd:string
property_value: IAO:0000117 "https://orcid.org/0000-0002-7702-4495" xsd:string
property_value: IAO:0000117 "https://orcid.org/0000-0003-2687-1982" xsd:string
property_value: IAO:0000118 "Conservation" xsd:string

[Term]
id: T4FS:0000018
name: data categorisation
is_a: T4FS:0000036 ! curation
property_value: IAO:0000118 "Data Categorization" xsd:string
property_value: IAO:0000118 "Data Classification" xsd:string
created_by: https://orcid.org/0000-0003-2687-1982
creation_date: 2021-02-17T22:30:31.531624Z

[Term]
id: T4FS:0000019
name: data registration
def: "Curation process on a data object by which it receives a persistent identifier (PID) from a trusted registration authority. Registration must be accompanied by the step(s) to create and submit metadata describing the object to the registry." [] {IAO:0000119="RDMT. https://terms.codata.org/rdmt/data-registration"}
is_a: T4FS:0000021 ! exposing data
property_value: IAO:0000117 "https://orcid.org/0000-0002-5214-4466" xsd:string
property_value: IAO:0000117 "https://orcid.org/0000-0002-7702-4495" xsd:string
property_value: IAO:0000117 "https://orcid.org/0000-0003-2687-1982" xsd:string

[Term]
id: T4FS:0000020
name: interoperability
def: "The capability to communicate, execute programs, or transfer data among various functional units in a useful and meaningful manner that requires the user to have little or no knowledge of the unique characteristics of those units. Foundational, syntactic, and semantic interoperability are the three necessary aspects of interoperability." [] {IAO:0000119="Definition from now-deprecated CASRAI Glossary term: interoperability"}
is_a: T4FS:0000372 ! data stewardship technical concept
relationship: T4FS:0000563 T4FS:0000014 ! contributes to the implementation of interoperability of digital assets
property_value: IAO:0000117 "v" xsd:string

[Term]
id: T4FS:0000021
name: exposing data
def: "Exposing data is the activity of exposing your data to collaborators, the public, or other interested parties. A data producer makes the data accessible to external users in a machine- and/or human-readable way." [] {IAO:0000119="[PMQ 3.2022, AL 15.3.22]"}
comment: AL 15.3.22: Was "expose your data", which was not in the style of other term labels. Also updated definition, but might need revisiting later for a more formal definition.
is_a: T4FS:0000012 ! data stewardship activity
property_value: IAO:0000117 "https://orcid.org/0000-0002-7702-4495" xsd:string
property_value: IAO:0000117 "https://orcid.org/0000-0003-2687-1982" xsd:string

[Term]
id: T4FS:0000023
name: aptitudes for workflow technologies management
def: "Bin for Aptitudes related to Workflow technologies management." []
is_a: T4FS:0000177 ! workflow technologies management
property_value: IAO:0000117 "leightonlc" xsd:string

[Term]
id: T4FS:0000024
name: de facto standard
def: "A standard that is widely accepted and used, but lacks formal approval by a recognized standards developing organization (e.g., the QWERTY keyboard)." [] {IAO:0000119="Definition from now-deprecated CASRAI Glossary term: de-facto-standard"}
is_a: T4FS:0000372 ! data stewardship technical concept
relationship: T4FS:0000563 T4FS:0000137 ! contributes to the implementation of I1. (meta)data use a formal, accessible, shared, and broadly applicable language for knowledge representation
property_value: IAO:0000117 "https://orcid.org/0000-0002-5214-4466" xsd:string
property_value: IAO:0000117 "https://orcid.org/0000-0003-2687-1982" xsd:string

[Term]
id: T4FS:0000025
name: data entity
def: "Object, event or phenomenon about which data are stored in a database and which has intermediate representation in a Data Model." [] {IAO:0000119="RDMT. https://terms.codata.org/rdmt/data-entity"}
is_a: T4FS:0000372 ! data stewardship technical concept
property_value: IAO:0000117 "https://orcid.org/0000-0002-5214-4466" xsd:string
property_value: IAO:0000117 "https://orcid.org/0000-0003-2687-1982" xsd:string

[Term]
id: T4FS:0000026
name: real-time data
def: "Data that are being received, processed and stored at the time of their occurrence with only small delays. Examples include: stock quotes, manufacturing statistics, Web server loads, data warehouse activity and sensor feeds to data collectors. Real-time data are often used for navigation or tracking. Real-time data are data streams that are typically generated by sensors and received via direct networking connections." [] {IAO:0000119="RDMT. https://terms.codata.org/rdmt/real-time-data"}
is_a: T4FS:0000430 ! data
property_value: IAO:0000117 "https://orcid.org/0000-0002-5214-4466" xsd:string
property_value: IAO:0000117 "https://orcid.org/0000-0002-7702-4495" xsd:string
property_value: IAO:0000117 "https://orcid.org/0000-0003-2687-1982" xsd:string

[Term]
id: T4FS:0000027
name: storage security risk assessment and mitigation
def: "Detect and analysis security risk of storage periodically, and minimize the impact of the risks detected" []
is_a: T4FS:0000470 ! storage security management
property_value: IAO:0000117 "Angus Whyte" xsd:string
property_value: IAO:0000117 "Celia van Gelder" xsd:string
property_value: IAO:0000117 "Mateusz Kuzak" xsd:string
property_value: IAO:0000117 "Yan Wang" xsd:string

[Term]
id: T4FS:0000028
name: remote access
def: "The ability to get access to a computer or a network from a remote distance. Access may be through an Internet service provider (ISP) or through a dedicated line between a computer or a remote local area network and the central or main corporate local area network. A dedicated line is more expensive and less flexible but offers faster data rates." [] {IAO:0000119="Definition from now-deprecated CASRAI Glossary term: remote-access"}
is_a: T4FS:0000372 ! data stewardship technical concept
property_value: IAO:0000117 "https://orcid.org/0000-0002-5214-4466" xsd:string
property_value: IAO:0000117 "https://orcid.org/0000-0002-7702-4495" xsd:string
property_value: IAO:0000117 "https://orcid.org/0000-0003-2687-1982" xsd:string

[Term]
id: T4FS:0000029
name: fair stewardship supervising
def: "The activity of supervision of other people to ensure FAIR data practices." [] {IAO:0000119="PMQ"}
is_a: T4FS:0000259 ! fair training
property_value: IAO:0000117 "https://orcid.org/0000-0002-7702-4495" xsd:string
property_value: IAO:0000117 "https://orcid.org/0000-0003-2687-1982" xsd:string
property_value: IAO:0000117 "Philippe Rocca-Serra" xsd:string
property_value: IAO:0000117 "Susanna Sansone" xsd:string

[Term]
id: T4FS:0000030
name: skills related to high performance computing management
def: "Bin for Skills needed for High performance computing management." []
is_a: T4FS:0000308 ! high performance computing management
property_value: IAO:0000117 "leightonlc" xsd:string

[Term]
id: T4FS:0000031
name: fair metrics selection skills
def: "Ability to select the appropriate FAIR metrics among the existing ones in relation to the type of digital object concerned." []
is_a: T4FS:0000252 ! fairness assessment
property_value: IAO:0000117 "Kristina Hettne" xsd:string
property_value: IAO:0000117 "Victoria Dominguez Del Angel" xsd:string
property_value: IAO:0000117 "Yann Le Franc" xsd:string

[Term]
id: T4FS:0000032
name: relational database
def: "A collection of data items organized as a set of formally-described tables from which data can be accessed or reassembled in many different ways without having to reorganize the database tables. The standard user and application program interface to a relational database is the structured query language (SQL)." [] {IAO:0000119="Definition from now-deprecated CASRAI Glossary term: relational-database"}
is_a: T4FS:0000372 ! data stewardship technical concept
property_value: IAO:0000117 "https://orcid.org/0000-0002-5214-4466" xsd:string
property_value: IAO:0000117 "https://orcid.org/0000-0002-7702-4495" xsd:string
property_value: IAO:0000117 "https://orcid.org/0000-0003-2687-1982" xsd:string

[Term]
id: T4FS:0000033
name: non identifiable data
def: "Data that could not lead to the identification of a specific object of interest. These may be data that have been de-identified, or that could not lead to identifiable information in the first place." [] {IAO:0000119="Modified by AL on 6.5.22 from CASRAI. https://casrai.org/term/non-identifiable-data/"}
comment: AL 6.5.22: Modifed CASRAI definition to distinguish this term from 'non personally identifiable information.' Further work may determine whether or not both terms are required.
is_a: T4FS:0000430 ! data
property_value: IAO:0000117 "https://orcid.org/0000-0002-7702-4495" xsd:string
property_value: IAO:0000117 "https://orcid.org/0000-0003-2687-1982" xsd:string

[Term]
id: T4FS:0000034
name: database developer
relationship: T4FS:0000558 T4FS:0000012 ! has/wants competency in data stewardship activity
relationship: T4FS:0000559 T4FS:0000372 ! has/wants knowledge about data stewardship technical concept
relationship: T4FS:0000559 T4FS:0000446 ! has/wants knowledge about data stewardship guideline
relationship: T4FS:0000561 T4FS:0000372 ! has/wants practical skill about data stewardship technical concept
relationship: T4FS:0000562 T4FS:0000548 ! has aptitude for data stewardship soft skill

[Term]
id: T4FS:0000036
name: curation
def: "Managing and promoting the use of assets from their point of creation to ensure that they are fit for contemporary purpose and available for discovery and reuse. For dynamic datasets this may mean continuous enrichment or updating to keep them fit for purpose. Higher levels of curation will also involve links with annotation and with other published materials." [] {IAO:0000119="RDMT. https://terms.codata.org/rdmt/curation"}
is_a: T4FS:0000012 ! data stewardship activity
property_value: IAO:0000117 "https://orcid.org/0000-0002-5214-4466" xsd:string
property_value: IAO:0000117 "https://orcid.org/0000-0003-2687-1982" xsd:string

[Term]
id: T4FS:0000038
name: A1. (meta)data are retrievable by their identifier using a standardised communications protocol
is_a: T4FS:0000478 ! accessibility of digital assets
property_value: IAO:0000117 "https://orcid.org/0000-0003-2687-1982" xsd:string

[Term]
id: T4FS:0000039
name: version control
def: "Control over time of data, computer code, software, and documents that allows for the ability to revert to a previous revision, which is critical for data traceability, tracking edits, and correcting mistakes. Version control generates a (changed) copy of a data object that is uniquely labelled with a version number. The intent is to track changes to a data object, by making versioned copies. Note that a version is different from a backup copy, which is typically a copy made at a specific point in time, or a replica." [] {IAO:0000119="RDMT. https://terms.codata.org/rdmt/version-control"}
is_a: T4FS:0000372 ! data stewardship technical concept
property_value: IAO:0000117 "https://orcid.org/0000-0002-5214-4466" xsd:string
property_value: IAO:0000117 "https://orcid.org/0000-0002-7702-4495" xsd:string
property_value: IAO:0000117 "https://orcid.org/0000-0003-2687-1982" xsd:string
property_value: IAO:0000118 "Versioning, Revision control, Source control" xsd:string

[Term]
id: T4FS:0000041
name: understanding fair and open research challenges in your organization
def: "Understand the FAIR and open research practices, and the research landscape / current data management practices in the organization." []
is_a: T4FS:0000008 ! develop open research strategy and vision
property_value: IAO:0000117 "Angus Whyte" xsd:string
property_value: IAO:0000117 "Celia van Gelder" xsd:string
property_value: IAO:0000117 "Mateusz Kuzak" xsd:string
property_value: IAO:0000117 "Yan Wang" xsd:string

[Term]
id: T4FS:0000042
name: ethical application of patents, licenses
is_a: T4FS:0000106 ! publish data

[Term]
id: T4FS:0000043
name: data access protocol
def: "System that allows users to be granted access to a database under specified conditions." [] {IAO:0000119="RDMT.  https://terms.codata.org/rdmt/data-access-protocol"}
is_a: T4FS:0000283 ! access
property_value: IAO:0000117 "https://orcid.org/0000-0002-5214-4466" xsd:string
property_value: IAO:0000117 "https://orcid.org/0000-0003-2687-1982" xsd:string

[Term]
id: T4FS:0000044
name: data processing
def: "Generic concept referring to all kinds of procedures being executed on data at any point in the data lifecycle." [] {IAO:0000119="RDMT. https://terms.codata.org/rdmt/data-processing"}
is_a: T4FS:0000036 ! curation
property_value: IAO:0000117 "https://orcid.org/0000-0002-5214-4466" xsd:string
property_value: IAO:0000117 "https://orcid.org/0000-0003-2687-1982" xsd:string

[Term]
id: T4FS:0000045
name: data organization
def: "Set of measures that are used by a repository to form aggregations of data objects (including collections and metadata) to describe the properties of data objects, to register PIDs, to build the PID records, to link between all components, and to set up the containers (in the form of the software stack) that are used to store all components." [] {IAO:0000119="RDMT. https://terms.codata.org/rdmt/data-organisation"}
is_a: T4FS:0000372 ! data stewardship technical concept
relationship: T4FS:0000563 T4FS:0000447 ! contributes to the implementation of fair principle
property_value: IAO:0000117 "https://orcid.org/0000-0002-5214-4466" xsd:string
property_value: IAO:0000117 "https://orcid.org/0000-0003-2687-1982" xsd:string

[Term]
id: T4FS:0000046
name: data rescue
def: "Recovery and/or transformation and digitization of dark data and at-risk data so that they can be preserved, accessed, shared, and used. Data rescue also involves the addition of rich metadata to make the content understandable and more easily re-usable." [] {IAO:0000119="RDMT. https://terms.codata.org/rdmt/data-rescue"}
is_a: T4FS:0000156 ! archiving
property_value: IAO:0000117 "https://orcid.org/0000-0002-5214-4466" xsd:string
property_value: IAO:0000117 "https://orcid.org/0000-0002-7702-4495" xsd:string
property_value: IAO:0000117 "https://orcid.org/0000-0003-2687-1982" xsd:string

[Term]
id: T4FS:0000047
name: understand societal impact of research
def: "Anticipate possible implications of the research and making its outputs FAIR, reflecting on rmotivations and areas of uncertainty" []
is_a: T4FS:0000525 ! research integrity, attribution, impact awareness
property_value: IAO:0000117 "Angus Whyte" xsd:string
property_value: IAO:0000117 "Celia van Gelder" xsd:string
property_value: IAO:0000117 "Mateusz Kuzak" xsd:string
property_value: IAO:0000117 "Yan Wang" xsd:string

[Term]
id: T4FS:0000048
name: searching via algorithms and software
def: "To be able to search using software with a GUI or terminal access. For example using BLAST or genomic search tools in the life sciences." [] {IAO:0000119="[PMQ]"}
is_a: T4FS:0000145 ! search repositories and knowledge-bases
property_value: IAO:0000117 "https://orcid.org/0000-0003-2687-1982" xsd:string
property_value: IAO:0000118 "Algorithm searching" xsd:string
property_value: IAO:0000118 "batch search" xsd:string
property_value: IAO:0000118 "Programmatic search" xsd:string

[Term]
id: T4FS:0000049
name: audit
def: "Evaluation of an organisation, system, group, project or product with respect to its data and processes around this, often in accordance with a standard, guide, or framework used to structure the work. This can involve assessing, describing, and classifying any data held. An audit can be carried out internally by those who have access to the data or participate in related processes regularly, or by an independent, external actor." [] {IAO:0000119="RDMT. https://terms.codata.org/rdmt/audit"}
is_a: T4FS:0000126 ! assessment
property_value: IAO:0000117 "https://orcid.org/0000-0002-5214-4466" xsd:string
property_value: IAO:0000117 "https://orcid.org/0000-0003-2687-1982" xsd:string

[Term]
id: T4FS:0000050
name: wiki site
is_a: T4FS:0000095 ! online documentation
created_by: https://orcid.org/0000-0003-2687-1982
creation_date: 2020-10-01T21:03:37.147424Z

[Term]
id: T4FS:0000051
name: skills related to authorisation management
def: "Bin for Skills needed for Authorization management." []
is_a: T4FS:0000142 ! authorisation management
property_value: IAO:0000117 "leightonlc" xsd:string

[Term]
id: T4FS:0000053
name: storage management
def: "The term storage management encompasses the technologies and processes organizations use to maximize or improve the performance of their data storage resources. It is a broad category that includes  virtualization, replication, mirroring, security, compression, traffic analysis, process automation, storage provisioning and related techniques." [] {IAO:0000119="(webopedia.com/TERM/S/storage_management.html)[VDA]"}
is_a: T4FS:0000353 ! resource management
property_value: IAO:0000117 "Kristina Hettne" xsd:string
property_value: IAO:0000117 "Simon Hodson" xsd:string
property_value: IAO:0000117 "Victoria Dominguez Del Angel" xsd:string

[Term]
id: T4FS:0000054
name: data warehouse
def: "Central repository for all or significant parts of the data that an organisation’s various business systems collect, containing harmonised, highly-structured, quality data integrated from multiple sources. Data warehousing emphasises the capture of data from diverse sources for useful analysis and access, but does not generally start from the point-of-view of the end user who may need access to specialised data marts. There are two approaches to data warehousing: The top-down approach spins off data marts for specific groups of users after the complete data warehouse has been created. The bottom-up approach builds the data marts first and then combines them into a single, all-encompassing data warehouse." [] {IAO:0000119="RDMT. https://terms.codata.org/rdmt/data-warehouse"}
is_a: T4FS:0000215 ! data store
property_value: IAO:0000117 "https://orcid.org/0000-0002-5214-4466" xsd:string
property_value: IAO:0000117 "https://orcid.org/0000-0003-2687-1982" xsd:string

[Term]
id: T4FS:0000055
name: data driven disaster
def: "Serious problem caused by one or more ineffective data analysis processes." [] {IAO:0000119="RDMT. https://terms.codata.org/rdmt/data-driven-disaster"}
is_a: T4FS:0000012 ! data stewardship activity
property_value: IAO:0000117 "https://orcid.org/0000-0002-5214-4466" xsd:string
property_value: IAO:0000117 "https://orcid.org/0000-0003-2687-1982" xsd:string

[Term]
id: T4FS:0000056
name: data identifier
def: "An identifier that uniquely distinguishes one set of data from all others." [] {IAO:0000119="Definition from now-deprecated CASRAI Glossary term: data-identifier"}
is_a: T4FS:0000453 ! persistent identifier
property_value: IAO:0000117 "https://orcid.org/0000-0002-5214-4466" xsd:string
property_value: IAO:0000117 "https://orcid.org/0000-0003-2687-1982" xsd:string

[Term]
id: T4FS:0000057
name: data splitting
def: "Protecting sensitive data from unauthorised access by encrypting the data and storing different portions of a file on different servers. An unauthorised person would need to know the locations of the servers containing the parts, be able to get access to each server, know what data to combine, and how to decrypt it. Data splitting can be made even more effective by periodically retrieving and recombining the parts, and then splitting the data in a different way among different servers, and using a different encryption key." [] {IAO:0000119="RDMT. https://terms.codata.org/rdmt/data-splitting"}
is_a: T4FS:0000107 ! information security
property_value: IAO:0000117 "https://orcid.org/0000-0002-5214-4466" xsd:string
property_value: IAO:0000117 "https://orcid.org/0000-0002-7702-4495" xsd:string
property_value: IAO:0000117 "https://orcid.org/0000-0003-2687-1982" xsd:string

[Term]
id: T4FS:0000058
name: manage access
def: "Monitor the status of information access of different stakeholder groups. Evaluate new access request and authorize or decline it. Update the organizational information access overview." []
is_a: T4FS:0000107 ! information security
property_value: IAO:0000117 "Angus Whyte" xsd:string
property_value: IAO:0000117 "Celia van Gelder" xsd:string
property_value: IAO:0000117 "Mateusz Kuzak" xsd:string
property_value: IAO:0000117 "Yan Wang" xsd:string

[Term]
id: T4FS:0000059
name: system metadata
def: "Digital entity properties that are generated by the data management system (e.g., creation time; owner; storage location; data retention period; the length of time a digital entity will be retained)." [] {IAO:0000119="RDMT. https://terms.codata.org/rdmt/system-metadata"}
is_a: T4FS:0000527 ! metadata
property_value: IAO:0000117 "https://orcid.org/0000-0002-5214-4466" xsd:string
property_value: IAO:0000117 "https://orcid.org/0000-0002-7702-4495" xsd:string
property_value: IAO:0000117 "https://orcid.org/0000-0003-2687-1982" xsd:string

[Term]
id: T4FS:0000060
name: tactical/short-term planning
is_a: T4FS:0000320 ! project management activities
property_value: IAO:0000117 "https://orcid.org/0000-0002-7702-4495" xsd:string
property_value: IAO:0000117 "https://orcid.org/0000-0003-2687-1982" xsd:string
property_value: IAO:0000117 "Philippe Rocca-Serra" xsd:string
property_value: IAO:0000117 "Susanna Sansone" xsd:string

[Term]
id: T4FS:0000061
name: electronic medical record
def: "Electronic version of the paper record that doctors have traditionally maintained for their patients and which is typically only accessible within the facility or office that controls it." [] {IAO:0000119="RDMT. https://terms.codata.org/rdmt/electronic-medical-record"}
is_a: T4FS:0000372 ! data stewardship technical concept
property_value: IAO:0000117 "https://orcid.org/0000-0002-5214-4466" xsd:string
property_value: IAO:0000117 "https://orcid.org/0000-0003-2687-1982" xsd:string

[Term]
id: T4FS:0000062
name: aptitudes for provenance information management
def: "Bin for Aptitudes related to Provenance information management." []
is_a: T4FS:0000368 ! provenance information management
property_value: IAO:0000117 "leightonlc" xsd:string

[Term]
id: T4FS:0000065
name: data modeling
def: "Formalising and documenting existing processes and events. A first step in analysing a system of objects with which users interact is to identify each object and its relationship to other objects. This process is called data modelling and results in a picture of object relationships. Data modellers often use multiple models to view the same data and ensure that all processes, entities, relationships and data flows have been identified. There are several different approaches to data modelling, including: Conceptual Data Modelling (identifies the highest-level relationships between different entities); Enterprise Data Modelling (similar to conceptual data modelling, but addresses the unique requirements of a specific organisation); Logical Data Modelling (illustrates the specific entities, attributes and relationships involved in a business function. Serves as the basis for the creation of the physical data model); Physical Data Modelling (represents an application and database-specific implementation of a logical data model)." [] {IAO:0000119="RDMT. https://terms.codata.org/rdmt/data-modelling"}
is_a: T4FS:0000036 ! curation
property_value: IAO:0000117 "https://orcid.org/0000-0002-5214-4466" xsd:string
property_value: IAO:0000117 "https://orcid.org/0000-0003-2687-1982" xsd:string

[Term]
id: T4FS:0000067
name: use of aggregator sites
def: "To be able to search and understand the results from dataset aggregrator sites. To understand the implications of the provenance of the data and how to integrate and analyse data with differing metadata." [] {IAO:0000119="[PMQ]"}
is_a: T4FS:0000145 ! search repositories and knowledge-bases
property_value: IAO:0000117 "https://orcid.org/0000-0003-2687-1982" xsd:string
property_value: IAO:0000118 "Searching aggregator sites" xsd:string

[Term]
id: T4FS:0000068
name: manage metadata catalog
def: "Implement the policies that govern the choice of metadata schema, reserved vocabularies, metadata organization in tables, and metadata properties (creation date, access control, ownership, etc.)." [] {IAO:0000119="Definition from now-deprecated CASRAI Glossary term: manage-metadata-catalog"}
is_a: T4FS:0000353 ! resource management
property_value: IAO:0000117 "https://orcid.org/0000-0002-5214-4466" xsd:string
property_value: IAO:0000117 "https://orcid.org/0000-0002-7702-4495" xsd:string
property_value: IAO:0000117 "https://orcid.org/0000-0003-2687-1982" xsd:string

[Term]
id: T4FS:0000069
name: data transformation
def: "Manipulation of raw data to produce a single output." [] {IAO:0000119="RDMT. https://terms.codata.org/rdmt/data-transformation"}
is_a: T4FS:0000352 ! data analysis
property_value: IAO:0000117 "https://orcid.org/0000-0002-5214-4466" xsd:string
property_value: IAO:0000117 "https://orcid.org/0000-0002-7702-4495" xsd:string
property_value: IAO:0000117 "https://orcid.org/0000-0003-2687-1982" xsd:string

[Term]
id: T4FS:0000070
name: cataloguing
def: "An intellectual process of describing objects in accordance with accepted library principles, particularly those of subject and classification order." [] {IAO:0000119="RDMT. https://terms.codata.org/rdmt/catalogue-verb"}
is_a: T4FS:0000036 ! curation
property_value: IAO:0000117 "https://orcid.org/0000-0002-5214-4466" xsd:string
property_value: IAO:0000117 "https://orcid.org/0000-0003-2687-1982" xsd:string

[Term]
id: T4FS:0000071
name: design and apply processes for attribution
def: "Iniitate and develop processes for crediting the contributions of researchers and professional groups towards making FAIR outputs" []
is_a: T4FS:0000525 ! research integrity, attribution, impact awareness
property_value: IAO:0000117 "Angus Whyte" xsd:string
property_value: IAO:0000117 "Celia van Gelder" xsd:string
property_value: IAO:0000117 "Mateusz Kuzak" xsd:string
property_value: IAO:0000117 "Yan Wang" xsd:string

[Term]
id: T4FS:0000072
name: dataset series
def: "Collection of datasets sharing the same product specification. A dataset series is a type of aggregation or collection with some “logical grouping” such as by a topic (specification) with the (product) unit being a dataset series." [] {IAO:0000119="RDMT. https://terms.codata.org/rdmt/dataset-series"}
is_a: T4FS:0000397 ! database
property_value: IAO:0000117 "https://orcid.org/0000-0002-5214-4466" xsd:string
property_value: IAO:0000117 "https://orcid.org/0000-0003-2687-1982" xsd:string

[Term]
id: T4FS:0000073
name: data dictionary
def: "Collection of descriptions of the data objects or items in a data model. After each data object or item is given a descriptive name, its relationship is described (or it becomes part of some structure that implicitly describes relationship), the type of data (such as text or image or binary value) is described, possible predefined values are listed, and a brief textual description is provided. This collection can be organised for reference into a data dictionary." [] {IAO:0000119="RDMT. https://terms.codata.org/rdmt/data-dictionary"}
is_a: T4FS:0000372 ! data stewardship technical concept
property_value: IAO:0000117 "https://orcid.org/0000-0002-5214-4466" xsd:string
property_value: IAO:0000117 "https://orcid.org/0000-0003-2687-1982" xsd:string

[Term]
id: T4FS:0000074
name: data selection
def: "Process that creates a new dataset from an original source." [] {IAO:0000119="RDMT. https://terms.codata.org/rdmt/data-selection"}
is_a: T4FS:0000231 ! data acquisition
property_value: IAO:0000117 "https://orcid.org/0000-0002-5214-4466" xsd:string
property_value: IAO:0000117 "https://orcid.org/0000-0002-7702-4495" xsd:string
property_value: IAO:0000117 "https://orcid.org/0000-0003-2687-1982" xsd:string

[Term]
id: T4FS:0000075
name: apply data access policy
def: "Define data access policy based on project requirements. Provide access to autorised parties." []
is_a: T4FS:0000469 ! access control and management
property_value: IAO:0000117 "Celia van Gelder" xsd:string
property_value: IAO:0000117 "Mateusz Kuzak" xsd:string
property_value: IAO:0000117 "Yan Wang" xsd:string

[Term]
id: T4FS:0000076
name: data discovery
def: "The ability to find and comprehend data produced by people other than yourself." [] {IAO:0000119="[PMQ]"}
comment: AL 15.3.22: tidied label from "discover other peoples data" to "Data discovery
is_a: T4FS:0000012 ! data stewardship activity
property_value: IAO:0000117 "https://orcid.org/0000-0002-7702-4495" xsd:string
property_value: IAO:0000117 "https://orcid.org/0000-0003-2687-1982" xsd:string
property_value: IAO:0000118 "Data search" xsd:string

[Term]
id: T4FS:0000078
name: documented data
def: "Data that are delivered with all associated metadata, data dictionary, description of methods and instruments used to collect and process the data, and other supporting data (such as duplicate sample results, replicate analyses, percent recovery, etc.) with the purpose of providing the full context in which the data were created." [] {IAO:0000119="RDMT. https://terms.codata.org/rdmt/documented-data"}
is_a: T4FS:0000430 ! data
property_value: IAO:0000117 "https://orcid.org/0000-0002-5214-4466" xsd:string
property_value: IAO:0000117 "https://orcid.org/0000-0003-2687-1982" xsd:string

[Term]
id: T4FS:0000079
name: conducting operations
is_a: T4FS:0000320 ! project management activities
property_value: IAO:0000117 "https://orcid.org/0000-0002-7702-4495" xsd:string
property_value: IAO:0000117 "https://orcid.org/0000-0003-2687-1982" xsd:string
property_value: IAO:0000117 "Philippe Rocca-Serra" xsd:string
property_value: IAO:0000117 "Susanna Sansone" xsd:string

[Term]
id: T4FS:0000080
name: dynamic data
def: "Data that are changing frequently and at asynchronous moments." [] {IAO:0000119="RDMT. https://terms.codata.org/rdmt/dynamic-data"}
is_a: T4FS:0000372 ! data stewardship technical concept
property_value: IAO:0000117 "https://orcid.org/0000-0002-5214-4466" xsd:string
property_value: IAO:0000117 "https://orcid.org/0000-0002-7702-4495" xsd:string
property_value: IAO:0000117 "https://orcid.org/0000-0003-2687-1982" xsd:string

[Term]
id: T4FS:0000081
name: reference model
def: "Design covering a class of frameworks with the following characteristics: (1) it can be used to generate more specific models that still belong to the class and (2) it can be used to compare a concrete framework design to identify whether it belongs to the same class." [] {IAO:0000119="RDMT. https://terms.codata.org/rdmt/reference-model"}
is_a: T4FS:0000372 ! data stewardship technical concept
relationship: T4FS:0000563 T4FS:0000137 ! contributes to the implementation of I1. (meta)data use a formal, accessible, shared, and broadly applicable language for knowledge representation
property_value: IAO:0000117 "https://orcid.org/0000-0002-5214-4466" xsd:string
property_value: IAO:0000117 "https://orcid.org/0000-0002-7702-4495" xsd:string
property_value: IAO:0000117 "https://orcid.org/0000-0003-2687-1982" xsd:string

[Term]
id: T4FS:0000082
name: online workbook
is_a: T4FS:0000095 ! online documentation
created_by: https://orcid.org/0000-0003-2687-1982
creation_date: 2020-10-01T20:52:57.551905Z

[Term]
id: T4FS:0000084
name: engaging in open innovation beyond academia
is_a: T4FS:0000106 ! publish data

[Term]
id: T4FS:0000085
name: registered data
def: "Data that have gone through a registration process and have been assigned an identifier metadata to aid in their search and retrieval." [] {IAO:0000119="RDMT. https://terms.codata.org/rdmt/registered-data"}
is_a: T4FS:0000430 ! data
property_value: IAO:0000117 "https://orcid.org/0000-0002-5214-4466" xsd:string
property_value: IAO:0000117 "https://orcid.org/0000-0002-7702-4495" xsd:string
property_value: IAO:0000117 "https://orcid.org/0000-0003-2687-1982" xsd:string

[Term]
id: T4FS:0000086
name: integrity
def: "In the context of data and network security, assurance that information can only be accessed or modified by those authorised to do so. Measures taken to ensure integrity include controlling the physical environment of networked terminals and servers, restricting access to data, and maintaining rigorous authentication practices. Data integrity can also be threatened by environmental hazards, such as heat, dust, and electrical surges." [] {IAO:0000119="RDMT. https://terms.codata.org/rdmt/integrity"}
is_a: T4FS:0000012 ! data stewardship activity
property_value: IAO:0000117 "https://orcid.org/0000-0002-5214-4466" xsd:string
property_value: IAO:0000117 "https://orcid.org/0000-0002-7702-4495" xsd:string
property_value: IAO:0000117 "https://orcid.org/0000-0003-2687-1982" xsd:string

[Term]
id: T4FS:0000087
name: digital scholarship
def: "Scholarship which is dependent upon digital methods, tools or resources. May include building a digital collection of information for further study and analysis; creating appropriate tools for collection-building; creating appropriate tools for the analysis and study of collections; using digital collections and analytical tools to generate new intellectual products; or creating authoring tools for these new intellectual products, either in traditional forms or in digital form." [] {IAO:0000119="RDMT. https://terms.codata.org/rdmt/digital-scholarship"}
is_a: T4FS:0000012 ! data stewardship activity
property_value: IAO:0000117 "https://orcid.org/0000-0002-5214-4466" xsd:string
property_value: IAO:0000117 "https://orcid.org/0000-0002-7702-4495" xsd:string
property_value: IAO:0000117 "https://orcid.org/0000-0003-2687-1982" xsd:string

[Term]
id: T4FS:0000088
name: a knowledge for resource management
def: "Bin for types of Knowledge related to Resource management" []
is_a: T4FS:0000353 ! resource management
property_value: IAO:0000117 "leightonlc" xsd:string

[Term]
id: T4FS:0000089
name: aptitudes for resource management
def: "Bin for Aptitudes related to Resource management." []
is_a: T4FS:0000353 ! resource management
property_value: IAO:0000117 "leightonlc" xsd:string

[Term]
id: T4FS:0000091
name: knowledge of storage management
def: "Bin for types of Knowledge related to Storage management." []
is_a: T4FS:0000053 ! storage management
property_value: IAO:0000117 "leightonlc" xsd:string

[Term]
id: T4FS:0000092
name: understand open access publishing
def: "Know about the open access publishing procedure, journals' policies on OA publishing, project funder and institutions policy as well as the financial support on OA publishing" []
is_a: T4FS:0000193 ! open access publishing
property_value: IAO:0000117 "Celia van Gelder" xsd:string
property_value: IAO:0000117 "Mateusz Kuzak" xsd:string
property_value: IAO:0000117 "Yan Wang" xsd:string

[Term]
id: T4FS:0000093
name: use of persistent, resolvable identifiers (pids)
def: "OBSOLETE. The use of persistent identifiers or PIDs to uniquely and persistently identify an entity." [] {IAO:0000119="[PMQ 3.2022]"}
comment: This term is redundant with http://purl.obolibrary.org/obo/T4FS_0000388 and has been deprecated.
property_value: IAO:0000117 "https://orcid.org/0000-0002-7702-4495" xsd:string
property_value: IAO:0000117 "https://orcid.org/0000-0003-2687-1982" xsd:string
property_value: IAO:0000117 "Nancy Hoebelheinrich" xsd:string
property_value: IAO:0000233 "https://github.com/terms4fairskills/FAIRterminology/issues/21" xsd:string
is_obsolete: true

[Term]
id: T4FS:0000094
name: record standardization
def: "Process in which files are first parsed (assigned to appropriate fields in a record) and then translated to a common format. Data often lack consistency simply because there are many ways of saying the same thing. Standardising the record ensures that when a query is run for a particular field, accurate results will be returned." [] {IAO:0000119="RDMT. https://terms.codata.org/rdmt/record-standardisation"}
is_a: T4FS:0000012 ! data stewardship activity
property_value: IAO:0000117 "https://orcid.org/0000-0002-5214-4466" xsd:string
property_value: IAO:0000117 "https://orcid.org/0000-0002-7702-4495" xsd:string
property_value: IAO:0000117 "https://orcid.org/0000-0003-2687-1982" xsd:string
property_value: IAO:0000233 "https://github.com/terms4fairskills/FAIRterminology/issues/32" xsd:string

[Term]
id: T4FS:0000095
name: online documentation
is_a: T4FS:0000519 ! learning medium
property_value: IAO:0000117 "https://orcid.org/0000-0003-2687-1982" xsd:string
created_by: https://orcid.org/0000-0003-2687-1982
creation_date: 2020-10-01T20:53:59.107153Z

[Term]
id: T4FS:0000096
name: metadata catalogue
def: "Catalogue containing metadata records that enables services to find data and services." [] {IAO:0000119="RDMT. https://terms.codata.org/rdmt/metadata-catalogue"}
is_a: T4FS:0000372 ! data stewardship technical concept
relationship: T4FS:0000563 T4FS:0000393 ! contributes to the implementation of F4. (meta)data are registered or indexed in a searchable resource
property_value: IAO:0000117 "https://orcid.org/0000-0002-5214-4466" xsd:string
property_value: IAO:0000117 "https://orcid.org/0000-0002-7702-4495" xsd:string
property_value: IAO:0000117 "https://orcid.org/0000-0003-2687-1982" xsd:string
created_by: https://orcid.org/0000-0003-2687-1982

[Term]
id: T4FS:0000097
name: understand legal background of patents
def: "Learn about the types of patents and its legal implications. Understand the application procedure of patents." []
is_a: T4FS:0000042 ! ethical application of patents, licenses
property_value: IAO:0000117 "Celia van Gelder" xsd:string
property_value: IAO:0000117 "Mateusz Kuzak" xsd:string
property_value: IAO:0000117 "Yan Wang" xsd:string

[Term]
id: T4FS:0000098
name: data file format
def: "Layout of a file in terms of how the data within the file are organised and encoded for storage." [] {IAO:0000119="RDMT. https://terms.codata.org/rdmt/data-file-format"}
is_a: T4FS:0000372 ! data stewardship technical concept
property_value: IAO:0000117 "https://orcid.org/0000-0002-5214-4466" xsd:string
property_value: IAO:0000117 "https://orcid.org/0000-0003-2687-1982" xsd:string
property_value: IAO:0000118 "Research data format" xsd:string

[Term]
id: T4FS:0000100
name: data catalogue
def: "Curated collection of metadata records describing datasets and their data elements. Curated and organised using a formal metadata schema appropriate to data and data sets (e.g. ReCollect etc)." [] {IAO:0000119="RDMT. https://terms.codata.org/rdmt/data-catalogue"}
is_a: T4FS:0000215 ! data store
property_value: IAO:0000117 "https://orcid.org/0000-0002-5214-4466" xsd:string
property_value: IAO:0000117 "https://orcid.org/0000-0003-2687-1982" xsd:string

[Term]
id: T4FS:0000102
name: curation workflow
def: "A type of workflow that includes active steps to curate data as an aid to on-going management of data through its lifecycle." [] {IAO:0000119="Definition from now–deprecated CASRAI Glossary term: curation-workflow"}
is_a: T4FS:0000372 ! data stewardship technical concept
property_value: IAO:0000117 "https://orcid.org/0000-0002-5214-4466" xsd:string
property_value: IAO:0000117 "https://orcid.org/0000-0003-2687-1982" xsd:string

[Term]
id: T4FS:0000103
name: A1.1 the protocol is open, free, and universally implementable
is_a: T4FS:0000038 ! A1. (meta)data are retrievable by their identifier using a standardised communications protocol
property_value: IAO:0000117 "https://orcid.org/0000-0003-2687-1982" xsd:string

[Term]
id: T4FS:0000104
name: preservation costs management
def: "Planning for and controlling the present and future costs of the conservation of data, including technical storage, fixed costs, and staff resources." [] {IAO:0000119="Based on https://www.cessda.eu/About/Projects/Past-projects/CESSDA-SaW/WP4/Cost-Benefit-Advocacy-Toolkit/Costs-Factsheet [LLC]"}
is_a: T4FS:0000353 ! resource management
property_value: IAO:0000117 "Kristina Hettne" xsd:string
property_value: IAO:0000117 "Leighton Christiansen" xsd:string
property_value: IAO:0000117 "Simon Hodson" xsd:string
property_value: IAO:0000117 "Victoria Dominguez Del Angel" xsd:string

[Term]
id: T4FS:0000105
name: project manager
def: "The person who is tasked with delivering a project within the boundaries and framework established by the program manager. The project manager is and should be delivery and execution focused and is judged on the elements of time, cost, and scope of the project. The person responsible for ensuring that the Project Team completes the project. The Project Manager develops the Project Plan with the team and manages the teamís performance of project tasks. It is also the responsibility of the Project Manager to secure acceptance and approval of deliverables from the Project Sponsor and Stakeholders. The Project Manager is responsible for communication, including status reporting, risk management, escalation of issues that cannot be resolved in the team, and, in general, making sure the project is delivered in budget, on schedule, and within scope." [] {IAO:0000119="Definition from now-deprecated CASRAI Glossary term: project-manager"}
is_a: T4FS:0000415 ! manager
property_value: IAO:0000117 "https://orcid.org/0000-0002-5214-4466" xsd:string
property_value: IAO:0000117 "https://orcid.org/0000-0002-7702-4495" xsd:string
property_value: IAO:0000117 "https://orcid.org/0000-0003-2687-1982" xsd:string

[Term]
id: T4FS:0000106
name: publish data
comment: AL 9.3.22. Removed from 'FAIR4S defined activity' class to better integrate with the T4FS hierarchy. AL 5.5.22: removed "Publishing and archiving data" and "Publish and archive data" alternative terms, as the two actions are not the same.
is_a: T4FS:0000021 ! exposing data
property_value: IAO:0000117 "Celia van Gelder" xsd:string
property_value: IAO:0000117 "https://orcid.org/0000-0002-7702-4495" xsd:string
property_value: IAO:0000117 "https://orcid.org/0000-0003-2687-1982" xsd:string
property_value: IAO:0000117 "Mateusz Kuzak" xsd:string
property_value: IAO:0000117 "Yan Wang" xsd:string
property_value: IAO:0000118 "Release data" xsd:string

[Term]
id: T4FS:0000107
name: information security
comment: AL 16.3.22: Changed 'information security and access management' such that access management went in as an alternative term. If required in future, we may wish to separate it out completely.
is_a: T4FS:0000012 ! data stewardship activity
property_value: IAO:0000117 "https://orcid.org/0000-0002-7702-4495" xsd:string
property_value: IAO:0000118 "Access management" xsd:string

[Term]
id: T4FS:0000108
name: data production
def: "All activities involved in the planning, collecting, processing, analysis and maintenance of data in the original research project. Among these activities are selecting a study design, constructing instruments for data collection, conducting data collection/creation, performing data editing/verification/validation, analysing data, backing up data versions and preparing and tagging metadata." [] {IAO:0000119="RDMT. https://terms.codata.org/rdmt/data-production"}
is_a: T4FS:0000231 ! data acquisition
property_value: IAO:0000117 "https://orcid.org/0000-0002-5214-4466" xsd:string
property_value: IAO:0000117 "https://orcid.org/0000-0003-2687-1982" xsd:string

[Term]
id: T4FS:0000109
name: raw data
def: "Data that have not been processed for meaningful use. Although raw data have the potential to become information, they require selective extraction, organisation, and sometimes analysis and formatting for presentation." [] {IAO:0000119="RDMT. https://terms.codata.org/rdmt/raw-data"}
is_a: T4FS:0000430 ! data
property_value: IAO:0000117 "https://orcid.org/0000-0002-5214-4466" xsd:string
property_value: IAO:0000117 "https://orcid.org/0000-0002-7702-4495" xsd:string
property_value: IAO:0000117 "https://orcid.org/0000-0003-2687-1982" xsd:string
property_value: IAO:0000118 "Source data" xsd:string

[Term]
id: T4FS:0000112
name: interface testing
def: "Testing conducted to evaluate whether systems or components pass data and control correctly to each other." [] {IAO:0000119="Definition from now-deprecated CASRAI Glossary term: interface-testing"}
is_a: T4FS:0000126 ! assessment
property_value: IAO:0000117 "https://orcid.org/0000-0002-5214-4466" xsd:string
property_value: IAO:0000117 "https://orcid.org/0000-0002-7702-4495" xsd:string
property_value: IAO:0000117 "https://orcid.org/0000-0003-2687-1982" xsd:string

[Term]
id: T4FS:0000113
name: digital object
def: "Machine-independent data structure consisting of one or more elements in digital form that can be parsed by different information systems; the structure helps to enable interoperability among diverse information systems. A digital object is composed of a structured sequence of bits/bytes. The bit sequence realising the object can be identified and accessed by a unique and persistent identifier or by use of referencing attributes describing its properties." [] {IAO:0000119="RDMT. https://terms.codata.org/rdmt/digital-object"}
is_a: T4FS:0000372 ! data stewardship technical concept
property_value: IAO:0000117 "https://orcid.org/0000-0002-5214-4466" xsd:string
property_value: IAO:0000117 "https://orcid.org/0000-0002-7702-4495" xsd:string
property_value: IAO:0000117 "https://orcid.org/0000-0003-2687-1982" xsd:string
property_value: IAO:0000118 "Digital entity" xsd:string

[Term]
id: T4FS:0000114
name: digital materials
def: "A broad term encompassing: (a) digital surrogates created as a result of converting analogue materials to digital form (digitisation); (b) born digital for which there has never been and is never intended to be an analogue equivalent; and, (c) digital records." [] {IAO:0000119="RDMT. https://terms.codata.org/rdmt/digital-materials"}
is_a: T4FS:0000372 ! data stewardship technical concept
property_value: IAO:0000117 "https://orcid.org/0000-0002-5214-4466" xsd:string
property_value: IAO:0000117 "https://orcid.org/0000-0002-7702-4495" xsd:string
property_value: IAO:0000117 "https://orcid.org/0000-0003-2687-1982" xsd:string

[Term]
id: T4FS:0000116
name: define access policy
def: "Understand the needs and conditions of information access for different stakeholder groups. Identify the responsibility and rights for each stakeholder group on informaiton access. Build up a catalogue of risk profiles. For each risk profile, develope mitigation protocols." []
is_a: T4FS:0000107 ! information security
property_value: IAO:0000117 "Angus Whyte" xsd:string
property_value: IAO:0000117 "Celia van Gelder" xsd:string
property_value: IAO:0000117 "Mateusz Kuzak" xsd:string
property_value: IAO:0000117 "Yan Wang" xsd:string

[Term]
id: T4FS:0000117
name: skills related to provenance information management
def: "Bin for Skills needed for Provenance information management." []
is_a: T4FS:0000368 ! provenance information management
created_by: leightonlc
creation_date: 2019-10-17T15:17:02.313138Z

[Term]
id: T4FS:0000118
name: remote data access
def: "Ability to access and download data from a repository." [] {IAO:0000119="RDMT. https://terms.codata.org/rdmt/remote-data-access"}
is_a: T4FS:0000372 ! data stewardship technical concept
property_value: IAO:0000117 "https://orcid.org/0000-0002-5214-4466" xsd:string
property_value: IAO:0000117 "https://orcid.org/0000-0002-7702-4495" xsd:string
property_value: IAO:0000117 "https://orcid.org/0000-0003-2687-1982" xsd:string

[Term]
id: T4FS:0000119
name: disambiguation
def: "The act of interpreting an author's intended use of a word that has multiple meanings or spellings." [] {IAO:0000119="Definition from now-deprecated CASRAI Glossary term: dissambuation"}
is_a: T4FS:0000036 ! curation
property_value: IAO:0000117 "https://orcid.org/0000-0002-5214-4466" xsd:string
property_value: IAO:0000117 "https://orcid.org/0000-0002-7702-4495" xsd:string
property_value: IAO:0000117 "https://orcid.org/0000-0003-2687-1982" xsd:string

[Term]
id: T4FS:0000120
name: data compliance
def: "Ongoing processes to ensure adherence of data to both enterprise business rules (government department, university, industry, or agency), and to legal, regulatory and accreditation requirements. Includes five areas: controls, audit, legal compliance, regulatory compliance, and accreditation conformance." [] {IAO:0000119="RDMT. https://terms.codata.org/rdmt/data-compliance"}
is_a: T4FS:0000372 ! data stewardship technical concept
property_value: IAO:0000117 "https://orcid.org/0000-0002-5214-4466" xsd:string
property_value: IAO:0000117 "https://orcid.org/0000-0003-2687-1982" xsd:string

[Term]
id: T4FS:0000121
name: re-use
def: "The re-analysis of a dataset or combination of datasets outside of the original research purpose for which the dataset was created." [] {IAO:0000119="RDMT. https://terms.codata.org/rdmt/re-use"}
comment: AL 2.3.23: Removed because of its high level of similarity with the 'R' FAIR principle.
property_value: IAO:0000117 "https://orcid.org/0000-0002-5214-4466" xsd:string
property_value: IAO:0000117 "https://orcid.org/0000-0002-7702-4495" xsd:string
property_value: IAO:0000117 "https://orcid.org/0000-0003-2687-1982" xsd:string
property_value: IAO:0000233 "https://github.com/terms4fairskills/FAIRterminology/issues/15" xsd:string
is_obsolete: true

[Term]
id: T4FS:0000122
name: trainer/teacher
relationship: T4FS:0000558 T4FS:0000012 ! has/wants competency in data stewardship activity
relationship: T4FS:0000559 T4FS:0000372 ! has/wants knowledge about data stewardship technical concept
relationship: T4FS:0000559 T4FS:0000446 ! has/wants knowledge about data stewardship guideline
relationship: T4FS:0000561 T4FS:0000372 ! has/wants practical skill about data stewardship technical concept
relationship: T4FS:0000562 T4FS:0000548 ! has aptitude for data stewardship soft skill

[Term]
id: T4FS:0000123
name: aptitudes for identity management
def: "Bin for Aptitudes related to Identity management." []
is_a: T4FS:0000169 ! identity management
property_value: IAO:0000117 "leightonlc" xsd:string

[Term]
id: T4FS:0000124
name: understand information security challenges
def: "Know the security requirements on the organization regarding different types of information Know the current organizational policy, infrastructure and capacity on information security." []
is_a: T4FS:0000107 ! information security
property_value: IAO:0000117 "Angus Whyte" xsd:string
property_value: IAO:0000117 "Celia van Gelder" xsd:string
property_value: IAO:0000117 "Mateusz Kuzak" xsd:string
property_value: IAO:0000117 "Yan Wang" xsd:string

[Term]
id: T4FS:0000125
name: aptitudes for authorisation management
def: "Bin for Aptitudes related to Authorization management." []
is_a: T4FS:0000142 ! authorisation management
property_value: IAO:0000117 "leightonlc" xsd:string

[Term]
id: T4FS:0000126
name: assessment
comment: AL 17.3.22: Updated to "Assessment" to match the style of its sibling classes. AL 3.22: Was "govern and assess", which is a compound concept. Split into two classes, Assess and Governance. Original source: FAIR4S defined activity.
is_a: T4FS:0000012 ! data stewardship activity
property_value: IAO:0000117 "Angus Whyte" xsd:string
property_value: IAO:0000117 "Celia van Gelder" xsd:string
property_value: IAO:0000117 "https://orcid.org/0000-0002-7702-4495" xsd:string
property_value: IAO:0000117 "Mateusz Kuzak" xsd:string
property_value: IAO:0000117 "Yan Wang" xsd:string

[Term]
id: T4FS:0000127
name: personal information privacy
def: "The World Wide Web Consortium’s Platform for Personal Privacy Project (P3P) offers specific recommendations for practices that will let users define and share personal information with Web sites that they agree to share it with. The P3P incorporates a number of industry proposals, including the Open Profiling Standard (OPS). Using software that adheres to the P3P recommendations, users will be able to create a personal profile, all or parts of which can be made accessible to a Web site as the user directs. A tool that will help a user decide whether to trust a given website with personal information is a Statement of Privacy Policy that a website can post." [] {IAO:0000119="RDMT. https://terms.codata.org/rdmt/personal-information-privacy"}
is_a: T4FS:0000372 ! data stewardship technical concept
property_value: IAO:0000117 "https://orcid.org/0000-0002-5214-4466" xsd:string
property_value: IAO:0000117 "https://orcid.org/0000-0002-7702-4495" xsd:string
property_value: IAO:0000117 "https://orcid.org/0000-0003-2687-1982" xsd:string

[Term]
id: T4FS:0000129
name: ability to solve fair implementation problems collaboratively
def: "Demonstrate ability to involve others and share responsibility for applying FAIR principles." [] {IAO:0000119="[PMQ, 3.2022]"}
is_a: T4FS:0000399 ! ability to learn new techniques for fair implementation
property_value: IAO:0000117 "Angus Whyte" xsd:string

[Term]
id: T4FS:0000131
name: skills related to cloud computing environment management
def: "Bin for Skills needed for Cloud computing environment management." []
is_a: T4FS:0000479 ! cloud computing environment management
created_by: leightonlc
creation_date: 2019-10-17T15:14:37.180683Z

[Term]
id: T4FS:0000132
name: data curation
def: "Managed process throughout the data lifecycle, by which data/data collections are cleansed, documented, standardised, formatted and inter-related. This includes versioning data, or forming a new collection from several data sources, annotating with metadata, adding codes to raw data (e.g., classifying a galaxy image with a galaxy type such as “spiral”). Higher levels of curation involve maintaining links with annotation and with other published materials. Thus a dataset may include a citation link to publication whose analysis was based on the data. The goal of curation is to manage and promote the use of data from its point of creation to ensure it is fit for contemporary purpose and available for discovery and re-use. For dynamic datasets this may mean continuous enrichment or updating to keep it fit for purpose. Special forms of curation may be available in data repositories. The data curation process itself must be documented as part of curation. Thus curation and provenance are highly related." [] {IAO:0000119="RDMT. https://terms.codata.org/rdmt/data-curation"}
is_a: T4FS:0000036 ! curation
property_value: IAO:0000117 "https://orcid.org/0000-0002-5214-4466" xsd:string
property_value: IAO:0000117 "https://orcid.org/0000-0003-2687-1982" xsd:string

[Term]
id: T4FS:0000133
name: cite contributions
def: "Cite contributions to data work in published literature which draws upon that data." [] {IAO:0000119="[LM]"}
is_a: T4FS:0000021 ! exposing data
property_value: IAO:0000117 "https://orcid.org/0000-0003-2687-1982" xsd:string
property_value: IAO:0000117 "Laura Molloy" xsd:string

[Term]
id: T4FS:0000134
name: operational management
def: "Ongoing organizational activities associated with supporting functional elements, as opposed to project elements. Operational management also includes support of products that the organization has created through project activity." [] {IAO:0000119="Definition from now-deprecated CASRAI Glossary term: operational-management"}
is_a: T4FS:0000548 ! data stewardship soft skill
property_value: IAO:0000117 "https://orcid.org/0000-0002-5214-4466" xsd:string
property_value: IAO:0000117 "https://orcid.org/0000-0002-7702-4495" xsd:string
property_value: IAO:0000117 "https://orcid.org/0000-0003-2687-1982" xsd:string

[Term]
id: T4FS:0000135
name: high quality data
def: "Data that are complete, timely, accurate, consistent, relevant, reliable, traceable, cleaned, validated, and well documented." [] {IAO:0000119="RDMT. https://terms.codata.org/rdmt/high-quality-data"}
is_a: T4FS:0000372 ! data stewardship technical concept
property_value: IAO:0000117 "https://orcid.org/0000-0002-5214-4466" xsd:string
property_value: IAO:0000117 "https://orcid.org/0000-0003-2687-1982" xsd:string

[Term]
id: T4FS:0000136
name: how to make your data reuseable
def: "Understand what reuse is permitted according to the licenses or terms and conditions applicable to services, tools and their content." []
is_a: T4FS:0000481 ! the use of fair and open research tools or services
property_value: IAO:0000117 "Angus Whyte" xsd:string

[Term]
id: T4FS:0000137
name: I1. (meta)data use a formal, accessible, shared, and broadly applicable language for knowledge representation
is_a: T4FS:0000014 ! interoperability of digital assets
property_value: IAO:0000117 "https://orcid.org/0000-0003-2687-1982" xsd:string

[Term]
id: T4FS:0000138
name: schema
name: schema (database)
def: "Organisation or structure for a database. The activity of data modelling leads to a schema. (The plural form is schemata.) The term is used in discussing both relational databases and object-oriented databases. The term sometimes refers to a visualisation of a structure and sometimes to a formal text-oriented description." [] {IAO:0000119="RDMT. https://terms.codata.org/rdmt/schema-database"}
is_a: T4FS:0000372 ! data stewardship technical concept
property_value: IAO:0000117 "https://orcid.org/0000-0002-5214-4466" xsd:string
property_value: IAO:0000117 "https://orcid.org/0000-0002-7702-4495" xsd:string
property_value: IAO:0000117 "https://orcid.org/0000-0003-2687-1982" xsd:string

[Term]
id: T4FS:0000139
name: pid service
def: "Service that provides a connection between a PID and its target object." [] {IAO:0000119="RDMT. https://terms.codata.org/rdmt/pid-service"}
is_a: T4FS:0000453 ! persistent identifier
property_value: IAO:0000117 "https://orcid.org/0000-0002-5214-4466" xsd:string
property_value: IAO:0000117 "https://orcid.org/0000-0002-7702-4495" xsd:string
property_value: IAO:0000117 "https://orcid.org/0000-0003-2687-1982" xsd:string

[Term]
id: T4FS:0000140
name: foundational interoperability
def: "Set of conditions that allow data exchange from one information technology system to be received by another and does not require the ability for the receiving information technology system to interpret the data." [] {IAO:0000119="RDMT. https://terms.codata.org/rdmt/foundational-interoperability"}
is_a: T4FS:0000020 ! interoperability
property_value: IAO:0000117 "https://orcid.org/0000-0002-5214-4466" xsd:string
property_value: IAO:0000117 "https://orcid.org/0000-0003-2687-1982" xsd:string

[Term]
id: T4FS:0000141
name: data management
def: "The activities of data policies, data planning, data element standardization, information management control, data synchronization, data sharing, and database development, including practices and projects that acquire, control, protect, deliver and enhance the value of data and information." [] {IAO:0000119="Definition from now-deprecated CASRAI Glossary term: data-management"}
is_a: T4FS:0000353 ! resource management
property_value: IAO:0000117 "https://orcid.org/0000-0002-5214-4466" xsd:string
property_value: IAO:0000117 "https://orcid.org/0000-0003-2687-1982" xsd:string

[Term]
id: T4FS:0000142
name: authorisation management
def: "Authorization management is concerned with people's access to different objects, most often to data or physical objects, such as land, buildings, rooms or infrastructure." [] {IAO:0000119="https://managementmania.com/en/authorization-management"}
is_a: T4FS:0000353 ! resource management
property_value: IAO:0000117 "Kristina Hettne" xsd:string
property_value: IAO:0000117 "Leighton Christiansen" xsd:string
property_value: IAO:0000117 "Simon Hodson" xsd:string
property_value: IAO:0000117 "Victoria Dominguez Del Angel" xsd:string

[Term]
id: T4FS:0000143
name: knowledge of authorisation management
def: "Bin for types of Knowledge related to Authorization management." []
is_a: T4FS:0000142 ! authorisation management
property_value: IAO:0000117 "leightonlc" xsd:string

[Term]
id: T4FS:0000145
name: search repositories and knowledge-bases
def: "The ability to search repositories and knowledge-bases." [] {IAO:0000119="[PMQ]"}
is_a: T4FS:0000076 ! data discovery
property_value: IAO:0000117 "https://orcid.org/0000-0003-2687-1982" xsd:string
property_value: IAO:0000118 "database search" xsd:string
property_value: IAO:0000118 "Repository search" xsd:string
property_value: IAO:0000118 "searching databases" xsd:string
property_value: IAO:0000118 "searching repositories" xsd:string

[Term]
id: T4FS:0000146
name: cloud ecosystem
def: "Ecosystem that includes software, infrastructure, consultants, integrators, partners, third parties and anything else in the specified environment that has a bearing on the other components." [] {IAO:0000119="RDMT. https://terms.codata.org/rdmt/cloud-ecosystem"}
is_a: T4FS:0000372 ! data stewardship technical concept
property_value: IAO:0000117 "https://orcid.org/0000-0002-5214-4466" xsd:string
property_value: IAO:0000117 "https://orcid.org/0000-0003-2687-1982" xsd:string

[Term]
id: T4FS:0000148
name: understand legal background of licensing
def: "Learn about  data licensing, the types of data licences and its legal implications. Understand the application procedure of data licences." []
is_a: T4FS:0000042 ! ethical application of patents, licenses
property_value: IAO:0000117 "Celia van Gelder" xsd:string
property_value: IAO:0000117 "Mateusz Kuzak" xsd:string
property_value: IAO:0000117 "Yan Wang" xsd:string

[Term]
id: T4FS:0000149
name: archive
def: "A place or collection containing static records, documents, or other materials for long-term preservation." [] {IAO:0000119="RDMT. https://terms.codata.org/rdmt/archive"}
is_a: T4FS:0000372 ! data stewardship technical concept
property_value: IAO:0000117 "https://orcid.org/0000-0002-5214-4466" xsd:string
property_value: IAO:0000117 "https://orcid.org/0000-0003-2687-1982" xsd:string

[Term]
id: T4FS:0000150
name: trusted digital repository
def: "An infrastructure component that provides reliable, long-term access to managed digital resources. It stores, manages, and curates digital objects and returns their bit streams when a request is issued. Trusted repositories undergo regular assessments according to a set of rules such as defined by Data Seal of Approval (DSA) or TRAC (ISO 16363). It is well understood that such an assessment has the potential of increasing trust from its depositors and users, but it will not be the only criterion for users. Repositories can be at different stages of assessments. However, it is evident that certain quality criteria need to be met to distinguish trusted repositories from all types of other entities that store data such as notebooks or lab servers." [] {IAO:0000119="Definition from now-deprecated CASRAI Glossary term: trusted-digital-repository"}
is_a: T4FS:0000372 ! data stewardship technical concept
property_value: IAO:0000117 "https://orcid.org/0000-0002-5214-4466" xsd:string
property_value: IAO:0000117 "https://orcid.org/0000-0002-7702-4495" xsd:string
property_value: IAO:0000117 "https://orcid.org/0000-0003-2687-1982" xsd:string

[Term]
id: T4FS:0000151
name: database administration
def: "Managing the physical aspects of data resources, including database design and integrity, backup and recovery, performance and tuning." [] {IAO:0000119="RDMT. https://terms.codata.org/rdmt/database-administration"}
is_a: T4FS:0000141 ! data management
property_value: IAO:0000117 "https://orcid.org/0000-0002-5214-4466" xsd:string
property_value: IAO:0000117 "https://orcid.org/0000-0002-7702-4495" xsd:string
property_value: IAO:0000117 "https://orcid.org/0000-0003-2687-1982" xsd:string

[Term]
id: T4FS:0000152
name: knowledge of identity management
def: "Bin for types of Knowledge related to Identity management" []
is_a: T4FS:0000169 ! identity management
property_value: IAO:0000117 "leightonlc" xsd:string

[Term]
id: T4FS:0000153
name: quality assessment
is_a: T4FS:0000126 ! assessment
property_value: IAO:0000117 "Angus Whyte" xsd:string
property_value: IAO:0000117 "Celia van Gelder" xsd:string
property_value: IAO:0000117 "Mateusz Kuzak" xsd:string
property_value: IAO:0000117 "Yan Wang" xsd:string

[Term]
id: T4FS:0000154
name: data structure
def: "Specialised format for organising and storing data. General data structure types include the array, the file, the record, the table, the tree, and so on. Any data structure is designed to organise data to suit a specific purpose so that it can be accessed and worked with in appropriate ways. In computer programming, a data structure may be selected or designed to store data for the purpose of working on it with various algorithms." [] {IAO:0000119="RDMT. https://terms.codata.org/rdmt/data-structure"}
is_a: T4FS:0000372 ! data stewardship technical concept
property_value: IAO:0000117 "https://orcid.org/0000-0002-5214-4466" xsd:string
property_value: IAO:0000117 "https://orcid.org/0000-0003-2687-1982" xsd:string
property_value: IAO:0000118 "Data format" xsd:string

[Term]
id: T4FS:0000155
name: information technology specialist
def: "Information systems and technology infrastructure manager, expert, or technician." [] {IAO:0000119="RDMT. https://terms.codata.org/rdmt/information-technology-specialist"}
relationship: T4FS:0000558 T4FS:0000012 ! has/wants competency in data stewardship activity
relationship: T4FS:0000559 T4FS:0000372 ! has/wants knowledge about data stewardship technical concept
relationship: T4FS:0000559 T4FS:0000446 ! has/wants knowledge about data stewardship guideline
relationship: T4FS:0000561 T4FS:0000372 ! has/wants practical skill about data stewardship technical concept
relationship: T4FS:0000562 T4FS:0000548 ! has aptitude for data stewardship soft skill
property_value: IAO:0000117 "https://orcid.org/0000-0002-5214-4466" xsd:string
property_value: IAO:0000117 "https://orcid.org/0000-0003-2687-1982" xsd:string

[Term]
id: T4FS:0000156
name: archiving
def: "A curation activity that ensures that data are properly selected, stored, and can be accessed, and for which logical and physical integrity are maintained over time, including security and authenticity." [] {IAO:0000119="RDMT. https://terms.codata.org/rdmt/archive-verb"}
is_a: T4FS:0000012 ! data stewardship activity
property_value: IAO:0000117 "https://orcid.org/0000-0002-5214-4466" xsd:string
property_value: IAO:0000117 "https://orcid.org/0000-0003-2687-1982" xsd:string

[Term]
id: T4FS:0000157
name: knowledge of preservation costs management
def: "Bin for types of Knowledge related to Preservation costs management." []
is_a: T4FS:0000104 ! preservation costs management
created_by: leightonlc
creation_date: 2019-10-17T15:17:32.816776Z

[Term]
id: T4FS:0000158
name: user acceptance testing
def: "A phase of development where the product is tested in the real world by the intended audience. The experiences of the early users are forwarded back to the developers who make final changes before releasing the product." [] {IAO:0000119="Definition from now-deprecated CASRAI Glossary term: user-acceptance-testing/"}
is_a: T4FS:0000012 ! data stewardship activity
property_value: IAO:0000117 "https://orcid.org/0000-0002-5214-4466" xsd:string
property_value: IAO:0000117 "https://orcid.org/0000-0002-7702-4495" xsd:string
property_value: IAO:0000117 "https://orcid.org/0000-0003-2687-1982" xsd:string

[Term]
id: T4FS:0000159
name: minimal metadata
def: "Description of a digital object with a limited number of fields including at least a name and persistent identifier." [] {IAO:0000119="RDMT. https://terms.codata.org/rdmt/minimal-metadata"}
is_a: T4FS:0000527 ! metadata
property_value: IAO:0000117 "https://orcid.org/0000-0002-5214-4466" xsd:string
property_value: IAO:0000117 "https://orcid.org/0000-0002-7702-4495" xsd:string

[Term]
id: T4FS:0000160
name: metadata exposure
def: "Metadata exposure is the process of finding, identifying, selecting and acquiring/obtaining access to a metadata entity." [] {IAO:0000119="AL 22.3.22, and see also FRBR User Tasks at: https://sites.google.com/site/metadatastandards/chapter-6/6-3-frbr-user-tasks."}
comment: AL 22.3.22: Refactored from 'metadata creation and exposure'. Metadata creation has moved to the Curation hierarchy.
is_a: T4FS:0000021 ! exposing data
property_value: IAO:0000117 "https://orcid.org/0000-0002-7702-4495" xsd:string
property_value: IAO:0000117 "Nancy Hoebelheinrich" xsd:string

[Term]
id: T4FS:0000161
name: data destruction
def: "Process of destroying data stored on tapes, hard disks and other forms of electronic media so that it is completely unreadable and cannot be accessed or used." [] {IAO:0000119="RDMT. https://terms.codata.org/rdmt/data-destruction"}
is_a: T4FS:0000107 ! information security
property_value: IAO:0000117 "https://orcid.org/0000-0002-5214-4466" xsd:string

[Term]
id: T4FS:0000162
name: fair stewardship training
def: "The provision of training materials and events in and around good data stewardship." [] {IAO:0000119="PMQ"}
is_a: T4FS:0000259 ! fair training
property_value: IAO:0000117 "https://orcid.org/0000-0002-7702-4495" xsd:string
property_value: IAO:0000117 "https://orcid.org/0000-0003-2687-1982" xsd:string
property_value: IAO:0000117 "Philippe Rocca-Serra" xsd:string
property_value: IAO:0000117 "Susanna Sansone" xsd:string

[Term]
id: T4FS:0000165
name: creativity
def: "The ability to have an innovative approach to research by creating new or modified current concepts, theories, approaches and/or solutions." [] {IAO:0000119="Definition from now-deprecated CASRAI Glossary term: creativity"}
is_a: T4FS:0000548 ! data stewardship soft skill
property_value: IAO:0000117 "https://orcid.org/0000-0002-5214-4466" xsd:string
property_value: IAO:0000117 "https://orcid.org/0000-0003-2687-1982" xsd:string

[Term]
id: T4FS:0000166
name: data table attribute
name: data table attribute (field)
def: "Field or column in a database table. It is an abbreviation for ‘physical data attribute’ which is a single data element related to a data object, such as a table in a database. The database schema associates one or more attributes with each database entity (i.e. table)." [] {IAO:0000119="RDMT. https://terms.codata.org/rdmt/data-table-attribute-field"}
is_a: T4FS:0000372 ! data stewardship technical concept
property_value: IAO:0000117 "https://orcid.org/0000-0002-5214-4466" xsd:string
property_value: IAO:0000117 "https://orcid.org/0000-0003-2687-1982" xsd:string

[Term]
id: T4FS:0000168
name: consensus standard
def: "A standard developed through the cooperation of all parties who have an interest in participating in its development and/or use." [] {IAO:0000119="Definition from now-deprecated CASRAI Glossary term: consensus-standard"}
is_a: T4FS:0000372 ! data stewardship technical concept
relationship: T4FS:0000563 T4FS:0000137 ! contributes to the implementation of I1. (meta)data use a formal, accessible, shared, and broadly applicable language for knowledge representation
property_value: IAO:0000117 "https://orcid.org/0000-0002-5214-4466" xsd:string
property_value: IAO:0000117 "https://orcid.org/0000-0003-2687-1982" xsd:string
property_value: IAO:0000118 "Community standard" xsd:string

[Term]
id: T4FS:0000169
name: identity management
def: "Identity Management (IdM), also called Identity and Access Management (IAM) refers to a framework of policies and technologies for ensuring that the proper  user in an organisation has the appropriate access to technology resources  systems fall under the overarching umbrella of IT security.  IdM systems not only identify, but authenticate and authorize individuals  who will be using IT resources, but also the hardware and applications users need to access." [] {IAO:0000119="https://en.wikipedia.org/wiki/Identity_management"}
is_a: T4FS:0000353 ! resource management
property_value: IAO:0000117 "Kristina Hettne" xsd:string
property_value: IAO:0000117 "Leighton Christiansen" xsd:string
property_value: IAO:0000117 "Simon Hodson" xsd:string
property_value: IAO:0000117 "Victoria Dominguez Del Angel" xsd:string
property_value: IAO:0000118 "IAM" xsd:string
property_value: IAO:0000118 "Identity and Access Management" xsd:string
property_value: IAO:0000118 "IdM" xsd:string

[Term]
id: T4FS:0000170
name: reuse of digital assets
is_a: T4FS:0000447 ! fair principle
property_value: IAO:0000117 "https://orcid.org/0000-0003-2687-1982" xsd:string

[Term]
id: T4FS:0000172
name: investigate open innovation opportunities
def: "Explore the potential application domain/sociental implication of the project work and the communities of users/partners." []
is_a: T4FS:0000084 ! engaging in open innovation beyond academia
property_value: IAO:0000117 "Celia van Gelder" xsd:string
property_value: IAO:0000117 "Mateusz Kuzak" xsd:string
property_value: IAO:0000117 "Yan Wang" xsd:string

[Term]
id: T4FS:0000173
name: data recovery
def: "The process of restoring data that have been lost, accidentally deleted, corrupted or made inaccessible for any reason. The data recovery process may vary, depending on the circumstances of the data loss, the data recovery software used to create backups, and backup target media. In some cases, end users may be able to restore lost..." [] {IAO:0000119="Definition from now-deprecated CASRAI Glossary term: data-quality-review"}
is_a: T4FS:0000156 ! archiving
property_value: IAO:0000117 "https://orcid.org/0000-0002-5214-4466" xsd:string
property_value: IAO:0000117 "https://orcid.org/0000-0003-2687-1982" xsd:string

[Term]
id: T4FS:0000174
name: R1. (meta)data are richly described with a plurality of accurate and relevant attributes
is_a: T4FS:0000170 ! reuse of digital assets
property_value: IAO:0000117 "https://orcid.org/0000-0003-2687-1982" xsd:string

[Term]
id: T4FS:0000175
name: fair evaluation of repositories for data deposition
def: "To be able to define and deploy appropriate criteria, based on the FAIR principles, to identify the appropriate repository for a dataset. This may, for example, involve discovering the mark-up of the repository, the exchange formats and data models used, and the licensing information for each repository. Tools such as the FAIR evaluator or FAIRshake may be used to assess the FAIRness of a repository based on human-entered questionnaires or FAIRsharing resource metadata." [] {IAO:0000119="[PMQ]"}
is_a: T4FS:0000021 ! exposing data
property_value: IAO:0000117 "https://orcid.org/0000-0003-2687-1982" xsd:string
property_value: IAO:0000118 "FAIR data submission" xsd:string
property_value: IAO:0000118 "Repository FAIRness" xsd:string

[Term]
id: T4FS:0000176
name: regional standard
def: "A Regional standard is one that applies across a multi-nation region. Most countries have their own national standards-making bodies, which in turn may also group together to make regional standards. For example, national standards bodies in Europe are also members of the European Committee for Standardization (CEN) as well as members of ISO. The use of such standards may be voluntary, or they may be referenced in regulation (therefore mandatory)." [] {IAO:0000119="Adapted by AL from ISO. https://www.iso.org/sites/ConsumersStandards/1_standards.html#section1_2"}
comment: AL 9.3.22: Removed reference to CASRAI (https://casrai.org/term/regional-standard/), as the definition was unsuitable.
is_a: T4FS:0000372 ! data stewardship technical concept
property_value: IAO:0000117 "https://orcid.org/0000-0002-7702-4495" xsd:string
property_value: IAO:0000117 "https://orcid.org/0000-0003-2687-1982" xsd:string

[Term]
id: T4FS:0000177
name: workflow technologies management
def: "The process of setting up environments for workflow technologies." [] {IAO:0000119="KH"}
is_a: T4FS:0000353 ! resource management
property_value: IAO:0000117 "Kristina Hettne" xsd:string
property_value: IAO:0000117 "Simon Hodson" xsd:string
property_value: IAO:0000117 "Victoria Dominguez Del Angel" xsd:string

[Term]
id: T4FS:0000178
name: data steward
def: "Data steward is an umbrella term for numerous support roles that involve the creation, management and usage of research data. A data steward facilitates the quality, integrity and access to (meta)data in a manner that is consistent with the appropriate laws and institutional policies, ensuring professional treatment of data throughout all stages of the research project." [] {IAO:0000119="The Turing Way. https://book.the-turing-way.org/collaboration/research-infrastructure-roles/data-steward.html"}
relationship: T4FS:0000558 T4FS:0000162 ! has/wants competency in fair stewardship training
relationship: T4FS:0000558 T4FS:0000297 ! has/wants competency in research data management
relationship: T4FS:0000558 T4FS:0000492 ! has/wants competency in understanding persistent identifiers
relationship: T4FS:0000559 T4FS:0000372 ! has/wants knowledge about data stewardship technical concept
relationship: T4FS:0000559 T4FS:0000446 ! has/wants knowledge about data stewardship guideline
relationship: T4FS:0000561 T4FS:0000372 ! has/wants practical skill about data stewardship technical concept
relationship: T4FS:0000562 T4FS:0000548 ! has aptitude for data stewardship soft skill
property_value: IAO:0000117 "https://orcid.org/0000-0002-5214-4466" xsd:string
property_value: IAO:0000117 "https://orcid.org/0000-0003-2687-1982" xsd:string
created_by: https://orcid.org/0000-0003-2687-1982

[Term]
id: T4FS:0000180
name: skills related to preservation costs management
def: "Bin for Skills needed for Preservation costs management." []
is_a: T4FS:0000104 ! preservation costs management
created_by: leightonlc
creation_date: 2019-10-17T15:17:32.816013Z

[Term]
id: T4FS:0000181
name: repository certification schemes
is_a: T4FS:0000489 ! repository
created_by: https://orcid.org/0000-0003-2687-1982
creation_date: 2021-02-17T22:10:11.837519Z

[Term]
id: T4FS:0000182
name: registry
def: "Database containing information about trusted repositories that are provided by repository managers and are useful for human and machine users. These registries do not contain information about all metadata descriptions of digital objects, nor do they offer a list of PIDs of all stored digital objects. They do offer information based on standardised types on how to retrieve such information (e.g., the port under which OAI-PMH can be accessed to offer metadata). A registry requires the assignment of a permanent, unique and unambiguous identifier to each item." [] {IAO:0000119="RDMT. https://terms.codata.org/rdmt/registry"}
is_a: T4FS:0000372 ! data stewardship technical concept
property_value: IAO:0000117 "https://orcid.org/0000-0002-5214-4466" xsd:string
property_value: IAO:0000117 "https://orcid.org/0000-0002-7702-4495" xsd:string
property_value: IAO:0000117 "https://orcid.org/0000-0003-2687-1982" xsd:string
property_value: IAO:0000118 "Data registry" xsd:string

[Term]
id: T4FS:0000183
name: recognise and acknowledge contributions
def: "To clearly communicate the existence of contributions from different individuals / projects to the compilation of a given dataset, in such a way that can be consistently cited." [] {IAO:0000119="[LM]"}
is_a: T4FS:0000021 ! exposing data
property_value: IAO:0000117 "Laura Molloy" xsd:string
property_value: IAO:0000118 "attribution" xsd:string
property_value: IAO:0000118 "credit" xsd:string

[Term]
id: T4FS:0000184
name: linked open data
def: "Data where relationships/connections between them are available to allow easy data access." [] {IAO:0000119="RDMT. https://terms.codata.org/rdmt/linked-open-data"}
is_a: T4FS:0000372 ! data stewardship technical concept
property_value: IAO:0000117 "https://orcid.org/0000-0002-5214-4466" xsd:string
property_value: IAO:0000117 "https://orcid.org/0000-0002-7702-4495" xsd:string
property_value: IAO:0000117 "https://orcid.org/0000-0003-2687-1982" xsd:string

[Term]
id: T4FS:0000185
name: research data format
def: "Research data format is a generic term encompassing the concept of a standardised format for research data." [] {IAO:0000119="AL, 9.3.22"}
comment: AL 9.3.2022: The original CASRAI definition is unsuitable (https://casrai.org/term/research-data-format), therefore I have changed the definition to something more generic.
is_a: T4FS:0000372 ! data stewardship technical concept
property_value: IAO:0000117 "https://orcid.org/0000-0002-7702-4495" xsd:string
property_value: IAO:0000117 "https://orcid.org/0000-0003-2687-1982" xsd:string

[Term]
id: T4FS:0000186
name: research governance
def: "Activities and policies that ensure that the benefits to society of research outweigh any risks, from both an ethical and legal perspective." [] {IAO:0000119="RDMT. https://terms.codata.org/rdmt/research-governance"}
is_a: T4FS:0000472 ! governance
property_value: IAO:0000117 "https://orcid.org/0000-0002-5214-4466" xsd:string
property_value: IAO:0000117 "https://orcid.org/0000-0002-7702-4495" xsd:string
property_value: IAO:0000117 "https://orcid.org/0000-0003-2687-1982" xsd:string

[Term]
id: T4FS:0000188
name: semantic interoperability
def: "Ability of computer systems to transmit data with unambiguous, shared meaning. Semantic interoperability is a requirement to enable machine computable logic, inferencing, knowledge discovery, and data federation between information systems. Semantic interoperability is achieved when the information transferred has, in its communicated form, all of the meaning required for the receiving system to interpret it correctly, even when the algorithms used by the receiving system are unknown to the sending system. Syntactic interoperability is a prerequisite to semantic interoperability. Semantic interoperability ensures that the precise format and meaning of exchanged data and information is preserved and understood throughout exchanges between parties; in other words, what is sent is what is understood." [] {IAO:0000119="RDMT. https://terms.codata.org/rdmt/semantic-interoperability"}
is_a: T4FS:0000372 ! data stewardship technical concept
relationship: T4FS:0000563 T4FS:0000361 ! contributes to the implementation of I2. (meta)data use vocabularies that follow fair principles
property_value: IAO:0000117 "https://orcid.org/0000-0002-5214-4466" xsd:string
property_value: IAO:0000117 "https://orcid.org/0000-0002-7702-4495" xsd:string
property_value: IAO:0000117 "https://orcid.org/0000-0003-2687-1982" xsd:string

[Term]
id: T4FS:0000189
name: international chemical identifier
def: "A non-proprietary identifier for chemical substances that can be used in printed and electronic data sources thus enabling easier linking of diverse data compilations." [] {IAO:0000119="RDMT. https://terms.codata.org/rdmt/international-chemical-identifier"}
is_a: T4FS:0000453 ! persistent identifier
property_value: IAO:0000117 "https://orcid.org/0000-0002-5214-4466" xsd:string
property_value: IAO:0000117 "https://orcid.org/0000-0003-2687-1982" xsd:string

[Term]
id: T4FS:0000190
name: research data publication workflow
def: "Activities and processes in a digital environment that lead to the publication of research data, associated metadata and accompanying documentation and software code on the Web. In contrast to interim or final published products, workflows are the means to curate, document, and review, and thus ensure and enhance the value of the published product. Workflows can involve both humans and machines and often humans are supported by technology as they perform steps in the workflow. Similar workflows may vary in the details depending on the research discipline, data publishing product and/or the host institution of the workflow." [] {IAO:0000119="RDMT. https://terms.codata.org/rdmt/research-data-publication-workflow"}
is_a: T4FS:0000012 ! data stewardship activity
property_value: IAO:0000117 "https://orcid.org/0000-0002-5214-4466" xsd:string
property_value: IAO:0000117 "https://orcid.org/0000-0002-7702-4495" xsd:string
property_value: IAO:0000117 "https://orcid.org/0000-0003-2687-1982" xsd:string

[Term]
id: T4FS:0000191
name: data completeness
def: "Degree to which all required measurements are known. Values may be designated as “missing” in order not to have empty cells, or missing values may be replaced with default or interpolated values. In the case of default or interpolated values, these must be flagged as such to distinguish them from actual measurements or observations. Missing, default, or interpolated values do not imply that the dataset has been made complete." [] {IAO:0000119="RDMT. https://terms.codata.org/rdmt/data-completeness"}
is_a: T4FS:0000372 ! data stewardship technical concept
property_value: IAO:0000117 "https://orcid.org/0000-0002-5214-4466" xsd:string
property_value: IAO:0000117 "https://orcid.org/0000-0003-2687-1982" xsd:string

[Term]
id: T4FS:0000192
name: privacy-preserving data linkage
def: "Data linkage where the resulting product has been de-identified." [] {IAO:0000119="RDMT. https://terms.codata.org/rdmt/privacy-preserving-data-linkage"}
is_a: T4FS:0000372 ! data stewardship technical concept
property_value: IAO:0000117 "https://orcid.org/0000-0002-5214-4466" xsd:string
property_value: IAO:0000117 "https://orcid.org/0000-0002-7702-4495" xsd:string
property_value: IAO:0000117 "https://orcid.org/0000-0003-2687-1982" xsd:string

[Term]
id: T4FS:0000193
name: open access publishing
comment: AL 22.3.22: refactored 'open access publishing and self-archiving' to be two separate concepts ('open access publishing', and 'self-archiving') according to T4FS best practices. Self-archiving did not have to be created because we already had self-archive, which was then moved to the Archiving hierarchy. 'publish open access' was also removed in favour of this term as they were too similar to have without the potential for confusion by users.
is_a: T4FS:0000106 ! publish data
property_value: IAO:0000117 "Celia van Gelder" xsd:string
property_value: IAO:0000117 "https://orcid.org/0000-0002-7702-4495" xsd:string
property_value: IAO:0000117 "Mateusz Kuzak" xsd:string
property_value: IAO:0000117 "Yan Wang" xsd:string

[Term]
id: T4FS:0000194
name: self-archiving
def: "Prepare the data in preferred types and the data documentation. Choose the data repository and data license, deposit the data in the repository." []
is_a: T4FS:0000534 ! data archiving
property_value: IAO:0000117 "Celia van Gelder" xsd:string
property_value: IAO:0000117 "https://orcid.org/0000-0002-7702-4495" xsd:string
property_value: IAO:0000117 "Mateusz Kuzak" xsd:string
property_value: IAO:0000117 "Yan Wang" xsd:string

[Term]
id: T4FS:0000195
name: information management advisor
def: "Person with broad knowledge of information management disciplines and who provides guidance and support to program and staff functions on all aspects of managing the information resource." [] {IAO:0000119="RDMT. https://terms.codata.org/rdmt/information-management-advisor"}
relationship: T4FS:0000558 T4FS:0000012 ! has/wants competency in data stewardship activity
relationship: T4FS:0000559 T4FS:0000372 ! has/wants knowledge about data stewardship technical concept
relationship: T4FS:0000559 T4FS:0000446 ! has/wants knowledge about data stewardship guideline
relationship: T4FS:0000561 T4FS:0000372 ! has/wants practical skill about data stewardship technical concept
relationship: T4FS:0000562 T4FS:0000548 ! has aptitude for data stewardship soft skill
property_value: IAO:0000117 "https://orcid.org/0000-0002-5214-4466" xsd:string
property_value: IAO:0000117 "https://orcid.org/0000-0003-2687-1982" xsd:string

[Term]
id: T4FS:0000196
name: data management plan
def: "Statement describing how research data will be managed throughout a specified research project's life cycle - during and after the active phase of the research project - including terms regarding archiving and potential preservation of the data in a data repository. The DMP is considered to be a 'living' document, i.e. one which can be updated when necessary." [] {IAO:0000119="RDMT. https://terms.codata.org/rdmt/data-management-plan"}
is_a: T4FS:0000372 ! data stewardship technical concept
relationship: T4FS:0000563 T4FS:0000447 ! contributes to the implementation of fair principle
property_value: IAO:0000117 "https://orcid.org/0000-0002-5214-4466" xsd:string
property_value: IAO:0000117 "https://orcid.org/0000-0003-2687-1982" xsd:string
property_value: IAO:0000118 "DMP" xsd:string

[Term]
id: T4FS:0000199
name: F2. data are described with rich metadata
is_a: T4FS:0000248 ! findability of digital assets
property_value: IAO:0000117 "https://orcid.org/0000-0003-2687-1982" xsd:string

[Term]
id: T4FS:0000200
name: R1.1 (meta)data are released with a clear and accessible data usage license
is_a: T4FS:0000174 ! R1. (meta)data are richly described with a plurality of accurate and relevant attributes
property_value: IAO:0000117 "https://orcid.org/0000-0003-2687-1982" xsd:string
property_value: IAO:0000118 "Data license" xsd:string

[Term]
id: T4FS:0000201
name: data stream
def: "Sequence of digitally encoded, coherent signals used to send or receive a representation of information content as transmitted." [] {IAO:0000119="RDMT. https://terms.codata.org/rdmt/data-stream"}
is_a: T4FS:0000372 ! data stewardship technical concept
property_value: IAO:0000117 "https://orcid.org/0000-0002-5214-4466" xsd:string
property_value: IAO:0000117 "https://orcid.org/0000-0003-2687-1982" xsd:string

[Term]
id: T4FS:0000202
name: data librarian
def: "Librarian who manages the sharing and publishing of datasets as openly as possible and as closed as necessary, and the management and curation of repositories required to achieve this. Broad role requirements include support for sharing and publishing datasets, finding, accessing, interoperating and re-using these datasets, reviewing and supporting Data Management Plans and training delivery." [] {IAO:0000119="RDMT. https://terms.codata.org/rdmt/data-librarian"}
relationship: T4FS:0000558 T4FS:0000012 ! has/wants competency in data stewardship activity
relationship: T4FS:0000559 T4FS:0000372 ! has/wants knowledge about data stewardship technical concept
relationship: T4FS:0000559 T4FS:0000446 ! has/wants knowledge about data stewardship guideline
relationship: T4FS:0000561 T4FS:0000372 ! has/wants practical skill about data stewardship technical concept
relationship: T4FS:0000562 T4FS:0000548 ! has aptitude for data stewardship soft skill
property_value: IAO:0000117 "https://orcid.org/0000-0002-5214-4466" xsd:string
property_value: IAO:0000117 "https://orcid.org/0000-0003-2687-1982" xsd:string

[Term]
id: T4FS:0000203
name: program governance
def: "The process of developing, communicating, implementing, monitoring, and assuring the policies, procedures, organizational structures, and practices associated with a given program." [] {IAO:0000119="Definition from now-deprecated CASRAI Glossary term: program-governance"}
is_a: T4FS:0000472 ! governance
property_value: IAO:0000117 "https://orcid.org/0000-0002-5214-4466" xsd:string
property_value: IAO:0000117 "https://orcid.org/0000-0002-7702-4495" xsd:string
property_value: IAO:0000117 "https://orcid.org/0000-0003-2687-1982" xsd:string

[Term]
id: T4FS:0000206
name: knowledge of workflow technologies management
def: "Bin for types of Knowledge related to Workflow technologies management." []
is_a: T4FS:0000177 ! workflow technologies management
created_by: leightonlc
creation_date: 2019-10-17T15:16:10.561925Z

[Term]
id: T4FS:0000209
name: access risk assessment and mitigation
def: "Obtain an overview of information access status for different stakeholder groups. Check this overview against the organizational information access policy and risk catalogue, identify the type of information security risks based on the mismatch between the current status and policy. Choose and implement the right protocal to mitigate the risk." []
is_a: T4FS:0000107 ! information security
property_value: IAO:0000117 "Angus Whyte" xsd:string
property_value: IAO:0000117 "Celia van Gelder" xsd:string
property_value: IAO:0000117 "Mateusz Kuzak" xsd:string
property_value: IAO:0000117 "Yan Wang" xsd:string

[Term]
id: T4FS:0000210
name: usable data
def: "Data that can be used: delivered in a form that meets the needs of different end-user audiences, is ready for the tasks that the end-user needs to accomplish, and that has been adapted to the end-user’s needs. Usable data have been cleaned, structured, are in machine readable format, fully documented, and ready for analysis and interpretation." [] {IAO:0000119="RDMT. https://terms.codata.org/rdmt/usable-data"}
is_a: T4FS:0000430 ! data
property_value: IAO:0000117 "https://orcid.org/0000-0002-5214-4466" xsd:string
property_value: IAO:0000117 "https://orcid.org/0000-0002-7702-4495" xsd:string
property_value: IAO:0000117 "https://orcid.org/0000-0003-2687-1982" xsd:string

[Term]
id: T4FS:0000211
name: presentation slides
is_a: T4FS:0000519 ! learning medium
property_value: IAO:0000117 "https://orcid.org/0000-0003-2687-1982" xsd:string
created_by: https://orcid.org/0000-0003-2687-1982
creation_date: 2020-10-01T20:52:43.543314Z

[Term]
id: T4FS:0000212
name: implement secure storage
def: "Configure secure storage and monitor its usage" []
is_a: T4FS:0000470 ! storage security management
property_value: IAO:0000117 "Angus Whyte" xsd:string
property_value: IAO:0000117 "Celia van Gelder" xsd:string
property_value: IAO:0000117 "Mateusz Kuzak" xsd:string
property_value: IAO:0000117 "Yan Wang" xsd:string

[Term]
id: T4FS:0000213
name: data lifecycle
name: research data lifecycle
def: "Entire period of time that research data exists. This lifecycle describes the flow of research data starting from planning, collecting, processing, analysing, preserving, sharing and finally reusing the research data. Research data often have a longer lifespan than the research project." [] {IAO:0000119="RDMT. https://terms.codata.org/rdmt/research-data-lifecycle"}
is_a: T4FS:0000372 ! data stewardship technical concept
property_value: IAO:0000117 "https://orcid.org/0000-0002-5214-4466" xsd:string
property_value: IAO:0000117 "https://orcid.org/0000-0003-2687-1982" xsd:string

[Term]
id: T4FS:0000214
name: format and media migration
is_a: T4FS:0000156 ! archiving
property_value: IAO:0000117 "Kristina Hettne" xsd:string
property_value: IAO:0000117 "Victoria Dominguez Del Angel" xsd:string
property_value: IAO:0000117 "Yann Le Franc" xsd:string

[Term]
id: T4FS:0000215
name: data store
def: "Repository for persistently storing collections of data, such as a database, a file system or a directory. The data stored can be of any type that can be rendered in digital format and placed in electronic media." [] {IAO:0000119="RDMT. https://terms.codata.org/rdmt/data-store"}
is_a: T4FS:0000372 ! data stewardship technical concept
property_value: IAO:0000117 "https://orcid.org/0000-0002-5214-4466" xsd:string
property_value: IAO:0000117 "https://orcid.org/0000-0003-2687-1982" xsd:string

[Term]
id: T4FS:0000216
name: design processes for research integrity
def: "Initiate and develop processes to ensure outputs are made FAIR consistently with research integrity principles, and with ethical oversight." []
is_a: T4FS:0000525 ! research integrity, attribution, impact awareness
property_value: IAO:0000117 "Angus Whyte" xsd:string
property_value: IAO:0000117 "Celia van Gelder" xsd:string
property_value: IAO:0000117 "Mateusz Kuzak" xsd:string
property_value: IAO:0000117 "Yan Wang" xsd:string

[Term]
id: T4FS:0000217
name: core trust seal
def: "CoreTrustSeal offers to any interested data repository a core level certification based on the DSA–WDS Core Trustworthy Data Repositories Requirements catalogue and procedures. This universal catalogue of requirements reflects the core characteristics of trustworthy data repositories and is the culmination of a cooperative effort between DSA and WDS under the umbrella of the Research Data Alliance to merge their data repositories certifications." [] {IAO:0000119="https://www.coretrustseal.org/about/"}
is_a: T4FS:0000181 ! repository certification schemes
property_value: IAO:0000117 "https://orcid.org/0000-0003-2687-1982" xsd:string
property_value: IAO:0000118 "CTS" xsd:string
created_by: https://orcid.org/0000-0003-2687-1982
creation_date: 2021-02-17T22:12:12.996581Z

[Term]
id: T4FS:0000218
name: project management lifecycle
def: "Defines how to manage a project. It will always be the same, regardless of the project lifecycle being employed." [] {IAO:0000119="Definition from now-deprecated CASRAI Glossary term: project-management-lifecycle"}
is_a: T4FS:0000372 ! data stewardship technical concept
property_value: IAO:0000117 "https://orcid.org/0000-0002-5214-4466" xsd:string
property_value: IAO:0000117 "https://orcid.org/0000-0002-7702-4495" xsd:string
property_value: IAO:0000117 "https://orcid.org/0000-0003-2687-1982" xsd:string

[Term]
id: T4FS:0000219
name: authenticity metadata
def: "Type of metadata that conveys information needed to link a data object to its original source." [] {IAO:0000119="RDMT. https://terms.codata.org/rdmt/authenticity-metadata"}
is_a: T4FS:0000372 ! data stewardship technical concept
relationship: T4FS:0000563 T4FS:0000137 ! contributes to the implementation of I1. (meta)data use a formal, accessible, shared, and broadly applicable language for knowledge representation
property_value: IAO:0000117 "https://orcid.org/0000-0002-5214-4466" xsd:string
property_value: IAO:0000117 "https://orcid.org/0000-0003-2687-1982" xsd:string

[Term]
id: T4FS:0000220
name: researcher
relationship: T4FS:0000558 T4FS:0000012 ! has/wants competency in data stewardship activity
relationship: T4FS:0000559 T4FS:0000372 ! has/wants knowledge about data stewardship technical concept
relationship: T4FS:0000559 T4FS:0000446 ! has/wants knowledge about data stewardship guideline
relationship: T4FS:0000561 T4FS:0000372 ! has/wants practical skill about data stewardship technical concept
relationship: T4FS:0000562 T4FS:0000548 ! has aptitude for data stewardship soft skill

[Term]
id: T4FS:0000221
name: skills related to service level management
def: "Bin for Skills needed for Service level management." []
is_a: T4FS:0000466 ! service level management
created_by: leightonlc
creation_date: 2019-10-17T15:18:53.731967Z

[Term]
id: T4FS:0000222
name: personally identifiable information
def: "Data that relate to a living individual who can be identified from those data or those data plus other information which is in the possession of, or is likely to come into the possession of, the data controller, and includes any expression of opinion about the individual and any indication of the intentions of the data controller or any other person in respect of the individual. Any information that can be used to distinguish one person from another and can be used for de-anonymising anonymous data can be considered personally identifiable data." [] {IAO:0000119="RDMT. https://terms.codata.org/rdmt/personally-identifiable-information"}
is_a: T4FS:0000127 ! personal information privacy
property_value: IAO:0000117 "https://orcid.org/0000-0002-5214-4466" xsd:string
property_value: IAO:0000117 "https://orcid.org/0000-0002-7702-4495" xsd:string
property_value: IAO:0000117 "https://orcid.org/0000-0003-2687-1982" xsd:string
property_value: IAO:0000118 "Personal data" xsd:string

[Term]
id: T4FS:0000223
name: understand storage security challanges
def: "Understand the current storage security status and the preferred status, as well as the barriers between them." []
is_a: T4FS:0000470 ! storage security management
property_value: IAO:0000117 "Angus Whyte" xsd:string
property_value: IAO:0000117 "Celia van Gelder" xsd:string
property_value: IAO:0000117 "Mateusz Kuzak" xsd:string
property_value: IAO:0000117 "Yan Wang" xsd:string

[Term]
id: T4FS:0000224
name: normalization
def: "Organising data into tables so that the results of using the database are always unambiguous and as intended. Normalisation is typically a refinement process after the initial exercise of identifying the data objects that should be in the database, identifying their relationships, and defining the tables required and the columns within each table. First normal form (1NF) is the “basic” level of normalisation: Data and information are contained in two-dimensional tables with rows and columns. Each column corresponds to a sub-object or an attribute of the object represented by the entire table. Each row represents a unique instance of that sub-object or attribute and must be different in some way from any other row (that is, no duplicate rows are possible). All entries in any column must be of the same kind. For example, in the column labelled “Date,” only dates are permitted. In Second normal form (2NF), the tables are in first normal form and, in addition, each column in a table that is not a determiner of the contents of another column must itself be a function of the other columns in the table. At the second normal form, modifications are still possible because a change to one row in a table may affect data that refers to this information from another table. In Third normal form (3NF), the tables are in second normal form and, in addition, there is no transitive functional dependency. For example, if A is functionally dependent on B, and B is functionally dependent on C, then C is transitively dependent on A via B. In Domain/key normal form (DKNF), a key uniquely identifies each row in a table. A domain is the set of permissible values for an attribute. By enforcing key and domain restrictions, the database is assured of being freed from modification anomalies. DKNF is the normalisation level that most designers aim to achieve." [] {IAO:0000119="RDMT. https://terms.codata.org/rdmt/normalisation"}
is_a: T4FS:0000372 ! data stewardship technical concept
property_value: IAO:0000117 "https://orcid.org/0000-0002-5214-4466" xsd:string
property_value: IAO:0000117 "https://orcid.org/0000-0002-7702-4495" xsd:string
property_value: IAO:0000117 "https://orcid.org/0000-0003-2687-1982" xsd:string

[Term]
id: T4FS:0000225
name: evaluation
def: "Evaluation is a decision about significance, value, or quality of something, based on careful study of its good and bad features." [] {IAO:0000119="Definition from now-deprecated CASRAI Glossary term: evaluation"}
comment: AL 17.3.22: We may wish to make this an alternative term of Assessment.
is_a: T4FS:0000126 ! assessment
property_value: IAO:0000117 "https://orcid.org/0000-0002-5214-4466" xsd:string
property_value: IAO:0000117 "https://orcid.org/0000-0002-7702-4495" xsd:string
property_value: IAO:0000117 "https://orcid.org/0000-0003-2687-1982" xsd:string

[Term]
id: T4FS:0000226
name: data item
def: "Type of data element that expresses a proposition that binds one or more property values to some data entity." [] {IAO:0000119="RDMT. https://terms.codata.org/rdmt/data-item"}
is_a: T4FS:0000372 ! data stewardship technical concept
property_value: IAO:0000117 "https://orcid.org/0000-0002-5214-4466" xsd:string
property_value: IAO:0000117 "https://orcid.org/0000-0003-2687-1982" xsd:string

[Term]
id: T4FS:0000227
name: confidentiality
def: "Duty and practice of ensuring that personal or sensitive information only flows from one entity to another according to legislated or otherwise broadly accepted norms and policies. This can be done by either restricting access to the data or certain variables in the data, and/or by protecting personal or sensitive information using an anonymisation method." [] {IAO:0000119="RDMT. https://terms.codata.org/rdmt/confidentiality"}
is_a: T4FS:0000372 ! data stewardship technical concept
property_value: IAO:0000117 "https://orcid.org/0000-0002-5214-4466" xsd:string
property_value: IAO:0000117 "https://orcid.org/0000-0003-2687-1982" xsd:string

[Term]
id: T4FS:0000228
name: knowledge of data management costs management
def: "Bin for types of Knowledge needed for Data management costs management." []
is_a: T4FS:0000232 ! data management costs management
property_value: IAO:0000117 "leightonlc" xsd:string

[Term]
id: T4FS:0000229
name: logistical support
is_a: T4FS:0000320 ! project management activities
property_value: IAO:0000117 "https://orcid.org/0000-0002-7702-4495" xsd:string
property_value: IAO:0000117 "https://orcid.org/0000-0003-2687-1982" xsd:string
property_value: IAO:0000117 "Philippe Rocca-Serra" xsd:string
property_value: IAO:0000117 "Susanna Sansone" xsd:string

[Term]
id: T4FS:0000230
name: aptitudes for data management costs management
def: "Bin for Aptitudes related to Data management costs management." []
is_a: T4FS:0000232 ! data management costs management
property_value: IAO:0000117 "leightonlc" xsd:string

[Term]
id: T4FS:0000231
name: data acquisition
def: "The process of acquiring data from some source. For example, data may be acquired by download from a repository, transfer from a data logger, data capture, etc." [] {IAO:0000119="RDMT. https://terms.codata.org/rdmt/data-acquisition"}
comment: AL 15.3.22: Removed "data and metadata capture" as was too similar to this term. Added alternative term "data capture".
is_a: T4FS:0000012 ! data stewardship activity
property_value: IAO:0000117 "https://orcid.org/0000-0002-5214-4466" xsd:string
property_value: IAO:0000117 "https://orcid.org/0000-0002-7702-4495" xsd:string
property_value: IAO:0000117 "https://orcid.org/0000-0003-2687-1982" xsd:string
property_value: IAO:0000118 "data capture" xsd:string
property_value: IAO:0000118 "data download" xsd:string
property_value: IAO:0000118 "data reception" xsd:string

[Term]
id: T4FS:0000232
name: data management costs management
def: "Planning for and controlling expenditures related to the data management lifecycle, including, but not limited to, labor and infrastructure expenses for data collection; data documentation; data storage; data access and security; data preservation; data sharing; and data disposition." [] {IAO:0000119="Written by LLC, based on list at https://www.uu.nl/en/research/research-data-management/guides/costs-of-data-management"}
is_a: T4FS:0000353 ! resource management
property_value: IAO:0000117 "Kristina Hettne" xsd:string
property_value: IAO:0000117 "Simon Hodson" xsd:string
property_value: IAO:0000117 "Victoria Dominguez Del Angel" xsd:string

[Term]
id: T4FS:0000233
name: text file
def: "A Text file is a kind of computer file that is structured as a sequence of lines of electronic text. A text file exists stored as data within a computer file system." [] {IAO:0000119="AL, Adapted from Wikipedia. https://en.wikipedia.org/wiki/Text_file"}
comment: AL 9.3.22: The CASRAI term (https://casrai.org/term/text-file) had an unsuitable definition, and therefore was removed.
is_a: T4FS:0000372 ! data stewardship technical concept
relationship: T4FS:0000563 T4FS:0000137 ! contributes to the implementation of I1. (meta)data use a formal, accessible, shared, and broadly applicable language for knowledge representation
property_value: IAO:0000117 "https://orcid.org/0000-0002-7702-4495" xsd:string
property_value: IAO:0000117 "https://orcid.org/0000-0003-2687-1982" xsd:string

[Term]
id: T4FS:0000236
name: human-readable format
def: "Data and code that are commented so that humans can understand what they represent, their design, and their purpose." [] {IAO:0000119="RDMT. https://terms.codata.org/rdmt/human-readable-format"}
is_a: T4FS:0000372 ! data stewardship technical concept
relationship: T4FS:0000563 T4FS:0000137 ! contributes to the implementation of I1. (meta)data use a formal, accessible, shared, and broadly applicable language for knowledge representation
property_value: IAO:0000117 "https://orcid.org/0000-0002-5214-4466" xsd:string
property_value: IAO:0000117 "https://orcid.org/0000-0003-2687-1982" xsd:string

[Term]
id: T4FS:0000238
name: data validation
def: "Checks that data are valid, sensible, reasonable, clean, usable, and secure before they are processed. Provides well-defined guarantees for fitness, accuracy, and consistency for any of various kinds of user input into an application or automated system. Failures or omissions in data validation can lead to data corruption, security vulnerability. Improperly validated data can cause computer code processing the data to crash, generate error messages, behave in an unanticipated manner, or generate incorrect results that may be difficult or impossible to detect." [] {IAO:0000119="RDMT. https://terms.codata.org/rdmt/data-validation"}
is_a: T4FS:0000036 ! curation
property_value: IAO:0000117 "https://orcid.org/0000-0002-5214-4466" xsd:string
property_value: IAO:0000117 "https://orcid.org/0000-0003-2687-1982" xsd:string

[Term]
id: T4FS:0000239
name: pid record
def: "Type of record (and organisation) that stores an instance of an executable/understandable PID. The content of a PID record distinguishes a registered digital or data object from other digital objects. A PID record is a type of record that includes property information that characterises the digital object it is identifying. Important parts of a PID record are location and checksum. However there is a large variation in usage. In some data models the PID is simply used as a unique label with an empty record. A PID record has a lifecycle including creation, publication, curation and destruction." [] {IAO:0000119="RDMT. https://terms.codata.org/rdmt/pid-record"}
is_a: T4FS:0000453 ! persistent identifier
property_value: IAO:0000117 "https://orcid.org/0000-0002-5214-4466" xsd:string
property_value: IAO:0000117 "https://orcid.org/0000-0002-7702-4495" xsd:string
property_value: IAO:0000117 "https://orcid.org/0000-0003-2687-1982" xsd:string

[Term]
id: T4FS:0000240
name: appreciate importance of research integrity
def: "Take proactive approach to ensure outputs are made FAIR consistently with research integrity principles." []
is_a: T4FS:0000525 ! research integrity, attribution, impact awareness
property_value: IAO:0000117 "Angus Whyte" xsd:string
property_value: IAO:0000117 "Celia van Gelder" xsd:string
property_value: IAO:0000117 "Mateusz Kuzak" xsd:string
property_value: IAO:0000117 "Yan Wang" xsd:string

[Term]
id: T4FS:0000241
name: structural metadata
name: structural metadata (information)
def: "A type of metadata that indicates how compound objects are put together." [] {IAO:0000119="RDMT. https://terms.codata.org/rdmt/structural-metadata-information"}
is_a: T4FS:0000527 ! metadata
property_value: IAO:0000117 "https://orcid.org/0000-0002-5214-4466" xsd:string
property_value: IAO:0000117 "https://orcid.org/0000-0002-7702-4495" xsd:string
property_value: IAO:0000117 "https://orcid.org/0000-0003-2687-1982" xsd:string

[Term]
id: T4FS:0000244
name: non personally identifiable information
def: "Data that could not lead to the identification of a specific individual, to distinguishing one person from another, or to personally identifiable information. These may be data that have been de-identified, or that could not lead to personally identifiable information in the first place." [] {IAO:0000119="Definition from now-deprecated CASRAI Glossary term: non-personally-identifiable-information"}
is_a: T4FS:0000372 ! data stewardship technical concept
property_value: IAO:0000117 "https://orcid.org/0000-0002-5214-4466" xsd:string
property_value: IAO:0000117 "https://orcid.org/0000-0002-7702-4495" xsd:string
property_value: IAO:0000117 "https://orcid.org/0000-0003-2687-1982" xsd:string

[Term]
id: T4FS:0000245
name: digitisation
def: "Process of creating digital files by scanning or otherwise converting analogue materials. The resulting digital copy, or digital surrogate, would then be classed as digital material and then subject to the same broad challenges involved in preserving access to it, as born-digital materials." [] {IAO:0000119="RDMT. https://terms.codata.org/rdmt/digitisation"}
is_a: T4FS:0000036 ! curation
property_value: IAO:0000117 "https://orcid.org/0000-0002-5214-4466" xsd:string
property_value: IAO:0000117 "https://orcid.org/0000-0002-7702-4495" xsd:string
property_value: IAO:0000117 "https://orcid.org/0000-0003-2687-1982" xsd:string

[Term]
id: T4FS:0000247
name: data publication
def: "Release of research data, associated metadata, accompanying documentation, and software code (in cases where the raw data have been processed or manipulated) for re-use and analysis in such a manner that they can be discovered on the Web and referred to in a unique and persistent way. Data publication occurs via dedicated data repositories and/or (data) journals which ensure that the published research objects are findable, accessible, interoperable and re-usable." [] {IAO:0000119="RDMT. https://terms.codata.org/rdmt/data-publication"}
is_a: T4FS:0000021 ! exposing data
property_value: IAO:0000117 "https://orcid.org/0000-0002-5214-4466" xsd:string
property_value: IAO:0000117 "https://orcid.org/0000-0003-2687-1982" xsd:string

[Term]
id: T4FS:0000248
name: findability of digital assets
is_a: T4FS:0000447 ! fair principle
property_value: IAO:0000117 "https://orcid.org/0000-0003-2687-1982" xsd:string

[Term]
id: T4FS:0000249
name: community building
comment: AL 9.3.22: renamed to prevent compound term. Was 'Influencing/community building'
is_a: T4FS:0000320 ! project management activities
property_value: IAO:0000117 "https://orcid.org/0000-0002-7702-4495" xsd:string
property_value: IAO:0000117 "https://orcid.org/0000-0003-2687-1982" xsd:string
property_value: IAO:0000117 "Philippe Rocca-Serra" xsd:string
property_value: IAO:0000117 "Susanna Sansone" xsd:string

[Term]
id: T4FS:0000250
name: citable data
def: "Standalone dataset that can be cited in a similar manner to other research outputs. The dataset appears in a data repository, data paper or project website, and has a Persistent Identifier. Most current referencing systems provide a format for citing datasets." [] {IAO:0000119="RDMT. https://terms.codata.org/rdmt/citable-data"}
is_a: T4FS:0000430 ! data
relationship: T4FS:0000563 T4FS:0000512 ! contributes to the implementation of F1. (meta)data are assigned a globally unique and persistent identifier
property_value: IAO:0000117 "https://orcid.org/0000-0002-5214-4466" xsd:string
property_value: IAO:0000117 "https://orcid.org/0000-0003-2687-1982" xsd:string

[Term]
id: T4FS:0000251
name: big data
def: "Voluminous amount of structured, semi-structured and/or unstructured data that have the potential to be mined for information, primarily characterised by big volume, extensive variety, high velocity (creation and use), and/or variability that together require a scalable architecture for efficient data storage, manipulation, and analysis. The definition is evolving and can vary by sector, depending on what kind of software tools are commonly available and what sizes of datasets are common in a particular discipline. With those caveats, big data in many sectors today will range from a few dozen terabytes to multiple petabytes." [] {IAO:0000119="RDMT. https://terms.codata.org/rdmt/big-data"}
is_a: T4FS:0000430 ! data
property_value: IAO:0000117 "https://orcid.org/0000-0002-5214-4466" xsd:string
property_value: IAO:0000117 "https://orcid.org/0000-0003-2687-1982" xsd:string

[Term]
id: T4FS:0000252
name: fairness assessment
def: "Ability to apply knowledge about FAIR metrics and assessing FAIRness using FAIR assessment tools." []
is_a: T4FS:0000126 ! assessment
property_value: IAO:0000117 "Kristina Hettne" xsd:string
property_value: IAO:0000117 "Victoria Dominguez Del Angel" xsd:string
property_value: IAO:0000117 "Yann Le Franc" xsd:string

[Term]
id: T4FS:0000254
name: data archive
def: "Service providing long-term, permanent care and accessibility for digital objects with research value. The standard for such repositories is the Open Archival Information System reference model." [] {IAO:0000119="RDMT. https://terms.codata.org/rdmt/data-archive"}
is_a: T4FS:0000372 ! data stewardship technical concept
property_value: IAO:0000117 "https://orcid.org/0000-0002-5214-4466" xsd:string
property_value: IAO:0000117 "https://orcid.org/0000-0003-2687-1982" xsd:string

[Term]
id: T4FS:0000255
name: technical metadata
def: "Information describing the technical processes used to produce, or required to use a digital object." [] {IAO:0000119="RDMT. https://terms.codata.org/rdmt/technical-metadata"}
is_a: T4FS:0000527 ! metadata
property_value: IAO:0000117 "https://orcid.org/0000-0002-5214-4466" xsd:string
property_value: IAO:0000117 "https://orcid.org/0000-0002-7702-4495" xsd:string
property_value: IAO:0000117 "https://orcid.org/0000-0003-2687-1982" xsd:string

[Term]
id: T4FS:0000256
name: machine readable
def: "In a form that can be used and understood by a computer." [] {IAO:0000119="RDMT. https://terms.codata.org/rdmt/machine-readable"}
comment: AL 5.12.22: Deprecated because of its similarity with http://purl.obolibrary.org/obo/T4FS_0000551. We don't need to be going to the level of granularity that the concept of machine readability needs to be modelled as well as machine readable format.
property_value: IAO:0000117 "https://orcid.org/0000-0002-5214-4466" xsd:string
property_value: IAO:0000117 "https://orcid.org/0000-0002-7702-4495" xsd:string
property_value: IAO:0000117 "https://orcid.org/0000-0003-2687-1982" xsd:string
is_obsolete: true

[Term]
id: T4FS:0000257
name: integrated access management
def: "Combination of business processes, policies and technologies that allows organisations to provide secure access to confidential data. Integrated access management software is used by enterprises to control the flow of sensitive data in and out of a network." [] {IAO:0000119="RDMT. https://terms.codata.org/rdmt/integrated-access-management"}
is_a: T4FS:0000012 ! data stewardship activity
property_value: IAO:0000117 "https://orcid.org/0000-0002-5214-4466" xsd:string
property_value: IAO:0000117 "https://orcid.org/0000-0002-7702-4495" xsd:string
property_value: IAO:0000117 "https://orcid.org/0000-0003-2687-1982" xsd:string

[Term]
id: T4FS:0000258
name: noisy data
def: "Meaningless data, including any data that cannot be understood and interpreted correctly by machines such as unstructured text; any data that has been received, stored, or changed in such a manner that it cannot be read or used by the program that originally created it." [] {IAO:0000119="RDMT. https://terms.codata.org/rdmt/noisy-data"}
is_a: T4FS:0000430 ! data
property_value: IAO:0000117 "https://orcid.org/0000-0002-5214-4466" xsd:string
property_value: IAO:0000117 "https://orcid.org/0000-0002-7702-4495" xsd:string
property_value: IAO:0000117 "https://orcid.org/0000-0003-2687-1982" xsd:string

[Term]
id: T4FS:0000259
name: fair training
def: "Activities in and around the provision of training, mentorship and teaching opportunities for good data management and the implementation of FAIR practices." [] {IAO:0000119="PMQ"}
is_a: T4FS:0000012 ! data stewardship activity
property_value: IAO:0000117 "https://orcid.org/0000-0002-7702-4495" xsd:string
property_value: IAO:0000117 "https://orcid.org/0000-0003-2687-1982" xsd:string
property_value: IAO:0000117 "Philippe Rocca-Serra" xsd:string
property_value: IAO:0000117 "Susanna Sansone" xsd:string

[Term]
id: T4FS:0000260
name: software
def: "A set of instructions that direct a computer to do a specific task." [] {IAO:0000119="Definition from now-deprecated CASRAI Glossary term: software"}
is_a: T4FS:0000372 ! data stewardship technical concept
property_value: IAO:0000117 "https://orcid.org/0000-0002-5214-4466" xsd:string
property_value: IAO:0000117 "https://orcid.org/0000-0002-7702-4495" xsd:string
property_value: IAO:0000117 "https://orcid.org/0000-0003-2687-1982" xsd:string

[Term]
id: T4FS:0000263
name: data standardization
def: "Conversion of multiple datasets to a single common format and structure." [] {IAO:0000119="RDMT. https://terms.codata.org/rdmt/data-standardisation"}
is_a: T4FS:0000012 ! data stewardship activity
property_value: IAO:0000117 "https://orcid.org/0000-0002-5214-4466" xsd:string
property_value: IAO:0000117 "https://orcid.org/0000-0003-2687-1982" xsd:string
property_value: IAO:0000233 "https://github.com/terms4fairskills/FAIRterminology/issues/32" xsd:string

[Term]
id: T4FS:0000264
name: open data
def: "Data that are accessible, machine-readable, usable, intelligible, and freely shared. Open data can be freely used, re-used, built on, and redistributed by anyone – subject only, at most, to the requirement to attribute and sharealike." [] {IAO:0000119="RDMT. https://terms.codata.org/rdmt/open-data"}
is_a: T4FS:0000430 ! data
property_value: IAO:0000117 "https://orcid.org/0000-0002-5214-4466" xsd:string
property_value: IAO:0000117 "https://orcid.org/0000-0002-7702-4495" xsd:string
property_value: IAO:0000117 "https://orcid.org/0000-0003-2687-1982" xsd:string

[Term]
id: T4FS:0000265
name: curated data
def: "The output of a data curation activity. Such data has generally already been cleaned, standardised, documented. Additional metadata relevant to the data object has also been added, via either manual or automatic methods." [] {IAO:0000119="AL 9.5.22"}
comment: AL 9.5.22: The orginal label ("data curation") matched a term within the Data stewardship activity hierarchy. Changing the class label to "Curated data" better fit the model.
is_a: T4FS:0000430 ! data
relationship: T4FS:0000563 T4FS:0000174 ! contributes to the implementation of R1. (meta)data are richly described with a plurality of accurate and relevant attributes
relationship: T4FS:0000563 T4FS:0000361 ! contributes to the implementation of I2. (meta)data use vocabularies that follow fair principles
relationship: T4FS:0000563 T4FS:0000435 ! contributes to the implementation of F3. metadata clearly and explicitly include the identifier of the data they describe
property_value: IAO:0000117 "https://orcid.org/0000-0002-7702-4495" xsd:string
property_value: IAO:0000117 "https://orcid.org/0000-0003-2687-1982" xsd:string
created_by: https://orcid.org/0000-0003-2687-1982

[Term]
id: T4FS:0000267
name: skills related to funding acquisition management
def: "Bin for Skills needed for Funding acquisition management." []
is_a: T4FS:0000426 ! funding acquisition management
property_value: IAO:0000117 "leightonlc" xsd:string

[Term]
id: T4FS:0000268
name: universally unique identifier
def: "128-bit number used to guarantee unique identity for objects on the internet over time." [] {IAO:0000119="RDMT. https://terms.codata.org/rdmt/universally-unique-identifier"}
is_a: T4FS:0000529 ! identifier
property_value: IAO:0000117 "https://orcid.org/0000-0002-5214-4466" xsd:string
property_value: IAO:0000117 "https://orcid.org/0000-0002-7702-4495" xsd:string
property_value: IAO:0000117 "https://orcid.org/0000-0003-2687-1982" xsd:string
property_value: IAO:0000118 "UUID, GUID" xsd:string

[Term]
id: T4FS:0000270
name: authentication
def: "The process of confirming the identity of a principal entity." [] {IAO:0000119="Definition from now-deprecated CASRAI Glossary: authentication"}
is_a: T4FS:0000107 ! information security
property_value: IAO:0000117 "https://orcid.org/0000-0002-5214-4466" xsd:string
property_value: IAO:0000117 "https://orcid.org/0000-0003-2687-1982" xsd:string

[Term]
id: T4FS:0000271
name: cloud computing
def: "Large-scale distributed computing paradigm that is driven by economies of scale, in which a pool of abstracted, virtualised, dynamically-scalable, managed computing power, storage, platforms and services are delivered on demand to external customers over the Internet. Key features are that: it is a specialised distributed computing paradigm; it is massively scalable; it can be encapsulated as an abstract entity that delivers different levels of services to customers outside the Cloud; it is driven by economies of scale; and the services can be dynamically configured (via virtualisation or other approaches) and delivered on demand." [] {IAO:0000119="RDMT. https://terms.codata.org/rdmt/cloud-computing"}
is_a: T4FS:0000372 ! data stewardship technical concept
property_value: IAO:0000117 "https://orcid.org/0000-0002-5214-4466" xsd:string
property_value: IAO:0000117 "https://orcid.org/0000-0003-2687-1982" xsd:string

[Term]
id: T4FS:0000273
name: short-term preservation
def: "Access to digital materials either for a defined period of time while use is predicted but which does not extend beyond the foreseeable future and/or until it becomes inaccessible because of changes in technology." [] {IAO:0000119="RDMT. https://terms.codata.org/rdmt/short-term-preservation"}
is_a: T4FS:0000372 ! data stewardship technical concept
property_value: IAO:0000117 "https://orcid.org/0000-0002-5214-4466" xsd:string
property_value: IAO:0000117 "https://orcid.org/0000-0002-7702-4495" xsd:string
property_value: IAO:0000117 "https://orcid.org/0000-0003-2687-1982" xsd:string

[Term]
id: T4FS:0000274
name: international standard
def: "Standard that is used in multiple nations and whose development process is open to representatives from all countries." [] {IAO:0000119="RDMT. https://terms.codata.org/rdmt/international-standard"}
is_a: T4FS:0000372 ! data stewardship technical concept
relationship: T4FS:0000563 T4FS:0000137 ! contributes to the implementation of I1. (meta)data use a formal, accessible, shared, and broadly applicable language for knowledge representation
property_value: IAO:0000117 "https://orcid.org/0000-0002-5214-4466" xsd:string
property_value: IAO:0000117 "https://orcid.org/0000-0003-2687-1982" xsd:string

[Term]
id: T4FS:0000275
name: conformance
def: "Satisfaction of the requirements of a specific standard(s) and/or specification(s). Conformance is used with respect to voluntary standards and specifications, whereas compliance is used with respect to mandatory standards and regulations." [] {IAO:0000119="RDMT. https://terms.codata.org/rdmt/conformance"}
is_a: T4FS:0000372 ! data stewardship technical concept
property_value: IAO:0000117 "https://orcid.org/0000-0002-5214-4466" xsd:string
property_value: IAO:0000117 "https://orcid.org/0000-0003-2687-1982" xsd:string

[Term]
id: T4FS:0000276
name: data custodian
def: "Individual or organisation responsible for the IT infrastructure providing and protecting data in conformance with the policies and practices prescribed by data governance." [] {IAO:0000119="RDMT. https://terms.codata.org/rdmt/data-custodian"}
relationship: T4FS:0000558 T4FS:0000012 ! has/wants competency in data stewardship activity
relationship: T4FS:0000559 T4FS:0000372 ! has/wants knowledge about data stewardship technical concept
relationship: T4FS:0000559 T4FS:0000446 ! has/wants knowledge about data stewardship guideline
relationship: T4FS:0000561 T4FS:0000372 ! has/wants practical skill about data stewardship technical concept
relationship: T4FS:0000562 T4FS:0000548 ! has aptitude for data stewardship soft skill
property_value: IAO:0000117 "https://orcid.org/0000-0002-5214-4466" xsd:string
property_value: IAO:0000117 "https://orcid.org/0000-0003-2687-1982" xsd:string
property_value: IAO:0000118 "Data manager" xsd:string
property_value: IAO:0000118 "Technical data steward" xsd:string

[Term]
id: T4FS:0000277
name: aptitudes for high performance computing management
def: "Bin for Aptitudes related to High performance computing management." []
is_a: T4FS:0000308 ! high performance computing management
property_value: IAO:0000117 "leightonlc" xsd:string

[Term]
id: T4FS:0000278
name: manage datasets in a repository
def: "Implement the policies that govern the arrangement, naming, descriptive metadata, provenance metadata, representation metadata, administrative metadata, access controls, retention, disposition, integrity, and replication of digital objects." [] {IAO:0000119="Definition from now-deprecated CASRAI Glossary term: manage-datasets-in-a-repository"}
is_a: T4FS:0000141 ! data management
property_value: IAO:0000117 "https://orcid.org/0000-0002-5214-4466" xsd:string
property_value: IAO:0000117 "https://orcid.org/0000-0002-7702-4495" xsd:string
property_value: IAO:0000117 "https://orcid.org/0000-0003-2687-1982" xsd:string

[Term]
id: T4FS:0000280
name: data de-noising
def: "Removing noise from data." [] {IAO:0000119="RDMT. https://terms.codata.org/rdmt/data-de-noising"}
is_a: T4FS:0000036 ! curation
property_value: IAO:0000117 "https://orcid.org/0000-0002-5214-4466" xsd:string
property_value: IAO:0000117 "https://orcid.org/0000-0003-2687-1982" xsd:string

[Term]
id: T4FS:0000282
name: governance and accountability model
def: "Provides the relationship and process context for working together to ensure outcomes are achieved." [] {IAO:0000119="Definition from now-deprecated CASRAI Glossary term: governance-and-accountability-model"}
is_a: T4FS:0000372 ! data stewardship technical concept
property_value: IAO:0000117 "https://orcid.org/0000-0002-5214-4466" xsd:string
property_value: IAO:0000117 "https://orcid.org/0000-0002-7702-4495" xsd:string
property_value: IAO:0000117 "https://orcid.org/0000-0003-2687-1982" xsd:string

[Term]
id: T4FS:0000283
name: access
def: "Continued availability and ongoing usability of a digital resource, retaining all qualities of authenticity, accuracy and functionality deemed to be essential for the purposes the digital material was created and/or acquired for. Users who have access can retrieve, understand, manipulate, and store copies." [] {IAO:0000119="RDMT. https://terms.codata.org/rdmt/access"}
is_a: T4FS:0000372 ! data stewardship technical concept
property_value: IAO:0000117 "https://orcid.org/0000-0002-5214-4466" xsd:string
property_value: IAO:0000117 "https://orcid.org/0000-0003-2687-1982" xsd:string

[Term]
id: T4FS:0000285
name: develop fair and open research strategy
def: "Find the people with a good understand of FAIR and open research challenges in your organiation, and create a work agenda." []
is_a: T4FS:0000008 ! develop open research strategy and vision
property_value: IAO:0000117 "Angus Whyte" xsd:string
property_value: IAO:0000117 "Celia van Gelder" xsd:string
property_value: IAO:0000117 "Mateusz Kuzak" xsd:string
property_value: IAO:0000117 "Yan Wang" xsd:string

[Term]
id: T4FS:0000286
name: patent application
def: "Choose the proper type of patent for the project data and apply for the patent chosen." []
is_a: T4FS:0000042 ! ethical application of patents, licenses
property_value: IAO:0000117 "Celia van Gelder" xsd:string
property_value: IAO:0000117 "Mateusz Kuzak" xsd:string
property_value: IAO:0000117 "Yan Wang" xsd:string

[Term]
id: T4FS:0000287
name: collection management identification
def: "Type of data provenance indication that adds metadata to identify data collections. The organisation doing the collection management is stated in the metadata along with the provenance of collection management events such as source of data acquisition, conservation, and movement." [] {IAO:0000119="RDMT. https://terms.codata.org/rdmt/collection-management-identification"}
is_a: T4FS:0000372 ! data stewardship technical concept
property_value: IAO:0000117 "https://orcid.org/0000-0002-5214-4466" xsd:string
property_value: IAO:0000117 "https://orcid.org/0000-0003-2687-1982" xsd:string

[Term]
id: T4FS:0000288
name: assess fairness
def: "Activity/Process whereby digital objects are evaluated with the relevant FAIR metrics and assessment tools." [] {IAO:0000119="[YLF, VDA, KH]"}
is_a: T4FS:0000126 ! assessment
property_value: IAO:0000117 "Kristina Hettne" xsd:string
property_value: IAO:0000117 "Victoria Dominguez Del Angel" xsd:string
property_value: IAO:0000117 "Yann Le Franc" xsd:string

[Term]
id: T4FS:0000289
name: knowledge of change management
def: "Bin for types of Knowledge related to Change management." []
is_a: T4FS:0000411 ! change management
property_value: IAO:0000117 "leightonlc" xsd:string

[Term]
id: T4FS:0000290
name: data ingestion
def: "Process of obtaining, importing, and processing data for later use or storage in a database. This process often involves altering individual files by editing their content and/or formatting them to fit into a larger document. An effective data ingestion methodology begins by validating the individual files, then prioritises the sources for optimum processing, and finally validates the results. When numerous data sources exist in diverse formats (the sources may number in the hundreds and the formats in the dozens), maintaining reasonable speed and efficiency can become a major challenge. To that end, several vendors offer programs tailored to the task of data ingestion in specific applications or environments." [] {IAO:0000119="RDMT. https://terms.codata.org/rdmt/data-ingestion"}
is_a: T4FS:0000231 ! data acquisition
property_value: IAO:0000117 "https://orcid.org/0000-0002-5214-4466" xsd:string
property_value: IAO:0000117 "https://orcid.org/0000-0003-2687-1982" xsd:string

[Term]
id: T4FS:0000291
name: data wrangling
def: "Manually or semi-automatically converting or mapping data from one form into another format that allows for more convenient consumption of the data with the help of semi-automated tools. Gathering and organising disparate data from different sources, often collected by many different investigators. Activities include developing and supporting search tools that utilise standardised metadata, harmonising the coding of data for specific variables, engineering new methods of combining data. with the help of semi-automated tools. The result of data wrangling is repurposed data." [] {IAO:0000119="RDMT. https://terms.codata.org/rdmt/data-wrangling"}
is_a: T4FS:0000036 ! curation
property_value: IAO:0000117 "https://orcid.org/0000-0002-5214-4466" xsd:string
property_value: IAO:0000117 "https://orcid.org/0000-0003-2687-1982" xsd:string

[Term]
id: T4FS:0000292
name: research data management infrastructure
def: "Configuration of staff, services and tools assembled to support data management across the research lifecycle and to provide comprehensive coverage of the stages making up the data lifecycle. It can be organised locally and/or globally to support research data activities across the research lifecycle." [] {IAO:0000119="RDMT. https://terms.codata.org/rdmt/research-data%20management-infrastructure"}
is_a: T4FS:0000372 ! data stewardship technical concept
property_value: IAO:0000117 "https://orcid.org/0000-0002-5214-4466" xsd:string
property_value: IAO:0000117 "https://orcid.org/0000-0002-7702-4495" xsd:string
property_value: IAO:0000117 "https://orcid.org/0000-0003-2687-1982" xsd:string

[Term]
id: T4FS:0000293
name: flexibility in relating fair criteria to openness
def: "Appreciate the need for flexibility in applying FAIR criteria to make data as open as possible, as closed as necessary." []
is_a: T4FS:0000259 ! fair training
property_value: IAO:0000117 "Angus Whyte" xsd:string

[Term]
id: T4FS:0000294
name: choosing the appropriate terminology for your data
def: "To be able to research and identify the appropriate taxonomy for your project. This may involve using resources such as FAIRsharing, which captures metadata on taxonomies and provides an assessment of their FAIRness." [] {IAO:0000119="[PMQ]"}
is_a: T4FS:0000175 ! fair evaluation of repositories for data deposition
property_value: IAO:0000117 "https://orcid.org/0000-0003-2687-1982" xsd:string
property_value: IAO:0000118 "Controlled Vocabulary identification" xsd:string
property_value: IAO:0000118 "Ontology identification" xsd:string
property_value: IAO:0000118 "Taxonomy identification" xsd:string
property_value: IAO:0000118 "Thesaurus identification" xsd:string

[Term]
id: T4FS:0000295
name: structured data
def: "Data elements that have been organised into a consistent format and data structure within a defined data model such that the elements can be easily addressed, organised and accessed in various combinations to make better use of the information, such as in a relational database." [] {IAO:0000119="RDMT. https://terms.codata.org/rdmt/structured-data"}
is_a: T4FS:0000430 ! data
property_value: IAO:0000117 "https://orcid.org/0000-0002-5214-4466" xsd:string
property_value: IAO:0000117 "https://orcid.org/0000-0002-7702-4495" xsd:string
property_value: IAO:0000117 "https://orcid.org/0000-0003-2687-1982" xsd:string
property_value: IAO:0000118 "Structured information" xsd:string

[Term]
id: T4FS:0000296
name: knowledge to contextualise fair principles to domain
def: "Know how data handling practices in the domain make FAIR criteria more or less easy to implement." []
is_a: T4FS:0000259 ! fair training
property_value: IAO:0000117 "Angus Whyte" xsd:string

[Term]
id: T4FS:0000297
name: research data management
def: "Storage, access and preservation of data created or collected in the course of research. Research data management practices cover the entire lifecycle of the data, from planning the investigation to conducting it, and from backing up data as it is created and used to long term preservation of data deliverables after the research investigation has concluded. Specific activities and issues that fall within the category of data management include: File naming (the proper way to name computer files); data quality control and quality assurance; data access; data documentation (including levels of uncertainty); metadata creation and controlled vocabularies; data storage; data archiving and preservation; data sharing and reuse; data integrity; data security; data privacy; data rights; notebook protocols (lab or field) as required." [] {IAO:0000119="RDMT. https://terms.codata.org/rdmt/research-data-management"}
is_a: T4FS:0000141 ! data management
property_value: IAO:0000117 "https://orcid.org/0000-0002-5214-4466" xsd:string
property_value: IAO:0000117 "https://orcid.org/0000-0002-7702-4495" xsd:string
property_value: IAO:0000117 "https://orcid.org/0000-0003-2687-1982" xsd:string

[Term]
id: T4FS:0000298
name: publish output in a repository
def: "Deposit research output (software, data and publication together with documentation) in  previousy selected repositories." []
is_a: T4FS:0000106 ! publish data
property_value: IAO:0000117 "Celia van Gelder" xsd:string
property_value: IAO:0000117 "Mateusz Kuzak" xsd:string
property_value: IAO:0000117 "Yan Wang" xsd:string

[Term]
id: T4FS:0000300
name: metadata search via metadata providers
def: "To be able to identify and process metadata over the internet, sourced from a variety of metadata providers and schemata." [] {IAO:0000119="[PMQ]"}
is_a: T4FS:0000076 ! data discovery
property_value: IAO:0000117 "https://orcid.org/0000-0003-2687-1982" xsd:string
property_value: IAO:0000118 "Metadata processing" xsd:string
property_value: IAO:0000118 "Metadata search" xsd:string

[Term]
id: T4FS:0000301
name: record provenance information
def: "Information for a data object that includes: the person who deposited the data object in the repository, the source of the data object, the date when the object was deposited, and authenticity information needed to link the data object to its original source." [] {IAO:0000119="RDMT. https://terms.codata.org/rdmt/record-provenance-information"}
is_a: T4FS:0000527 ! metadata
property_value: IAO:0000117 "https://orcid.org/0000-0002-5214-4466" xsd:string
property_value: IAO:0000117 "https://orcid.org/0000-0002-7702-4495" xsd:string
property_value: IAO:0000117 "https://orcid.org/0000-0003-2687-1982" xsd:string

[Term]
id: T4FS:0000302
name: data citation
def: "Process of citing a dataset in a similar manner to other research outputs. The dataset must be a standalone output that appears in a data repository, data paper or project website, and has a Persistent Identifier. Most current referencing systems provide a format for citing datasets." [] {IAO:0000119="RDMT. https://terms.codata.org/rdmt/data-citation"}
is_a: T4FS:0000021 ! exposing data
property_value: IAO:0000117 "https://orcid.org/0000-0002-5214-4466" xsd:string
property_value: IAO:0000117 "https://orcid.org/0000-0003-2687-1982" xsd:string

[Term]
id: T4FS:0000305
name: book
is_a: T4FS:0000519 ! learning medium
property_value: IAO:0000117 "https://orcid.org/0000-0003-2687-1982" xsd:string
created_by: https://orcid.org/0000-0003-2687-1982
creation_date: 2020-10-01T20:54:08.535183Z

[Term]
id: T4FS:0000306
name: intellectual leadership
def: "The capacity to influence stakeholders and the direction of research activities; the ability to shape others' understanding in ways that capture interest, inform and gain support; and, the capacity to influence the actions and opinions of others." [] {IAO:0000119="Definition from now-deprecated CASRAI Glossary term: intellectual-leadership/"}
is_a: T4FS:0000548 ! data stewardship soft skill
property_value: IAO:0000117 "https://orcid.org/0000-0002-5214-4466" xsd:string
property_value: IAO:0000117 "https://orcid.org/0000-0002-7702-4495" xsd:string
property_value: IAO:0000117 "https://orcid.org/0000-0003-2687-1982" xsd:string

[Term]
id: T4FS:0000307
name: innovation
def: "In the context of a researcher's activities, innovation is the development of modified or novel approaches, theories, concepts, ideas or solutions. Innovation is one of four valued outcomes." [] {IAO:0000119="Definition from now-deprecated CASRAI Glossary term: innovation"}
is_a: T4FS:0000012 ! data stewardship activity
property_value: IAO:0000117 "https://orcid.org/0000-0002-5214-4466" xsd:string
property_value: IAO:0000117 "https://orcid.org/0000-0002-7702-4495" xsd:string
property_value: IAO:0000117 "https://orcid.org/0000-0003-2687-1982" xsd:string

[Term]
id: T4FS:0000308
name: high performance computing management
def: "High-performance computing (HPC) is a process for using of super computers and parallel processing techniques for solving complex computational problems. HPC technology focuses on developing parallel processing algorithms and systems by incorporating both administration and parallel computational techniques." [] {IAO:0000119="(modified from wikipedia)[VDA]"}
is_a: T4FS:0000353 ! resource management
property_value: IAO:0000117 "Kristina Hettne" xsd:string
property_value: IAO:0000117 "Simon Hodson" xsd:string
property_value: IAO:0000117 "Victoria Dominguez Del Angel" xsd:string
property_value: IAO:0000118 "HPC management" xsd:string

[Term]
id: T4FS:0000309
name: provenance
def: "A type of historical information or metadata about the origin, location or the source of something, or the history of the ownership or location of an object or resource including digital objects. For example, information about the Principal Investigator who recorded the data, and the information concerning its storage, handling, and migration." [] {IAO:0000119="RDMT. https://terms.codata.org/rdmt/provenance"}
is_a: T4FS:0000372 ! data stewardship technical concept
relationship: T4FS:0000563 T4FS:0000014 ! contributes to the implementation of interoperability of digital assets
property_value: IAO:0000117 "https://orcid.org/0000-0002-5214-4466" xsd:string
property_value: IAO:0000117 "https://orcid.org/0000-0002-7702-4495" xsd:string
property_value: IAO:0000117 "https://orcid.org/0000-0003-2687-1982" xsd:string

[Term]
id: T4FS:0000310
name: digital record
def: "A record created digitally in the day-to-day business of the organisation and assigned formal status by the organisation. Examples include: word processing documents, emails, databases, or intranet web pages." [] {IAO:0000119="Definition from now-deprecated CASRAI Glossary term: digital"}
comment: AL 8.2.22: Updated label from the CASRAI "Digital" to "Digital record" to better match the definition and intent of the term, and to provide clarity.
is_a: T4FS:0000372 ! data stewardship technical concept
property_value: IAO:0000117 "https://orcid.org/0000-0002-5214-4466" xsd:string
property_value: IAO:0000117 "https://orcid.org/0000-0002-7702-4495" xsd:string
property_value: IAO:0000117 "https://orcid.org/0000-0003-2687-1982" xsd:string
property_value: IAO:0000118 "Electronic record" xsd:string

[Term]
id: T4FS:0000311
name: analytical quality control
def: "Processes and procedures designed to ensure that the results of laboratory analysis are consistent, comparable, accurate and within specified limits of precision." [] {IAO:0000119="Definition from now-deprecated CASRAI Glossary term: analytical-quality-control"}
is_a: T4FS:0000372 ! data stewardship technical concept
property_value: IAO:0000117 "https://orcid.org/0000-0002-5214-4466" xsd:string
property_value: IAO:0000117 "https://orcid.org/0000-0003-2687-1982" xsd:string

[Term]
id: T4FS:0000312
name: digital research data
def: "Research data in digital form. It may have been originally created in digital form, or it may have been converted from paper, or other non-digital form to a digital representation." [] {IAO:0000119="RDMT. https://terms.codata.org/rdmt/digital-research-data"}
is_a: T4FS:0000430 ! data
property_value: IAO:0000117 "https://orcid.org/0000-0002-5214-4466" xsd:string
property_value: IAO:0000117 "https://orcid.org/0000-0002-7702-4495" xsd:string
property_value: IAO:0000117 "https://orcid.org/0000-0003-2687-1982" xsd:string

[Term]
id: T4FS:0000314
name: managing research
def: "In the context of a researcher’s activities, Managing research is the processes related to the planning, organizing, setting objectives, controlling and evaluating of RDA activities and their associated human and financial resources. It includes the provision of leadership to, and assessment of, other scientists, engineers, technologists, and/or other staff. Managing research is one of the three research contexts in which a researcher is expected to conduct his/her activities. Managing research is distinct from the position-based role of a research manager." [] {IAO:0000119="Definition from now-deprecated CASRAI Glossary term: managing-research"}
is_a: T4FS:0000012 ! data stewardship activity
property_value: IAO:0000117 "https://orcid.org/0000-0002-5214-4466" xsd:string
property_value: IAO:0000117 "https://orcid.org/0000-0002-7702-4495" xsd:string
property_value: IAO:0000117 "https://orcid.org/0000-0003-2687-1982" xsd:string

[Term]
id: T4FS:0000315
name: evaluation of how to publish your data
def: "To be able to define and deploy appropriate criteria, based on the FAIR principles, to identify the appropriate publishing platform for a dataset. This may, for example, involve discovering the mark-up of the platform, the exchange formats and data models used, and the licensing information for each repository. Tools such as the FAIR evaluator or FAIRshake may be used to assess the FAIRnessbased on human-entered questionnaires or FAIRsharing resource metadata." [] {IAO:0000119="[PMQ]"}
is_a: T4FS:0000021 ! exposing data
property_value: IAO:0000117 "https://orcid.org/0000-0003-2687-1982" xsd:string

[Term]
id: T4FS:0000316
name: accession number
def: "Numbers used by the National Center for Biotechnology Information (NCBI) that are unique and citable." [] {IAO:0000119="Definition from now-deprecated CASRAI Glossary term: accession-number"}
is_a: T4FS:0000529 ! identifier
property_value: IAO:0000117 "https://orcid.org/0000-0002-5214-4466" xsd:string
property_value: IAO:0000117 "https://orcid.org/0000-0003-2687-1982" xsd:string

[Term]
id: T4FS:0000318
name: digital preservation
def: "Series of managed activities necessary to ensure continued access to digital materials for as long as necessary. All of the actions required to maintain access to digital materials beyond the limits of media failure or technological change. Those materials may be records created during the day-to-day business of an organisation; born-digital materials created for a specific purpose (such as teaching resources); or the products of digitisation projects. This definition specifically excludes the potential use of digital technology to preserve the original artefacts through digitisation." [] {IAO:0000119="RDMT. https://terms.codata.org/rdmt/digital-preservation Also drawn from https://www.dpconline.org/digipres/what-is-digipres"}
is_a: T4FS:0000372 ! data stewardship technical concept
property_value: IAO:0000117 "https://orcid.org/0000-0002-5214-4466" xsd:string
property_value: IAO:0000117 "https://orcid.org/0000-0002-7702-4495" xsd:string
property_value: IAO:0000117 "https://orcid.org/0000-0003-2687-1982" xsd:string

[Term]
id: T4FS:0000320
name: project management activities
def: "The practice of initiating, planning, executing, controlling, and closing the work of a team in relation to FAIR data stewardship." [] {IAO:0000119="PMQ"}
is_a: T4FS:0000012 ! data stewardship activity
property_value: IAO:0000117 "https://orcid.org/0000-0002-7702-4495" xsd:string
property_value: IAO:0000117 "https://orcid.org/0000-0003-2687-1982" xsd:string
property_value: IAO:0000117 "Philippe Rocca-Serra" xsd:string
property_value: IAO:0000117 "Susanna Sansone" xsd:string

[Term]
id: T4FS:0000321
name: knowledge of funding acquisition management
def: "Bin for types of Knowledge related to Funding acquisition management." []
is_a: T4FS:0000426 ! funding acquisition management
property_value: IAO:0000117 "leightonlc" xsd:string

[Term]
id: T4FS:0000322
name: manage access control
def: "Monitor the authorised parties' access to data and keep it up to date." []
is_a: T4FS:0000469 ! access control and management
property_value: IAO:0000117 "Celia van Gelder" xsd:string
property_value: IAO:0000117 "Mateusz Kuzak" xsd:string
property_value: IAO:0000117 "Yan Wang" xsd:string

[Term]
id: T4FS:0000323
name: project management
def: "The practice of initiating, planning, executing, controlling, and closing the work of a team to achieve specific goals and meet specific success criteria at the specified time." [] {IAO:0000119="KH"}
is_a: T4FS:0000353 ! resource management
property_value: IAO:0000117 "Kristina Hettne" xsd:string
property_value: IAO:0000117 "Simon Hodson" xsd:string
property_value: IAO:0000117 "Victoria Dominguez Del Angel" xsd:string
property_value: IAO:0000118 "PM" xsd:string

[Term]
id: T4FS:0000324
name: data retention policy
def: "Established protocol of an organisation for retaining information for operational or regulatory compliance needs. The objectives of a data retention policy are to keep important information for future use or reference, to organise information so it can be searched and accessed at a later date, and to dispose of information that is no longer needed. A data retention policy must consider both the value of data over time, and regulations to which the data may be subject." [] {IAO:0000119="RDMT. https://terms.codata.org/rdmt/data-retention-policy"}
is_a: T4FS:0000372 ! data stewardship technical concept
property_value: IAO:0000117 "https://orcid.org/0000-0002-5214-4466" xsd:string
property_value: IAO:0000117 "https://orcid.org/0000-0003-2687-1982" xsd:string

[Term]
id: T4FS:0000326
name: data representation
def: "Object describing the context of the data, including provenance, description, structural, and administrative information." [] {IAO:0000119="RDMT. https://terms.codata.org/rdmt/data-representation"}
is_a: T4FS:0000036 ! curation
property_value: IAO:0000117 "https://orcid.org/0000-0002-5214-4466" xsd:string
property_value: IAO:0000117 "https://orcid.org/0000-0002-7702-4495" xsd:string
property_value: IAO:0000117 "https://orcid.org/0000-0003-2687-1982" xsd:string

[Term]
id: T4FS:0000327
name: metadata dataset
def: "The set of metadata describing a specific dataset." [] {IAO:0000119="Definition from now-deprecated CASRAI Glossary term: metadata-dataset"}
is_a: T4FS:0000517 ! metadata record
property_value: IAO:0000117 "https://orcid.org/0000-0002-5214-4466" xsd:string
property_value: IAO:0000117 "https://orcid.org/0000-0002-7702-4495" xsd:string
property_value: IAO:0000117 "https://orcid.org/0000-0003-2687-1982" xsd:string

[Term]
id: T4FS:0000328
name: long-term preservation
def: "Continued access to digital materials, or at least to the information contained in them, indefinitely." [] {IAO:0000119="RDMT. https://terms.codata.org/rdmt/long-term-preservation"}
is_a: T4FS:0000017 ! preservation
property_value: IAO:0000117 "https://orcid.org/0000-0002-5214-4466" xsd:string
property_value: IAO:0000117 "https://orcid.org/0000-0002-7702-4495" xsd:string
property_value: IAO:0000117 "https://orcid.org/0000-0003-2687-1982" xsd:string

[Term]
id: T4FS:0000329
name: research metadata format
def: "Research metadata format is a generic term encompassing the concept of a standardised format for research metadata." [] {IAO:0000119="AL, 9.3.2022"}
comment: AL 9.3.2022: The original CASRAI definition is unsuitable (https://casrai.org/term/research-metadata-format), therefore I have changed the definition to something more generic
is_a: T4FS:0000372 ! data stewardship technical concept
relationship: T4FS:0000563 T4FS:0000137 ! contributes to the implementation of I1. (meta)data use a formal, accessible, shared, and broadly applicable language for knowledge representation
property_value: IAO:0000117 "https://orcid.org/0000-0002-7702-4495" xsd:string
property_value: IAO:0000117 "https://orcid.org/0000-0003-2687-1982" xsd:string

[Term]
id: T4FS:0000330
name: data residency
def: "Physical or geographic location of an organisation’s data or information. Data residency also refers to the legal or regulatory requirements imposed on data based on the country or region in which it resides. Cloud computing, which allows organisations to deliver hosted services over the Internet, can create data residency concerns." [] {IAO:0000119="RDMT. https://terms.codata.org/rdmt/data-residency"}
is_a: T4FS:0000012 ! data stewardship activity
property_value: IAO:0000117 "https://orcid.org/0000-0002-5214-4466" xsd:string
property_value: IAO:0000117 "https://orcid.org/0000-0003-2687-1982" xsd:string

[Term]
id: T4FS:0000331
name: information governance
def: "Information governance, is the overall strategy for information at an organization. Information governance balances the risk that information presents with the value that information provides. Information governance helps with legal compliance, operational transparency, and reducing expenditures associated with legal discovery." [] {IAO:0000119="https://en.wikipedia.org/wiki/Information_governance, accessed 8.2.22"}
comment: CASRAI is the source for the term, with the definition provided separately.
is_a: T4FS:0000107 ! information security
property_value: IAO:0000117 "https://orcid.org/0000-0002-7702-4495" xsd:string
property_value: IAO:0000117 "https://orcid.org/0000-0003-2687-1982" xsd:string

[Term]
id: T4FS:0000332
name: data element
def: "Unit of data for which the definition, identification, representation (term used to represent it), and permissible values are specified by means of a set of attributes." [] {IAO:0000119="RDMT. https://terms.codata.org/rdmt/data-element"}
is_a: T4FS:0000372 ! data stewardship technical concept
property_value: IAO:0000117 "https://orcid.org/0000-0002-5214-4466" xsd:string
property_value: IAO:0000117 "https://orcid.org/0000-0003-2687-1982" xsd:string

[Term]
id: T4FS:0000333
name: data policy
def: "Set of high-level principles that establish a guiding framework for data-related issues. A data policy may contain subsidiary sections that define approaches to strategic aspects such as data access; data protection; data management, custodianship or stewardship; data preservation; relevant legal matters; data acquisition; data ethics and other data-related issues. Distinct from a data management policy which is the subset of data policy addressing the management of a specified set of data assets." [] {IAO:0000119="RDMT. https://terms.codata.org/rdmt/data-policy"}
is_a: T4FS:0000372 ! data stewardship technical concept
relationship: T4FS:0000563 T4FS:0000447 ! contributes to the implementation of fair principle
property_value: IAO:0000117 "https://orcid.org/0000-0002-5214-4466" xsd:string
property_value: IAO:0000117 "https://orcid.org/0000-0003-2687-1982" xsd:string

[Term]
id: T4FS:0000334
name: legacy data
def: "Older data that can no longer be accessed or processed easily because they are stored in obsolete formats or systems." [] {IAO:0000119="RDMT. https://terms.codata.org/rdmt/legacy-data"}
is_a: T4FS:0000430 ! data
property_value: IAO:0000117 "https://orcid.org/0000-0002-5214-4466" xsd:string
property_value: IAO:0000117 "https://orcid.org/0000-0002-7702-4495" xsd:string
property_value: IAO:0000117 "https://orcid.org/0000-0003-2687-1982" xsd:string

[Term]
id: T4FS:0000335
name: controlled vocabulary
def: "List of standardised terminology, words, or phrases, used for indexing or content analysis and information retrieval, usually in a defined information domain." [] {IAO:0000119="RDMT. https://terms.codata.org/rdmt/controlled-vocabulary"}
is_a: T4FS:0000372 ! data stewardship technical concept
relationship: T4FS:0000563 T4FS:0000452 ! contributes to the implementation of I3. (meta)data include qualified references to other (meta)data
property_value: IAO:0000117 "https://orcid.org/0000-0002-5214-4466" xsd:string
property_value: IAO:0000117 "https://orcid.org/0000-0003-2687-1982" xsd:string

[Term]
id: T4FS:0000336
name: data integrity
name: data integrity (access)
def: "Assurance that information can only be accessed or modified by those authorised to do so." [] {IAO:0000119="RDMT. https://terms.codata.org/rdmt/data-integrity-access"}
is_a: T4FS:0000372 ! data stewardship technical concept
property_value: IAO:0000117 "https://orcid.org/0000-0002-5214-4466" xsd:string
property_value: IAO:0000117 "https://orcid.org/0000-0003-2687-1982" xsd:string

[Term]
id: T4FS:0000337
name: pid attribute
def: "Single data element related to a PID and part of its record content." [] {IAO:0000119="RDMT. https://terms.codata.org/rdmt/pid-attribute"}
is_a: T4FS:0000453 ! persistent identifier
property_value: IAO:0000117 "https://orcid.org/0000-0002-5214-4466" xsd:string
property_value: IAO:0000117 "https://orcid.org/0000-0002-7702-4495" xsd:string
property_value: IAO:0000117 "https://orcid.org/0000-0003-2687-1982" xsd:string

[Term]
id: T4FS:0000338
name: aptitudes for change management
def: "Bin for Aptitudes related to Change management." []
is_a: T4FS:0000411 ! change management
property_value: IAO:0000117 "leightonlc" xsd:string

[Term]
id: T4FS:0000339
name: medium-term preservation
def: "Continued access to digital materials beyond changes in technology for a defined period of time but not indefinitely." [] {IAO:0000119="RDMT. https://terms.codata.org/rdmt/medium-term-preservation"}
is_a: T4FS:0000017 ! preservation
property_value: IAO:0000117 "https://orcid.org/0000-0002-5214-4466" xsd:string
property_value: IAO:0000117 "https://orcid.org/0000-0002-7702-4495" xsd:string
property_value: IAO:0000117 "https://orcid.org/0000-0003-2687-1982" xsd:string

[Term]
id: T4FS:0000340
name: project lifecycle
def: "Describes the processes and tasks that must be completed to produce a product or service. Different project lifecycles exist for specific products and services. (For example, the lifecycle followed to build a house is very different from the lifecycle followed to develop a software package." [] {IAO:0000119="Definition from now-deprecated CASRAI Glossary term: project-lifecycle"}
is_a: T4FS:0000372 ! data stewardship technical concept
property_value: IAO:0000117 "https://orcid.org/0000-0002-5214-4466" xsd:string
property_value: IAO:0000117 "https://orcid.org/0000-0002-7702-4495" xsd:string
property_value: IAO:0000117 "https://orcid.org/0000-0003-2687-1982" xsd:string

[Term]
id: T4FS:0000341
name: knowledge to relate fair data assessment to research community norms
def: "Know how the acceptability of research data FAIRness depends on the research community norms e.g. concepts of data and methods for deriving valid knowledge." []
is_a: T4FS:0000259 ! fair training
property_value: IAO:0000117 "Angus Whyte" xsd:string

[Term]
id: T4FS:0000342
name: data traceability
def: "Data traceability follows the lifecycle of data to track all access and changes to the data. It helps demonstrate transparency, compliance and adherence to regulations. Data traceability, along with data compliance, can be considered part of a data audit process. Data traceability is fundamental to reproducible research." [] {IAO:0000119="RDMT. https://terms.codata.org/rdmt/data-traceability"}
is_a: T4FS:0000372 ! data stewardship technical concept
property_value: IAO:0000117 "https://orcid.org/0000-0002-5214-4466" xsd:string
property_value: IAO:0000117 "https://orcid.org/0000-0003-2687-1982" xsd:string

[Term]
id: T4FS:0000343
name: maintaining persistent identifiers
is_a: T4FS:0000492 ! understanding persistent identifiers
created_by: https://orcid.org/0000-0003-2687-1982
creation_date: 2020-10-02T14:23:22.115275Z

[Term]
id: T4FS:0000345
name: select and apply license
def: "Choose the proper license considering types of project data and clearly indicate (apply) the license chosen in the project work." []
is_a: T4FS:0000042 ! ethical application of patents, licenses
property_value: IAO:0000117 "Celia van Gelder" xsd:string
property_value: IAO:0000117 "Mateusz Kuzak" xsd:string
property_value: IAO:0000117 "Yan Wang" xsd:string

[Term]
id: T4FS:0000346
name: relations
def: "Indicates how the different components within a system are linked to fulfill the tasks. Relations are thus defined by the services they are making use of and by the interface specifications." [] {IAO:0000119="Definition from now-deprecated CASRAI Glossary term: relations"}
is_a: T4FS:0000372 ! data stewardship technical concept
property_value: IAO:0000117 "https://orcid.org/0000-0002-5214-4466" xsd:string
property_value: IAO:0000117 "https://orcid.org/0000-0002-7702-4495" xsd:string
property_value: IAO:0000117 "https://orcid.org/0000-0003-2687-1982" xsd:string

[Term]
id: T4FS:0000347
name: dataset
def: "Organised collection of data or objects in a computational format, that are generated or collected by researchers in the course of their investigations, regardless of their form or method, that form the object on which researchers test a hypothesis. This includes the full range of data: raw, unprocessed datasets, proprietary generated and processed data and secondary data obtained from third parties. The presentation of the data in the application is enabled through metadata." [] {IAO:0000119="RDMT. https://terms.codata.org/rdmt/dataset"}
is_a: T4FS:0000072 ! dataset series
property_value: IAO:0000117 "https://orcid.org/0000-0002-5214-4466" xsd:string
property_value: IAO:0000117 "https://orcid.org/0000-0003-2687-1982" xsd:string

[Term]
id: T4FS:0000348
name: aptitudes for service level management
def: "Bin for Aptitudes related to Service level management." []
is_a: T4FS:0000466 ! service level management
property_value: IAO:0000117 "leightonlc" xsd:string

[Term]
id: T4FS:0000350
name: extensible markup language
def: "Text format derived from Standard Generalized Markup Language or ‘SGML’ (ISO 8879). Originally designed to meet the challenges of large-scale electronic publishing, XML is also playing an increasingly important role in the exchange of a wide variety of data on the Web and elsewhere." [] {IAO:0000119="RDMT. https://terms.codata.org/rdmt/extensible-markup-language"}
is_a: T4FS:0000372 ! data stewardship technical concept
relationship: T4FS:0000563 T4FS:0000137 ! contributes to the implementation of I1. (meta)data use a formal, accessible, shared, and broadly applicable language for knowledge representation
property_value: IAO:0000117 "https://orcid.org/0000-0002-5214-4466" xsd:string
property_value: IAO:0000117 "https://orcid.org/0000-0002-7702-4495" xsd:string
property_value: IAO:0000117 "https://orcid.org/0000-0003-2687-1982" xsd:string
property_value: IAO:0000118 "XML" xsd:string

[Term]
id: T4FS:0000351
name: skills related to change management
def: "Bin for Skills needed for Change management." []
is_a: T4FS:0000411 ! change management
property_value: IAO:0000117 "leightonlc" xsd:string

[Term]
id: T4FS:0000352
name: data analysis
def: "Techniques that produce synthesised knowledge from organised information. Process of inspecting, cleaning, transforming, and modelling data with the goal of highlighting useful information suggesting conclusions, and supporting decision making. Data analysis has multiple facets and approaches, encompassing diverse techniques under a variety of names, in different business, science, and social science domains." [] {IAO:0000119="RDMT. https://terms.codata.org/rdmt/data-analysis"}
is_a: T4FS:0000012 ! data stewardship activity
property_value: IAO:0000117 "https://orcid.org/0000-0002-5214-4466" xsd:string
property_value: IAO:0000117 "https://orcid.org/0000-0003-2687-1982" xsd:string

[Term]
id: T4FS:0000353
name: resource management
def: "Resource management is the efficient and effective development of an organization's resources when they are needed. Such resources may include the financial resources, inventory, human skills, production resources, or information technology (IT) and natural resources." [] {IAO:0000119="[LLC, https://en.wikipedia.org/wiki/Resource_management]"}
is_a: T4FS:0000012 ! data stewardship activity
property_value: IAO:0000117 "Kristina Hettne" xsd:string
property_value: IAO:0000117 "Leighton Christiansen" xsd:string
property_value: IAO:0000117 "Simon Hodson" xsd:string
property_value: IAO:0000117 "Victoria Dominguez Del Angel" xsd:string

[Term]
id: T4FS:0000354
name: data exploration
def: "Summarising the main characteristics of a dataset using visualisation." [] {IAO:0000119="RDMT. https://terms.codata.org/rdmt/data-exploration"}
is_a: T4FS:0000352 ! data analysis
property_value: IAO:0000117 "https://orcid.org/0000-0002-5214-4466" xsd:string
property_value: IAO:0000117 "https://orcid.org/0000-0003-2687-1982" xsd:string

[Term]
id: T4FS:0000355
name: aptitudes for storage management
def: "Bin for Aptitudes related to Storage management." []
is_a: T4FS:0000053 ! storage management
property_value: IAO:0000117 "leightonlc" xsd:string

[Term]
id: T4FS:0000356
name: advise and mentor
def: "Management and provision of good data stewardship practice." [] {IAO:0000119="PMQ"}
comment: AL 9.3.22. Removed from 'FAIR4S defined activity' class to better integrate with the T4FS hierarchy.
is_a: T4FS:0000012 ! data stewardship activity
property_value: IAO:0000117 "https://orcid.org/0000-0002-7702-4495" xsd:string
property_value: IAO:0000117 "https://orcid.org/0000-0003-2687-1982" xsd:string
property_value: IAO:0000117 "Philippe Rocca-Serra" xsd:string
property_value: IAO:0000117 "Susanna Sansone" xsd:string
property_value: IAO:0000118 "Advise and enable" xsd:string
property_value: IAO:0000118 "data management and open research" xsd:string
property_value: IAO:0000118 "Data Stewardship and FAIR mentorship activity" xsd:string

[Term]
id: T4FS:0000357
name: skills related to workflow technologies management
def: "Bin for Skills needed for Workflow technologies management." []
is_a: T4FS:0000177 ! workflow technologies management
created_by: leightonlc
creation_date: 2019-10-17T15:15:55.86138Z

[Term]
id: T4FS:0000358
name: digital infrastructure
def: "Those layers that sit between base technology (a computer science concern) and discipline-specific science. Value-added systems and services that can be widely shared across scientific domains, both supporting and enabling large increases in multi- and interdisciplinary science while reducing duplication of effort and resources (including hardware, software, personnel, services and organisations)." [] {IAO:0000119="RDMT. https://terms.codata.org/rdmt/digital-infrastructure"}
is_a: T4FS:0000372 ! data stewardship technical concept
property_value: IAO:0000117 "https://orcid.org/0000-0002-5214-4466" xsd:string
property_value: IAO:0000117 "https://orcid.org/0000-0002-7702-4495" xsd:string
property_value: IAO:0000117 "https://orcid.org/0000-0003-2687-1982" xsd:string

[Term]
id: T4FS:0000359
name: skills related to data management cost management
def: "Bin for Skills needed for Data management cost management." []
is_a: T4FS:0000232 ! data management costs management
property_value: IAO:0000117 "leightonlc" xsd:string

[Term]
id: T4FS:0000360
name: pid system
def: "Consists of at least one PID resolver, a name schema and a defined mechanism for issuing PIDs that conform to the name schema." [] {IAO:0000119="RDMT. https://terms.codata.org/rdmt/pid-system"}
is_a: T4FS:0000453 ! persistent identifier
property_value: IAO:0000117 "https://orcid.org/0000-0002-5214-4466" xsd:string
property_value: IAO:0000117 "https://orcid.org/0000-0002-7702-4495" xsd:string
property_value: IAO:0000117 "https://orcid.org/0000-0003-2687-1982" xsd:string

[Term]
id: T4FS:0000361
name: I2. (meta)data use vocabularies that follow fair principles
is_a: T4FS:0000014 ! interoperability of digital assets
property_value: IAO:0000117 "https://orcid.org/0000-0003-2687-1982" xsd:string

[Term]
id: T4FS:0000362
name: cross-disciplinary
def: "Research approach that explains aspects of one discipline in terms of another (e.g., the physics of music; the politics of literature)." [] {IAO:0000119="RDMT. https://terms.codata.org/rdmt/cross-disciplinary"}
is_a: T4FS:0000372 ! data stewardship technical concept
property_value: IAO:0000117 "https://orcid.org/0000-0002-5214-4466" xsd:string
property_value: IAO:0000117 "https://orcid.org/0000-0003-2687-1982" xsd:string

[Term]
id: T4FS:0000364
name: semantic data
def: "Data that are tagged with particular metadata that can be used to derive relationships between data." [] {IAO:0000119="RDMT. https://terms.codata.org/rdmt/semantic-data"}
is_a: T4FS:0000430 ! data
relationship: T4FS:0000563 T4FS:0000361 ! contributes to the implementation of I2. (meta)data use vocabularies that follow fair principles
property_value: IAO:0000117 "https://orcid.org/0000-0002-5214-4466" xsd:string
property_value: IAO:0000117 "https://orcid.org/0000-0002-7702-4495" xsd:string
property_value: IAO:0000117 "https://orcid.org/0000-0003-2687-1982" xsd:string

[Term]
id: T4FS:0000365
name: pid domain
def: "For a single identifier, the class of entity it refers to. For a PID system, the typical class of entities it is intended to be used for, such as digital objects, physical objects, bodies, actors." [] {IAO:0000119="RDMT. https://terms.codata.org/rdmt/pid-domain"}
is_a: T4FS:0000453 ! persistent identifier
property_value: IAO:0000117 "https://orcid.org/0000-0002-5214-4466" xsd:string
property_value: IAO:0000117 "https://orcid.org/0000-0002-7702-4495" xsd:string
property_value: IAO:0000117 "https://orcid.org/0000-0003-2687-1982" xsd:string

[Term]
id: T4FS:0000367
name: knowledge to choose fair data handling approaches appropriate to the research phenomena
def: "Select data handling approaches likely to make data as FAIR as possible, considering what the data is about and its purpose in the research." []
is_a: T4FS:0000259 ! fair training
property_value: IAO:0000117 "Angus Whyte" xsd:string

[Term]
id: T4FS:0000368
name: provenance information management
def: "The activity of recording provenance for data and software. Knowledge about provenance vocabularies, for example PROV-O and models provenance such as nanopublications." [] {IAO:0000119="KH"}
is_a: T4FS:0000353 ! resource management
property_value: IAO:0000117 "Kristina Hettne" xsd:string
property_value: IAO:0000117 "Simon Hodson" xsd:string
property_value: IAO:0000117 "Victoria Dominguez Del Angel" xsd:string

[Term]
id: T4FS:0000370
name: reproducible research
def: "Results that can be replicated using the documented data, code, and methods employed by the author or provider without the need for any additional information or needing to communicate with the author or provider." [] {IAO:0000119="RDMT. https://terms.codata.org/rdmt/reproducible-research"}
is_a: T4FS:0000170 ! reuse of digital assets
property_value: IAO:0000117 "https://orcid.org/0000-0002-5214-4466" xsd:string
property_value: IAO:0000117 "https://orcid.org/0000-0002-7702-4495" xsd:string
property_value: IAO:0000117 "https://orcid.org/0000-0003-2687-1982" xsd:string

[Term]
id: T4FS:0000371
name: A1.2 the protocol allows for an authentication and authorisation procedure, where necessary
is_a: T4FS:0000038 ! A1. (meta)data are retrievable by their identifier using a standardised communications protocol
property_value: IAO:0000117 "https://orcid.org/0000-0003-2687-1982" xsd:string

[Term]
id: T4FS:0000372
name: data stewardship technical concept
relationship: T4FS:0000563 T4FS:0000446 ! contributes to the implementation of data stewardship guideline
property_value: IAO:0000117 "https://orcid.org/0000-0002-7702-4495" xsd:string
property_value: IAO:0000117 "https://orcid.org/0000-0003-2687-1982" xsd:string

[Term]
id: T4FS:0000373
name: canonical data collection
def: "Data collection that has been normalised by some established criteria to allow for effective data management. Examples include: data files that belong to a certain experiment, all files that are created by one specific simulation, all files that belong to a specific observation (same day, same place, etc.)." [] {IAO:0000119="RDMT. https://terms.codata.org/rdmt/canonical-data-collection"}
is_a: T4FS:0000372 ! data stewardship technical concept
property_value: IAO:0000117 "https://orcid.org/0000-0002-5214-4466" xsd:string
property_value: IAO:0000117 "https://orcid.org/0000-0003-2687-1982" xsd:string

[Term]
id: T4FS:0000374
name: archival documentation of software
def: "Ability to clean up existing source code and version control systems, get Unique ID for the code, choose the appropriate code repository/registry [YLF, VDA, KH]" []
is_a: T4FS:0000156 ! archiving
property_value: IAO:0000117 "https://orcid.org/0000-0002-7702-4495" xsd:string
property_value: IAO:0000117 "Kristina Hettne" xsd:string
property_value: IAO:0000117 "Victoria Dominguez Del Angel" xsd:string
property_value: IAO:0000117 "Yann Le Franc" xsd:string

[Term]
id: T4FS:0000375
name: data harmonization
def: "Data harmonization is the process of making data from different sources comparable." [] {IAO:0000119="Modified from CASRAI. https://casrai.org/term/data-harmonization/"}
is_a: T4FS:0000036 ! curation
property_value: IAO:0000117 "https://orcid.org/0000-0002-7702-4495" xsd:string
property_value: IAO:0000117 "https://orcid.org/0000-0003-2687-1982" xsd:string
property_value: IAO:0000233 "https://github.com/terms4fairskills/FAIRterminology/issues/17" xsd:string

[Term]
id: T4FS:0000376
name: data mart
def: "Repository of data designed to serve a particular community of knowledge workers. A data mart contains harmonised, highly-structured, quality data integrated from multiple sources (which is also a characteristic of the data warehouse). It's also optimised to support well-known, predefined and repeatable analytic queries, rather than ad-hoc analysis." [] {IAO:0000119="RDMT. https://terms.codata.org/rdmt/data-mart"}
is_a: T4FS:0000215 ! data store
property_value: IAO:0000117 "https://orcid.org/0000-0002-5214-4466" xsd:string
property_value: IAO:0000117 "https://orcid.org/0000-0003-2687-1982" xsd:string

[Term]
id: T4FS:0000377
name: access workflow
def: "Type of access entity that contains the services and functions which make the data object holdings and their information content and related services visible to data consumers." [] {IAO:0000119="RDMT. https://terms.codata.org/rdmt/access-workflow"}
is_a: T4FS:0000283 ! access
property_value: IAO:0000117 "https://orcid.org/0000-0002-5214-4466" xsd:string
property_value: IAO:0000117 "https://orcid.org/0000-0003-2687-1982" xsd:string

[Term]
id: T4FS:0000378
name: knowledge of service level management
def: "Bin for types of Knowledge related to Service level management." []
is_a: T4FS:0000466 ! service level management
created_by: leightonlc
creation_date: 2019-10-17T15:18:53.73274Z

[Term]
id: T4FS:0000379
name: data model
def: "Model that specifies the structure or schema of a dataset. The model provides a documented description of the data and thus is an instance of metadata. It is a logical, relational data model showing an organised dataset as a collection of tables with entity, attributes and relations." [] {IAO:0000119="RDMT. https://terms.codata.org/rdmt/data-model"}
is_a: T4FS:0000372 ! data stewardship technical concept
property_value: IAO:0000117 "https://orcid.org/0000-0002-5214-4466" xsd:string
property_value: IAO:0000117 "https://orcid.org/0000-0003-2687-1982" xsd:string

[Term]
id: T4FS:0000380
name: appreciate security and usability trade-offs
def: "Be aware of the potential conflicts between security and usability. Understand the importance of having information security policy and keeping a balance between the information security and usability. Willing to establish both organization and technical information security measurements." []
is_a: T4FS:0000107 ! information security
property_value: IAO:0000117 "Angus Whyte" xsd:string
property_value: IAO:0000117 "Celia van Gelder" xsd:string
property_value: IAO:0000117 "Mateusz Kuzak" xsd:string
property_value: IAO:0000117 "Yan Wang" xsd:string

[Term]
id: T4FS:0000381
name: standard
def: "Set of agreed-upon and documented guidelines, specifications, accepted practices, technical requirements, or terminologies that have been prepared by a standards developing organisation or group, and published in accordance with established procedures. These can be mandatory or voluntary and are distinct from Acts, regulations, and codes, although standards can be referenced in those legal instruments." [] {IAO:0000119="RDMT. https://terms.codata.org/rdmt/standard"}
is_a: T4FS:0000372 ! data stewardship technical concept
property_value: IAO:0000117 "https://orcid.org/0000-0002-5214-4466" xsd:string
property_value: IAO:0000117 "https://orcid.org/0000-0002-7702-4495" xsd:string
property_value: IAO:0000117 "https://orcid.org/0000-0003-2687-1982" xsd:string

[Term]
id: T4FS:0000382
name: university teaching
def: "The application of a comprehensive knowledge of a discipline or disciplines to the development of expertise and the generation of new knowledge through research, and the planning and presentation of courses of study for undergraduates and graduates in universities." [] {IAO:0000119="Definition from now-deprecated CASRAI Glossary term: university-teaching"}
is_a: T4FS:0000012 ! data stewardship activity
property_value: IAO:0000117 "https://orcid.org/0000-0002-5214-4466" xsd:string
property_value: IAO:0000117 "https://orcid.org/0000-0002-7702-4495" xsd:string
property_value: IAO:0000117 "https://orcid.org/0000-0003-2687-1982" xsd:string

[Term]
id: T4FS:0000383
name: data migration
def: "Transfer of data between storage types, formats, information technologies, or computer systems. A data migration project is usually undertaken to replace or upgrade servers or storage equipment, for a website consolidation, to conduct server maintenance or to relocate a data centre." [] {IAO:0000119="RDMT. https://terms.codata.org/rdmt/data-migration"}
is_a: T4FS:0000141 ! data management
property_value: IAO:0000117 "https://orcid.org/0000-0002-5214-4466" xsd:string
property_value: IAO:0000117 "https://orcid.org/0000-0003-2687-1982" xsd:string

[Term]
id: T4FS:0000384
name: data cleaning
def: "Process of detecting and correcting corrupt or inaccurate records from a dataset. Data cleaning is a continuous process that requires corrective actions throughout the data lifecycle. Data cleaning involves identifying, replacing, modifying or deleting incomplete, incorrect, inaccurate, inconsistent, irrelevant, and improperly formatted data. Typically, the process involves updating, correcting, standardising, and de-duplicating records to create a single view of the data, even if they are stored in multiple disparate systems." [] {IAO:0000119="RDMT. https://terms.codata.org/rdmt/data-cleaning"}
is_a: T4FS:0000036 ! curation
property_value: IAO:0000117 "https://orcid.org/0000-0002-5214-4466" xsd:string
property_value: IAO:0000117 "https://orcid.org/0000-0003-2687-1982" xsd:string

[Term]
id: T4FS:0000385
name: R1.2 (meta)data are associated with detailed provenance
is_a: T4FS:0000174 ! R1. (meta)data are richly described with a plurality of accurate and relevant attributes
property_value: IAO:0000117 "https://orcid.org/0000-0003-2687-1982" xsd:string

[Term]
id: T4FS:0000387
name: skills related to identity management
def: "Bin for Skills needed for Identity management." []
is_a: T4FS:0000169 ! identity management
property_value: IAO:0000117 "leightonlc" xsd:string

[Term]
id: T4FS:0000388
name: using persistent identifiers
def: "The use of persistent identifiers or PIDs to uniquely and persistently identify an entity." [] {IAO:0000119="[PMQ 3.2022]"}
is_a: T4FS:0000492 ! understanding persistent identifiers
property_value: IAO:0000117 "https://orcid.org/0000-0002-7702-4495" xsd:string
property_value: IAO:0000117 "https://orcid.org/0000-0003-2687-1982" xsd:string
property_value: IAO:0000117 "Nancy Hoebelheinrich" xsd:string
created_by: https://orcid.org/0000-0003-2687-1982
creation_date: 2020-10-02T14:22:51.569762Z

[Term]
id: T4FS:0000389
name: data curator
comment: AL 15.3.22: Updated label to 'data curator' to encompass curation beyond just in databases.
relationship: T4FS:0000558 T4FS:0000012 ! has/wants competency in data stewardship activity
relationship: T4FS:0000559 T4FS:0000372 ! has/wants knowledge about data stewardship technical concept
relationship: T4FS:0000559 T4FS:0000446 ! has/wants knowledge about data stewardship guideline
relationship: T4FS:0000561 T4FS:0000372 ! has/wants practical skill about data stewardship technical concept
relationship: T4FS:0000562 T4FS:0000548 ! has aptitude for data stewardship soft skill
property_value: IAO:0000117 "https://orcid.org/0000-0002-7702-4495" xsd:string
property_value: IAO:0000118 "database curator" xsd:string

[Term]
id: T4FS:0000390
name: engage innovation partners
def: "Learn about innovation partners' interests and concerns, analyze them and position the project work/outcome properly. Reach out to innovation partners with proactive and pragmatic innovation plan which is in compliance with FAIR principles." []
is_a: T4FS:0000084 ! engaging in open innovation beyond academia
property_value: IAO:0000117 "Celia van Gelder" xsd:string
property_value: IAO:0000117 "Mateusz Kuzak" xsd:string
property_value: IAO:0000117 "Yan Wang" xsd:string

[Term]
id: T4FS:0000391
name: R1.3 (meta)data meet domain-relevant community standards
is_a: T4FS:0000174 ! R1. (meta)data are richly described with a plurality of accurate and relevant attributes
property_value: IAO:0000117 "https://orcid.org/0000-0003-2687-1982" xsd:string

[Term]
id: T4FS:0000392
name: data reduction
def: "Process of reducing the amount or size of stored data. This may be achieved by eliminating redundant copies of data files, deduplicating data files by removing redundant records, or by compressing the data files." [] {IAO:0000119="RDMT. https://terms.codata.org/rdmt/data-reduction"}
is_a: T4FS:0000141 ! data management
property_value: IAO:0000117 "https://orcid.org/0000-0002-5214-4466" xsd:string
property_value: IAO:0000117 "https://orcid.org/0000-0003-2687-1982" xsd:string

[Term]
id: T4FS:0000393
name: F4. (meta)data are registered or indexed in a searchable resource
is_a: T4FS:0000248 ! findability of digital assets
property_value: IAO:0000117 "https://orcid.org/0000-0003-2687-1982" xsd:string

[Term]
id: T4FS:0000394
name: data type registry
def: "Registry for data types supporting their standardisation, uniqueness and discoverability. Data types range from complex digital objects to simple categories that occur in digital objects. An additional functionality may be to link data types to executable data processing functions." [] {IAO:0000119="RDMT. https://terms.codata.org/rdmt/data-type-registry"}
is_a: T4FS:0000215 ! data store
property_value: IAO:0000117 "https://orcid.org/0000-0002-5214-4466" xsd:string
property_value: IAO:0000117 "https://orcid.org/0000-0003-2687-1982" xsd:string

[Term]
id: T4FS:0000397
name: database
def: "Collection of data that is organised according to a conceptual structure/model describing the characteristics of these data and the relationships among their corresponding entities, supporting one or more application areas. A database allows its contents to be easily accessed, managed and updated. The type of database used depends on the requirements of the study. A common type is the relational database, where data are related to each other in a systematic manner so that they can be reorganised and accessed in a number of different ways. A database may house one or many datasets." [] {IAO:0000119="RDMT. https://terms.codata.org/rdmt/database"}
is_a: T4FS:0000215 ! data store
property_value: IAO:0000117 "https://orcid.org/0000-0002-5214-4466" xsd:string
property_value: IAO:0000117 "https://orcid.org/0000-0003-2687-1982" xsd:string

[Term]
id: T4FS:0000398
name: appreciation of fair and open research
def: "Recognize the added value of FAIR and open research, encourage researchers to practise FAIR and open research." []
is_a: T4FS:0000008 ! develop open research strategy and vision
property_value: IAO:0000117 "Angus Whyte" xsd:string
property_value: IAO:0000117 "Celia van Gelder" xsd:string
property_value: IAO:0000117 "Mateusz Kuzak" xsd:string
property_value: IAO:0000117 "Yan Wang" xsd:string

[Term]
id: T4FS:0000399
name: ability to learn new techniques for fair implementation
def: "Demonstrate willingness to engage with new ways of applying FAIR principles." []
is_a: T4FS:0000408 ! aptitudes associated with using fair tools and services
relationship: T4FS:0000556 T4FS:0000548 {all_only="true"} ! requires/improves personal attribute data stewardship soft skill
property_value: IAO:0000117 "Angus Whyte" xsd:string

[Term]
id: T4FS:0000400
name: aptitudes for funding acquisition management
def: "Bin for Aptitudes related to Funding acquisition management." []
is_a: T4FS:0000426 ! funding acquisition management
property_value: IAO:0000117 "leightonlc" xsd:string

[Term]
id: T4FS:0000401
name: choosing the appropriate model or format for your data
def: "To be able to choose the correct data model and/or exchange format for your data, based on the repository where you plan to deposit your data." [] {IAO:0000119="[PMQ]"}
is_a: T4FS:0000175 ! fair evaluation of repositories for data deposition
property_value: IAO:0000117 "https://orcid.org/0000-0003-2687-1982" xsd:string
property_value: IAO:0000118 "Which data model to use" xsd:string
property_value: IAO:0000118 "Which format to use" xsd:string

[Term]
id: T4FS:0000402
name: provenance metadata
def: "Information concerning the creation, attribution, or version history of managed data. Provenance metadata indicates the relationship between two versions of data objects and is generated whenever a new version of a dataset is created. Provenance information is gathered along the data lifecycle as part of curation processes. A finer level of provenance metadata would be concerned only with data flowing between various stores such as curated databases and managed repositories. Provenance metadata is designed to allow queries over the relationship between versions, and includes either or both fine-grained and coarse-grained provenance data. Different applications may store different provenance data." [] {IAO:0000119="RDMT. https://terms.codata.org/rdmt/provenance-metadata"}
is_a: T4FS:0000527 ! metadata
property_value: IAO:0000117 "https://orcid.org/0000-0002-5214-4466" xsd:string
property_value: IAO:0000117 "https://orcid.org/0000-0002-7702-4495" xsd:string

[Term]
id: T4FS:0000404
name: data availability
def: "State when data are available in a timely manner in the place and form as needed by the user." [] {IAO:0000119="RDMT. https://terms.codata.org/rdmt/data-availability"}
is_a: T4FS:0000372 ! data stewardship technical concept
property_value: IAO:0000117 "https://orcid.org/0000-0002-5214-4466" xsd:string
property_value: IAO:0000117 "https://orcid.org/0000-0003-2687-1982" xsd:string

[Term]
id: T4FS:0000406
name: data review
def: "Activity through which the correctness conditions of the data are verified. It also includes the specification of the type of the error or condition not met, and the qualification of the data and its division into “error-free” or “erroneous” data. Data review consists of both error detection and data analysis, and can be carried out in manual or automated mode." [] {IAO:0000119="RDMT. https://terms.codata.org/rdmt/data-review"}
is_a: T4FS:0000352 ! data analysis
property_value: IAO:0000117 "https://orcid.org/0000-0002-5214-4466" xsd:string
property_value: IAO:0000117 "https://orcid.org/0000-0002-7702-4495" xsd:string
property_value: IAO:0000117 "https://orcid.org/0000-0003-2687-1982" xsd:string

[Term]
id: T4FS:0000408
name: aptitudes associated with using fair tools and services
is_a: T4FS:0000508 ! using fair and open research tools or services
created_by: HughShanahan
creation_date: 2019-10-18T08:56:32.673701Z

[Term]
id: T4FS:0000410
name: preservation metadata
def: "Documents actions that have been undertaken to preserve a digital resource such as migrations and checks sum calculations." [] {IAO:0000119="RDMT. https://terms.codata.org/rdmt/preservation-metadata"}
is_a: T4FS:0000527 ! metadata
property_value: IAO:0000117 "https://orcid.org/0000-0002-5214-4466" xsd:string
property_value: IAO:0000117 "https://orcid.org/0000-0002-7702-4495" xsd:string
property_value: IAO:0000117 "https://orcid.org/0000-0003-2687-1982" xsd:string

[Term]
id: T4FS:0000411
name: change management
def: "Change management is a broad subject and can be applied to all different types of organizational change. The most common change drivers include:  technological evolution, process reviews, crisis, and consumer habit changes; pressure from new business entrants, acquisitions, mergers, and organizational restructuring." [] {IAO:0000119="https://www.hucmi.com/en/hcmbok/"}
is_a: T4FS:0000353 ! resource management
property_value: IAO:0000117 "Kristina Hettne" xsd:string
property_value: IAO:0000117 "Leighton Christiansen" xsd:string
property_value: IAO:0000117 "Simon Hodson" xsd:string
property_value: IAO:0000117 "Victoria Dominguez Del Angel" xsd:string
property_value: IAO:0000118 "CM" xsd:string

[Term]
id: T4FS:0000413
name: original repository
def: "Type of repository where the original copy of data was stored and probably a data identifier registered." [] {IAO:0000119="RDMT. https://terms.codata.org/rdmt/original-repository"}
is_a: T4FS:0000215 ! data store
property_value: IAO:0000117 "https://orcid.org/0000-0002-5214-4466" xsd:string
property_value: IAO:0000117 "https://orcid.org/0000-0002-7702-4495" xsd:string
property_value: IAO:0000117 "https://orcid.org/0000-0003-2687-1982" xsd:string

[Term]
id: T4FS:0000414
name: de-identification
def: "Techniques designed to make the risk of identifying a particular individual in a dataset negligible, whilst retaining the re-usability of the dataset. The purpose is to protect the privacy of the individual and comply with legislation, whilst enabling data sharing. Methods include removing direct and indirect identifiers such as names, addresses, social insurance numbers, or dates of birth, or using obfuscation methods such as encryption, hashing, generalisation, pseudonymisation, and perturbation." [] {IAO:0000119="RDMT. https://terms.codata.org/rdmt/de-identification"}
is_a: T4FS:0000107 ! information security
property_value: IAO:0000117 "https://orcid.org/0000-0002-5214-4466" xsd:string
property_value: IAO:0000117 "https://orcid.org/0000-0002-7702-4495" xsd:string
property_value: IAO:0000117 "https://orcid.org/0000-0003-2687-1982" xsd:string

[Term]
id: T4FS:0000415
name: manager
def: "Program delivery managers and support function managers, at all levels in an institution who are accountable for the direct delivery and support of programs and services within their domain of business responsibility." [] {IAO:0000119="Definition from now-deprecated CASRAI Glossary term: manager"}
relationship: T4FS:0000558 T4FS:0000012 ! has/wants competency in data stewardship activity
relationship: T4FS:0000559 T4FS:0000372 ! has/wants knowledge about data stewardship technical concept
relationship: T4FS:0000559 T4FS:0000446 ! has/wants knowledge about data stewardship guideline
relationship: T4FS:0000561 T4FS:0000372 ! has/wants practical skill about data stewardship technical concept
relationship: T4FS:0000562 T4FS:0000548 ! has aptitude for data stewardship soft skill
property_value: IAO:0000117 "https://orcid.org/0000-0002-5214-4466" xsd:string
property_value: IAO:0000117 "https://orcid.org/0000-0002-7702-4495" xsd:string
property_value: IAO:0000117 "https://orcid.org/0000-0003-2687-1982" xsd:string

[Term]
id: T4FS:0000417
name: organizational leadership
def: "Organizational leadership is: (a) The ability to attract, assess, mobilize and focus energies and talent to work towards a shared purpose aligned with the mandate of the organization; (b) The ability to change culture, processes and priorities within the organization; and, (c) The ability to mentor." [] {IAO:0000119="Definition from now-deprecated CASRAI Glossary term: organizational-leadership"}
is_a: T4FS:0000548 ! data stewardship soft skill
property_value: IAO:0000117 "https://orcid.org/0000-0002-5214-4466" xsd:string
property_value: IAO:0000117 "https://orcid.org/0000-0002-7702-4495" xsd:string
property_value: IAO:0000117 "https://orcid.org/0000-0003-2687-1982" xsd:string

[Term]
id: T4FS:0000418
name: data dredging
def: "Data mining practice in which large volumes of data are analysed seeking any possible relationships between data. The traditional scientific method, in contrast, begins with a hypothesis and follows with an examination of the data. Data dredging often circumvents traditional data mining techniques and may lead to premature conclusions. Uncovered patterns may be presented as statistically significant without any specific hypothesis as to the underlying causality." [] {IAO:0000119="RDMT. https://terms.codata.org/rdmt/data-dredging"}
is_a: T4FS:0000352 ! data analysis
property_value: IAO:0000117 "https://orcid.org/0000-0002-5214-4466" xsd:string
property_value: IAO:0000117 "https://orcid.org/0000-0003-2687-1982" xsd:string
property_value: IAO:0000118 "Data fishing" xsd:string

[Term]
id: T4FS:0000420
name: unstructured data
def: "Data that have not been organised into a format and identifiable data structure that makes them easy to access and process. These data can often be searched as long as they are digital, but they are difficult to use for computer analyses." [] {IAO:0000119="RDMT. https://terms.codata.org/rdmt/unstructured-data"}
is_a: T4FS:0000430 ! data
property_value: IAO:0000117 "https://orcid.org/0000-0002-5214-4466" xsd:string
property_value: IAO:0000117 "https://orcid.org/0000-0002-7702-4495" xsd:string
property_value: IAO:0000117 "https://orcid.org/0000-0003-2687-1982" xsd:string
property_value: IAO:0000118 "Unstructured information" xsd:string

[Term]
id: T4FS:0000421
name: presentation slides with interactive exercises
is_a: T4FS:0000211 ! presentation slides
created_by: https://orcid.org/0000-0003-2687-1982
creation_date: 2020-11-16T22:18:14.764875Z

[Term]
id: T4FS:0000422
name: creating persistent identifiers
is_a: T4FS:0000492 ! understanding persistent identifiers
created_by: https://orcid.org/0000-0003-2687-1982
creation_date: 2020-10-02T14:23:05.600474Z

[Term]
id: T4FS:0000423
name: data linkage
def: "The process of bringing together from two or more different sources, data that relate to the same individual, family, place or event)." [] {IAO:0000119="RDMT. https://terms.codata.org/rdmt/data-linkage"}
is_a: T4FS:0000372 ! data stewardship technical concept
property_value: IAO:0000117 "https://orcid.org/0000-0002-5214-4466" xsd:string
property_value: IAO:0000117 "https://orcid.org/0000-0003-2687-1982" xsd:string
property_value: IAO:0000118 "Linkage" xsd:string

[Term]
id: T4FS:0000425
name: catalogue
def: "A type of collection that describes, and points to features of another collection." [] {IAO:0000119="RDMT. https://terms.codata.org/rdmt/catalogue"}
is_a: T4FS:0000372 ! data stewardship technical concept
property_value: IAO:0000117 "https://orcid.org/0000-0002-5214-4466" xsd:string
property_value: IAO:0000117 "https://orcid.org/0000-0003-2687-1982" xsd:string

[Term]
id: T4FS:0000426
name: funding acquisition management
def: "The consideration of available monetary resources for a specific time period to serve a specific purpose." [] {IAO:0000119="KH"}
is_a: T4FS:0000353 ! resource management
property_value: IAO:0000117 "Kristina Hettne" xsd:string
property_value: IAO:0000117 "Simon Hodson" xsd:string
property_value: IAO:0000117 "Victoria Dominguez Del Angel" xsd:string

[Term]
id: T4FS:0000427
name: machine access via api
def: "To be able to use programmatic methods to access a resource's API to query and extract an appropriate subset of data." [] {IAO:0000119="PMQ"}
is_a: T4FS:0000372 ! data stewardship technical concept
property_value: IAO:0000117 "https://orcid.org/0000-0003-2687-1982" xsd:string
property_value: IAO:0000118 "API access" xsd:string
property_value: IAO:0000118 "Machine actionable search" xsd:string

[Term]
id: T4FS:0000428
name: data structure continuum
def: "Continuum of data structure that includes unstructured data, semi-structured data, and structured data." [] {IAO:0000119="RDMT. https://terms.codata.org/rdmt/data-structure-continuum"}
is_a: T4FS:0000372 ! data stewardship technical concept
property_value: IAO:0000117 "https://orcid.org/0000-0002-5214-4466" xsd:string
property_value: IAO:0000117 "https://orcid.org/0000-0003-2687-1982" xsd:string

[Term]
id: T4FS:0000430
name: data
def: "Facts, measurements, recordings, records, or observations about the world, collected by researchers, that are yet to be processed/interpreted/analysed. Data may be in any format or medium taking the form of writings, notes, numbers, symbols, text, images, films, video, sound recordings, pictorial reproductions, drawings, designs or other graphical representations, procedural manuals, forms, diagrams, work flow charts, equipment descriptions, data files, data processing algorithms, or statistical records." [] {IAO:0000119="RDMT. https://terms.codata.org/rdmt/data"}
is_a: T4FS:0000372 ! data stewardship technical concept
property_value: IAO:0000117 "https://orcid.org/0000-0002-5214-4466" xsd:string
property_value: IAO:0000117 "https://orcid.org/0000-0003-2687-1982" xsd:string

[Term]
id: T4FS:0000431
name: semi-structured data
def: "Data that have not been organised into a specialised repository, such as a database, but that nevertheless have associated information, such as metadata, that makes them more amenable to processing than raw data. Semi-structured data lie somewhere between structured and unstructured data. They are not organised in a complex manner that makes sophisticated access and analysis possible. However, they may have information associated with them, such as metadata tagging that allows elements contained to be addressed." [] {IAO:0000119="RDMT. https://terms.codata.org/rdmt/semi-structured-data"}
is_a: T4FS:0000430 ! data
property_value: IAO:0000117 "https://orcid.org/0000-0002-5214-4466" xsd:string
property_value: IAO:0000117 "https://orcid.org/0000-0002-7702-4495" xsd:string
property_value: IAO:0000117 "https://orcid.org/0000-0003-2687-1982" xsd:string

[Term]
id: T4FS:0000432
name: book chapter
is_a: T4FS:0000305 ! book
created_by: https://orcid.org/0000-0003-2687-1982
creation_date: 2020-10-01T20:53:37.24517Z

[Term]
id: T4FS:0000433
name: research scientist
def: "A scientist who conducts activities in: (1) Research, development and analysis (RDA); (2) Managing research; and, (3) Representation and client services." [] {IAO:0000119="Definition from now-deprecated CASRAI Glossary term: research-scientist"}
is_a: T4FS:0000220 ! researcher
property_value: IAO:0000117 "https://orcid.org/0000-0002-5214-4466" xsd:string
property_value: IAO:0000117 "https://orcid.org/0000-0002-7702-4495" xsd:string
property_value: IAO:0000117 "https://orcid.org/0000-0003-2687-1982" xsd:string

[Term]
id: T4FS:0000434
name: digital object identifier
def: "Type of digital Persistent Identifier (PID) issued by the International DOI Foundation. This permanent digital identifier is associated with an object that permits the object to be referenced reliably even if its location and metadata undergo change over time." [] {IAO:0000119="RDMT. https://terms.codata.org/rdmt/digital-object-identifier"}
is_a: T4FS:0000453 ! persistent identifier
property_value: IAO:0000117 "https://orcid.org/0000-0002-5214-4466" xsd:string
property_value: IAO:0000117 "https://orcid.org/0000-0002-7702-4495" xsd:string
property_value: IAO:0000117 "https://orcid.org/0000-0003-2687-1982" xsd:string
property_value: IAO:0000118 "DOI" xsd:string

[Term]
id: T4FS:0000435
name: F3. metadata clearly and explicitly include the identifier of the data they describe
is_a: T4FS:0000248 ! findability of digital assets
property_value: IAO:0000117 "https://orcid.org/0000-0003-2687-1982" xsd:string

[Term]
id: T4FS:0000437
name: information management specialist
def: "Expert in one or more of the information management disciplines that support the effective and efficient management of information." [] {IAO:0000119="RDMT. https://terms.codata.org/rdmt/information-management-specialist"}
relationship: T4FS:0000558 T4FS:0000012 ! has/wants competency in data stewardship activity
relationship: T4FS:0000559 T4FS:0000372 ! has/wants knowledge about data stewardship technical concept
relationship: T4FS:0000559 T4FS:0000446 ! has/wants knowledge about data stewardship guideline
relationship: T4FS:0000561 T4FS:0000372 ! has/wants practical skill about data stewardship technical concept
relationship: T4FS:0000562 T4FS:0000548 ! has aptitude for data stewardship soft skill
property_value: IAO:0000117 "https://orcid.org/0000-0002-5214-4466" xsd:string
property_value: IAO:0000117 "https://orcid.org/0000-0003-2687-1982" xsd:string

[Term]
id: T4FS:0000438
name: A2. metadata are accessible, even when the data are no longer available
is_a: T4FS:0000478 ! accessibility of digital assets
property_value: IAO:0000117 "https://orcid.org/0000-0003-2687-1982" xsd:string

[Term]
id: T4FS:0000439
name: stakeholder engagement on societal impact
def: "Identify and engage in dialogue with stakeholders affected by the research, or by making its outputs FAIR." []
is_a: T4FS:0000525 ! research integrity, attribution, impact awareness
property_value: IAO:0000117 "Angus Whyte" xsd:string
property_value: IAO:0000117 "Celia van Gelder" xsd:string
property_value: IAO:0000117 "Mateusz Kuzak" xsd:string
property_value: IAO:0000117 "Yan Wang" xsd:string

[Term]
id: T4FS:0000441
name: principal investigator
def: "The Principal Investigator (P.I.) is a researcher who has a research leadership role and is the point of contact for a project or partnership that applies the scientific method, historical method, or other research methodology for the advancement of knowledge resulting in independent, objective, high quality, traceable, and reproducible results. The P.I. has primary responsibility for the intellectual direction and integrity of the research or research-related activity, including data production, findings and results, and ensures ethical conduct in all aspects of the research process including but not limited to the treatment of human and animal subjects, conflicts of interest, data acquisition, sharing and ownership, publication practices, responsible authorship, and collaborative research and reporting. While various tasks may be delegated to team members, some of whom may have greater expertise in specific areas, the P.I. is familiar with the various technical and scientific aspects of a project and how they fit together, is able to identify and remediate gaps, and ensure communication within the team and with users of the research data and results." [] {IAO:0000119="Definition from now-deprecated CASRAI Glossary term: principal-investigator"}
is_a: T4FS:0000415 ! manager
property_value: IAO:0000117 "https://orcid.org/0000-0002-5214-4466" xsd:string
property_value: IAO:0000117 "https://orcid.org/0000-0002-7702-4495" xsd:string
property_value: IAO:0000117 "https://orcid.org/0000-0003-2687-1982" xsd:string

[Term]
id: T4FS:0000442
name: program manager
def: "The person responsible for creating the organizational environment culture by providing clear direction and circumstances that allow people to be successful. The program manager is judged on the elements time, cost, and scope, cumulatively for all the projects and operations within the program. Program management decisions are both tactical and strategic in nature. The strategy aspects of these decisions must consider multidimensional impacts beyond the near-term delivery dates of the project. In addition to delivery and execution, the program manager has to also be concerned with the overall health and effectiveness of the program over the long term." [] {IAO:0000119="Definition from now-deprecated CASRAI Glossary term: program-manager"}
is_a: T4FS:0000415 ! manager
property_value: IAO:0000117 "https://orcid.org/0000-0002-5214-4466" xsd:string
property_value: IAO:0000117 "https://orcid.org/0000-0002-7702-4495" xsd:string
property_value: IAO:0000117 "https://orcid.org/0000-0003-2687-1982" xsd:string

[Term]
id: T4FS:0000443
name: persistent uniform resource locator
def: "URL that points to an intermediate resolution service. The PURL resolution service associates the PURL with the actual URL and returns that URL to the client." [] {IAO:0000119="RDMT. https://terms.codata.org/rdmt/persistent-uniform-resource-locator"}
is_a: T4FS:0000453 ! persistent identifier
property_value: IAO:0000117 "https://orcid.org/0000-0002-5214-4466" xsd:string
property_value: IAO:0000117 "https://orcid.org/0000-0002-7702-4495" xsd:string
property_value: IAO:0000117 "https://orcid.org/0000-0003-2687-1982" xsd:string
property_value: IAO:0000118 "PURL" xsd:string

[Term]
id: T4FS:0000445
name: dublin core
def: "Widely used metadata element set, formally titled ISO 15836-1:2017, Information and documentation — The Dublin Core metadata element set — Part 1: Core elements." [] {IAO:0000119="RDMT. https://terms.codata.org/rdmt/dublin-core"}
is_a: T4FS:0000372 ! data stewardship technical concept
relationship: T4FS:0000563 T4FS:0000137 ! contributes to the implementation of I1. (meta)data use a formal, accessible, shared, and broadly applicable language for knowledge representation
property_value: IAO:0000117 "https://orcid.org/0000-0002-5214-4466" xsd:string
property_value: IAO:0000117 "https://orcid.org/0000-0002-7702-4495" xsd:string
property_value: IAO:0000117 "https://orcid.org/0000-0003-2687-1982" xsd:string

[Term]
id: T4FS:0000446
name: data stewardship guideline
property_value: IAO:0000117 "Yann Le Franc" xsd:string
created_by: ylefranc
creation_date: 2021-03-17T16:34:14.943152Z

[Term]
id: T4FS:0000447
name: fair principle
def: "The FAIR principles are guidelines to improve the Findability, Accessibility, Interoperability, and Reuse of digital assets. The principles emphasise machine-actionability (i.e., the capacity of computational systems to find, access, interoperate, and reuse data with none or minimal human intervention) because humans increasingly rely on computational support to deal with data as a result of the increase in volume, complexity, and creation speed of data. The principles refer to three types of entities: data (or any digital object), metadata (information about that digital object), and infrastructure." [] {IAO:0000119="https://www.go-fair.org/fair-principles/"}
is_a: T4FS:0000446 ! data stewardship guideline
property_value: IAO:0000117 "https://orcid.org/0000-0003-2687-1982" xsd:string
created_by: https://orcid.org/0000-0003-2687-1982
creation_date: 2020-10-02T14:56:15.031154Z

[Term]
id: T4FS:0000448
name: aptitudes for cloud computing environment management
def: "Bin for Aptitudes related to Cloud computing environment management." []
is_a: T4FS:0000479 ! cloud computing environment management
property_value: IAO:0000117 "leightonlc" xsd:string

[Term]
id: T4FS:0000449
name: repurposed data
def: "New datasets obtained by combining data appropriately from a variety of existing files, generating new data products that did not previously exist. Repurposed data result from data wrangling." [] {IAO:0000119="RDMT. https://terms.codata.org/rdmt/repurposed-data"}
is_a: T4FS:0000430 ! data
property_value: IAO:0000117 "https://orcid.org/0000-0002-5214-4466" xsd:string
property_value: IAO:0000117 "https://orcid.org/0000-0002-7702-4495" xsd:string
property_value: IAO:0000117 "https://orcid.org/0000-0003-2687-1982" xsd:string

[Term]
id: T4FS:0000450
name: document type definition
def: "Definition of the structure and the legal elements and attributes of an XML document." [] {IAO:0000119="RDMT. https://terms.codata.org/rdmt/document-type-definition"}
is_a: T4FS:0000372 ! data stewardship technical concept
relationship: T4FS:0000563 T4FS:0000137 ! contributes to the implementation of I1. (meta)data use a formal, accessible, shared, and broadly applicable language for knowledge representation
property_value: IAO:0000117 "https://orcid.org/0000-0002-5214-4466" xsd:string
property_value: IAO:0000117 "https://orcid.org/0000-0002-7702-4495" xsd:string
property_value: IAO:0000117 "https://orcid.org/0000-0003-2687-1982" xsd:string

[Term]
id: T4FS:0000452
name: I3. (meta)data include qualified references to other (meta)data
is_a: T4FS:0000014 ! interoperability of digital assets
property_value: IAO:0000117 "https://orcid.org/0000-0003-2687-1982" xsd:string

[Term]
id: T4FS:0000453
name: persistent identifier
def: "Long-lasting digital reference to an object that gives information about that object regardless of what happens to that object. Developed to address link rot, a persistent identifier can be resolved to provide an appropriate representation of an object whether that object changes its online location or goes offline." [] {IAO:0000119="RDMT. https://terms.codata.org/rdmt/persistent-identifier"}
is_a: T4FS:0000529 ! identifier
property_value: IAO:0000117 "https://orcid.org/0000-0002-5214-4466" xsd:string
property_value: IAO:0000117 "https://orcid.org/0000-0002-7702-4495" xsd:string
property_value: IAO:0000117 "https://orcid.org/0000-0003-2687-1982" xsd:string
property_value: IAO:0000118 "PID" xsd:string

[Term]
id: T4FS:0000454
name: scientist
def: "A person who is studying or has expert knowledge of one or more of the natural or physical sciences." [] {IAO:0000119="Definition from now-deprecated CASRAI Glossary term: scientist"}
is_a: T4FS:0000220 ! researcher
property_value: IAO:0000117 "https://orcid.org/0000-0002-5214-4466" xsd:string
property_value: IAO:0000117 "https://orcid.org/0000-0002-7702-4495" xsd:string
property_value: IAO:0000117 "https://orcid.org/0000-0003-2687-1982" xsd:string

[Term]
id: T4FS:0000455
name: integration
def: "1. The act of bringing together smaller components into a single system that functions as one. 2. In the context of information technology: The end result of a process that aims to stitch together different, often disparate, subsystems so that the data contained in each becomes part of a larger, more comprehensive system that, ideally, quickly and easily shares data when needed. This often requires that organizations build a customized architecture or structure of applications to combine new or existing hardware, software and other communications." [] {IAO:0000119="Definition from now-deprecated CASRAI Glossary term: integration"}
is_a: T4FS:0000012 ! data stewardship activity
property_value: IAO:0000117 "https://orcid.org/0000-0002-7702-4495" xsd:string
property_value: IAO:0000117 "https://orcid.org/0000-0003-2687-1982" xsd:string

[Term]
id: T4FS:0000456
name: knowledge of high performance computing management
def: "Bin for types of Knowledge related to High performance computing management." []
is_a: T4FS:0000308 ! high performance computing management
property_value: IAO:0000117 "leightonlc" xsd:string

[Term]
id: T4FS:0000457
name: fair mentoring
def: "The act of mentoring around FAIR data stewardship." [] {IAO:0000119="PMQ"}
is_a: T4FS:0000259 ! fair training
property_value: IAO:0000117 "https://orcid.org/0000-0002-7702-4495" xsd:string
property_value: IAO:0000117 "https://orcid.org/0000-0003-2687-1982" xsd:string
property_value: IAO:0000117 "Philippe Rocca-Serra" xsd:string
property_value: IAO:0000117 "Susanna Sansone" xsd:string

[Term]
id: T4FS:0000458
name: data governance
def: "Exercise of authority, control and shared decision making (planning, monitoring and enforcement) over the management of data assets. Overall management of the availability, usability, integrity, and security of the data employed in an organisation. A sound data governance program includes a governing body or council, a defined set of procedures, and a plan to execute those procedures." [] {IAO:0000119="RDMT. https://terms.codata.org/rdmt/data-governance"}
is_a: T4FS:0000472 ! governance
property_value: IAO:0000117 "https://orcid.org/0000-0002-5214-4466" xsd:string
property_value: IAO:0000117 "https://orcid.org/0000-0003-2687-1982" xsd:string

[Term]
id: T4FS:0000460
name: extensible resource identifier
def: "Scheme used for identification of resources (including people and organisations) and the sharing of data across domains, enterprises, and applications. XRI TC will define a Uniform Resource Identifier (URI) scheme and a corresponding Uniform Resource Namespace (URN)." [] {IAO:0000119="RDMT. https://terms.codata.org/rdmt/extensible-resource-identifier"}
is_a: T4FS:0000529 ! identifier
property_value: IAO:0000117 "https://orcid.org/0000-0002-5214-4466" xsd:string
property_value: IAO:0000117 "https://orcid.org/0000-0003-2687-1982" xsd:string

[Term]
id: T4FS:0000462
name: impact
def: "In the context of a researcher's activities, impact is the consequence of the research and new knowledge on the advancement of the specialty. Science-based policies, regulations, services and technology transfers are some examples of ways target results can be achieved and impact demonstrated." [] {IAO:0000119="Definition from now-deprecated CASRAI Glossary term: impact"}
is_a: T4FS:0000372 ! data stewardship technical concept
property_value: IAO:0000117 "https://orcid.org/0000-0002-5214-4466" xsd:string
property_value: IAO:0000117 "https://orcid.org/0000-0003-2687-1982" xsd:string

[Term]
id: T4FS:0000463
name: access control list
def: "A list used to grant permission matched against credentials." [] {IAO:0000119="Definition from now-deprecated CASRAI Glossary term: access-control-list."}
is_a: T4FS:0000283 ! access
property_value: IAO:0000117 "https://orcid.org/0000-0002-5214-4466" xsd:string
property_value: IAO:0000117 "https://orcid.org/0000-0003-2687-1982" xsd:string

[Term]
id: T4FS:0000464
name: understand data ownership and access policies
def: "Learn about data copyright laws, licennsing and other legal aspects of data access. Understand the application of those laws at the project level." []
is_a: T4FS:0000469 ! access control and management
property_value: IAO:0000117 "Celia van Gelder" xsd:string
property_value: IAO:0000117 "Mateusz Kuzak" xsd:string
property_value: IAO:0000117 "Yan Wang" xsd:string

[Term]
id: T4FS:0000465
name: meeting/conference organisation
def: "Meeting/conference organisation is a project management activity that encompasses all of the steps required to run a meeting or conference." []
is_a: T4FS:0000320 ! project management activities
property_value: IAO:0000117 "https://orcid.org/0000-0002-7702-4495" xsd:string
property_value: IAO:0000117 "https://orcid.org/0000-0003-2687-1982" xsd:string
property_value: IAO:0000117 "Philippe Rocca-Serra" xsd:string
property_value: IAO:0000117 "Susanna Sansone" xsd:string

[Term]
id: T4FS:0000466
name: service level management
def: "It can be considered as a negotiated agreement between the customer and vendor which are acceptable to both parties with respect to costs and expectations in order to support the business process." [] {IAO:0000119="https://www.techopedia.com/definition/13848/service-level-management-slm [LLC]"}
is_a: T4FS:0000353 ! resource management
property_value: IAO:0000117 "Kristina Hettne" xsd:string
property_value: IAO:0000117 "Leighton Christiansen" xsd:string
property_value: IAO:0000117 "Simon Hodson" xsd:string
property_value: IAO:0000117 "Victoria Dominguez Del Angel" xsd:string
property_value: IAO:0000118 "SLM" xsd:string

[Term]
id: T4FS:0000467
name: national standard
def: "From an official perspective, a national standard is adopted by a national standards body (e.g., Standards Council of Canada, American National Standards Institute, British Standards Institution) and made available to the public. Practically speaking, however, a national standard is any standard that is widely used and recognized within a country. In this context, even government standards, such as those issued by the Occupational Safety and Health Administration (OSHA), can be considered national standards." [] {IAO:0000119="Definition from now-deprecated CASRAI Glossary term: national-standard"}
is_a: T4FS:0000372 ! data stewardship technical concept
relationship: T4FS:0000563 T4FS:0000137 ! contributes to the implementation of I1. (meta)data use a formal, accessible, shared, and broadly applicable language for knowledge representation
property_value: IAO:0000117 "https://orcid.org/0000-0002-5214-4466" xsd:string
property_value: IAO:0000117 "https://orcid.org/0000-0002-7702-4495" xsd:string
property_value: IAO:0000117 "https://orcid.org/0000-0003-2687-1982" xsd:string

[Term]
id: T4FS:0000468
name: open government
def: "A governing culture that holds that the public has the right to access the documents and proceedings of government to allow for greater openness, accountability, and engagement." [] {IAO:0000119="Definition from now-deprecated CASRAI Glossary term: open-government"}
is_a: T4FS:0000372 ! data stewardship technical concept
property_value: IAO:0000117 "https://orcid.org/0000-0002-5214-4466" xsd:string
property_value: IAO:0000117 "https://orcid.org/0000-0002-7702-4495" xsd:string
property_value: IAO:0000117 "https://orcid.org/0000-0003-2687-1982" xsd:string

[Term]
id: T4FS:0000469
name: access control and management
is_a: T4FS:0000106 ! publish data

[Term]
id: T4FS:0000470
name: storage security management
def: "Manage the assessment, implementation and monitoring of secure storage protocols." []
is_a: T4FS:0000107 ! information security
property_value: IAO:0000117 "Angus Whyte" xsd:string
property_value: IAO:0000117 "Celia van Gelder" xsd:string
property_value: IAO:0000117 "Mateusz Kuzak" xsd:string
property_value: IAO:0000117 "Yan Wang" xsd:string

[Term]
id: T4FS:0000472
name: governance
def: "1. Exercising authority to provide direction and to undertake, coordinate, and regulate activities in support of achieving this direction and desired outcomes. Governance can be thought of as the role of an organization's board of directors or its equivalent that is focused on defining that organization's purpose and the development of the strategies, objectives, values, and policies that frame how that purpose will be pursued. It includes the development of such things as mission statements, statements of organizational objectives and values, logic models, organizational performance metrics, risk management frameworks, policies and guidelines for financial and operational matters, stakeholder relations, etc." [] {IAO:0000119="Definition from now-deprecated CASRAI Glossary term: governance"}
is_a: T4FS:0000012 ! data stewardship activity
property_value: IAO:0000117 "https://orcid.org/0000-0002-5214-4466" xsd:string
property_value: IAO:0000117 "https://orcid.org/0000-0003-2687-1982" xsd:string

[Term]
id: T4FS:0000474
name: open archives initiative protocol for metadata harvesting
def: "Low-barrier mechanism for repository interoperability. Data Providers are repositories that expose structured metadata via OAI-PMH. Service Providers then make OAI-PMH service requests to harvest that metadata. OAI-PMH is a set of six verbs or services that are invoked within HTTP." [] {IAO:0000119="RDMT. https://terms.codata.org/rdmt/open-archives-initiative-protocol-for-metadata-harvesting"}
is_a: T4FS:0000427 ! machine access via api
property_value: IAO:0000117 "https://orcid.org/0000-0002-5214-4466" xsd:string
property_value: IAO:0000117 "https://orcid.org/0000-0003-2687-1982" xsd:string

[Term]
id: T4FS:0000475
name: computer code
def: "A series of computer instructions written in some human readable computer language, usually stored in a text file." [] {IAO:0000119="Definition from now-deprecated CASRAI Glossary term: computer-code"}
is_a: T4FS:0000372 ! data stewardship technical concept
property_value: IAO:0000117 "https://orcid.org/0000-0002-5214-4466" xsd:string
property_value: IAO:0000117 "https://orcid.org/0000-0003-2687-1982" xsd:string

[Term]
id: T4FS:0000476
name: syntactic interoperability
def: "Defines the structure or format of data exchange and is achieved through tools such as XML or SQL standards." [] {IAO:0000119="RDMT. https://terms.codata.org/rdmt/syntactic-interoperability"}
is_a: T4FS:0000372 ! data stewardship technical concept
property_value: IAO:0000117 "https://orcid.org/0000-0002-5214-4466" xsd:string
property_value: IAO:0000117 "https://orcid.org/0000-0002-7702-4495" xsd:string
property_value: IAO:0000117 "https://orcid.org/0000-0003-2687-1982" xsd:string

[Term]
id: T4FS:0000477
name: aptitudes for preservation costs management
def: "Bin for Aptitudes related to Preservation costs management." []
is_a: T4FS:0000104 ! preservation costs management
property_value: IAO:0000117 "leightonlc" xsd:string

[Term]
id: T4FS:0000478
name: accessibility of digital assets
is_a: T4FS:0000447 ! fair principle
property_value: IAO:0000117 "https://orcid.org/0000-0003-2687-1982" xsd:string

[Term]
id: T4FS:0000479
name: cloud computing environment management
def: "The activity of bringing computer system resources, especially data storage and computing power on demand via Internet." [] {IAO:0000119="(modified from wikipedia) [VDA]"}
is_a: T4FS:0000353 ! resource management
property_value: IAO:0000117 "Kristina Hettne" xsd:string
property_value: IAO:0000117 "Simon Hodson" xsd:string
property_value: IAO:0000117 "Victoria Dominguez Del Angel" xsd:string

[Term]
id: T4FS:0000480
name: corpus
def: "Set of documents that has a scientific meaning. A corpus can be produced by an individual researcher's activity (including its archival materials) or from a laboratory's research, a field campaign, a survey, or any other discrete research activity." [] {IAO:0000119="RDMT. https://terms.codata.org/rdmt/corpus"}
is_a: T4FS:0000372 ! data stewardship technical concept
property_value: IAO:0000117 "https://orcid.org/0000-0002-5214-4466" xsd:string
property_value: IAO:0000117 "https://orcid.org/0000-0003-2687-1982" xsd:string

[Term]
id: T4FS:0000481
name: the use of fair and open research tools or services
def: "Understand how to use FAIR and open research tools and services." []
is_a: T4FS:0000508 ! using fair and open research tools or services
property_value: IAO:0000117 "Hugh Shanahan" xsd:string

[Term]
id: T4FS:0000482
name: data sharing
def: "Practice of making data available for checking, reproducing or reusing. The mechanisms available for achieving this are: making data available on request, as supplementary information to journal articles, or as published datasets in data repositories." [] {IAO:0000119="RDMT. https://terms.codata.org/rdmt/data-sharing"}
is_a: T4FS:0000021 ! exposing data
property_value: IAO:0000117 "https://orcid.org/0000-0002-5214-4466" xsd:string
property_value: IAO:0000117 "https://orcid.org/0000-0002-7702-4495" xsd:string
property_value: IAO:0000117 "https://orcid.org/0000-0003-2687-1982" xsd:string
property_value: IAO:0000118 "Data dissemination" xsd:string
property_value: IAO:0000118 "Data posting" xsd:string

[Term]
id: T4FS:0000483
name: appreciate importance of crediting research contributions
def: "Understand how the rewards for effort depend on crediting the contributions of researchers and professional groups towards making FAIR outputs." []
is_a: T4FS:0000525 ! research integrity, attribution, impact awareness
property_value: IAO:0000117 "Angus Whyte" xsd:string
property_value: IAO:0000117 "Celia van Gelder" xsd:string
property_value: IAO:0000117 "Mateusz Kuzak" xsd:string
property_value: IAO:0000117 "Yan Wang" xsd:string

[Term]
id: T4FS:0000485
name: reference resolution
def: "The process of resolving a reference to useful information by using a globally available system." [] {IAO:0000119="Definition from now-deprecated CASRAI Glossary term: reference-resolution"}
is_a: T4FS:0000372 ! data stewardship technical concept
property_value: IAO:0000117 "https://orcid.org/0000-0002-5214-4466" xsd:string
property_value: IAO:0000117 "https://orcid.org/0000-0002-7702-4495" xsd:string
property_value: IAO:0000117 "https://orcid.org/0000-0003-2687-1982" xsd:string

[Term]
id: T4FS:0000486
name: research manager
def: "The person who manages or coordinates resources, personnel, facilities, and operating funds-allocations in an organization conducting research, development and analysis (RDA) in the natural and physical sciences. A research manager determines the nature, priority objectives and the resources committed to their achievement within and across the organizations, and evaluates program outputs in relation to organizational objectives and policies. A research manager provides scientific advice on the direction, conduct and management of these programs. A research manager does not personally conduct research development and analysis (RDA), control and coordinate projects, or control and coordinate contracted RDA." [] {IAO:0000119="Definition from now-deprecated CASRAI Glossary term: research-manager"}
is_a: T4FS:0000220 ! researcher
property_value: IAO:0000117 "https://orcid.org/0000-0002-5214-4466" xsd:string
property_value: IAO:0000117 "https://orcid.org/0000-0002-7702-4495" xsd:string
property_value: IAO:0000117 "https://orcid.org/0000-0003-2687-1982" xsd:string

[Term]
id: T4FS:0000487
name: data integration
def: "Combining diverse datasets from disparate sources into one unified dataset or database. Data are accessed and extracted, moved, validated, cleaned, transformed and loaded." [] {IAO:0000119="RDMT. https://terms.codata.org/rdmt/data-integration"}
is_a: T4FS:0000036 ! curation
property_value: IAO:0000117 "https://orcid.org/0000-0002-5214-4466" xsd:string
property_value: IAO:0000117 "https://orcid.org/0000-0002-7702-4495" xsd:string
property_value: IAO:0000117 "https://orcid.org/0000-0003-2687-1982" xsd:string

[Term]
id: T4FS:0000488
name: standard operating procedure
name: Standard operating procedure for the collection of harmonised or integrated data
def: "Written methods, instructions, and tools that, when applied in different data collection contexts produce data that are ready to be harmonised or integrated without further manipulation." [] {IAO:0000119="RDMT. https://terms.codata.org/rdmt/standard-operating-procedure-harmonised-integrated-data"}
comment: AL, LM 22.1.25: Refined the definition of this term to apply specifically to data stewardship tasks, and to align with RDMT.
is_a: T4FS:0000372 ! data stewardship technical concept
property_value: IAO:0000117 "https://orcid.org/0000-0002-5214-4466" xsd:string
property_value: IAO:0000117 "https://orcid.org/0000-0002-7702-4495" xsd:string
property_value: IAO:0000117 "https://orcid.org/0000-0003-2687-1982" xsd:string

[Term]
id: T4FS:0000489
name: repository
def: "Physical or digital storage location that can house, preserve, manage, and provide access to many types of digital and physical materials in a variety of formats. Materials in online repositories are curated to enable search, discovery, and reuse. There must be sufficient control for the physical and digital material to be authentic, reliable, accessible and usable on a continuing basis." [] {IAO:0000119="RDMT. https://terms.codata.org/rdmt/repository"}
is_a: T4FS:0000372 ! data stewardship technical concept
property_value: IAO:0000117 "https://orcid.org/0000-0002-5214-4466" xsd:string
property_value: IAO:0000117 "https://orcid.org/0000-0002-7702-4495" xsd:string
property_value: IAO:0000117 "https://orcid.org/0000-0003-2687-1982" xsd:string

[Term]
id: T4FS:0000490
name: knowledge of theories underlying fair implementation
def: "Understand the concepts underpinning FAIR criteria." []
is_a: T4FS:0000259 ! fair training
property_value: IAO:0000117 "Angus Whyte" xsd:string

[Term]
id: T4FS:0000491
name: document in lay terms
def: "Know the purpose of the public use, choose the proper subjects for the audience and describe the project work for the purpose/audience chosen." []
is_a: T4FS:0000106 ! publish data
property_value: IAO:0000117 "Celia van Gelder" xsd:string
property_value: IAO:0000117 "Mateusz Kuzak" xsd:string
property_value: IAO:0000117 "Yan Wang" xsd:string

[Term]
id: T4FS:0000492
name: understanding persistent identifiers
is_a: T4FS:0000021 ! exposing data
created_by: https://orcid.org/0000-0003-2687-1982
creation_date: 2020-10-02T14:54:27.168274Z

[Term]
id: T4FS:0000493
name: data upload database
def: "Collection of interrelated data often with controlled redundancy, organised according to a scheme to serve one or more applications; the data are stored so that they can be used by several programs without concern for data structures or organisation." [] {IAO:0000119="RDMT. https://terms.codata.org/rdmt/data-upload-database"}
is_a: T4FS:0000215 ! data store
property_value: IAO:0000117 "https://orcid.org/0000-0002-5214-4466" xsd:string
property_value: IAO:0000117 "https://orcid.org/0000-0003-2687-1982" xsd:string

[Term]
id: T4FS:0000494
name: uniform resource identifier
def: "A string of characters used to identify or name a resource on the Internet. Such identification enables interaction with representations of the resource over a network, typically the World Wide Web, using specific protocols. MIT data management and publishing" [] {IAO:0000119="Definition from now-deprecated CASRAI Glossary term: uniform-resource-identifier"}
is_a: T4FS:0000529 ! identifier
property_value: IAO:0000117 "https://orcid.org/0000-0002-5214-4466" xsd:string
property_value: IAO:0000117 "https://orcid.org/0000-0002-7702-4495" xsd:string
property_value: IAO:0000117 "https://orcid.org/0000-0003-2687-1982" xsd:string

[Term]
id: T4FS:0000495
name: how to find fair research data tools/services (catalogues)
def: "Know how to search for and identify FAIR services or tools that fit project needs." []
is_a: T4FS:0000481 ! the use of fair and open research tools or services
property_value: IAO:0000117 "Angus Whyte" xsd:string

[Term]
id: T4FS:0000496
name: data reference model
def: "A framework whose primary purpose is to enable information sharing and reuse via the standard description and discovery of common data and the promotion of uniform data management practices." [] {IAO:0000119="Definition from now-deprecated CASRAI Glossary: data-reference-model"}
is_a: T4FS:0000379 ! data model
property_value: IAO:0000117 "https://orcid.org/0000-0002-5214-4466" xsd:string
property_value: IAO:0000117 "https://orcid.org/0000-0003-2687-1982" xsd:string

[Term]
id: T4FS:0000498
name: peer review
def: "A process by which a scholarly work (such as a paper or a research proposal) is checked by a group of experts in the same field to make sure it meets the necessary standards before it is published or accepted." [] {IAO:0000119="Definition from now-deprecated CASRAI Glossary term: peer-review"}
is_a: T4FS:0000126 ! assessment
property_value: IAO:0000117 "https://orcid.org/0000-0002-5214-4466" xsd:string
property_value: IAO:0000117 "https://orcid.org/0000-0002-7702-4495" xsd:string
property_value: IAO:0000117 "https://orcid.org/0000-0003-2687-1982" xsd:string

[Term]
id: T4FS:0000499
name: knowledge of provenance information management
def: "Bin for types of Knowledge related to Provenance information management." []
is_a: T4FS:0000368 ! provenance information management
created_by: leightonlc
creation_date: 2019-10-17T15:17:02.313897Z

[Term]
id: T4FS:0000500
name: record
def: "(noun) Sometimes called a row, a group of fields (sometimes called columns) within a table that are relevant to a specific entity. Multiple records are contained in a file or dataset." [] {IAO:0000119="RDMT. https://terms.codata.org/rdmt/record"}
is_a: T4FS:0000372 ! data stewardship technical concept
property_value: IAO:0000117 "https://orcid.org/0000-0002-5214-4466" xsd:string
property_value: IAO:0000117 "https://orcid.org/0000-0002-7702-4495" xsd:string
property_value: IAO:0000117 "https://orcid.org/0000-0003-2687-1982" xsd:string
property_value: IAO:0000118 "Data record" xsd:string

[Term]
id: T4FS:0000501
name: de-anonymization
def: "Reverse engineering process in which de-identified data are cross-referenced with other data sources to re-identify the personally identifiable information. This could occur if a de-identification process had not been not successfully performed, or had not been undertaken in the first place." [] {IAO:0000119="RDMT. https://terms.codata.org/rdmt/de-anonymisation"}
is_a: T4FS:0000107 ! information security
property_value: IAO:0000117 "https://orcid.org/0000-0002-5214-4466" xsd:string
property_value: IAO:0000117 "https://orcid.org/0000-0002-7702-4495" xsd:string
property_value: IAO:0000117 "https://orcid.org/0000-0003-2687-1982" xsd:string

[Term]
id: T4FS:0000502
name: application of fair tools and services
is_a: T4FS:0000508 ! using fair and open research tools or services
created_by: HughShanahan
creation_date: 2019-10-18T08:45:02.980527Z

[Term]
id: T4FS:0000503
name: mandatory standard
def: "Requires compliance because of a government statute or regulation, an organization internal policy, or contractual requirement. Failure to comply with a mandatory standard usually carries a sanction, such as civil or criminal penalties, or loss of employment." [] {IAO:0000119="Definition from now-deprecated CASRAI Glossary term: mandatory-standard"}
is_a: T4FS:0000372 ! data stewardship technical concept
relationship: T4FS:0000563 T4FS:0000137 ! contributes to the implementation of I1. (meta)data use a formal, accessible, shared, and broadly applicable language for knowledge representation
property_value: IAO:0000117 "https://orcid.org/0000-0002-5214-4466" xsd:string
property_value: IAO:0000117 "https://orcid.org/0000-0002-7702-4495" xsd:string
property_value: IAO:0000117 "https://orcid.org/0000-0003-2687-1982" xsd:string

[Term]
id: T4FS:0000504
name: data driven decision management
def: "Approach to governance that values decisions that can be backed up with data that can be verified. The success of the data-driven approach is reliant upon the quality of the data gathered and the effectiveness of its analysis and interpretation. Errors can creep into data analytics processes at any stage of the endeavour and serious issues can result when they do." [] {IAO:0000119="RDMT. https://terms.codata.org/rdmt/data-driven-decision-management"}
is_a: T4FS:0000472 ! governance
property_value: IAO:0000117 "https://orcid.org/0000-0002-5214-4466" xsd:string
property_value: IAO:0000117 "https://orcid.org/0000-0003-2687-1982" xsd:string
property_value: IAO:0000118 "DDDM" xsd:string

[Term]
id: T4FS:0000505
name: golden record
def: "Single, well-defined version of all the data entities in an organisational ecosystem. Encompasses all the data in every system of record within a particular organisation. A well-maintained, current golden record should be a fundamental element of the master data management policy for every enterprise. The word “golden” is sometimes used in information technology to express the importance of some type of source. In the context of virtualization, for example, a golden image is a template for a virtual machine, virtual desktop, servers, or hard disk drive." [] {IAO:0000119="RDMT. https://terms.codata.org/rdmt/golden-record"}
is_a: T4FS:0000372 ! data stewardship technical concept
property_value: IAO:0000117 "https://orcid.org/0000-0002-5214-4466" xsd:string
property_value: IAO:0000117 "https://orcid.org/0000-0002-7702-4495" xsd:string
property_value: IAO:0000117 "https://orcid.org/0000-0003-2687-1982" xsd:string

[Term]
id: T4FS:0000507
name: data quality
def: "Reliability and application efficiency of data. Perception or assessment of a dataset's fitness to serve its purpose in a given context. Aspects of data quality include: Accuracy, Completeness, Update status, Relevance, Consistency across data sources, Reliability, Appropriate presentation, Accessibility. Data quality is affected by the way data are entered, stored and managed. Maintaining data quality requires going through the data periodically and scrubbing it. Typically this involves updating, standardising, and de-duplicating records to create a single view of the data, even if it is stored in multiple disparate systems." [] {IAO:0000119="RDMT. https://terms.codata.org/rdmt/data-quality"}
is_a: T4FS:0000372 ! data stewardship technical concept
property_value: IAO:0000117 "https://orcid.org/0000-0002-5214-4466" xsd:string
property_value: IAO:0000117 "https://orcid.org/0000-0003-2687-1982" xsd:string

[Term]
id: T4FS:0000508
name: using fair and open research tools or services
is_a: T4FS:0000259 ! fair training
created_by: HughShanahan
creation_date: 2019-10-18T08:38:59.038306Z

[Term]
id: T4FS:0000510
name: webinar
is_a: T4FS:0000519 ! learning medium
property_value: IAO:0000117 "https://orcid.org/0000-0003-2687-1982" xsd:string
created_by: https://orcid.org/0000-0003-2687-1982
creation_date: 2020-10-01T20:53:15.691824Z

[Term]
id: T4FS:0000511
name: digital data
def: "Data in the form of digital materials." [] {IAO:0000119="RDMT. https://terms.codata.org/rdmt/digital-data"}
is_a: T4FS:0000430 ! data
property_value: IAO:0000117 "https://orcid.org/0000-0002-5214-4466" xsd:string
property_value: IAO:0000117 "https://orcid.org/0000-0002-7702-4495" xsd:string
property_value: IAO:0000117 "https://orcid.org/0000-0003-2687-1982" xsd:string

[Term]
id: T4FS:0000512
name: F1. (meta)data are assigned a globally unique and persistent identifier
is_a: T4FS:0000248 ! findability of digital assets
property_value: IAO:0000117 "https://orcid.org/0000-0003-2687-1982" xsd:string

[Term]
id: T4FS:0000514
name: strategic/long-term planning
def: "An organization's process of defining its strategy or direction in the context of FAIR project management activities, both in the context of current knowledge and unknown factors in the future." [] {IAO:0000119="AL, and https://en.wikipedia.org/wiki/Strategic_planning [17.10.19]"}
is_a: T4FS:0000320 ! project management activities
property_value: IAO:0000117 "https://orcid.org/0000-0002-7702-4495" xsd:string
property_value: IAO:0000117 "https://orcid.org/0000-0003-2687-1982" xsd:string
property_value: IAO:0000117 "Philippe Rocca-Serra" xsd:string
property_value: IAO:0000117 "Susanna Sansone" xsd:string

[Term]
id: T4FS:0000515
name: data hygiene
def: "Collective processes conducted to ensure the cleanliness of data. Data are considered clean when they are relatively error-free." [] {IAO:0000119="RDMT. https://terms.codata.org/rdmt/data-hygiene"}
is_a: T4FS:0000036 ! curation
property_value: IAO:0000117 "https://orcid.org/0000-0002-5214-4466" xsd:string
property_value: IAO:0000117 "https://orcid.org/0000-0003-2687-1982" xsd:string

[Term]
id: T4FS:0000516
name: data profiling
def: "Statistical analysis and assessment of the quality of data values within a dataset for consistency, uniqueness and logic. The data profiling process cannot identify inaccurate data; it can only identify rule violations and anomalies. The insight gained by data profiling can be used to determine how difficult it will be to use existing data for other purposes. It can also be used to provide metrics to assess data quality and help determine whether or not metadata accurately describes the source data. Profiling tools evaluate the actual content, structure and quality of the data by exploring relationships that exist between value collections both within and across datasets." [] {IAO:0000119="RDMT. https://terms.codata.org/rdmt/data-profiling"}
is_a: T4FS:0000352 ! data analysis
property_value: IAO:0000117 "https://orcid.org/0000-0002-5214-4466" xsd:string
property_value: IAO:0000117 "https://orcid.org/0000-0003-2687-1982" xsd:string

[Term]
id: T4FS:0000517
name: metadata record
def: "Set of metadata elements and their values that describe an object. Metadata elements in the record may derive from a metadata profile or standard, and may include different types of metadata (descriptive, administrative, etc.). A metadata record is typically stored within a metadata catalogue or repository." [] {IAO:0000119="RDMT. https://terms.codata.org/rdmt/metadata-record"}
is_a: T4FS:0000096 ! metadata catalogue
property_value: IAO:0000117 "https://orcid.org/0000-0002-5214-4466" xsd:string
property_value: IAO:0000117 "https://orcid.org/0000-0002-7702-4495" xsd:string
property_value: IAO:0000117 "https://orcid.org/0000-0003-2687-1982" xsd:string

[Term]
id: T4FS:0000518
name: research data
def: "Data that are used as primary sources to support technical or scientific enquiry, research, scholarship, or artistic activity, and that are used as evidence in the research process and/or are commonly accepted in the research community as necessary to validate research findings and results. All other digital and non-digital content have the potential of becoming research data. Research data may be experimental data, observational data, operational data, third party data, public sector data, monitoring data, processed data, or repurposed data." [] {IAO:0000119="RDMT. https://terms.codata.org/rdmt/research-data"}
is_a: T4FS:0000430 ! data
property_value: IAO:0000117 "https://orcid.org/0000-0002-5214-4466" xsd:string
property_value: IAO:0000117 "https://orcid.org/0000-0002-7702-4495" xsd:string
property_value: IAO:0000117 "https://orcid.org/0000-0003-2687-1982" xsd:string

[Term]
id: T4FS:0000519
name: learning medium
def: "The medium through which learning has been provided. For example, through a course, slides, video presentation, online documentation, wiki pages or others." []
relationship: T4FS:0000554 T4FS:0000012 ! confers competency about data stewardship activity
relationship: T4FS:0000555 T4FS:0000372 ! confers knowledge about data stewardship technical concept
relationship: T4FS:0000556 T4FS:0000548 ! requires/improves personal attribute data stewardship soft skill
relationship: T4FS:0000557 T4FS:0000372 ! confers practical skill about data stewardship technical concept
relationship: T4FS:0000560 T4FS:0000446 ! supports implementation of data stewardship guideline
relationship: T4FS:0000576 T4FS:0000012 ! requires competency about data stewardship activity
relationship: T4FS:0000577 T4FS:0000372 ! requires knowledge about data stewardship technical concept
relationship: T4FS:0000578 T4FS:0000372 ! requires practical skill about data stewardship technical concept
property_value: IAO:0000117 "https://orcid.org/0000-0002-7702-4495" xsd:string
property_value: IAO:0000117 "https://orcid.org/0000-0003-2687-1982" xsd:string
created_by: https://orcid.org/0000-0003-2687-1982
creation_date: 2020-09-22T13:19:57.012225Z

[Term]
id: T4FS:0000520
name: data manager
is_a: T4FS:0000415 ! manager

[Term]
id: T4FS:0000521
name: electronic health record
def: "Compilation of core electronic health data submitted by various healthcare providers and organisations, accessible by numerous authorised parties from a number of points of care, possibly even from different jurisdictions. Electronic health records typically include: contact information, information about visits to health care professionals, allergies, insurance information, family history, immunisation status, information about any conditions or diseases, a list of medications, records of hospitalisation, information about any surgeries or procedures performed." [] {IAO:0000119="RDMT. https://terms.codata.org/rdmt/electronic-health-record"}
is_a: T4FS:0000372 ! data stewardship technical concept
property_value: IAO:0000117 "https://orcid.org/0000-0002-5214-4466" xsd:string
property_value: IAO:0000117 "https://orcid.org/0000-0002-7702-4495" xsd:string
property_value: IAO:0000117 "https://orcid.org/0000-0003-2687-1982" xsd:string
property_value: IAO:0000118 "Digital medical record" xsd:string

[Term]
id: T4FS:0000522
name: data scaling
def: "Techniques used to deal with parameters having different units and scales." [] {IAO:0000119="RDMT. https://terms.codata.org/rdmt/data-scaling"}
is_a: T4FS:0000352 ! data analysis
property_value: IAO:0000117 "https://orcid.org/0000-0002-5214-4466" xsd:string
property_value: IAO:0000117 "https://orcid.org/0000-0002-7702-4495" xsd:string
property_value: IAO:0000117 "https://orcid.org/0000-0003-2687-1982" xsd:string
property_value: IAO:0000118 "Data rescaling" xsd:string

[Term]
id: T4FS:0000523
name: access controls
def: "Definitions of the access relationships between the following metadata: data object name, a user name (or user group, or user role), and access permission(s). The information can be stored as metadata information associated with each data object. The information can be generated dynamically by applying the access controls of the collection that organises the data objects (if a collection sticky bit is turned on)." [] {IAO:0000119="RDMT. https://terms.codata.org/rdmt/access-controls"}
is_a: T4FS:0000283 ! access
property_value: IAO:0000117 "https://orcid.org/0000-0002-5214-4466" xsd:string
property_value: IAO:0000117 "https://orcid.org/0000-0003-2687-1982" xsd:string

[Term]
id: T4FS:0000524
name: privacy governance
def: "Monitoring the risk to privacy posed by data requests from researchers, and the practices of data custodians in providing data (information governance) to ensure that confidentiality is protected. Such governance requires specialised knowledge of technology, law, and statistical methods." [] {IAO:0000119="RDMT. https://terms.codata.org/rdmt/privacy-governance"}
is_a: T4FS:0000472 ! governance
property_value: IAO:0000117 "https://orcid.org/0000-0002-5214-4466" xsd:string
property_value: IAO:0000117 "https://orcid.org/0000-0002-7702-4495" xsd:string
property_value: IAO:0000117 "https://orcid.org/0000-0003-2687-1982" xsd:string

[Term]
id: T4FS:0000525
name: research integrity, attribution, impact awareness
is_a: T4FS:0000126 ! assessment
property_value: IAO:0000117 "Angus Whyte" xsd:string
property_value: IAO:0000117 "Celia van Gelder" xsd:string
property_value: IAO:0000117 "Mateusz Kuzak" xsd:string
property_value: IAO:0000117 "Yan Wang" xsd:string

[Term]
id: T4FS:0000526
name: knowledge of cloud computing environment management
def: "Bin for types of Knowledge related to Cloud computing environment management." []
is_a: T4FS:0000479 ! cloud computing environment management
property_value: IAO:0000117 "leightonlc" xsd:string

[Term]
id: T4FS:0000527
name: metadata
def: "Data about data. It is data (or information) that defines and describes the characteristics of other data. It is used to improve the understanding and use of the data." [] {IAO:0000119="RDMT. https://terms.codata.org/rdmt/metadata"}
is_a: T4FS:0000372 ! data stewardship technical concept
relationship: T4FS:0000563 T4FS:0000199 ! contributes to the implementation of F2. data are described with rich metadata
property_value: IAO:0000117 "https://orcid.org/0000-0002-5214-4466" xsd:string
property_value: IAO:0000117 "https://orcid.org/0000-0002-7702-4495" xsd:string
property_value: IAO:0000117 "https://orcid.org/0000-0003-2687-1982" xsd:string
property_value: IAO:0000118 "Data documentation" xsd:string

[Term]
id: T4FS:0000528
name: comma separated values
def: "Values in a table presented as a series of ASCII text lines organised so that each column value is separated by a comma from the next column’s value and each row starts a new line. Along with pipe- and tab-separated values, comma-separated values are a specific example of a record-oriented data structure (usually of fixed dimension) with fields separated by an agreed delimiter." [] {IAO:0000119="RDMT. https://terms.codata.org/rdmt/comma-separated-values"}
comment: Maybe remove as shouldn't have formats here.
is_a: T4FS:0000372 ! data stewardship technical concept
relationship: T4FS:0000563 T4FS:0000137 ! contributes to the implementation of I1. (meta)data use a formal, accessible, shared, and broadly applicable language for knowledge representation
property_value: IAO:0000117 "https://orcid.org/0000-0002-5214-4466" xsd:string
property_value: IAO:0000117 "https://orcid.org/0000-0003-2687-1982" xsd:string
property_value: IAO:0000118 "CSV" xsd:string

[Term]
id: T4FS:0000529
name: identifier
is_a: T4FS:0000372 ! data stewardship technical concept
relationship: T4FS:0000563 T4FS:0000512 ! contributes to the implementation of F1. (meta)data are assigned a globally unique and persistent identifier
property_value: IAO:0000117 "https://orcid.org/0000-0003-2687-1982" xsd:string

[Term]
id: T4FS:0000530
name: project team member
def: "Responsible for executing tasks and producing deliverables as outlined in the Project Plan and directed by the Project Manager, at whatever level of effort or participation has been defined for them." [] {IAO:0000119="Definition from now-deprecated CASRAI Glossary term: project-team-member"}
relationship: T4FS:0000558 T4FS:0000012 ! has/wants competency in data stewardship activity
relationship: T4FS:0000559 T4FS:0000372 ! has/wants knowledge about data stewardship technical concept
relationship: T4FS:0000559 T4FS:0000446 ! has/wants knowledge about data stewardship guideline
relationship: T4FS:0000561 T4FS:0000372 ! has/wants practical skill about data stewardship technical concept
relationship: T4FS:0000562 T4FS:0000548 ! has aptitude for data stewardship soft skill
property_value: IAO:0000117 "https://orcid.org/0000-0002-5214-4466" xsd:string
property_value: IAO:0000117 "https://orcid.org/0000-0002-7702-4495" xsd:string
property_value: IAO:0000117 "https://orcid.org/0000-0003-2687-1982" xsd:string

[Term]
id: T4FS:0000531
name: descriptive metadata
def: "Metadata that describe a dataset or resource in such a way that people can discover and identify it. Contains information that aids with findability such as information (metadata elements) on the creator(s), affiliation(s), title, abstract, keywords, persistent identifier, related publications, etc." [] {IAO:0000119="RDMT. https://terms.codata.org/rdmt/descriptive-metadata"}
is_a: T4FS:0000527 ! metadata
property_value: IAO:0000117 "https://orcid.org/0000-0002-5214-4466" xsd:string
property_value: IAO:0000117 "https://orcid.org/0000-0002-7702-4495" xsd:string
property_value: IAO:0000117 "https://orcid.org/0000-0003-2687-1982" xsd:string
property_value: IAO:0000233 "https://github.com/terms4fairskills/FAIRterminology/issues/13" xsd:string

[Term]
id: T4FS:0000532
name: github repository
is_a: T4FS:0000519 ! learning medium
property_value: IAO:0000117 "https://orcid.org/0000-0003-2687-1982" xsd:string
created_by: https://orcid.org/0000-0003-2687-1982
creation_date: 2020-10-01T21:03:55.425579Z

[Term]
id: T4FS:0000533
name: data mining
def: "Analysing multivariate datasets using pattern recognition or other knowledge discovery techniques to identify potentially unknown and potentially meaningful data content, relationships, classification or trends. Data mining parameters include: Association (looking for patterns where one event is connected to another event); Sequence or path analysis (looking for patterns where one event leads to another later event); Classification (looking for new patterns); Clustering (finding and visually documenting groups of facts not previously known); Forecasting, or predictive analytics (discovering patterns in data that can lead to reasonable predictions about the future." [] {IAO:0000119="RDMT. https://terms.codata.org/rdmt/data-mining"}
is_a: T4FS:0000352 ! data analysis
property_value: IAO:0000117 "https://orcid.org/0000-0002-5214-4466" xsd:string
property_value: IAO:0000117 "https://orcid.org/0000-0003-2687-1982" xsd:string

[Term]
id: T4FS:0000534
name: data archiving
is_a: T4FS:0000156 ! archiving
property_value: IAO:0000117 "https://orcid.org/0000-0002-7702-4495" xsd:string
property_value: IAO:0000117 "https://orcid.org/0000-0003-2687-1982" xsd:string
property_value: IAO:0000118 "Data preservation" xsd:string
created_by: https://orcid.org/0000-0003-2687-1982
creation_date: 2021-02-17T22:18:22.641817Z

[Term]
id: T4FS:0000535
name: encoding schema
def: "Machine processable specifications which define the structure and syntax of metadata specifications in a formal schema language." [] {IAO:0000119="RDMT. https://terms.codata.org/rdmt/encoding-schema"}
comment: AL 5.12.22 Moved from 'findability of digital assets' as it is definitely not a particular data stewardship guideline.
is_a: T4FS:0000372 ! data stewardship technical concept
property_value: IAO:0000117 "https://orcid.org/0000-0002-5214-4466" xsd:string
property_value: IAO:0000117 "https://orcid.org/0000-0002-7702-4495" xsd:string
property_value: IAO:0000117 "https://orcid.org/0000-0003-2687-1982" xsd:string

[Term]
id: T4FS:0000537
name: digital archiving
name: digital archiving (computing)
def: "In the context of computing, the process of backup and ongoing maintenance as opposed to strategies for long-term digital preservation." [] {IAO:0000119="RDMT. https://terms.codata.org/rdmt/digital-archiving-computing"}
is_a: T4FS:0000156 ! archiving
property_value: IAO:0000117 "https://orcid.org/0000-0002-5214-4466" xsd:string
property_value: IAO:0000117 "https://orcid.org/0000-0002-7702-4495" xsd:string
property_value: IAO:0000117 "https://orcid.org/0000-0003-2687-1982" xsd:string

[Term]
id: T4FS:0000540
name: pid resolution
def: "The process of resolving a PID to a useful state of information about a digital object by using a globally available system." [] {IAO:0000119="RDMT. https://terms.codata.org/rdmt/pid-resolution"}
is_a: T4FS:0000453 ! persistent identifier
property_value: IAO:0000117 "https://orcid.org/0000-0002-5214-4466" xsd:string
property_value: IAO:0000117 "https://orcid.org/0000-0002-7702-4495" xsd:string
property_value: IAO:0000117 "https://orcid.org/0000-0003-2687-1982" xsd:string

[Term]
id: T4FS:0000541
name: skills related to storage management
def: "Bin for Skills needed for Storage management." []
is_a: T4FS:0000053 ! storage management
property_value: IAO:0000117 "leightonlc" xsd:string

[Term]
id: T4FS:0000544
name: data repository management
def: "Management of a national, discipline or institutional repository of published datasets. Provision of infrastructure, curation, policy and training that govern the organisation, control, and properties of the repository such as: required file formats, access control restrictions, integrity, replication, retention, disposal, etc." [] {IAO:0000119="RDMT. https://terms.codata.org/rdmt/data-repository-management"}
is_a: T4FS:0000353 ! resource management
property_value: IAO:0000117 "https://orcid.org/0000-0002-5214-4466" xsd:string
property_value: IAO:0000117 "https://orcid.org/0000-0002-7702-4495" xsd:string
property_value: IAO:0000117 "https://orcid.org/0000-0003-2687-1982" xsd:string

[Term]
id: T4FS:0000546
name: darwin information typing architecture
def: "A document creation and management specification that builds content reuse into the authoring process." [] {IAO:0000119="Definition from now-deprecated CASRAI Glossary term: darwin-information-typing-architecture/"}
is_a: T4FS:0000372 ! data stewardship technical concept
property_value: IAO:0000117 "https://orcid.org/0000-0002-5214-4466" xsd:string
property_value: IAO:0000117 "https://orcid.org/0000-0003-2687-1982" xsd:string

[Term]
id: T4FS:0000547
name: analytics
def: "The discovery of meaningful multidimensional patterns in data." [] {IAO:0000119="Definition from now-deprecated CASRAI Glossary term: analytics"}
is_a: T4FS:0000372 ! data stewardship technical concept
property_value: IAO:0000117 "https://orcid.org/0000-0002-5214-4466" xsd:string
property_value: IAO:0000117 "https://orcid.org/0000-0003-2687-1982" xsd:string

[Term]
id: T4FS:0000548
name: data stewardship soft skill
def: "The personal attributes necessary to perform a task." []
property_value: IAO:0000117 "https://orcid.org/0000-0003-2687-1982" xsd:string
property_value: T4FS:0000564 "Aptitude is the innate trait or talent that a person brings to a task or situation. It is the quality of being able to do something. An aptitude is not something that can be learned or developed unless it is there to begin with." xsd:string
property_value: T4FS:0000565 "Laura Molloy, Celia van Gelder:https://docs.google.com/presentation/d/12oNBFix39ZtsLAR4tkqESBXxMU5rVg3cCKoEDG2oK-M/edit#slide=id.p5" xsd:string

[Term]
id: T4FS:0000550
name: archival documentation of data
def: "Ability to apply the FAIR principles i.e. describe the data with community metadata standard for machine and human, align with existing semantic models (ontologies, controlled vocabularies, ...), get a persistent ID, attribute licence and credit for data creators, legal aspect related to data (ownership, confidentiality, ethics, ...) add data provenance." [] {IAO:0000119="[YLF, VDA, KH]"}
is_a: T4FS:0000156 ! archiving
property_value: IAO:0000117 "https://orcid.org/0000-0002-7702-4495" xsd:string
property_value: IAO:0000117 "Kristina Hettne" xsd:string
property_value: IAO:0000117 "Victoria Dominguez Del Angel" xsd:string
property_value: IAO:0000117 "Yann Le Franc" xsd:string

[Term]
id: T4FS:0000551
name: machine-readable format
def: "A machine-readable format is a structured format that can be processed by a computer. Such formats can either be intended solely for machine processing (e.g. XML or RDF), or may be both human and machine accessible via appropriate markup (e.g. HTML)." [] {IAO:0000119="Modified by AL from Wikipedia, https://en.wikipedia.org/wiki/Machine-readable_data, accessed 6.5.22"}
comment: AL 5.12.22: Merged with now-obsolete 'machine readable' (http://purl.obolibrary.org/obo/T4FS_0000256), as we do not need that level of granularity. AL 6.5.22: The original CASRAI term (https://casrai.org/term/machine-readable-format/) has an identical source definition with 'Digital materials', and therefore has been removed.
is_a: T4FS:0000372 ! data stewardship technical concept
property_value: IAO:0000117 "https://orcid.org/0000-0002-7702-4495" xsd:string
property_value: IAO:0000117 "https://orcid.org/0000-0003-2687-1982" xsd:string

[Term]
id: T4FS:0000552
name: confidential information
def: "Any information obtained by a person on the understanding that they will not disclose it to others, or obtained in circumstances where it is expected that they will not disclose it." [] {IAO:0000119="Definition from now-deprecated CASRAI Glossary term: confidential-information"}
is_a: T4FS:0000372 ! data stewardship technical concept
property_value: IAO:0000117 "https://orcid.org/0000-0002-5214-4466" xsd:string
property_value: IAO:0000117 "https://orcid.org/0000-0003-2687-1982" xsd:string

[Term]
id: T4FS:0000579
name: fair cookbook recipe
def: "The FAIR Cookbook’s recipes are a combination of guidance, technical, hands-on, background and review types to cover the operation steps of FAIR data management, and are classified according to the audience types, to serve all those involved in the data management life cycle. The FAIR Cookbook is for anyone working in the Life Sciences who needs guidance on applying the FAIR Principles in practice." [] {IAO:0000119="https://faircookbook.elixir-europe.org/content/recipes/introduction/FAIR-cookbook-audience.html"}
is_a: T4FS:0000095 ! online documentation
property_value: IAO:0000117 "https://orcid.org/0000-0002-7702-4495" xsd:string

[Term]
id: T4FS:0000580
name: evaluation indicator
def: "Evaluation indicators are designed to enable the measurement of the degree of compliance against a guideline using a set of criteria. The goals of such indicators are varied, but a good example would be to improve the re-usability of the digital asset being measured for increased discoverability, interoperability and overall machine actionability." [] {IAO:0000119="Definition by https://orcid.org/0000-0002-7702-4495 and drawn in part from https://fairplus.github.io/Data-Maturity/docs/Indicators"}
property_value: IAO:0000233 "https://github.com/terms4fairskills/FAIRterminology/issues/22" xsd:string

[Term]
id: T4FS:0000583
name: fairplus dataset maturity model indicator
def: "The fairplus dataset maturity model indicators are used within the context of the model, which is intended as a comprehensive reference model for state-of-FAIRness improvement in research datasets. Based on the FAIR guiding principles, the DSM model defines and classifies requirements that constitute an incremental path towards improving FAIRness level for a given research dataset." [] {IAO:0000119="https://fairplus.github.io/Data-Maturity/"}
is_a: T4FS:0000580 ! evaluation indicator
property_value: IAO:0000117 "https://orcid.org/0000-0002-7702-4495" xsd:string
property_value: IAO:0000118 "fairplus DSM model indicator" xsd:string

[Term]
id: T4FS:0000584
name: fairplus DSM content-related indicator
def: "The fairplus DSM content-related indicators relate to what is reported in the Dataset (data) & the Dataset Descriptor (metadata)." [] {IAO:0000119="https://fairplus.github.io/Data-Maturity/"}
is_a: T4FS:0000583 ! fairplus dataset maturity model indicator
property_value: IAO:0000117 "https://orcid.org/0000-0002-7702-4495" xsd:string

[Term]
id: T4FS:0000585
name: fairplus DSM representation and format indicator
def: "The fairplus DSM representation and format indicators relate to how the data object & metadata object are represented and formatted." [] {IAO:0000119="https://fairplus.github.io/Data-Maturity/"}
comment: AL 5.12.22: Please note that the 'and' in this label is a direct representation of the fairplus DSM model, and not a ontological design choice.
is_a: T4FS:0000583 ! fairplus dataset maturity model indicator
property_value: IAO:0000117 "https://orcid.org/0000-0002-7702-4495" xsd:string

[Term]
id: T4FS:0000586
name: fairplus DSM hosting-environment capabilities indicator
def: "The fairplus DSM hosting-environment capabilities indicator relate to the capabilities of the hosting environment that enables and supports the use of FAIR data" [] {IAO:0000119="https://fairplus.github.io/Data-Maturity/"}
is_a: T4FS:0000583 ! fairplus dataset maturity model indicator
property_value: IAO:0000117 "https://orcid.org/0000-0002-7702-4495" xsd:string

[Term]
id: T4FS:0000587
name: DSM-0-R2
def: "No representation of Data purposed for FAIR sharing is available" [] {IAO:0000119="https://fairplus.github.io/Data-Maturity/docs/Indicators/"}
is_a: T4FS:0000585 ! fairplus DSM representation and format indicator
property_value: IAO:0000117 "https://orcid.org/0000-0002-7702-4495" xsd:string

[Term]
id: T4FS:0000588
name: DSM-1-R2
def: "Structured and/or Unstructured Data are organised into Dataset(s) created for the purpose of FAIR sharing" [] {IAO:0000119="https://fairplus.github.io/Data-Maturity/docs/Indicators/"}
is_a: T4FS:0000585 ! fairplus DSM representation and format indicator
property_value: IAO:0000117 "https://orcid.org/0000-0002-7702-4495" xsd:string

[Term]
id: T4FS:0000589
name: DSM-2-R2
def: "Project collected Data are organized into structured Dataset(s) and conform to a locally defined Dataset Model" [] {IAO:0000119="https://fairplus.github.io/Data-Maturity/docs/Indicators/"}
is_a: T4FS:0000585 ! fairplus DSM representation and format indicator
property_value: IAO:0000117 "https://orcid.org/0000-0002-7702-4495" xsd:string

[Term]
id: T4FS:0000590
name: DSM-3-R2
def: "Structured Data are represented as Datasets and conform to relevant Standard Dataset Model(s) for FAIR sharing" [] {IAO:0000119="https://fairplus.github.io/Data-Maturity/docs/Indicators/"}
is_a: T4FS:0000585 ! fairplus DSM representation and format indicator
property_value: IAO:0000117 "https://orcid.org/0000-0002-7702-4495" xsd:string

[Term]
id: T4FS:0000591
name: DSM-4-R2
def: "Dataset(s) content is semantically represented using Linked Data Represetations conforming to a Semantic Data Model" [] {IAO:0000119="https://fairplus.github.io/Data-Maturity/docs/Indicators/"}
is_a: T4FS:0000585 ! fairplus DSM representation and format indicator
property_value: IAO:0000117 "https://orcid.org/0000-0002-7702-4495" xsd:string

[Term]
id: T4FS:0000592
name: DSM-5-R2
def: "Dataset(s) are granularly represented and managed at the Data Element Level (e.g. ISO 11179 MDR standard)" [] {IAO:0000119="https://fairplus.github.io/Data-Maturity/docs/Indicators/"}
is_a: T4FS:0000585 ! fairplus DSM representation and format indicator
property_value: IAO:0000117 "https://orcid.org/0000-0002-7702-4495" xsd:string

[Term]
id: T4FS:0000593
name: DSM-0-R3
def: "Dataset Metadata is NOT formally represented in a structured Dataset Descriptor" [] {IAO:0000119="https://fairplus.github.io/Data-Maturity/docs/Indicators/"}
is_a: T4FS:0000585 ! fairplus DSM representation and format indicator
property_value: IAO:0000117 "https://orcid.org/0000-0002-7702-4495" xsd:string

[Term]
id: T4FS:0000594
name: DSM-1-R0
def: "Dataset Metadata is formally represented in the form of an Identifiable Dataset Descriptor" [] {IAO:0000119="https://fairplus.github.io/Data-Maturity/docs/Indicators/"}
is_a: T4FS:0000585 ! fairplus DSM representation and format indicator
property_value: IAO:0000117 "https://orcid.org/0000-0002-7702-4495" xsd:string

[Term]
id: T4FS:0000595
name: DSM-1-R3
def: "A representation of the Dataset Descriptor conforming to a relevant General Purpose Metadata Schema is available" [] {IAO:0000119="https://fairplus.github.io/Data-Maturity/docs/Indicators/"}
is_a: T4FS:0000585 ! fairplus DSM representation and format indicator
property_value: IAO:0000117 "https://orcid.org/0000-0002-7702-4495" xsd:string

[Term]
id: T4FS:0000596
name: DSM-2-R3
def: "Dataset Descriptor(s) conforms to or extends a Standard Generic Dataset Descriptor Model to describe and represent structural metadata of Dataset(s)" [] {IAO:0000119="https://fairplus.github.io/Data-Maturity/docs/Indicators/"}
is_a: T4FS:0000585 ! fairplus DSM representation and format indicator
property_value: IAO:0000117 "https://orcid.org/0000-0002-7702-4495" xsd:string

[Term]
id: T4FS:0000597
name: DSM-3-R3
def: "Dataset Descriptor(s) use community-defined or domain-specific metadata standard" [] {IAO:0000119="https://fairplus.github.io/Data-Maturity/docs/Indicators/"}
is_a: T4FS:0000585 ! fairplus DSM representation and format indicator
relationship: T4FS:0000581 T4FS:0000391 ! confers compliance with R1.3 (meta)data meet domain-relevant community standards
property_value: IAO:0000117 "https://orcid.org/0000-0002-7702-4495" xsd:string

[Term]
id: T4FS:0000598
name: DSM-4-R3
def: "A Semantic Data Model (Metadata) used for data harmonisation across Datasets is formally defined and represented using Linked Data Representations" [] {IAO:0000119="https://fairplus.github.io/Data-Maturity/docs/Indicators/"}
is_a: T4FS:0000585 ! fairplus DSM representation and format indicator
relationship: T4FS:0000581 T4FS:0000137 ! confers compliance with I1. (meta)data use a formal, accessible, shared, and broadly applicable language for knowledge representation
property_value: IAO:0000117 "https://orcid.org/0000-0002-7702-4495" xsd:string

[Term]
id: T4FS:0000599
name: DSM-5-R3
def: "Common Data Elements and their value sets are defined and registered in a managed Metadata Registry" [] {IAO:0000119="https://fairplus.github.io/Data-Maturity/docs/Indicators/"}
is_a: T4FS:0000585 ! fairplus DSM representation and format indicator
property_value: IAO:0000117 "https://orcid.org/0000-0002-7702-4495" xsd:string

[Term]
id: T4FS:0000600
name: DSM-0-R1
def: "Contextual Metadata is NOT formally represented in any form" [] {IAO:0000119="https://fairplus.github.io/Data-Maturity/docs/Indicators/"}
is_a: T4FS:0000585 ! fairplus DSM representation and format indicator
property_value: IAO:0000117 "https://orcid.org/0000-0002-7702-4495" xsd:string

[Term]
id: T4FS:0000601
name: DSM-1-R1
def: "Contextual Metadata is reported at summary level and represented in the Dataset Descriptor" [] {IAO:0000119="https://fairplus.github.io/Data-Maturity/docs/Indicators/"}
is_a: T4FS:0000585 ! fairplus DSM representation and format indicator
property_value: IAO:0000117 "https://orcid.org/0000-0002-7702-4495" xsd:string

[Term]
id: T4FS:0000602
name: DSM-2-R1
def: "Contextual Metadata is formally represented in the form of a locally defined Domain Model" [] {IAO:0000119="https://fairplus.github.io/Data-Maturity/docs/Indicators/"}
is_a: T4FS:0000585 ! fairplus DSM representation and format indicator
property_value: IAO:0000117 "https://orcid.org/0000-0002-7702-4495" xsd:string

[Term]
id: T4FS:0000603
name: DSM-3-R1
def: "Contextual Metadata is formally represented and conforms to a standard defined Domain Model if available" [] {IAO:0000119="https://fairplus.github.io/Data-Maturity/docs/Indicators/"}
is_a: T4FS:0000585 ! fairplus DSM representation and format indicator
property_value: IAO:0000117 "https://orcid.org/0000-0002-7702-4495" xsd:string

[Term]
id: T4FS:0000604
name: DSM-4-R1
def: "Contextual Metadata is formally represented by a defined set Common Data Elements" [] {IAO:0000119="https://fairplus.github.io/Data-Maturity/docs/Indicators/"}
is_a: T4FS:0000585 ! fairplus DSM representation and format indicator
property_value: IAO:0000117 "https://orcid.org/0000-0002-7702-4495" xsd:string

[Term]
id: T4FS:0000605
name: DSM-5-R1
def: "Domain entities are represented by Managed Master Data Objects conforming to a Master Data Model used for data consolidation" [] {IAO:0000119="https://fairplus.github.io/Data-Maturity/docs/Indicators/"}
is_a: T4FS:0000585 ! fairplus DSM representation and format indicator
property_value: IAO:0000117 "https://orcid.org/0000-0002-7702-4495" xsd:string

[Term]
id: T4FS:0000606
name: DSM-0-R4
def: "Dataset Descriptor (metadata) is NOT available in a Machine Readable Format" [] {IAO:0000119="https://fairplus.github.io/Data-Maturity/docs/Indicators/"}
is_a: T4FS:0000585 ! fairplus DSM representation and format indicator
property_value: IAO:0000117 "https://orcid.org/0000-0002-7702-4495" xsd:string

[Term]
id: T4FS:0000607
name: DSM-1-R4
def: "Dataset Descriptor is available in Machine Readable Format" [] {IAO:0000119="https://fairplus.github.io/Data-Maturity/docs/Indicators/"}
is_a: T4FS:0000585 ! fairplus DSM representation and format indicator
property_value: IAO:0000117 "https://orcid.org/0000-0002-7702-4495" xsd:string

[Term]
id: T4FS:0000608
name: DSM-2-R4
def: "Contextual Metadata represented in the form of a Domain Model is available in a Human Readable Format" [] {IAO:0000119="https://fairplus.github.io/Data-Maturity/docs/Indicators/"}
is_a: T4FS:0000585 ! fairplus DSM representation and format indicator
property_value: IAO:0000117 "https://orcid.org/0000-0002-7702-4495" xsd:string

[Term]
id: T4FS:0000609
name: DSM-3-R4
def: "A formal documentation of the adopted Standard Dataset Model is available in a Machine Readable Format" [] {IAO:0000119="https://fairplus.github.io/Data-Maturity/docs/Indicators/"}
is_a: T4FS:0000585 ! fairplus DSM representation and format indicator
property_value: IAO:0000117 "https://orcid.org/0000-0002-7702-4495" xsd:string

[Term]
id: T4FS:0000610
name: DSM-4-R4
def: "A Semantic Data Model (Metadata) describing the data is represented in a Machine Readable and Machine Interptretable format" [] {IAO:0000119="https://fairplus.github.io/Data-Maturity/docs/Indicators/"}
is_a: T4FS:0000585 ! fairplus DSM representation and format indicator
property_value: IAO:0000117 "https://orcid.org/0000-0002-7702-4495" xsd:string

[Term]
id: T4FS:0000611
name: DSM-0-R5
def: "Dataset(s) are NOT available in a Machine Readable Format" [] {IAO:0000119="https://fairplus.github.io/Data-Maturity/docs/Indicators/"}
is_a: T4FS:0000585 ! fairplus DSM representation and format indicator
property_value: IAO:0000117 "https://orcid.org/0000-0002-7702-4495" xsd:string

[Term]
id: T4FS:0000612
name: DSM-1-R5
def: "Dataset(s) available in Machine Readable Format" [] {IAO:0000119="https://fairplus.github.io/Data-Maturity/docs/Indicators/"}
is_a: T4FS:0000585 ! fairplus DSM representation and format indicator
property_value: IAO:0000117 "https://orcid.org/0000-0002-7702-4495" xsd:string

[Term]
id: T4FS:0000613
name: DSM-3-R5
def: "If applicable, Dataset(s) available in non-proprietary Machine Readable Format relevant to the adopted standard Dataset Model" [] {IAO:0000119="https://fairplus.github.io/Data-Maturity/docs/Indicators/"}
is_a: T4FS:0000585 ! fairplus DSM representation and format indicator
property_value: IAO:0000117 "https://orcid.org/0000-0002-7702-4495" xsd:string

[Term]
id: T4FS:0000614
name: DSM-4-R5
def: "Datasets are available in a Machine Readable and Machine Interpretable format" [] {IAO:0000119="https://fairplus.github.io/Data-Maturity/docs/Indicators/"}
is_a: T4FS:0000585 ! fairplus DSM representation and format indicator
property_value: IAO:0000117 "https://orcid.org/0000-0002-7702-4495" xsd:string

[Term]
id: T4FS:0000615
name: DSM-4-R6
def: "If applicable, license information and/or permitted use and accessability to parts of the dataset is formally represented and encoded in a Machine Readable Format" [] {IAO:0000119="https://fairplus.github.io/Data-Maturity/docs/Indicators/"}
is_a: T4FS:0000585 ! fairplus DSM representation and format indicator
relationship: T4FS:0000581 T4FS:0000200 ! confers compliance with R1.1 (meta)data are released with a clear and accessible data usage license
property_value: IAO:0000117 "https://orcid.org/0000-0002-7702-4495" xsd:string

[Term]
id: T4FS:0000616
name: DSM-0-C0
def: "Dataset(s) are NOT Identifiable via Unique Identifiers" [] {IAO:0000119="https://fairplus.github.io/Data-Maturity/docs/Indicators/"}
is_a: T4FS:0000584 ! fairplus DSM content-related indicator
property_value: IAO:0000117 "https://orcid.org/0000-0002-7702-4495" xsd:string

[Term]
id: T4FS:0000617
name: DSM-1-C0
def: "Each Dataset purposed for FAIR sharing is assigned a unique identifier" [] {IAO:0000119="https://fairplus.github.io/Data-Maturity/docs/Indicators/"}
is_a: T4FS:0000584 ! fairplus DSM content-related indicator
relationship: T4FS:0000581 T4FS:0000512 ! confers compliance with F1. (meta)data are assigned a globally unique and persistent identifier
property_value: IAO:0000117 "https://orcid.org/0000-0002-7702-4495" xsd:string

[Term]
id: T4FS:0000618
name: DSM-2-C2
def: "Where applicable, data is structured in the Dataset according to the Tidy Data Principles" [] {IAO:0000119="https://fairplus.github.io/Data-Maturity/docs/Indicators/"}
is_a: T4FS:0000584 ! fairplus DSM content-related indicator
relationship: T4FS:0000581 T4FS:0000174 ! confers compliance with R1. (meta)data are richly described with a plurality of accurate and relevant attributes
property_value: IAO:0000117 "https://orcid.org/0000-0002-7702-4495" xsd:string

[Term]
id: T4FS:0000619
name: DSM-3-C2
def: "Where applicable, Dataset(s) scope and content are reported in compliance with relevant community-defined Data Reporting Guidelines" [] {IAO:0000119="https://fairplus.github.io/Data-Maturity/docs/Indicators/"}
is_a: T4FS:0000584 ! fairplus DSM content-related indicator
relationship: T4FS:0000581 T4FS:0000391 ! confers compliance with R1.3 (meta)data meet domain-relevant community standards
property_value: IAO:0000117 "https://orcid.org/0000-0002-7702-4495" xsd:string

[Term]
id: T4FS:0000620
name: DSM-4-C2
def: "Dataset(s) content is harmonised against a designed-for-purpose Semantic Data Model" [] {IAO:0000119="https://fairplus.github.io/Data-Maturity/docs/Indicators/"}
is_a: T4FS:0000584 ! fairplus DSM content-related indicator
relationship: T4FS:0000581 T4FS:0000137 ! confers compliance with I1. (meta)data use a formal, accessible, shared, and broadly applicable language for knowledge representation
property_value: IAO:0000117 "https://orcid.org/0000-0002-7702-4495" xsd:string

[Term]
id: T4FS:0000621
name: DSM-2-C3
def: "Dataset(s) include Reference Fields that enable joining related datasets" [] {IAO:0000119="https://fairplus.github.io/Data-Maturity/docs/Indicators/"}
is_a: T4FS:0000584 ! fairplus DSM content-related indicator
relationship: T4FS:0000581 T4FS:0000452 ! confers compliance with I3. (meta)data include qualified references to other (meta)data
property_value: IAO:0000117 "https://orcid.org/0000-0002-7702-4495" xsd:string

[Term]
id: T4FS:0000622
name: DSM-3-C3
def: "Where applicable, Dataset Field Names use standard controlled terms as recommended by the adopted Standard" [] {IAO:0000119="https://fairplus.github.io/Data-Maturity/docs/Indicators/"}
is_a: T4FS:0000584 ! fairplus DSM content-related indicator
relationship: T4FS:0000581 T4FS:0000137 ! confers compliance with I1. (meta)data use a formal, accessible, shared, and broadly applicable language for knowledge representation
property_value: IAO:0000117 "https://orcid.org/0000-0002-7702-4495" xsd:string

[Term]
id: T4FS:0000623
name: DSM-4-C3
def: "Key Dataset Fields are mapped to Common Data Elements as defined by the Semantic Data Model" [] {IAO:0000119="https://fairplus.github.io/Data-Maturity/docs/Indicators/"}
is_a: T4FS:0000584 ! fairplus DSM content-related indicator
property_value: IAO:0000117 "https://orcid.org/0000-0002-7702-4495" xsd:string

[Term]
id: T4FS:0000624
name: DSM-5-C3
def: "Dataset Fields are linked and harmonized against enterprise managed Metadata Elements (e.g. MDR registered Data Elements)" [] {IAO:0000119="https://fairplus.github.io/Data-Maturity/docs/Indicators/"}
is_a: T4FS:0000584 ! fairplus DSM content-related indicator
property_value: IAO:0000117 "https://orcid.org/0000-0002-7702-4495" xsd:string

[Term]
id: T4FS:0000625
name: DSM-2-C4
def: "Where applicable, Dataset Field Values are standardized against a locally defined Data Dictionary within and across related Datasets" [] {IAO:0000119="https://fairplus.github.io/Data-Maturity/docs/Indicators/"}
is_a: T4FS:0000584 ! fairplus DSM content-related indicator
relationship: T4FS:0000581 T4FS:0000174 ! confers compliance with R1. (meta)data are richly described with a plurality of accurate and relevant attributes
relationship: T4FS:0000581 T4FS:0000199 ! confers compliance with F2. data are described with rich metadata
property_value: IAO:0000117 "https://orcid.org/0000-0002-7702-4495" xsd:string

[Term]
id: T4FS:0000626
name: DSM-3-C4
def: "Where applicable, Dataset Field Values are standardised against domain-specific Controlled Terminologies and/or Ontology Terms" [] {IAO:0000119="https://fairplus.github.io/Data-Maturity/docs/Indicators/"}
is_a: T4FS:0000584 ! fairplus DSM content-related indicator
relationship: T4FS:0000581 T4FS:0000361 ! confers compliance with I2. (meta)data use vocabularies that follow fair principles
relationship: T4FS:0000581 T4FS:0000391 ! confers compliance with R1.3 (meta)data meet domain-relevant community standards
property_value: IAO:0000117 "https://orcid.org/0000-0002-7702-4495" xsd:string

[Term]
id: T4FS:0000627
name: DSM-4-C4
def: "Values for key Domain Entities reported in the Dataset(s) are standardised and assigned unique Standard Identifiers" [] {IAO:0000119="https://fairplus.github.io/Data-Maturity/docs/Indicators/"}
is_a: T4FS:0000584 ! fairplus DSM content-related indicator
relationship: T4FS:0000581 T4FS:0000435 ! confers compliance with F3. metadata clearly and explicitly include the identifier of the data they describe
property_value: IAO:0000117 "https://orcid.org/0000-0002-7702-4495" xsd:string

[Term]
id: T4FS:0000628
name: DSM-5-C4
def: "Dataset Field values are controlled and managed via enterprise managed Reference and Master Data" [] {IAO:0000119="https://fairplus.github.io/Data-Maturity/docs/Indicators/"}
is_a: T4FS:0000584 ! fairplus DSM content-related indicator
property_value: IAO:0000117 "https://orcid.org/0000-0002-7702-4495" xsd:string

[Term]
id: T4FS:0000629
name: DSM-0-C1
def: "Study/Project-Level metadata is NOT reported" [] {IAO:0000119="https://fairplus.github.io/Data-Maturity/docs/Indicators/"}
is_a: T4FS:0000584 ! fairplus DSM content-related indicator
property_value: IAO:0000117 "https://orcid.org/0000-0002-7702-4495" xsd:string

[Term]
id: T4FS:0000630
name: DSM-1-C1
def: "Dataset Descriptor includes Descriptive Study/Project-Level summary information" [] {IAO:0000119="https://fairplus.github.io/Data-Maturity/docs/Indicators/"}
is_a: T4FS:0000584 ! fairplus DSM content-related indicator
relationship: T4FS:0000581 T4FS:0000174 ! confers compliance with R1. (meta)data are richly described with a plurality of accurate and relevant attributes
relationship: T4FS:0000581 T4FS:0000199 ! confers compliance with F2. data are described with rich metadata
property_value: IAO:0000117 "https://orcid.org/0000-0002-7702-4495" xsd:string

[Term]
id: T4FS:0000631
name: DSM-2-C1
def: "A locally defined Domain Model contains concepts that describes the overall project/study design, the relationships between the Datasets, the key entities reported within the Datasets and the relationships between them." [] {IAO:0000119="https://fairplus.github.io/Data-Maturity/docs/Indicators/"}
is_a: T4FS:0000584 ! fairplus DSM content-related indicator
relationship: T4FS:0000581 T4FS:0000174 ! confers compliance with R1. (meta)data are richly described with a plurality of accurate and relevant attributes
property_value: IAO:0000117 "https://orcid.org/0000-0002-7702-4495" xsd:string

[Term]
id: T4FS:0000632
name: DSM-3-C1
def: "Where applicable, study-level / experimental metadata is reported in compliance with relevant Minimum Information Reporting Guidelines" [] {IAO:0000119="https://fairplus.github.io/Data-Maturity/docs/Indicators/"}
is_a: T4FS:0000584 ! fairplus DSM content-related indicator
relationship: T4FS:0000581 T4FS:0000391 ! confers compliance with R1.3 (meta)data meet domain-relevant community standards
property_value: IAO:0000117 "https://orcid.org/0000-0002-7702-4495" xsd:string

[Term]
id: T4FS:0000633
name: DSM-4-C1
def: "A Semantic Data Model includes study design Data Elements and the relationships between them" [] {IAO:0000119="https://fairplus.github.io/Data-Maturity/docs/Indicators/"}
is_a: T4FS:0000372 ! data stewardship technical concept
is_a: T4FS:0000584 ! fairplus DSM content-related indicator
relationship: T4FS:0000563 T4FS:0000137 ! contributes to the implementation of I1. (meta)data use a formal, accessible, shared, and broadly applicable language for knowledge representation
relationship: T4FS:0000581 T4FS:0000199 ! confers compliance with F2. data are described with rich metadata
property_value: IAO:0000117 "https://orcid.org/0000-0002-7702-4495" xsd:string

[Term]
id: T4FS:0000634
name: DSM-0-C2
def: "Dataset Descriptor does NOT include a reference to the Dataset it describes" [] {IAO:0000119="https://fairplus.github.io/Data-Maturity/docs/Indicators/"}
is_a: T4FS:0000584 ! fairplus DSM content-related indicator
property_value: IAO:0000117 "https://orcid.org/0000-0002-7702-4495" xsd:string

[Term]
id: T4FS:0000635
name: DSM-1-C2
def: "Dataset Descriptor includes Identifying & Descriptive Dataset-Level metadata" [] {IAO:0000119="https://fairplus.github.io/Data-Maturity/docs/Indicators/"}
is_a: T4FS:0000584 ! fairplus DSM content-related indicator
relationship: T4FS:0000581 T4FS:0000174 ! confers compliance with R1. (meta)data are richly described with a plurality of accurate and relevant attributes
relationship: T4FS:0000581 T4FS:0000435 ! confers compliance with F3. metadata clearly and explicitly include the identifier of the data they describe
property_value: IAO:0000117 "https://orcid.org/0000-0002-7702-4495" xsd:string

[Term]
id: T4FS:0000636
name: DSM-1-C3
def: "Dataset Descriptor contains access information for the Dataset" [] {IAO:0000119="https://fairplus.github.io/Data-Maturity/docs/Indicators/"}
is_a: T4FS:0000584 ! fairplus DSM content-related indicator
relationship: T4FS:0000581 T4FS:0000038 ! confers compliance with A1. (meta)data are retrievable by their identifier using a standardised communications protocol
property_value: IAO:0000117 "https://orcid.org/0000-0002-7702-4495" xsd:string

[Term]
id: T4FS:0000637
name: DSM-2-C5
def: "Dataset Descriptor includes reference to related Datasets and if applicable the relevant joining Dataset Fields" [] {IAO:0000119="https://fairplus.github.io/Data-Maturity/docs/Indicators/"}
is_a: T4FS:0000584 ! fairplus DSM content-related indicator
property_value: IAO:0000117 "https://orcid.org/0000-0002-7702-4495" xsd:string

[Term]
id: T4FS:0000638
name: DSM-3-C7
def: "Dataset Descriptor references a standard license under which the dataset can be re-used." [] {IAO:0000119="https://fairplus.github.io/Data-Maturity/docs/Indicators/"}
is_a: T4FS:0000584 ! fairplus DSM content-related indicator
relationship: T4FS:0000581 T4FS:0000199 ! confers compliance with F2. data are described with rich metadata
property_value: IAO:0000117 "https://orcid.org/0000-0002-7702-4495" xsd:string

[Term]
id: T4FS:0000639
name: DSM-2-C6
def: "Dataset Descriptor includes Field-level Metadata as prescribed by a locally defined Dataset Model" [] {IAO:0000119="https://fairplus.github.io/Data-Maturity/docs/Indicators/"}
is_a: T4FS:0000584 ! fairplus DSM content-related indicator
relationship: T4FS:0000581 T4FS:0000174 ! confers compliance with R1. (meta)data are richly described with a plurality of accurate and relevant attributes
relationship: T4FS:0000581 T4FS:0000199 ! confers compliance with F2. data are described with rich metadata
property_value: IAO:0000117 "https://orcid.org/0000-0002-7702-4495" xsd:string

[Term]
id: T4FS:0000640
name: DSM-3-C6
def: "Dataset Descriptor includes standard-compliant Field-level Metadata as prescribed by the adopted standard Dataset Model." [] {IAO:0000119="https://fairplus.github.io/Data-Maturity/docs/Indicators/"}
is_a: T4FS:0000584 ! fairplus DSM content-related indicator
property_value: IAO:0000117 "https://orcid.org/0000-0002-7702-4495" xsd:string

[Term]
id: T4FS:0000641
name: DSM-4-C5
def: "The Semantic Data Model includes a pre-defined set of Common Data Elements reported within the Datasets and the relationships between them" [] {IAO:0000119="https://fairplus.github.io/Data-Maturity/docs/Indicators/"}
is_a: T4FS:0000584 ! fairplus DSM content-related indicator
relationship: T4FS:0000581 T4FS:0000199 ! confers compliance with F2. data are described with rich metadata
property_value: IAO:0000117 "https://orcid.org/0000-0002-7702-4495" xsd:string

[Term]
id: T4FS:0000642
name: DSM-2-C7
def: "Dataset Descriptor includes Value-level Metadata or if applicable includes a reference to a locally defined Data Dictionary" [] {IAO:0000119="https://fairplus.github.io/Data-Maturity/docs/Indicators/"}
is_a: T4FS:0000584 ! fairplus DSM content-related indicator
relationship: T4FS:0000581 T4FS:0000174 ! confers compliance with R1. (meta)data are richly described with a plurality of accurate and relevant attributes
relationship: T4FS:0000581 T4FS:0000199 ! confers compliance with F2. data are described with rich metadata
property_value: IAO:0000117 "https://orcid.org/0000-0002-7702-4495" xsd:string

[Term]
id: T4FS:0000643
name: DSM-3-C5
def: "Value Level Metadata includes Resolvable Identifiers for Controlled and/or Standard Terms reported in the Dataset" [] {IAO:0000119="https://fairplus.github.io/Data-Maturity/docs/Indicators/"}
is_a: T4FS:0000584 ! fairplus DSM content-related indicator
relationship: T4FS:0000581 T4FS:0000038 ! confers compliance with A1. (meta)data are retrievable by their identifier using a standardised communications protocol
relationship: T4FS:0000581 T4FS:0000199 ! confers compliance with F2. data are described with rich metadata
relationship: T4FS:0000581 T4FS:0000361 ! confers compliance with I2. (meta)data use vocabularies that follow fair principles
relationship: T4FS:0000581 T4FS:0000435 ! confers compliance with F3. metadata clearly and explicitly include the identifier of the data they describe
relationship: T4FS:0000581 T4FS:0000452 ! confers compliance with I3. (meta)data include qualified references to other (meta)data
property_value: IAO:0000117 "https://orcid.org/0000-0002-7702-4495" xsd:string

[Term]
id: T4FS:0000644
name: DSM-0-H1
def: "Data or metadata is hosted in non-accessible storage (e.g., personal desktop, local file system or archive)" [] {IAO:0000119="https://fairplus.github.io/Data-Maturity/docs/Indicators/"}
is_a: T4FS:0000586 ! fairplus DSM hosting-environment capabilities indicator
property_value: IAO:0000117 "https://orcid.org/0000-0002-7702-4495" xsd:string

[Term]
id: T4FS:0000645
name: DSM-1-H1
def: "Metadata hosting environment stores and maintains an identifiable Dataset Descriptor for each identifiable Dataset" [] {IAO:0000119="https://fairplus.github.io/Data-Maturity/docs/Indicators/"}
is_a: T4FS:0000586 ! fairplus DSM hosting-environment capabilities indicator
relationship: T4FS:0000581 T4FS:0000038 ! confers compliance with A1. (meta)data are retrievable by their identifier using a standardised communications protocol
relationship: T4FS:0000581 T4FS:0000435 ! confers compliance with F3. metadata clearly and explicitly include the identifier of the data they describe
property_value: IAO:0000117 "https://orcid.org/0000-0002-7702-4495" xsd:string

[Term]
id: T4FS:0000646
name: DSM-2-H1
def: "The Data hosting environment's Persistence Model is aligned with a locally defined Domain Model to enable interpretation of Datasets" [] {IAO:0000119="https://fairplus.github.io/Data-Maturity/docs/Indicators/"}
is_a: T4FS:0000586 ! fairplus DSM hosting-environment capabilities indicator
relationship: T4FS:0000581 T4FS:0000174 ! confers compliance with R1. (meta)data are richly described with a plurality of accurate and relevant attributes
property_value: IAO:0000117 "https://orcid.org/0000-0002-7702-4495" xsd:string

[Term]
id: T4FS:0000647
name: DSM-3-H1
def: "The Data hosting environment's Persistence Model is aligned with a standard Dataset model or compliant with relevant Minimum Information Reporting Guidelines" [] {IAO:0000119="https://fairplus.github.io/Data-Maturity/docs/Indicators/"}
is_a: T4FS:0000586 ! fairplus DSM hosting-environment capabilities indicator
relationship: T4FS:0000581 T4FS:0000391 ! confers compliance with R1.3 (meta)data meet domain-relevant community standards
property_value: IAO:0000117 "https://orcid.org/0000-0002-7702-4495" xsd:string

[Term]
id: T4FS:0000648
name: DSM-4-H1
def: "Data Hosting environment stores data in a relevant linked data store (e.g., Triple Store or Graph Databaase)" [] {IAO:0000119="https://fairplus.github.io/Data-Maturity/docs/Indicators/"}
is_a: T4FS:0000586 ! fairplus DSM hosting-environment capabilities indicator
property_value: IAO:0000117 "https://orcid.org/0000-0002-7702-4495" xsd:string

[Term]
id: T4FS:0000649
name: DSM-0-H2
def: "Data or metadata hosted in an accessible resource but with no retrieval capability" [] {IAO:0000119="https://fairplus.github.io/Data-Maturity/docs/Indicators/"}
is_a: T4FS:0000586 ! fairplus DSM hosting-environment capabilities indicator
property_value: IAO:0000117 "https://orcid.org/0000-0002-7702-4495" xsd:string

[Term]
id: T4FS:0000650
name: DSM-1-H2
def: "The Dataset and its Descriptor are indexed and retrievable (in the same or separate hosting environments) via unique and persistent identifiers" [] {IAO:0000119="https://fairplus.github.io/Data-Maturity/docs/Indicators/"}
is_a: T4FS:0000586 ! fairplus DSM hosting-environment capabilities indicator
relationship: T4FS:0000581 T4FS:0000038 ! confers compliance with A1. (meta)data are retrievable by their identifier using a standardised communications protocol
property_value: IAO:0000117 "https://orcid.org/0000-0002-7702-4495" xsd:string

[Term]
id: T4FS:0000651
name: DSM-1-H3
def: "Retrieval of the Dataset and the Dataset Descriptor utilises a standardized communication protocol that is open, free and universally implementable" [] {IAO:0000119="https://fairplus.github.io/Data-Maturity/docs/Indicators/"}
is_a: T4FS:0000586 ! fairplus DSM hosting-environment capabilities indicator
relationship: T4FS:0000581 T4FS:0000103 ! confers compliance with A1.1 the protocol is open, free, and universally implementable
property_value: IAO:0000117 "https://orcid.org/0000-0002-7702-4495" xsd:string

[Term]
id: T4FS:0000652
name: DSM-2-H2
def: "Metadata hosting environment provides programmatic access and retrieval (API) for the Dataset Descriptor" [] {IAO:0000119="https://fairplus.github.io/Data-Maturity/docs/Indicators/"}
is_a: T4FS:0000586 ! fairplus DSM hosting-environment capabilities indicator
relationship: T4FS:0000581 T4FS:0000038 ! confers compliance with A1. (meta)data are retrievable by their identifier using a standardised communications protocol
property_value: IAO:0000117 "https://orcid.org/0000-0002-7702-4495" xsd:string

[Term]
id: T4FS:0000653
name: DSM-3-H2
def: "For each dataset, the hosting environment maintains a globally unique, persistent and resolvable identifier for access and retrieval" [] {IAO:0000119="https://fairplus.github.io/Data-Maturity/docs/Indicators/"}
is_a: T4FS:0000586 ! fairplus DSM hosting-environment capabilities indicator
relationship: T4FS:0000581 T4FS:0000512 ! confers compliance with F1. (meta)data are assigned a globally unique and persistent identifier
property_value: IAO:0000117 "https://orcid.org/0000-0002-7702-4495" xsd:string

[Term]
id: T4FS:0000654
name: DSM-3-H4
def: "If applicable, Dataset hosting environment offers dataset-level authentication and authorisation capabilities" [] {IAO:0000119="https://fairplus.github.io/Data-Maturity/docs/Indicators/"}
is_a: T4FS:0000586 ! fairplus DSM hosting-environment capabilities indicator
relationship: T4FS:0000581 T4FS:0000371 ! confers compliance with A1.2 the protocol allows for an authentication and authorisation procedure, where necessary
property_value: IAO:0000117 "https://orcid.org/0000-0002-7702-4495" xsd:string

[Term]
id: T4FS:0000655
name: DSM-4-H2
def: "Data Hosting Environment provides semantic querying capability" [] {IAO:0000119="https://fairplus.github.io/Data-Maturity/docs/Indicators/"}
is_a: T4FS:0000586 ! fairplus DSM hosting-environment capabilities indicator
property_value: IAO:0000117 "https://orcid.org/0000-0002-7702-4495" xsd:string

[Term]
id: T4FS:0000656
name: DSM-0-H3
def: "Dataset's Metadata is NOT searchable via keywords or elements within the Descriptor" [] {IAO:0000119="https://fairplus.github.io/Data-Maturity/docs/Indicators/"}
is_a: T4FS:0000586 ! fairplus DSM hosting-environment capabilities indicator
property_value: IAO:0000117 "https://orcid.org/0000-0002-7702-4495" xsd:string

[Term]
id: T4FS:0000657
name: DSM-1-H4
def: "Metadata hosting environment offers the capability to browse and search contents of the Dataset Descriptor" [] {IAO:0000119="https://fairplus.github.io/Data-Maturity/docs/Indicators/"}
is_a: T4FS:0000586 ! fairplus DSM hosting-environment capabilities indicator
relationship: T4FS:0000581 T4FS:0000393 ! confers compliance with F4. (meta)data are registered or indexed in a searchable resource
property_value: IAO:0000117 "https://orcid.org/0000-0002-7702-4495" xsd:string

[Term]
id: T4FS:0000658
name: DSM-2-H3
def: "Data hosting environment offers the capability to browse and search related Datasets" [] {IAO:0000119="https://fairplus.github.io/Data-Maturity/docs/Indicators/"}
is_a: T4FS:0000586 ! fairplus DSM hosting-environment capabilities indicator
relationship: T4FS:0000581 T4FS:0000393 ! confers compliance with F4. (meta)data are registered or indexed in a searchable resource
property_value: IAO:0000117 "https://orcid.org/0000-0002-7702-4495" xsd:string

[Term]
id: T4FS:0000659
name: DSM-3-H3
def: "Data Hosting environment utilises controlled terms and/or ontology terms to search within Dataset content." [] {IAO:0000119="https://fairplus.github.io/Data-Maturity/docs/Indicators/"}
is_a: T4FS:0000586 ! fairplus DSM hosting-environment capabilities indicator
relationship: T4FS:0000581 T4FS:0000512 ! confers compliance with F1. (meta)data are assigned a globally unique and persistent identifier
property_value: IAO:0000117 "https://orcid.org/0000-0002-7702-4495" xsd:string

[Term]
id: T4FS:0000660
name: DSM-4-H2
def: "Data Hosting Environment provides semantic querying capability" [] {IAO:0000119="https://fairplus.github.io/Data-Maturity/docs/Indicators/"}
is_a: T4FS:0000586 ! fairplus DSM hosting-environment capabilities indicator
property_value: IAO:0000117 "https://orcid.org/0000-0002-7702-4495" xsd:string

[Typedef]
id: T4FS:0000554
name: confers competency about
def: "Describes how a learning medium is intended to confer a competence or capability regarding a particular data stewardship activity, e.g. a presentation confering competency in metadata creation." [] {IAO:0000119="https://orcid.org/0000-0002-7702-4495"}
property_value: IAO:0000117 "https://orcid.org/0000-0002-7702-4495" xsd:string
property_value: IAO:0000117 "Peter McQuilton" xsd:string
domain: T4FS:0000519 ! learning medium
range: T4FS:0000012 ! data stewardship activity
inverse_of: T4FS:0000575 ! competency gained through
created_by: Peter McQuilton
creation_date: 2020-10-01T21:36:11.080721Z

[Typedef]
id: T4FS:0000555
name: confers knowledge about
def: "Describes how a learning medium is intended to confer knowledge of a particular data stewardship technical concept in order for that learning medium to perform its function, e.g. a presentation conferring competency in metadata." [] {IAO:0000119="https://orcid.org/0000-0002-7702-4495"}
property_value: IAO:0000117 "https://orcid.org/0000-0002-7702-4495" xsd:string
property_value: IAO:0000117 "Peter McQuilton" xsd:string
domain: T4FS:0000519 ! learning medium
range: T4FS:0000372 ! data stewardship technical concept
created_by: Peter McQuilton
creation_date: 2020-12-06 00:00:00

[Typedef]
id: T4FS:0000556
name: requires/improves personal attribute
property_value: IAO:0000117 "https://orcid.org/0000-0002-7702-4495" xsd:string
range: T4FS:0000548 ! data stewardship soft skill
created_by: Peter McQuilton

[Typedef]
id: T4FS:0000557
name: confers practical skill about
def: "Describes how a learning medium confers practical skills regarding a particular data stewardship technical concept in order for that learning medium to perform its function e.g. a workshop conferring a practical skill in repository access." [] {IAO:0000119="https://orcid.org/0000-0002-7702-4495"}
property_value: IAO:0000117 "https://orcid.org/0000-0002-7702-4495" xsd:string
property_value: IAO:0000117 "Peter McQuilton" xsd:string
domain: T4FS:0000519 ! learning medium
range: T4FS:0000372 ! data stewardship technical concept
created_by: Peter McQuilton
creation_date: 2020-12-06 00:00:00

[Typedef]
id: T4FS:0000558
name: has/wants competency in
def: "Describes how an expertise level or role (e.g. \"data steward\") is associated with a data stewardship activity (e.g. ‘workflow set-up and management’) to indicate whether someone has an awareness of the area, or an ability to do it, or expert knowledge of it." [] {IAO:0000119="https://orcid.org/0000-0002-7702-4495"}
comment: Definition added 8.2.22
property_value: IAO:0000117 "https://orcid.org/0000-0002-7702-4495" xsd:string
property_value: IAO:0000117 "Peter McQuilton" xsd:string
range: T4FS:0000012 ! data stewardship activity

[Typedef]
id: T4FS:0000559
name: has/wants knowledge about
property_value: IAO:0000117 "https://orcid.org/0000-0002-7702-4495" xsd:string
property_value: IAO:0000117 "Peter McQuilton" xsd:string

[Typedef]
id: T4FS:0000560
name: supports implementation of
property_value: IAO:0000117 "https://orcid.org/0000-0002-7702-4495" xsd:string
domain: T4FS:0000519 ! learning medium
range: T4FS:0000446 ! data stewardship guideline
created_by: Peter McQuilton

[Typedef]
id: T4FS:0000561
name: has/wants practical skill about
def: "Desires/has a competence or capability acquired or applied in a specific context, e.g. producing a research output or deploying a service. A skill may be specified in a ‘skills user story’. A badge or certificate may provide evidence that a skill has been acquired, and a publication, personal profile, portfolio or CV may provide evidence that a skill has been applied." [] {IAO:0000119="FAIR4S"}
property_value: IAO:0000117 "https://orcid.org/0000-0002-7702-4495" xsd:string
property_value: IAO:0000117 "Peter McQuilton" xsd:string
range: T4FS:0000372 ! data stewardship technical concept
created_by: Peter McQuilton

[Typedef]
id: T4FS:0000562
name: has aptitude for
property_value: IAO:0000117 "https://orcid.org/0000-0002-7702-4495" xsd:string
property_value: IAO:0000117 "Peter McQuilton" xsd:string
range: T4FS:0000548 ! data stewardship soft skill
created_by: Peter McQuilton
creation_date: 2021-03-24T15:33:43.476917Z

[Typedef]
id: T4FS:0000563
name: contributes to the implementation of
property_value: IAO:0000117 "https://orcid.org/0000-0002-7702-4495" xsd:string
property_value: IAO:0000117 "Peter McQuilton" xsd:string
domain: T4FS:0000372 ! data stewardship technical concept
range: T4FS:0000446 ! data stewardship guideline
created_by: Peter McQuilton
creation_date: 2021-03-22T15:25:13.443153Z

[Typedef]
id: T4FS:0000575
name: competency gained through
def: "The learning media that creates a competence or capability." [] {IAO:0000119="https://orcid.org/0000-0002-7702-4495"}
comment: Allyson Lister 13.9.22: This class is created as the inverse of confers/requires competency about to allow consistent reasoning and access to the Data stewardship guidelines for Data stewardship activities. It needs to be revisited by the entire team to check the model.
property_value: IAO:0000117 "https://orcid.org/0000-0002-7702-4495" xsd:string
domain: T4FS:0000012 ! data stewardship activity
range: T4FS:0000519 ! learning medium
created_by: https://orcid.org/0000-0002-7702-4495

[Typedef]
id: T4FS:0000576
name: requires competency about
def: "Describes how a learning medium requires competency in a particular data stewardship activity in order for that learning medium to perform its function, e.g. a presentation requiring competency in metadata creation prior to engaging with that learning medium." [] {IAO:0000119="https://orcid.org/0000-0002-7702-4495"}
domain: T4FS:0000519 ! learning medium
range: T4FS:0000012 ! data stewardship activity

[Typedef]
id: T4FS:0000577
name: requires knowledge about
def: "Describes how a learning medium requires knowledge of a particular data stewardship technical concept in order for that learning medium to perform its function, e.g. a presentation requiring knowledge of metadata." [] {IAO:0000119="https://orcid.org/0000-0002-7702-4495"}
domain: T4FS:0000519 ! learning medium
range: T4FS:0000372 ! data stewardship technical concept

[Typedef]
id: T4FS:0000578
name: requires practical skill about
def: "Describes how a learning medium requires practical skills of a particular data stewardship technical concept in order for that learning medium to perform its function e.g. a workshop requiring a practical skill in repository access." [] {IAO:0000119="https://orcid.org/0000-0002-7702-4495"}
domain: T4FS:0000519 ! learning medium
range: T4FS:0000372 ! data stewardship technical concept

[Typedef]
id: T4FS:0000581
name: confers compliance with
def: "Describes how an evaluation indicator may confer compliance with a particular guideline or set of guidelines" [] {IAO:0000119="https://orcid.org/0000-0002-7702-4495"}
property_value: IAO:0000117 "https://orcid.org/0000-0002-7702-4495" xsd:string
property_value: IAO:0000233 "https://github.com/terms4fairskills/FAIRterminology/issues/22" xsd:string
domain: T4FS:0000580 ! evaluation indicator
range: T4FS:0000446 ! data stewardship guideline

[Typedef]
id: T4FS:0000582
name: demonstrates how to fulfil the requirements for
def: "A learning medium may demonstrate how to meet the requirements for a particular evaluation indicator(s)." [] {IAO:0000119="https://orcid.org/0000-0002-7702-4495"}
property_value: IAO:0000117 "https://orcid.org/0000-0002-7702-4495" xsd:string
property_value: IAO:0000233 "https://github.com/terms4fairskills/FAIRterminology/issues/22" xsd:string
domain: T4FS:0000519 ! learning medium
range: T4FS:0000580 ! evaluation indicator

